# baseURI: http://w3id.org/ogeochem/def/samplecollection/ontology
# imports: http://purl.org/dc/elements/1.1/
# imports: http://www.w3.org/2000/01/rdf-schema
# imports: http://www.w3.org/2004/02/skos/core

@prefix dcterm: <http://purl.org/dc/terms/> .
@prefix dspl: <http://vocab.nerc.ac.uk/collection/P08/current/> .
@prefix grg: <http://www.isotc211.org/schemas/grg/> .
@prefix inst: <http://vocab.nerc.ac.uk/collection/L22/current/> .
@prefix owl: <http://www.w3.org/2002/07/owl#> .
@prefix pav: <http://purl.org/pav/> .
@prefix prov: <https://www.w3.org/ns/prov#> .
@prefix rdf: <http://www.w3.org/1999/02/22-rdf-syntax-ns#> .
@prefix rdfs: <http://www.w3.org/2000/01/rdf-schema#> .
@prefix sdev: <http://vocab.nerc.ac.uk/collection/L05/current/> .
@prefix sdnc: <http://vocab.nerc.ac.uk/collection/L21/current/> .
@prefix sdnd: <http://vocab.nerc.ac.uk/collection/C77/current/> .
@prefix sdnk: <http://vocab.nerc.ac.uk/collection/L19/current/> .
@prefix skos: <http://www.w3.org/2004/02/skos/core#> .
@prefix xml: <http://www.w3.org/XML/1998/namespace> .
@prefix xsd: <http://www.w3.org/2001/XMLSchema#> .

pav:authoredOn
  rdf:type owl:AnnotationProperty ;
.
pav:hasCurrentVersion
  rdf:type owl:AnnotationProperty ;
.
pav:hasVersion
  rdf:type owl:AnnotationProperty ;
.
pav:version
  rdf:type owl:AnnotationProperty ;
.
sdnd:B17
  rdf:type skos:Concept ;
  dcterm:date "2011-12-08 10:58:20.0" ;
  dcterm:identifier "SDN:C77::B17" ;
  pav:authoredOn "2011-12-08 10:58:20.0" ;
  pav:hasCurrentVersion <http://vocab.nerc.ac.uk/collection/C77/current/B17/1> ;
  owl:versionInfo "1" ;
  skos:broader <http://vocab.nerc.ac.uk/collection/L05/current/24> ;
  skos:definition "" ;
  skos:notation "SDN:C77::B17" ;
  skos:prefLabel "Phytobenthos"@en ;
.
sdnd:B18
  rdf:type skos:Concept ;
  dcterm:date "2011-12-08 10:58:20.0" ;
  dcterm:identifier "SDN:C77::B18" ;
  pav:authoredOn "2011-12-08 10:58:20.0" ;
  pav:hasCurrentVersion <http://vocab.nerc.ac.uk/collection/C77/current/B18/1> ;
  owl:versionInfo "1" ;
  skos:broader <http://vocab.nerc.ac.uk/collection/L05/current/24> ;
  skos:definition "" ;
  skos:notation "SDN:C77::B18" ;
  skos:prefLabel "Zoobenthos"@en ;
.
sdnd:B19
  rdf:type skos:Concept ;
  dcterm:date "2011-12-08 10:58:20.0" ;
  dcterm:identifier "SDN:C77::B19" ;
  pav:authoredOn "2011-12-08 10:58:20.0" ;
  pav:hasCurrentVersion <http://vocab.nerc.ac.uk/collection/C77/current/B19/1> ;
  owl:versionInfo "1" ;
  skos:broader <http://vocab.nerc.ac.uk/collection/L05/current/24> ;
  skos:definition "" ;
  skos:notation "SDN:C77::B19" ;
  skos:prefLabel "Demersal fish"@en ;
.
sdnd:G01
  rdf:type skos:Concept ;
  dcterm:date "2011-12-08 10:58:07.0" ;
  dcterm:identifier "SDN:C77::G01" ;
  pav:authoredOn "2011-12-08 10:58:07.0" ;
  pav:hasCurrentVersion <http://vocab.nerc.ac.uk/collection/C77/current/G01/1> ;
  owl:versionInfo "1" ;
  skos:broader sdnc:ICAT01 ;
  skos:definition "" ;
  skos:narrower <http://vocab.nerc.ac.uk/collection/L05/current/54> ;
  skos:narrower <http://vocab.nerc.ac.uk/collection/L05/current/60> ;
  skos:notation "SDN:C77::G01" ;
  skos:prefLabel "Dredge"@en ;
.
<http://vocab.nerc.ac.uk/collection/L05/current/11>
  rdf:type skos:Concept ;
  dcterm:date "2013-02-26 17:11:07.0" ;
  dcterm:identifier "SDN:L05::11" ;
  pav:authoredOn "2013-02-26 17:11:07.0" ;
  pav:hasCurrentVersion <http://vocab.nerc.ac.uk/collection/L05/current/11/2> ;
  pav:hasVersion <http://vocab.nerc.ac.uk/collection/L05/current/11/1> ;
  owl:versionInfo "2" ;
  skos:broader sdnc:ICAT01 ;
  skos:definition "A device that collects a sample of air from the atmosphere and stores it, usually under pressure, for subsequent analysis."@en ;
  skos:inScheme <http://vocab.nerc.ac.uk/scheme/EDMED_DCAT_THEMES/current> ;
  skos:inScheme <http://vocab.nerc.ac.uk/scheme/SDNDEV/current> ;
  skos:narrower inst:TOOL0544 ;
  skos:narrower inst:TOOL0545 ;
  skos:narrower inst:TOOL0588 ;
  skos:narrower <http://vocab.nerc.ac.uk/collection/W01/current/003> ;
  skos:notation "SDN:L05::11" ;
  skos:note "accepted"@en ;
  skos:prefLabel "discrete air samplers"@en ;
.
<http://vocab.nerc.ac.uk/collection/L05/current/12>
  rdf:type skos:Concept ;
  dcterm:date "2013-02-26 17:11:07.0" ;
  dcterm:identifier "SDN:L05::12" ;
  pav:authoredOn "2013-02-26 17:11:07.0" ;
  pav:hasCurrentVersion <http://vocab.nerc.ac.uk/collection/L05/current/12/2> ;
  pav:hasVersion <http://vocab.nerc.ac.uk/collection/L05/current/12/1> ;
  owl:versionInfo "2" ;
  skos:broader sdnc:ICAT01 ;
  skos:definition "A device that condenses a sample of fog from the atmosphere."@en ;
  skos:inScheme <http://vocab.nerc.ac.uk/scheme/EDMED_DCAT_THEMES/current> ;
  skos:inScheme <http://vocab.nerc.ac.uk/scheme/SDNDEV/current> ;
  skos:narrower <http://vocab.nerc.ac.uk/collection/W01/current/003> ;
  skos:notation "SDN:L05::12" ;
  skos:note "accepted"@en ;
  skos:prefLabel "fog samplers"@en ;
.
<http://vocab.nerc.ac.uk/collection/L05/current/13>
  rdf:type skos:Concept ;
  dcterm:date "2013-02-26 17:11:07.0" ;
  dcterm:identifier "SDN:L05::13" ;
  pav:authoredOn "2013-02-26 17:11:07.0" ;
  pav:hasCurrentVersion <http://vocab.nerc.ac.uk/collection/L05/current/13/2> ;
  pav:hasVersion <http://vocab.nerc.ac.uk/collection/L05/current/13/1> ;
  owl:versionInfo "2" ;
  skos:broader sdnc:ICAT01 ;
  skos:definition "A device that collects a sample of aerosol (dry particles or liquid droplets) from the atmosphere."@en ;
  skos:inScheme <http://vocab.nerc.ac.uk/scheme/EDMED_DCAT_THEMES/current> ;
  skos:inScheme <http://vocab.nerc.ac.uk/scheme/SDNDEV/current> ;
  skos:narrower inst:TOOL0550 ;
  skos:narrower inst:TOOL0551 ;
  skos:narrower inst:TOOL0554 ;
  skos:narrower <http://vocab.nerc.ac.uk/collection/W01/current/003> ;
  skos:notation "SDN:L05::13" ;
  skos:note "accepted"@en ;
  skos:prefLabel "aerosol samplers"@en ;
.
<http://vocab.nerc.ac.uk/collection/L05/current/14>
  rdf:type skos:Concept ;
  dcterm:date "2013-02-26 17:11:07.0" ;
  dcterm:identifier "SDN:L05::14" ;
  pav:authoredOn "2013-02-26 17:11:07.0" ;
  pav:hasCurrentVersion <http://vocab.nerc.ac.uk/collection/L05/current/14/2> ;
  pav:hasVersion <http://vocab.nerc.ac.uk/collection/L05/current/14/1> ;
  owl:versionInfo "2" ;
  skos:broader sdnc:ICAT01 ;
  skos:definition "A device that collects a sample of precipitation (rain, hail or snow) as it falls."@en ;
  skos:inScheme <http://vocab.nerc.ac.uk/scheme/EDMED_DCAT_THEMES/current> ;
  skos:inScheme <http://vocab.nerc.ac.uk/scheme/SDNDEV/current> ;
  skos:narrower inst:TOOL0541 ;
  skos:narrower <http://vocab.nerc.ac.uk/collection/W01/current/003> ;
  skos:notation "SDN:L05::14" ;
  skos:note "accepted"@en ;
  skos:prefLabel "precipitation samplers"@en ;
.
<http://vocab.nerc.ac.uk/collection/L05/current/182>
  rdf:type skos:Concept ;
  dcterm:date "2011-08-26 10:27:29.0" ;
  dcterm:identifier "SDN:L05::182" ;
  pav:authoredOn "2011-08-26 10:27:29.0" ;
  pav:hasCurrentVersion <http://vocab.nerc.ac.uk/collection/L05/current/182/2> ;
  pav:hasVersion <http://vocab.nerc.ac.uk/collection/L05/current/182/1> ;
  owl:versionInfo "2" ;
  skos:broader sdnc:ICAT01 ;
  skos:definition "There is no appropriate value. To be used in cases where metadata elements cannot be set null due to schema constraints."@en ;
  skos:inScheme <http://vocab.nerc.ac.uk/scheme/EDMED_DCAT_THEMES/current> ;
  skos:inScheme <http://vocab.nerc.ac.uk/scheme/SDNDEV/current> ;
  skos:narrower inst:TOOL000X ;
  skos:narrower <http://vocab.nerc.ac.uk/collection/W01/current/003> ;
  skos:notation "SDN:L05::182" ;
  skos:note "accepted"@en ;
  skos:prefLabel "inapplicable"@en ;
.
<http://vocab.nerc.ac.uk/collection/L05/current/21>
  rdf:type skos:Concept ;
  dcterm:date "2013-02-26 17:11:07.0" ;
  dcterm:identifier "SDN:L05::21" ;
  pav:authoredOn "2013-02-26 17:11:07.0" ;
  pav:hasCurrentVersion <http://vocab.nerc.ac.uk/collection/L05/current/21/2> ;
  pav:hasVersion <http://vocab.nerc.ac.uk/collection/L05/current/21/1> ;
  owl:versionInfo "2" ;
  skos:broader sdnc:ICAT01 ;
  skos:definition "A device that continuously samples a flow of water, separating and fixing plankton for subsequent identification and counting."@en ;
  skos:inScheme <http://vocab.nerc.ac.uk/scheme/EDMED_DCAT_THEMES/current> ;
  skos:inScheme <http://vocab.nerc.ac.uk/scheme/NETMAR_OCEAN/current> ;
  skos:inScheme <http://vocab.nerc.ac.uk/scheme/NETOC_INSTRUMENT/current> ;
  skos:inScheme <http://vocab.nerc.ac.uk/scheme/SDNDEV/current> ;
  skos:narrower inst:NETT0026 ;
  skos:narrower inst:NETT0047 ;
  skos:narrower inst:NETT0184 ;
  skos:narrower <http://vocab.nerc.ac.uk/collection/W01/current/003> ;
  skos:notation "SDN:L05::21" ;
  skos:note "accepted"@en ;
  skos:prefLabel "plankton recorders"@en ;
  skos:related <http://vocab.nerc.ac.uk/collection/P25/current/PHYTABUND> ;
.
<http://vocab.nerc.ac.uk/collection/L05/current/22>
  rdf:type skos:Concept ;
  dcterm:date "2018-02-20 17:43:56.0" ;
  dcterm:identifier "SDN:L05::22" ;
  pav:authoredOn "2018-02-20 17:43:56.0" ;
  pav:hasCurrentVersion <http://vocab.nerc.ac.uk/collection/L05/current/22/2> ;
  pav:hasVersion <http://vocab.nerc.ac.uk/collection/L05/current/22/1> ;
  owl:versionInfo "2" ;
  skos:broader sdnc:ICAT01 ;
  skos:definition "A fine-meshed net designed to collect small size organisms, aggregates, or litter in the water column including for example microzooplankton, mesozooplankton, nekton, microplastic or other litter."@en ;
  skos:inScheme <http://vocab.nerc.ac.uk/scheme/EDMED_DCAT_THEMES/current> ;
  skos:inScheme <http://vocab.nerc.ac.uk/scheme/SDNDEV/current> ;
  skos:narrower inst:NETT0001 ;
  skos:narrower inst:NETT0003 ;
  skos:narrower inst:NETT0006 ;
  skos:narrower inst:NETT0009 ;
  skos:narrower inst:NETT0010 ;
  skos:narrower inst:NETT0016 ;
  skos:narrower inst:NETT0019 ;
  skos:narrower inst:NETT0023 ;
  skos:narrower inst:NETT0024 ;
  skos:narrower inst:NETT0030 ;
  skos:narrower inst:NETT0031 ;
  skos:narrower inst:NETT0032 ;
  skos:narrower inst:NETT0034 ;
  skos:narrower inst:NETT0035 ;
  skos:narrower inst:NETT0036 ;
  skos:narrower inst:NETT0039 ;
  skos:narrower inst:NETT0040 ;
  skos:narrower inst:NETT0041 ;
  skos:narrower inst:NETT0042 ;
  skos:narrower inst:NETT0044 ;
  skos:narrower inst:NETT0045 ;
  skos:narrower inst:NETT0054 ;
  skos:narrower inst:NETT0074 ;
  skos:narrower inst:NETT0075 ;
  skos:narrower inst:NETT0077 ;
  skos:narrower inst:NETT0078 ;
  skos:narrower inst:NETT0079 ;
  skos:narrower inst:NETT0080 ;
  skos:narrower inst:NETT0090 ;
  skos:narrower inst:NETT0091 ;
  skos:narrower inst:NETT0092 ;
  skos:narrower inst:NETT0095 ;
  skos:narrower inst:NETT0098 ;
  skos:narrower inst:NETT0100 ;
  skos:narrower inst:NETT0102 ;
  skos:narrower inst:NETT0103 ;
  skos:narrower inst:NETT0104 ;
  skos:narrower inst:NETT0105 ;
  skos:narrower inst:NETT0106 ;
  skos:narrower inst:NETT0108 ;
  skos:narrower inst:NETT0122 ;
  skos:narrower inst:NETT0124 ;
  skos:narrower inst:NETT0125 ;
  skos:narrower inst:NETT0126 ;
  skos:narrower inst:NETT0127 ;
  skos:narrower inst:NETT0128 ;
  skos:narrower inst:NETT0129 ;
  skos:narrower inst:NETT0131 ;
  skos:narrower inst:NETT0132 ;
  skos:narrower inst:NETT0133 ;
  skos:narrower inst:NETT0134 ;
  skos:narrower inst:NETT0135 ;
  skos:narrower inst:NETT0136 ;
  skos:narrower inst:NETT0137 ;
  skos:narrower inst:NETT0138 ;
  skos:narrower inst:NETT0140 ;
  skos:narrower inst:NETT0141 ;
  skos:narrower inst:NETT0142 ;
  skos:narrower inst:NETT0143 ;
  skos:narrower inst:NETT0144 ;
  skos:narrower inst:NETT0147 ;
  skos:narrower inst:NETT0151 ;
  skos:narrower inst:NETT0153 ;
  skos:narrower inst:NETT0155 ;
  skos:narrower inst:NETT0163 ;
  skos:narrower inst:NETT0164 ;
  skos:narrower inst:NETT0166 ;
  skos:narrower inst:NETT0167 ;
  skos:narrower inst:NETT0169 ;
  skos:narrower inst:NETT0171 ;
  skos:narrower inst:NETT0173 ;
  skos:narrower inst:NETT0174 ;
  skos:narrower inst:NETT0176 ;
  skos:narrower inst:NETT0177 ;
  skos:narrower inst:NETT0199 ;
  skos:narrower inst:NETT0200 ;
  skos:narrower inst:NETT0201 ;
  skos:narrower inst:NETT0202 ;
  skos:narrower inst:TOOL0978 ;
  skos:narrower inst:TOOL0979 ;
  skos:narrower inst:TOOL0980 ;
  skos:narrower inst:TOOL0981 ;
  skos:narrower inst:TOOL0982 ;
  skos:narrower inst:TOOL0983 ;
  skos:narrower inst:TOOL0984 ;
  skos:narrower inst:TOOL0986 ;
  skos:narrower inst:TOOL0987 ;
  skos:narrower inst:TOOL0988 ;
  skos:narrower inst:TOOL0989 ;
  skos:narrower inst:TOOL0990 ;
  skos:narrower inst:TOOL0992 ;
  skos:narrower inst:TOOL0993 ;
  skos:narrower inst:TOOL0994 ;
  skos:narrower inst:TOOL0995 ;
  skos:narrower inst:TOOL0996 ;
  skos:narrower inst:TOOL0997 ;
  skos:narrower inst:TOOL1181 ;
  skos:narrower <http://vocab.nerc.ac.uk/collection/W01/current/003> ;
  skos:notation "SDN:L05::22" ;
  skos:note "accepted"@en ;
  skos:prefLabel "plankton nets"@en ;
.
<http://vocab.nerc.ac.uk/collection/L05/current/23>
  rdf:type skos:Concept ;
  dcterm:date "2007-11-20 08:50:03.0" ;
  dcterm:identifier "SDN:L05::23" ;
  pav:authoredOn "2007-11-20 08:50:03.0" ;
  pav:hasCurrentVersion <http://vocab.nerc.ac.uk/collection/L05/current/23/1> ;
  owl:sameAs sdnd:B14 ;
  owl:versionInfo "1" ;
  skos:broader <http://vocab.nerc.ac.uk/collection/L05/current/64> ;
  skos:broader sdnc:ICAT01 ;
  skos:definition "A net towed through the water column designed to sample free-swimming nekton or fish."@en ;
  skos:inScheme <http://vocab.nerc.ac.uk/scheme/EDMED_DCAT_THEMES/current> ;
  skos:inScheme <http://vocab.nerc.ac.uk/scheme/SDNDEV/current> ;
  skos:narrower inst:NETT0022 ;
  skos:narrower inst:NETT0043 ;
  skos:narrower inst:NETT0071 ;
  skos:narrower inst:NETT0072 ;
  skos:narrower inst:NETT0073 ;
  skos:narrower inst:NETT0150 ;
  skos:narrower inst:NETT0161 ;
  skos:narrower inst:NETT0162 ;
  skos:narrower inst:NETT0178 ;
  skos:narrower inst:NETT0179 ;
  skos:narrower inst:NETT0180 ;
  skos:narrower inst:NETT0181 ;
  skos:narrower inst:TOOL0985 ;
  skos:narrower <http://vocab.nerc.ac.uk/collection/W01/current/003> ;
  skos:notation "SDN:L05::23" ;
  skos:note "accepted"@en ;
  skos:prefLabel "pelagic trawl nets"@en ;
.
<http://vocab.nerc.ac.uk/collection/L05/current/24>
  rdf:type skos:Concept ;
  <http://purl.org/dc/terms/:replaces> <http://vocab.nerc.ac.uk/collection/L05/current/71> ;
  <http://purl.org/dc/terms/:replaces> <http://vocab.nerc.ac.uk/collection/L05/current/72> ;
  dcterm:date "2019-12-19 11:32:58.0" ;
  dcterm:identifier "SDN:L05::24" ;
  pav:authoredOn "2019-12-19 11:32:58.0" ;
  pav:hasCurrentVersion <http://vocab.nerc.ac.uk/collection/L05/current/24/4> ;
  pav:hasVersion <http://vocab.nerc.ac.uk/collection/L05/current/24/1> ;
  pav:hasVersion <http://vocab.nerc.ac.uk/collection/L05/current/24/2> ;
  pav:hasVersion <http://vocab.nerc.ac.uk/collection/L05/current/24/3> ;
  owl:versionInfo "4" ;
  skos:broader <http://vocab.nerc.ac.uk/collection/L05/current/64> ;
  skos:broader sdnc:ICAT01 ;
  skos:definition "A mechanical device that collects organisms from the seafloor. Includes dredges, sledges, weighted nets like beam trawls, and ROV manipulators."@en ;
  skos:inScheme <http://vocab.nerc.ac.uk/scheme/EDMED_DCAT_THEMES/current> ;
  skos:inScheme <http://vocab.nerc.ac.uk/scheme/SDNDEV/current> ;
  skos:narrower sdnd:B17 ;
  skos:narrower sdnd:B18 ;
  skos:narrower sdnd:B19 ;
  skos:narrower <http://vocab.nerc.ac.uk/collection/L05/current/61> ;
  skos:narrower <http://vocab.nerc.ac.uk/collection/L05/current/62> ;
  skos:narrower inst:NETT0040 ;
  skos:narrower inst:NETT0041 ;
  skos:narrower inst:NETT0042 ;
  skos:narrower inst:NETT0141 ;
  skos:narrower inst:NETT0142 ;
  skos:narrower inst:NETT0182 ;
  skos:narrower inst:NETT0186 ;
  skos:narrower inst:NETT0189 ;
  skos:narrower inst:NETT0190 ;
  skos:narrower inst:NETT0191 ;
  skos:narrower inst:NETT0192 ;
  skos:narrower inst:TOOL1165 ;
  skos:narrower inst:TOOL1166 ;
  skos:narrower inst:TOOL1378 ;
  skos:narrower inst:TOOL1379 ;
  skos:narrower inst:TOOL1462 ;
  skos:narrower inst:TOOL1815 ;
  skos:narrower <http://vocab.nerc.ac.uk/collection/W01/current/003> ;
  skos:notation "SDN:L05::24" ;
  skos:note "accepted"@en ;
  skos:prefLabel "benthos samplers"@en ;
.
<http://vocab.nerc.ac.uk/collection/L05/current/30>
  rdf:type skos:Concept ;
  dcterm:date "2013-02-26 17:11:07.0" ;
  dcterm:identifier "SDN:L05::30" ;
  pav:authoredOn "2013-02-26 17:11:07.0" ;
  pav:hasCurrentVersion <http://vocab.nerc.ac.uk/collection/L05/current/30/2> ;
  pav:hasVersion <http://vocab.nerc.ac.uk/collection/L05/current/30/1> ;
  owl:versionInfo "2" ;
  skos:broader sdnc:ICAT01 ;
  skos:definition "A device that collects an in-situ discrete water sample from any depth and returns it to the surface without contamination by the waters through which it passes, such as a water bottle."@en ;
  skos:inScheme <http://vocab.nerc.ac.uk/scheme/EDMED_DCAT_THEMES/current> ;
  skos:inScheme <http://vocab.nerc.ac.uk/scheme/NETMAR_OCEAN/current> ;
  skos:inScheme <http://vocab.nerc.ac.uk/scheme/NETOC_INSTRUMENT/current> ;
  skos:inScheme <http://vocab.nerc.ac.uk/scheme/SDNDEV/current> ;
  skos:narrower inst:NETT0175 ;
  skos:narrower inst:TOOL0235 ;
  skos:narrower inst:TOOL0236 ;
  skos:narrower inst:TOOL0248 ;
  skos:narrower inst:TOOL0381 ;
  skos:narrower inst:TOOL0412 ;
  skos:narrower inst:TOOL0418 ;
  skos:narrower inst:TOOL0427 ;
  skos:narrower inst:TOOL0501 ;
  skos:narrower inst:TOOL0502 ;
  skos:narrower inst:TOOL0503 ;
  skos:narrower inst:TOOL0504 ;
  skos:narrower inst:TOOL0505 ;
  skos:narrower inst:TOOL0506 ;
  skos:narrower inst:TOOL0508 ;
  skos:narrower inst:TOOL0535 ;
  skos:narrower inst:TOOL0536 ;
  skos:narrower inst:TOOL0537 ;
  skos:narrower inst:TOOL0538 ;
  skos:narrower inst:TOOL0540 ;
  skos:narrower inst:TOOL0542 ;
  skos:narrower inst:TOOL0543 ;
  skos:narrower inst:TOOL0546 ;
  skos:narrower inst:TOOL0547 ;
  skos:narrower inst:TOOL0548 ;
  skos:narrower inst:TOOL0552 ;
  skos:narrower inst:TOOL0556 ;
  skos:narrower inst:TOOL0557 ;
  skos:narrower inst:TOOL0660 ;
  skos:narrower inst:TOOL0828 ;
  skos:narrower inst:TOOL0939 ;
  skos:narrower inst:TOOL0940 ;
  skos:narrower inst:TOOL1253 ;
  skos:narrower inst:TOOL1326 ;
  skos:narrower inst:TOOL1339 ;
  skos:narrower inst:TOOL1463 ;
  skos:narrower inst:TOOL1464 ;
  skos:narrower inst:TOOL1465 ;
  skos:narrower inst:TOOL1466 ;
  skos:narrower inst:TOOL1467 ;
  skos:narrower inst:TOOL1576 ;
  skos:narrower inst:TOOL1654 ;
  skos:narrower <http://vocab.nerc.ac.uk/collection/W01/current/003> ;
  skos:notation "SDN:L05::30" ;
  skos:note "accepted"@en ;
  skos:prefLabel "discrete water samplers"@en ;
  skos:related <http://vocab.nerc.ac.uk/collection/P25/current/CHLA> ;
  skos:related <http://vocab.nerc.ac.uk/collection/P25/current/NO2> ;
  skos:related <http://vocab.nerc.ac.uk/collection/P25/current/NO3> ;
  skos:related <http://vocab.nerc.ac.uk/collection/P25/current/NO3NO2> ;
  skos:related <http://vocab.nerc.ac.uk/collection/P25/current/PHAEO> ;
  skos:related <http://vocab.nerc.ac.uk/collection/P25/current/PHYTABUND> ;
  skos:related <http://vocab.nerc.ac.uk/collection/P25/current/PO4> ;
  skos:related <http://vocab.nerc.ac.uk/collection/P25/current/SALIN> ;
  skos:related <http://vocab.nerc.ac.uk/collection/P25/current/SLCA> ;
.
<http://vocab.nerc.ac.uk/collection/L05/current/31>
  rdf:type skos:Concept ;
  dcterm:date "2013-02-26 17:11:07.0" ;
  dcterm:identifier "SDN:L05::31" ;
  pav:authoredOn "2013-02-26 17:11:07.0" ;
  pav:hasCurrentVersion <http://vocab.nerc.ac.uk/collection/L05/current/31/2> ;
  pav:hasVersion <http://vocab.nerc.ac.uk/collection/L05/current/31/1> ;
  owl:versionInfo "2" ;
  skos:broader sdnc:ICAT01 ;
  skos:definition "A device that continuously supplies a flow of water either to an analytical instrument, over a sensor or from which samples may be drawn."@en ;
  skos:inScheme <http://vocab.nerc.ac.uk/scheme/EDMED_DCAT_THEMES/current> ;
  skos:inScheme <http://vocab.nerc.ac.uk/scheme/NETMAR_OCEAN/current> ;
  skos:inScheme <http://vocab.nerc.ac.uk/scheme/NETOC_INSTRUMENT/current> ;
  skos:inScheme <http://vocab.nerc.ac.uk/scheme/SDNDEV/current> ;
  skos:narrower inst:TOOL0413 ;
  skos:narrower inst:TOOL0539 ;
  skos:narrower inst:TOOL0555 ;
  skos:narrower inst:TOOL0561 ;
  skos:narrower inst:TOOL0562 ;
  skos:narrower inst:TOOL1135 ;
  skos:narrower inst:TOOL1405 ;
  skos:narrower inst:TOOL1727 ;
  skos:narrower <http://vocab.nerc.ac.uk/collection/W01/current/003> ;
  skos:notation "SDN:L05::31" ;
  skos:note "accepted"@en ;
  skos:prefLabel "continuous water samplers"@en ;
  skos:related <http://vocab.nerc.ac.uk/collection/P25/current/CHLA> ;
  skos:related <http://vocab.nerc.ac.uk/collection/P25/current/NO2> ;
  skos:related <http://vocab.nerc.ac.uk/collection/P25/current/NO3> ;
  skos:related <http://vocab.nerc.ac.uk/collection/P25/current/NO3NO2> ;
  skos:related <http://vocab.nerc.ac.uk/collection/P25/current/PHAEO> ;
  skos:related <http://vocab.nerc.ac.uk/collection/P25/current/PO4> ;
  skos:related <http://vocab.nerc.ac.uk/collection/P25/current/SLCA> ;
.
<http://vocab.nerc.ac.uk/collection/L05/current/32>
  rdf:type skos:Concept ;
  dcterm:date "2007-11-20 08:50:03.0" ;
  dcterm:identifier "SDN:L05::32" ;
  pav:authoredOn "2007-11-20 08:50:03.0" ;
  pav:hasCurrentVersion <http://vocab.nerc.ac.uk/collection/L05/current/32/1> ;
  owl:versionInfo "1" ;
  skos:broader sdnc:ICAT01 ;
  skos:definition "A system that collects samples of water column particulates such as in-situ high volume filtration systems liks SAPs."@en ;
  skos:inScheme <http://vocab.nerc.ac.uk/scheme/EDMED_DCAT_THEMES/current> ;
  skos:inScheme <http://vocab.nerc.ac.uk/scheme/NETMAR_OCEAN/current> ;
  skos:inScheme <http://vocab.nerc.ac.uk/scheme/NETOC_INSTRUMENT/current> ;
  skos:inScheme <http://vocab.nerc.ac.uk/scheme/SDNDEV/current> ;
  skos:narrower <http://vocab.nerc.ac.uk/collection/W01/current/003> ;
  skos:notation "SDN:L05::32" ;
  skos:note "accepted"@en ;
  skos:prefLabel "particulates samplers"@en ;
  skos:related <http://vocab.nerc.ac.uk/collection/P25/current/CHLA> ;
  skos:related <http://vocab.nerc.ac.uk/collection/P25/current/PHAEO> ;
.
<http://vocab.nerc.ac.uk/collection/L05/current/33>
  rdf:type skos:Concept ;
  dcterm:date "2013-02-26 17:11:07.0" ;
  dcterm:identifier "SDN:L05::33" ;
  pav:authoredOn "2013-02-26 17:11:07.0" ;
  pav:hasCurrentVersion <http://vocab.nerc.ac.uk/collection/L05/current/33/2> ;
  pav:hasVersion <http://vocab.nerc.ac.uk/collection/L05/current/33/1> ;
  owl:sameAs sdnd:B73 ;
  owl:versionInfo "2" ;
  skos:broader sdnc:ICAT01 ;
  skos:definition "A collector of particulates as they sink through the water column."@en ;
  skos:inScheme <http://vocab.nerc.ac.uk/scheme/EDMED_DCAT_THEMES/current> ;
  skos:inScheme <http://vocab.nerc.ac.uk/scheme/SDNDEV/current> ;
  skos:narrower inst:TOOL0785 ;
  skos:narrower inst:TOOL0786 ;
  skos:narrower inst:TOOL0787 ;
  skos:narrower inst:TOOL0917 ;
  skos:narrower inst:TOOL1304 ;
  skos:narrower inst:TOOL1454 ;
  skos:narrower inst:TOOL1455 ;
  skos:narrower inst:TOOL1668 ;
  skos:narrower <http://vocab.nerc.ac.uk/collection/W01/current/003> ;
  skos:notation "SDN:L05::33" ;
  skos:note "accepted"@en ;
  skos:prefLabel "sediment traps"@en ;
.
<http://vocab.nerc.ac.uk/collection/L05/current/391>
  rdf:type skos:Concept ;
  dcterm:date "2019-12-19 15:01:25.0" ;
  dcterm:identifier "SDN:L05::391" ;
  pav:authoredOn "2019-12-19 15:01:25.0" ;
  pav:hasCurrentVersion <http://vocab.nerc.ac.uk/collection/L05/current/391/1> ;
  owl:versionInfo "1" ;
  skos:broader sdnc:ICAT01 ;
  skos:definition "Devices that collect samples from the sediment layer surface using suction. The mechanism of suction can be accomplished by either vacuum, by pressure difference between the air inside the sampler and surrounding water, by pumping water directly into the sampler or by under pressure air to elevate the sediment inside the sampler. Devices are typically diver- or remotely-operated."@en ;
  skos:inScheme <http://vocab.nerc.ac.uk/scheme/SDNDEV/current> ;
  skos:narrower inst:TOOL1371 ;
  skos:narrower inst:TOOL1372 ;
  skos:notation "SDN:L05::391" ;
  skos:note "accepted"@en ;
  skos:prefLabel "sediment suction samplers"@en ;
.
<http://vocab.nerc.ac.uk/collection/L05/current/392>
  rdf:type skos:Concept ;
  dcterm:date "2020-04-07 10:14:48.0" ;
  dcterm:identifier "SDN:L05::392" ;
  pav:authoredOn "2020-04-07 10:14:48.0" ;
  pav:hasCurrentVersion <http://vocab.nerc.ac.uk/collection/L05/current/392/1> ;
  owl:versionInfo "1" ;
  skos:altLabel "substrates"@en ;
  skos:broader sdnc:ICAT01 ;
  skos:definition "Natural or artificial materials deployed in a marine or artificial environment for a given period to act as standardised, passive settlement sampling devices (e.g. settlement plates). They are used to determine the extent of colonisation and/or the diversity of settled organisms."@en ;
  skos:inScheme <http://vocab.nerc.ac.uk/scheme/SDNDEV/current> ;
  skos:narrower inst:TOOL1413 ;
  skos:narrower inst:TOOL1414 ;
  skos:narrower inst:TOOL1415 ;
  skos:narrower inst:TOOL1416 ;
  skos:narrower inst:TOOL1417 ;
  skos:notation "SDN:L05::392" ;
  skos:note "accepted"@en ;
  skos:prefLabel "colonisation substrata"@en ;
.
<http://vocab.nerc.ac.uk/collection/L05/current/50>
  rdf:type skos:Concept ;
  dcterm:date "2007-11-20 08:50:03.0" ;
  dcterm:identifier "SDN:L05::50" ;
  pav:authoredOn "2007-11-20 08:50:03.0" ;
  pav:hasCurrentVersion <http://vocab.nerc.ac.uk/collection/L05/current/50/1> ;
  owl:sameAs sdnd:G02 ;
  owl:versionInfo "1" ;
  skos:broader sdnc:ICAT01 ;
  skos:definition "A device that collects a sample of surface sediment including manually deployed equipment like a shovel or bucket."@en ;
  skos:inScheme <http://vocab.nerc.ac.uk/scheme/EDMED_DCAT_THEMES/current> ;
  skos:inScheme <http://vocab.nerc.ac.uk/scheme/SDNDEV/current> ;
  skos:narrower inst:TOOL0653 ;
  skos:narrower inst:TOOL0788 ;
  skos:narrower inst:TOOL0960 ;
  skos:narrower inst:TOOL0961 ;
  skos:narrower inst:TOOL0962 ;
  skos:narrower inst:TOOL0963 ;
  skos:narrower inst:TOOL1214 ;
  skos:narrower inst:TOOL1215 ;
  skos:narrower inst:TOOL1216 ;
  skos:narrower inst:TOOL1487 ;
  skos:narrower inst:TOOL1533 ;
  skos:narrower inst:TOOL1535 ;
  skos:narrower <http://vocab.nerc.ac.uk/collection/W01/current/003> ;
  skos:notation "SDN:L05::50" ;
  skos:note "accepted"@en ;
  skos:prefLabel "sediment grabs"@en ;
.
<http://vocab.nerc.ac.uk/collection/L05/current/51>
  rdf:type skos:Concept ;
  dcterm:date "2014-11-12 11:08:53.0" ;
  dcterm:identifier "SDN:L05::51" ;
  pav:authoredOn "2014-11-12 11:08:53.0" ;
  pav:hasCurrentVersion <http://vocab.nerc.ac.uk/collection/L05/current/51/3> ;
  pav:hasVersion <http://vocab.nerc.ac.uk/collection/L05/current/51/1> ;
  pav:hasVersion <http://vocab.nerc.ac.uk/collection/L05/current/51/2> ;
  owl:sameAs sdnd:G04 ;
  owl:versionInfo "3" ;
  skos:broader sdnc:ICAT01 ;
  skos:definition "Devices designed to collect samples of unconsolidated sediment from between the surface and depths from centimetres to 10s of metres with minimal disturbance of the sediment structure."@en ;
  skos:inScheme <http://vocab.nerc.ac.uk/scheme/EDMED_DCAT_THEMES/current> ;
  skos:inScheme <http://vocab.nerc.ac.uk/scheme/SDNDEV/current> ;
  skos:narrower inst:TOOL0472 ;
  skos:narrower inst:TOOL0784 ;
  skos:narrower inst:TOOL0806 ;
  skos:narrower inst:TOOL0807 ;
  skos:narrower inst:TOOL1169 ;
  skos:narrower inst:TOOL1171 ;
  skos:narrower inst:TOOL1172 ;
  skos:narrower inst:TOOL1173 ;
  skos:narrower inst:TOOL1174 ;
  skos:narrower inst:TOOL1175 ;
  skos:narrower inst:TOOL1176 ;
  skos:narrower inst:TOOL1177 ;
  skos:narrower inst:TOOL1178 ;
  skos:narrower inst:TOOL1179 ;
  skos:narrower inst:TOOL1191 ;
  skos:narrower inst:TOOL1199 ;
  skos:narrower inst:TOOL1204 ;
  skos:narrower inst:TOOL1235 ;
  skos:narrower inst:TOOL1260 ;
  skos:narrower inst:TOOL1285 ;
  skos:narrower inst:TOOL1374 ;
  skos:narrower inst:TOOL1375 ;
  skos:narrower inst:TOOL1376 ;
  skos:narrower inst:TOOL1468 ;
  skos:narrower inst:TOOL1469 ;
  skos:narrower inst:TOOL1485 ;
  skos:narrower inst:TOOL1486 ;
  skos:narrower inst:TOOL1527 ;
  skos:narrower inst:TOOL1536 ;
  skos:narrower inst:TOOL1537 ;
  skos:narrower inst:TOOL1560 ;
  skos:narrower inst:TOOL1644 ;
  skos:narrower inst:TOOL1703 ;
  skos:narrower <http://vocab.nerc.ac.uk/collection/W01/current/003> ;
  skos:notation "SDN:L05::51" ;
  skos:note "accepted"@en ;
  skos:prefLabel "unconsolidated sediment corers"@en ;
.
<http://vocab.nerc.ac.uk/collection/L05/current/52>
  rdf:type skos:Concept ;
  dcterm:date "2007-11-20 08:50:03.0" ;
  dcterm:identifier "SDN:L05::52" ;
  pav:authoredOn "2007-11-20 08:50:03.0" ;
  pav:hasCurrentVersion <http://vocab.nerc.ac.uk/collection/L05/current/52/1> ;
  owl:versionInfo "1" ;
  skos:broader sdnc:ICAT01 ;
  skos:definition "A device that collects samples of pore water from various horizons below the seabed."@en ;
  skos:inScheme <http://vocab.nerc.ac.uk/scheme/EDMED_DCAT_THEMES/current> ;
  skos:inScheme <http://vocab.nerc.ac.uk/scheme/SDNDEV/current> ;
  skos:narrower inst:TOOL1741 ;
  skos:narrower <http://vocab.nerc.ac.uk/collection/W01/current/003> ;
  skos:notation "SDN:L05::52" ;
  skos:note "accepted"@en ;
  skos:prefLabel "sediment porewater samplers"@en ;
.
<http://vocab.nerc.ac.uk/collection/L05/current/53>
  rdf:type skos:Concept ;
  dcterm:date "2018-09-20 10:24:53.0" ;
  dcterm:identifier "SDN:L05::53" ;
  pav:authoredOn "2018-09-20 10:24:53.0" ;
  pav:hasCurrentVersion <http://vocab.nerc.ac.uk/collection/L05/current/53/3> ;
  pav:hasVersion <http://vocab.nerc.ac.uk/collection/L05/current/53/1> ;
  pav:hasVersion <http://vocab.nerc.ac.uk/collection/L05/current/53/2> ;
  owl:sameAs sdnd:G03 ;
  owl:versionInfo "3" ;
  skos:broader sdnc:ICAT01 ;
  skos:definition "A device that extracts rock either by chipping or drilling."@en ;
  skos:inScheme <http://vocab.nerc.ac.uk/scheme/EDMED_DCAT_THEMES/current> ;
  skos:inScheme <http://vocab.nerc.ac.uk/scheme/SDNDEV/current> ;
  skos:narrower inst:TOOL1170 ;
  skos:narrower inst:TOOL1172 ;
  skos:narrower <http://vocab.nerc.ac.uk/collection/W01/current/003> ;
  skos:notation "SDN:L05::53" ;
  skos:note "accepted"@en ;
  skos:prefLabel "rock corers"@en ;
.
<http://vocab.nerc.ac.uk/collection/L05/current/54>
  rdf:type skos:Concept ;
  dcterm:date "2007-11-20 08:50:03.0" ;
  dcterm:identifier "SDN:L05::54" ;
  pav:authoredOn "2007-11-20 08:50:03.0" ;
  pav:hasCurrentVersion <http://vocab.nerc.ac.uk/collection/L05/current/54/1> ;
  owl:versionInfo "1" ;
  skos:broader sdnd:G01 ;
  skos:broader sdnc:ICAT01 ;
  skos:definition "A device dragged across the seabed designed to collect loose rock samples."@en ;
  skos:inScheme <http://vocab.nerc.ac.uk/scheme/EDMED_DCAT_THEMES/current> ;
  skos:inScheme <http://vocab.nerc.ac.uk/scheme/SDNDEV/current> ;
  skos:narrower <http://vocab.nerc.ac.uk/collection/W01/current/003> ;
  skos:notation "SDN:L05::54" ;
  skos:note "accepted"@en ;
  skos:prefLabel "rock dredges"@en ;
.
<http://vocab.nerc.ac.uk/collection/L05/current/55>
  rdf:type skos:Concept ;
  dcterm:date "2007-11-20 08:50:03.0" ;
  dcterm:identifier "SDN:L05::55" ;
  pav:authoredOn "2007-11-20 08:50:03.0" ;
  pav:hasCurrentVersion <http://vocab.nerc.ac.uk/collection/L05/current/55/1> ;
  owl:versionInfo "1" ;
  skos:broader sdnc:ICAT01 ;
  skos:definition "A specialised water bottle that both collects water samples and provides a settling velocity experiment apparatus."@en ;
  skos:inScheme <http://vocab.nerc.ac.uk/scheme/EDMED_DCAT_THEMES/current> ;
  skos:inScheme <http://vocab.nerc.ac.uk/scheme/SDNDEV/current> ;
  skos:narrower <http://vocab.nerc.ac.uk/collection/W01/current/003> ;
  skos:notation "SDN:L05::55" ;
  skos:note "accepted"@en ;
  skos:prefLabel "sediment settling tubes"@en ;
.
<http://vocab.nerc.ac.uk/collection/L05/current/56>
  rdf:type skos:Concept ;
  dcterm:date "2013-02-26 17:11:07.0" ;
  dcterm:identifier "SDN:L05::56" ;
  pav:authoredOn "2013-02-26 17:11:07.0" ;
  pav:hasCurrentVersion <http://vocab.nerc.ac.uk/collection/L05/current/56/2> ;
  pav:hasVersion <http://vocab.nerc.ac.uk/collection/L05/current/56/1> ;
  owl:versionInfo "2" ;
  skos:broader sdnc:ICAT01 ;
  skos:definition "A device that collects a sample of frozen seawater or accumulated frozen precipitation."@en ;
  skos:inScheme <http://vocab.nerc.ac.uk/scheme/EDMED_DCAT_THEMES/current> ;
  skos:inScheme <http://vocab.nerc.ac.uk/scheme/NETMAR_OCEAN/current> ;
  skos:inScheme <http://vocab.nerc.ac.uk/scheme/NETOC_INSTRUMENT/current> ;
  skos:inScheme <http://vocab.nerc.ac.uk/scheme/SDNDEV/current> ;
  skos:narrower inst:TOOL1249 ;
  skos:narrower <http://vocab.nerc.ac.uk/collection/W01/current/003> ;
  skos:notation "SDN:L05::56" ;
  skos:note "accepted"@en ;
  skos:prefLabel "snow and ice samplers"@en ;
  skos:related <http://vocab.nerc.ac.uk/collection/P25/current/ICESSALIN> ;
.
<http://vocab.nerc.ac.uk/collection/L05/current/57>
  rdf:type skos:Concept ;
  dcterm:date "2013-02-26 17:11:07.0" ;
  dcterm:identifier "SDN:L05::57" ;
  pav:authoredOn "2013-02-26 17:11:07.0" ;
  pav:hasCurrentVersion <http://vocab.nerc.ac.uk/collection/L05/current/57/2> ;
  pav:hasVersion <http://vocab.nerc.ac.uk/collection/L05/current/57/1> ;
  owl:versionInfo "2" ;
  skos:broader sdnc:ICAT01 ;
  skos:definition "A simple tool like a hammer, saw or even just a hand for the collection of rock samples."@en ;
  skos:inScheme <http://vocab.nerc.ac.uk/scheme/EDMED_DCAT_THEMES/current> ;
  skos:inScheme <http://vocab.nerc.ac.uk/scheme/SDNDEV/current> ;
  skos:narrower <http://vocab.nerc.ac.uk/collection/W01/current/003> ;
  skos:notation "SDN:L05::57" ;
  skos:note "accepted"@en ;
  skos:prefLabel "manual rock samplers"@en ;
.
<http://vocab.nerc.ac.uk/collection/L05/current/58>
  rdf:type skos:Concept ;
  dcterm:date "2013-02-26 17:11:07.0" ;
  dcterm:identifier "SDN:L05::58" ;
  pav:authoredOn "2013-02-26 17:11:07.0" ;
  pav:hasCurrentVersion <http://vocab.nerc.ac.uk/collection/L05/current/58/2> ;
  pav:hasVersion <http://vocab.nerc.ac.uk/collection/L05/current/58/1> ;
  owl:versionInfo "2" ;
  skos:broader sdnc:ICAT01 ;
  skos:definition "A device that continuously supplies a flow of air either to an analytical instrument, over a sensor or from which discrete samples may be drawn."@en ;
  skos:inScheme <http://vocab.nerc.ac.uk/scheme/EDMED_DCAT_THEMES/current> ;
  skos:inScheme <http://vocab.nerc.ac.uk/scheme/SDNDEV/current> ;
  skos:narrower inst:TOOL0563 ;
  skos:narrower inst:TOOL0571 ;
  skos:narrower inst:TOOL0573 ;
  skos:narrower inst:TOOL0843 ;
  skos:narrower inst:TOOL1012 ;
  skos:narrower <http://vocab.nerc.ac.uk/collection/W01/current/003> ;
  skos:notation "SDN:L05::58" ;
  skos:note "accepted"@en ;
  skos:prefLabel "continuous air samplers"@en ;
.
<http://vocab.nerc.ac.uk/collection/L05/current/59>
  rdf:type skos:Concept ;
  dcterm:date "2014-06-05 09:44:31.0" ;
  dcterm:identifier "SDN:L05::59" ;
  pav:authoredOn "2014-06-05 09:44:31.0" ;
  pav:hasCurrentVersion <http://vocab.nerc.ac.uk/collection/L05/current/59/2> ;
  pav:hasVersion <http://vocab.nerc.ac.uk/collection/L05/current/59/1> ;
  owl:versionInfo "2" ;
  skos:broader sdnc:ICAT01 ;
  skos:definition "Devices that label the region within which sampling is to be confined such as permanent quadrats and location markers."@en ;
  skos:inScheme <http://vocab.nerc.ac.uk/scheme/EDMED_DCAT_THEMES/current> ;
  skos:inScheme <http://vocab.nerc.ac.uk/scheme/SDNDEV/current> ;
  skos:narrower inst:TOOL0817 ;
  skos:narrower inst:TOOL0818 ;
  skos:narrower inst:TOOL0819 ;
  skos:narrower <http://vocab.nerc.ac.uk/collection/W01/current/003> ;
  skos:notation "SDN:L05::59" ;
  skos:note "accepted"@en ;
  skos:prefLabel "sampling extent markers"@en ;
.
<http://vocab.nerc.ac.uk/collection/L05/current/60>
  rdf:type skos:Concept ;
  dcterm:date "2010-07-20 08:06:54.0" ;
  dcterm:identifier "SDN:L05::60" ;
  pav:authoredOn "2010-07-20 08:06:54.0" ;
  pav:hasCurrentVersion <http://vocab.nerc.ac.uk/collection/L05/current/60/1> ;
  owl:versionInfo "1" ;
  skos:broader sdnd:G01 ;
  skos:broader sdnc:ICAT01 ;
  skos:definition "Bucket-like containers hauled over the sea bed collecting integrated samples of surface sediment along a segment of ship track."@en ;
  skos:inScheme <http://vocab.nerc.ac.uk/scheme/EDMED_DCAT_THEMES/current> ;
  skos:inScheme <http://vocab.nerc.ac.uk/scheme/SDNDEV/current> ;
  skos:narrower inst:NETT0190 ;
  skos:narrower inst:TOOL1373 ;
  skos:narrower inst:TOOL1853 ;
  skos:narrower inst:TOOL1854 ;
  skos:narrower <http://vocab.nerc.ac.uk/collection/W01/current/003> ;
  skos:notation "SDN:L05::60" ;
  skos:note "accepted"@en ;
  skos:prefLabel "sediment dredges"@en ;
.
<http://vocab.nerc.ac.uk/collection/L05/current/61>
  rdf:type skos:Concept ;
  dcterm:date "2010-07-30 10:16:21.0" ;
  dcterm:identifier "SDN:L05::61" ;
  pav:authoredOn "2010-07-30 10:16:21.0" ;
  pav:hasCurrentVersion <http://vocab.nerc.ac.uk/collection/L05/current/61/1> ;
  owl:versionInfo "1" ;
  skos:broader <http://vocab.nerc.ac.uk/collection/L05/current/24> ;
  skos:broader <http://vocab.nerc.ac.uk/collection/L05/current/64> ;
  skos:broader sdnc:ICAT01 ;
  skos:definition "Nets towed over the sea floor designed to sample species living on or near the bottom."@en ;
  skos:inScheme <http://vocab.nerc.ac.uk/scheme/EDMED_DCAT_THEMES/current> ;
  skos:inScheme <http://vocab.nerc.ac.uk/scheme/SDNDEV/current> ;
  skos:narrower inst:NETT0039 ;
  skos:narrower inst:NETT0183 ;
  skos:narrower inst:NETT0193 ;
  skos:narrower inst:NETT0194 ;
  skos:narrower inst:NETT0195 ;
  skos:narrower inst:NETT0196 ;
  skos:narrower inst:NETT0197 ;
  skos:narrower inst:NETT0198 ;
  skos:narrower inst:TOOL0991 ;
  skos:narrower inst:TOOL1252 ;
  skos:narrower <http://vocab.nerc.ac.uk/collection/W01/current/003> ;
  skos:notation "SDN:L05::61" ;
  skos:note "accepted"@en ;
  skos:prefLabel "demersal trawl nets"@en ;
.
<http://vocab.nerc.ac.uk/collection/L05/current/62>
  rdf:type skos:Concept ;
  dcterm:date "2010-07-30 10:19:35.0" ;
  dcterm:identifier "SDN:L05::62" ;
  pav:authoredOn "2010-07-30 10:19:35.0" ;
  pav:hasCurrentVersion <http://vocab.nerc.ac.uk/collection/L05/current/62/1> ;
  owl:versionInfo "1" ;
  skos:broader <http://vocab.nerc.ac.uk/collection/L05/current/24> ;
  skos:broader <http://vocab.nerc.ac.uk/collection/L05/current/64> ;
  skos:broader sdnc:ICAT01 ;
  skos:definition "Nets towed over the sea floor having the horizontal net opening provided by a wooden or metal beam that disrupts the surface of the bed."@en ;
  skos:inScheme <http://vocab.nerc.ac.uk/scheme/EDMED_DCAT_THEMES/current> ;
  skos:inScheme <http://vocab.nerc.ac.uk/scheme/SDNDEV/current> ;
  skos:narrower inst:TOOL0651 ;
  skos:narrower inst:TOOL0652 ;
  skos:narrower <http://vocab.nerc.ac.uk/collection/W01/current/003> ;
  skos:notation "SDN:L05::62" ;
  skos:note "accepted"@en ;
  skos:prefLabel "beam trawls"@en ;
.
<http://vocab.nerc.ac.uk/collection/L05/current/63>
  rdf:type skos:Concept ;
  dcterm:date "2010-07-30 10:22:48.0" ;
  dcterm:identifier "SDN:L05::63" ;
  pav:authoredOn "2010-07-30 10:22:48.0" ;
  pav:hasCurrentVersion <http://vocab.nerc.ac.uk/collection/L05/current/63/1> ;
  owl:versionInfo "1" ;
  skos:broader sdnc:ICAT01 ;
  skos:definition "Apparatus where capture is based on the movement of the target species towards the gear (e.g. creels and fish traps)."@en ;
  skos:inScheme <http://vocab.nerc.ac.uk/scheme/EDMED_DCAT_THEMES/current> ;
  skos:inScheme <http://vocab.nerc.ac.uk/scheme/SDNDEV/current> ;
  skos:narrower <http://vocab.nerc.ac.uk/collection/L05/current/65> ;
  skos:narrower <http://vocab.nerc.ac.uk/collection/L05/current/70> ;
  skos:narrower inst:TOOL1574 ;
  skos:narrower inst:TOOL1575 ;
  skos:narrower <http://vocab.nerc.ac.uk/collection/W01/current/003> ;
  skos:notation "SDN:L05::63" ;
  skos:note "accepted"@en ;
  skos:prefLabel "passive fishing gear"@en ;
.
<http://vocab.nerc.ac.uk/collection/L05/current/64>
  rdf:type skos:Concept ;
  dcterm:date "2010-07-30 10:24:37.0" ;
  dcterm:identifier "SDN:L05::64" ;
  pav:authoredOn "2010-07-30 10:24:37.0" ;
  pav:hasCurrentVersion <http://vocab.nerc.ac.uk/collection/L05/current/64/1> ;
  owl:versionInfo "1" ;
  skos:broader sdnc:ICAT01 ;
  skos:definition "Apparatus where capture is based on chasing the target species (e.g. a trawl)."@en ;
  skos:inScheme <http://vocab.nerc.ac.uk/scheme/EDMED_DCAT_THEMES/current> ;
  skos:inScheme <http://vocab.nerc.ac.uk/scheme/SDNDEV/current> ;
  skos:narrower <http://vocab.nerc.ac.uk/collection/L05/current/23> ;
  skos:narrower <http://vocab.nerc.ac.uk/collection/L05/current/24> ;
  skos:narrower <http://vocab.nerc.ac.uk/collection/L05/current/61> ;
  skos:narrower <http://vocab.nerc.ac.uk/collection/L05/current/62> ;
  skos:narrower <http://vocab.nerc.ac.uk/collection/L05/current/71> ;
  skos:narrower <http://vocab.nerc.ac.uk/collection/L05/current/72> ;
  skos:narrower <http://vocab.nerc.ac.uk/collection/W01/current/003> ;
  skos:notation "SDN:L05::64" ;
  skos:note "accepted"@en ;
  skos:prefLabel "active fishing gear"@en ;
.
<http://vocab.nerc.ac.uk/collection/L05/current/65>
  rdf:type skos:Concept ;
  dcterm:date "2011-08-26 14:52:51.0" ;
  dcterm:identifier "SDN:L05::65" ;
  pav:authoredOn "2011-08-26 14:52:51.0" ;
  pav:hasCurrentVersion <http://vocab.nerc.ac.uk/collection/L05/current/65/1> ;
  owl:versionInfo "1" ;
  skos:broader <http://vocab.nerc.ac.uk/collection/L05/current/63> ;
  skos:broader sdnc:ICAT01 ;
  skos:definition "Nets drifting in the sea or standing on the sea floor in which fish become entangled, usually through their gill covers."@en ;
  skos:inScheme <http://vocab.nerc.ac.uk/scheme/EDMED_DCAT_THEMES/current> ;
  skos:inScheme <http://vocab.nerc.ac.uk/scheme/SDNDEV/current> ;
  skos:narrower inst:TOOL1259 ;
  skos:narrower <http://vocab.nerc.ac.uk/collection/W01/current/003> ;
  skos:notation "SDN:L05::65" ;
  skos:note "accepted"@en ;
  skos:prefLabel "gill nets"@en ;
.
<http://vocab.nerc.ac.uk/collection/L05/current/66>
  rdf:type skos:Concept ;
  dcterm:date "2011-08-26 14:59:54.0" ;
  dcterm:identifier "SDN:L05::66" ;
  pav:authoredOn "2011-08-26 14:59:54.0" ;
  pav:hasCurrentVersion <http://vocab.nerc.ac.uk/collection/L05/current/66/1> ;
  owl:versionInfo "1" ;
  skos:broader sdnc:ICAT01 ;
  skos:definition "Devices primarily designed to drill wells through sediment or rock that flush the drill spoil back to the surface where it is examined to provide lithological data through the process known as mud logging."@en ;
  skos:inScheme <http://vocab.nerc.ac.uk/scheme/SDNDEV/current> ;
  skos:narrower <http://vocab.nerc.ac.uk/collection/W01/current/003> ;
  skos:notation "SDN:L05::66" ;
  skos:note "accepted"@en ;
  skos:prefLabel "flushing drills"@en ;
.
<http://vocab.nerc.ac.uk/collection/L05/current/67>
  rdf:type skos:Concept ;
  dcterm:date "2011-11-25 11:45:36.0" ;
  dcterm:identifier "SDN:L05::67" ;
  pav:authoredOn "2011-11-25 11:45:36.0" ;
  pav:hasCurrentVersion <http://vocab.nerc.ac.uk/collection/L05/current/67/1> ;
  owl:versionInfo "1" ;
  skos:altLabel "HSS"@en ;
  skos:broader sdnc:ICAT01 ;
  skos:definition "A fine-meshed net or filter towed behind a moving vessel that collects a single sample for a tow. Samples microzooplankton, mesozooplankton and nekton."@en ;
  skos:inScheme <http://vocab.nerc.ac.uk/scheme/SDNDEV/current> ;
  skos:narrower inst:NETT0002 ;
  skos:narrower inst:NETT0005 ;
  skos:narrower inst:NETT0020 ;
  skos:narrower inst:NETT0052 ;
  skos:narrower inst:NETT0053 ;
  skos:narrower inst:NETT0055 ;
  skos:narrower inst:NETT0056 ;
  skos:narrower inst:NETT0057 ;
  skos:narrower inst:NETT0058 ;
  skos:narrower inst:NETT0059 ;
  skos:narrower inst:NETT0060 ;
  skos:narrower inst:NETT0061 ;
  skos:narrower inst:NETT0062 ;
  skos:narrower inst:NETT0063 ;
  skos:narrower inst:NETT0065 ;
  skos:narrower inst:NETT0066 ;
  skos:narrower inst:NETT0067 ;
  skos:narrower inst:NETT0068 ;
  skos:narrower inst:NETT0109 ;
  skos:narrower inst:NETT0125 ;
  skos:narrower inst:NETT0139 ;
  skos:narrower inst:NETT0154 ;
  skos:narrower inst:NETT0165 ;
  skos:narrower <http://vocab.nerc.ac.uk/collection/W01/current/003> ;
  skos:notation "SDN:L05::67" ;
  skos:note "accepted"@en ;
  skos:prefLabel "high-speed plankton samplers"@en ;
.
<http://vocab.nerc.ac.uk/collection/L05/current/68>
  rdf:type skos:Concept ;
  dcterm:date "2011-11-25 11:47:24.0" ;
  dcterm:identifier "SDN:L05::68" ;
  pav:authoredOn "2011-11-25 11:47:24.0" ;
  pav:hasCurrentVersion <http://vocab.nerc.ac.uk/collection/L05/current/68/1> ;
  owl:versionInfo "1" ;
  skos:broader sdnc:ICAT01 ;
  skos:definition "A system comprising several nets that can be opened and closed sequentially to collect a series of samples during a tow or haul. Samples microzooplankton, mesozooplankton and nekton."@en ;
  skos:inScheme <http://vocab.nerc.ac.uk/scheme/SDNDEV/current> ;
  skos:narrower inst:NETT0005 ;
  skos:narrower inst:NETT0030 ;
  skos:narrower inst:NETT0072 ;
  skos:narrower inst:NETT0073 ;
  skos:narrower inst:NETT0098 ;
  skos:narrower inst:NETT0134 ;
  skos:narrower inst:NETT0166 ;
  skos:narrower inst:NETT0179 ;
  skos:narrower inst:TOOL0985 ;
  skos:narrower inst:TOOL1274 ;
  skos:narrower <http://vocab.nerc.ac.uk/collection/W01/current/003> ;
  skos:notation "SDN:L05::68" ;
  skos:note "accepted"@en ;
  skos:prefLabel "multinet"@en ;
.
<http://vocab.nerc.ac.uk/collection/L05/current/69>
  rdf:type skos:Concept ;
  dcterm:date "2018-02-20 17:43:58.0" ;
  dcterm:identifier "SDN:L05::69" ;
  pav:authoredOn "2018-02-20 17:43:58.0" ;
  pav:hasCurrentVersion <http://vocab.nerc.ac.uk/collection/L05/current/69/2> ;
  pav:hasVersion <http://vocab.nerc.ac.uk/collection/L05/current/69/1> ;
  owl:versionInfo "2" ;
  skos:broader sdnc:ICAT01 ;
  skos:definition "A fine-meshed net designed to collect small size organisms, aggregates, or litter on top of or close to the surface of a water column (top 10 to 50 centimetres) including for example microzooplankton, mesozooplankton, nekton, microplastic or other litter."@en ;
  skos:inScheme <http://vocab.nerc.ac.uk/scheme/SDNDEV/current> ;
  skos:narrower inst:NETT0012 ;
  skos:narrower inst:NETT0027 ;
  skos:narrower inst:NETT0096 ;
  skos:narrower inst:NETT0111 ;
  skos:narrower inst:NETT0112 ;
  skos:narrower inst:NETT0113 ;
  skos:narrower inst:NETT0114 ;
  skos:narrower inst:NETT0115 ;
  skos:narrower inst:NETT0116 ;
  skos:narrower inst:NETT0118 ;
  skos:narrower inst:NETT0145 ;
  skos:narrower inst:NETT0177 ;
  skos:narrower inst:NETT0188 ;
  skos:narrower <http://vocab.nerc.ac.uk/collection/W01/current/003> ;
  skos:notation "SDN:L05::69" ;
  skos:note "accepted"@en ;
  skos:prefLabel "neuston net"@en ;
.
<http://vocab.nerc.ac.uk/collection/L05/current/70>
  rdf:type skos:Concept ;
  dcterm:date "2019-09-04 10:01:22.0" ;
  dcterm:identifier "SDN:L05::70" ;
  pav:authoredOn "2019-09-04 10:01:22.0" ;
  pav:hasCurrentVersion <http://vocab.nerc.ac.uk/collection/L05/current/70/3> ;
  pav:hasVersion <http://vocab.nerc.ac.uk/collection/L05/current/70/1> ;
  pav:hasVersion <http://vocab.nerc.ac.uk/collection/L05/current/70/2> ;
  owl:versionInfo "3" ;
  skos:altLabel "FAD"@en ;
  skos:broader <http://vocab.nerc.ac.uk/collection/L05/current/63> ;
  skos:broader sdnc:ICAT01 ;
  skos:definition "Any kind of permanent, semi-permanent or temporary structure designed to attract fishes (specially tunas) and used in ocean purse seine fisheries. FADs can be moored or drifting devices and consist of surface or sub-surface buoys or floats to which underwater ropes, lines or chains can be attached. The most sophisticated type can be equipped with an echo sounder to estimate the biomass under it, a GPS to locate the device, and either a VHF, Immarsat or Iridium connection to periodically send the information to the vessel which owns it."@en ;
  skos:inScheme <http://vocab.nerc.ac.uk/scheme/SDNDEV/current> ;
  skos:notation "SDN:L05::70" ;
  skos:note "accepted"@en ;
  skos:prefLabel "fish aggregating devices"@en ;
.
<http://vocab.nerc.ac.uk/collection/L05/current/71>
  rdf:type skos:Concept ;
  <http://purl.org/dc/terms/:isReplacedBy> <http://vocab.nerc.ac.uk/collection/L05/current/24> ;
  dcterm:date "2019-12-19 17:12:49.0" ;
  dcterm:identifier "SDN:L05::71" ;
  pav:authoredOn "2019-12-19 17:12:49.0" ;
  pav:hasCurrentVersion <http://vocab.nerc.ac.uk/collection/L05/current/71/3> ;
  pav:hasVersion <http://vocab.nerc.ac.uk/collection/L05/current/71/1> ;
  pav:hasVersion <http://vocab.nerc.ac.uk/collection/L05/current/71/2> ;
  owl:deprecated "true" ;
  owl:versionInfo "3" ;
  skos:broader <http://vocab.nerc.ac.uk/collection/L05/current/64> ;
  skos:broader sdnc:ICAT01 ;
  skos:definition "Code deprecated on 20Dec2019: created in error. Description was: Rigid structures with a chain mail collecting bag, towed on the seabed to target king scallops. Generally used by towing several dredges side by side behind the vessel (source: seafish.org)."@en ;
  skos:inScheme <http://vocab.nerc.ac.uk/scheme/SDNDEV/current> ;
  skos:notation "SDN:L05::71" ;
  skos:note "deprecated"@en ;
  skos:prefLabel "scallop dredges"@en ;
.
<http://vocab.nerc.ac.uk/collection/L05/current/72>
  rdf:type skos:Concept ;
  <http://purl.org/dc/terms/:isReplacedBy> <http://vocab.nerc.ac.uk/collection/L05/current/24> ;
  dcterm:date "2019-12-19 17:24:19.0" ;
  dcterm:identifier "SDN:L05::72" ;
  pav:authoredOn "2019-12-19 17:24:19.0" ;
  pav:hasCurrentVersion <http://vocab.nerc.ac.uk/collection/L05/current/72/3> ;
  pav:hasVersion <http://vocab.nerc.ac.uk/collection/L05/current/72/1> ;
  pav:hasVersion <http://vocab.nerc.ac.uk/collection/L05/current/72/2> ;
  owl:deprecated "true" ;
  owl:versionInfo "3" ;
  skos:broader <http://vocab.nerc.ac.uk/collection/L05/current/64> ;
  skos:broader sdnc:ICAT01 ;
  skos:definition "Code deprecated on 20Dec2019: created in error. Description was: The dredges used to target queen scallops are wider and higher than a traditional scallop dredge. They do not have tooth bar across the front, instead they have either a metal grid, or tickler chains to get the scallops to lift up off the seabed and swim into the dredge. The scallops then fall back into a bag made of metal rings. Some fishermen are replacing the tickler chain and metal grid with a strip of rubber matting across the front of the dredge (source seafish.org)."@en ;
  skos:inScheme <http://vocab.nerc.ac.uk/scheme/SDNDEV/current> ;
  skos:notation "SDN:L05::72" ;
  skos:note "deprecated"@en ;
  skos:prefLabel "queen scallop dredges"@en ;
.
<http://vocab.nerc.ac.uk/collection/L05/current/90>
  rdf:type skos:Concept ;
  dcterm:date "2013-02-26 17:11:07.0" ;
  dcterm:identifier "SDN:L05::90" ;
  pav:authoredOn "2013-02-26 17:11:07.0" ;
  pav:hasCurrentVersion <http://vocab.nerc.ac.uk/collection/L05/current/90/2> ;
  pav:hasVersion <http://vocab.nerc.ac.uk/collection/L05/current/90/1> ;
  owl:versionInfo "2" ;
  skos:broader sdnc:ICAT01 ;
  skos:definition "A simple tool like a hammer, saw or even just a hand for the collection of biota samples."@en ;
  skos:inScheme <http://vocab.nerc.ac.uk/scheme/EDMED_DCAT_THEMES/current> ;
  skos:inScheme <http://vocab.nerc.ac.uk/scheme/SDNDEV/current> ;
  skos:narrower <http://vocab.nerc.ac.uk/collection/W01/current/003> ;
  skos:notation "SDN:L05::90" ;
  skos:note "accepted"@en ;
  skos:prefLabel "manual biota samplers"@en ;
.
<http://vocab.nerc.ac.uk/collection/L05/current/999>
  rdf:type skos:Concept ;
  dcterm:date "2007-11-20 08:50:03.0" ;
  dcterm:identifier "SDN:L05::999" ;
  pav:authoredOn "2007-11-20 08:50:03.0" ;
  pav:hasCurrentVersion <http://vocab.nerc.ac.uk/collection/L05/current/999/1> ;
  owl:versionInfo "1" ;
  skos:broader sdnc:ICAT01 ;
  skos:definition "The correct value is not known to and not computable by the creator of this information. However a correct value probably exists."@en ;
  skos:inScheme <http://vocab.nerc.ac.uk/scheme/EDMED_DCAT_THEMES/current> ;
  skos:inScheme <http://vocab.nerc.ac.uk/scheme/SDNDEV/current> ;
  skos:narrower inst:TOOLZZZ ;
  skos:narrower <http://vocab.nerc.ac.uk/collection/W01/current/003> ;
  skos:notation "SDN:L05::999" ;
  skos:note "accepted"@en ;
  skos:prefLabel "unknown"@en ;
.
sdev:TFSAMP
  rdf:type skos:Concept ;
  dcterm:date "2013-04-23 12:55:37.0" ;
  dcterm:identifier "SDN:L05::TFSAMP" ;
  pav:authoredOn "2013-04-23 12:55:37.0" ;
  pav:hasCurrentVersion <http://vocab.nerc.ac.uk/collection/L05/current/TFSAMP/1> ;
  owl:versionInfo "1" ;
  skos:broader sdnc:ICAT01 ;
  skos:definition "Metal samplers comprising a filter, a diffusive gel layer and a resin layer that scavenge trace metals by diffusion from water bodies or in-situ sediment pore waters. A constant concentration gradient is set up in the gel from which the metal concentration in the sampled medium may be determined."@en ;
  skos:inScheme <http://vocab.nerc.ac.uk/scheme/SDNDEV/current> ;
  skos:narrower inst:TOOL0553 ;
  skos:narrower <http://vocab.nerc.ac.uk/collection/W01/current/003> ;
  skos:notation "SDN:L05::TFSAMP" ;
  skos:note "accepted"@en ;
  skos:prefLabel "thin film metal samplers"@en ;
.
sdnk:SDNKG17
  rdf:type skos:Collection ;
  dcterm:date "2021-07-07 10:53:52.0" ;
  dcterm:identifier "SDN:L19::SDNKG17" ;
  pav:authoredOn "2021-07-07 10:53:52.0" ;
  pav:hasCurrentVersion <http://vocab.nerc.ac.uk/collection/L19/current/SDNKG17/1> ;
  pav:version "1" ;
  owl:versionInfo "1" ;
  skos:altLabel "sensor_model"@en ;
  skos:definition "Keyword identifies a sensor model"@en ;
  skos:member inst:NETT0001 ;
  skos:member inst:NETT0002 ;
  skos:member inst:NETT0003 ;
  skos:member inst:NETT0005 ;
  skos:member inst:NETT0006 ;
  skos:member inst:NETT0009 ;
  skos:member inst:NETT0010 ;
  skos:member inst:NETT0012 ;
  skos:member inst:NETT0016 ;
  skos:member inst:NETT0019 ;
  skos:member inst:NETT0020 ;
  skos:member inst:NETT0022 ;
  skos:member inst:NETT0023 ;
  skos:member inst:NETT0024 ;
  skos:member inst:NETT0026 ;
  skos:member inst:NETT0027 ;
  skos:member inst:NETT0030 ;
  skos:member inst:NETT0031 ;
  skos:member inst:NETT0032 ;
  skos:member inst:NETT0034 ;
  skos:member inst:NETT0035 ;
  skos:member inst:NETT0036 ;
  skos:member inst:NETT0039 ;
  skos:member inst:NETT0040 ;
  skos:member inst:NETT0041 ;
  skos:member inst:NETT0042 ;
  skos:member inst:NETT0043 ;
  skos:member inst:NETT0044 ;
  skos:member inst:NETT0045 ;
  skos:member inst:NETT0047 ;
  skos:member inst:NETT0052 ;
  skos:member inst:NETT0053 ;
  skos:member inst:NETT0054 ;
  skos:member inst:NETT0055 ;
  skos:member inst:NETT0056 ;
  skos:member inst:NETT0057 ;
  skos:member inst:NETT0058 ;
  skos:member inst:NETT0059 ;
  skos:member inst:NETT0060 ;
  skos:member inst:NETT0061 ;
  skos:member inst:NETT0062 ;
  skos:member inst:NETT0063 ;
  skos:member inst:NETT0065 ;
  skos:member inst:NETT0066 ;
  skos:member inst:NETT0067 ;
  skos:member inst:NETT0068 ;
  skos:member inst:NETT0071 ;
  skos:member inst:NETT0072 ;
  skos:member inst:NETT0073 ;
  skos:member inst:NETT0074 ;
  skos:member inst:NETT0075 ;
  skos:member inst:NETT0077 ;
  skos:member inst:NETT0078 ;
  skos:member inst:NETT0079 ;
  skos:member inst:NETT0080 ;
  skos:member inst:NETT0090 ;
  skos:member inst:NETT0091 ;
  skos:member inst:NETT0092 ;
  skos:member inst:NETT0095 ;
  skos:member inst:NETT0096 ;
  skos:member inst:NETT0098 ;
  skos:member inst:NETT0100 ;
  skos:member inst:NETT0102 ;
  skos:member inst:NETT0103 ;
  skos:member inst:NETT0104 ;
  skos:member inst:NETT0105 ;
  skos:member inst:NETT0106 ;
  skos:member inst:NETT0108 ;
  skos:member inst:NETT0109 ;
  skos:member inst:NETT0111 ;
  skos:member inst:NETT0112 ;
  skos:member inst:NETT0113 ;
  skos:member inst:NETT0114 ;
  skos:member inst:NETT0115 ;
  skos:member inst:NETT0116 ;
  skos:member inst:NETT0118 ;
  skos:member inst:NETT0122 ;
  skos:member inst:NETT0124 ;
  skos:member inst:NETT0125 ;
  skos:member inst:NETT0126 ;
  skos:member inst:NETT0127 ;
  skos:member inst:NETT0128 ;
  skos:member inst:NETT0129 ;
  skos:member inst:NETT0131 ;
  skos:member inst:NETT0132 ;
  skos:member inst:NETT0133 ;
  skos:member inst:NETT0134 ;
  skos:member inst:NETT0135 ;
  skos:member inst:NETT0136 ;
  skos:member inst:NETT0137 ;
  skos:member inst:NETT0138 ;
  skos:member inst:NETT0139 ;
  skos:member inst:NETT0140 ;
  skos:member inst:NETT0141 ;
  skos:member inst:NETT0142 ;
  skos:member inst:NETT0143 ;
  skos:member inst:NETT0144 ;
  skos:member inst:NETT0145 ;
  skos:member inst:NETT0147 ;
  skos:member inst:NETT0150 ;
  skos:member inst:NETT0151 ;
  skos:member inst:NETT0153 ;
  skos:member inst:NETT0154 ;
  skos:member inst:NETT0155 ;
  skos:member inst:NETT0161 ;
  skos:member inst:NETT0162 ;
  skos:member inst:NETT0163 ;
  skos:member inst:NETT0164 ;
  skos:member inst:NETT0165 ;
  skos:member inst:NETT0166 ;
  skos:member inst:NETT0167 ;
  skos:member inst:NETT0169 ;
  skos:member inst:NETT0171 ;
  skos:member inst:NETT0173 ;
  skos:member inst:NETT0174 ;
  skos:member inst:NETT0175 ;
  skos:member inst:NETT0176 ;
  skos:member inst:NETT0177 ;
  skos:member inst:NETT0178 ;
  skos:member inst:NETT0179 ;
  skos:member inst:NETT0180 ;
  skos:member inst:NETT0181 ;
  skos:member inst:NETT0182 ;
  skos:member inst:NETT0183 ;
  skos:member inst:NETT0184 ;
  skos:member inst:NETT0186 ;
  skos:member inst:NETT0188 ;
  skos:member inst:NETT0189 ;
  skos:member inst:NETT0190 ;
  skos:member inst:NETT0191 ;
  skos:member inst:NETT0192 ;
  skos:member inst:NETT0193 ;
  skos:member inst:NETT0194 ;
  skos:member inst:NETT0195 ;
  skos:member inst:NETT0196 ;
  skos:member inst:NETT0197 ;
  skos:member inst:NETT0198 ;
  skos:member inst:TOOL000X ;
  skos:member inst:TOOL0235 ;
  skos:member inst:TOOL0236 ;
  skos:member inst:TOOL0248 ;
  skos:member inst:TOOL0353 ;
  skos:member inst:TOOL0354 ;
  skos:member inst:TOOL0355 ;
  skos:member inst:TOOL0356 ;
  skos:member inst:TOOL0357 ;
  skos:member inst:TOOL0358 ;
  skos:member inst:TOOL0381 ;
  skos:member inst:TOOL0412 ;
  skos:member inst:TOOL0413 ;
  skos:member inst:TOOL0418 ;
  skos:member inst:TOOL0427 ;
  skos:member inst:TOOL0472 ;
  skos:member inst:TOOL0501 ;
  skos:member inst:TOOL0502 ;
  skos:member inst:TOOL0503 ;
  skos:member inst:TOOL0504 ;
  skos:member inst:TOOL0505 ;
  skos:member inst:TOOL0506 ;
  skos:member inst:TOOL0508 ;
  skos:member inst:TOOL0535 ;
  skos:member inst:TOOL0536 ;
  skos:member inst:TOOL0537 ;
  skos:member inst:TOOL0538 ;
  skos:member inst:TOOL0539 ;
  skos:member inst:TOOL0540 ;
  skos:member inst:TOOL0541 ;
  skos:member inst:TOOL0542 ;
  skos:member inst:TOOL0543 ;
  skos:member inst:TOOL0544 ;
  skos:member inst:TOOL0545 ;
  skos:member inst:TOOL0546 ;
  skos:member inst:TOOL0547 ;
  skos:member inst:TOOL0548 ;
  skos:member inst:TOOL0550 ;
  skos:member inst:TOOL0551 ;
  skos:member inst:TOOL0552 ;
  skos:member inst:TOOL0553 ;
  skos:member inst:TOOL0554 ;
  skos:member inst:TOOL0555 ;
  skos:member inst:TOOL0556 ;
  skos:member inst:TOOL0557 ;
  skos:member inst:TOOL0561 ;
  skos:member inst:TOOL0562 ;
  skos:member inst:TOOL0563 ;
  skos:member inst:TOOL0571 ;
  skos:member inst:TOOL0573 ;
  skos:member inst:TOOL0588 ;
  skos:member inst:TOOL0651 ;
  skos:member inst:TOOL0652 ;
  skos:member inst:TOOL0653 ;
  skos:member inst:TOOL0660 ;
  skos:member inst:TOOL0784 ;
  skos:member inst:TOOL0785 ;
  skos:member inst:TOOL0786 ;
  skos:member inst:TOOL0787 ;
  skos:member inst:TOOL0788 ;
  skos:member inst:TOOL0806 ;
  skos:member inst:TOOL0807 ;
  skos:member inst:TOOL0817 ;
  skos:member inst:TOOL0818 ;
  skos:member inst:TOOL0819 ;
  skos:member inst:TOOL0828 ;
  skos:member inst:TOOL0843 ;
  skos:member inst:TOOL0917 ;
  skos:member inst:TOOL0939 ;
  skos:member inst:TOOL0940 ;
  skos:member inst:TOOL0960 ;
  skos:member inst:TOOL0961 ;
  skos:member inst:TOOL0962 ;
  skos:member inst:TOOL0963 ;
  skos:member inst:TOOL0978 ;
  skos:member inst:TOOL0979 ;
  skos:member inst:TOOL0980 ;
  skos:member inst:TOOL0981 ;
  skos:member inst:TOOL0982 ;
  skos:member inst:TOOL0983 ;
  skos:member inst:TOOL0984 ;
  skos:member inst:TOOL0985 ;
  skos:member inst:TOOL0986 ;
  skos:member inst:TOOL0987 ;
  skos:member inst:TOOL0988 ;
  skos:member inst:TOOL0989 ;
  skos:member inst:TOOL0990 ;
  skos:member inst:TOOL0991 ;
  skos:member inst:TOOL0992 ;
  skos:member inst:TOOL0993 ;
  skos:member inst:TOOL0994 ;
  skos:member inst:TOOL0995 ;
  skos:member inst:TOOL0996 ;
  skos:member inst:TOOL0997 ;
  skos:member inst:TOOL1012 ;
  skos:member inst:TOOL1135 ;
  skos:member inst:TOOL1165 ;
  skos:member inst:TOOL1166 ;
  skos:member inst:TOOL1169 ;
  skos:member inst:TOOL1170 ;
  skos:member inst:TOOL1171 ;
  skos:member inst:TOOL1172 ;
  skos:member inst:TOOL1173 ;
  skos:member inst:TOOL1174 ;
  skos:member inst:TOOL1175 ;
  skos:member inst:TOOL1176 ;
  skos:member inst:TOOL1177 ;
  skos:member inst:TOOL1178 ;
  skos:member inst:TOOL1179 ;
  skos:member inst:TOOL1181 ;
  skos:member inst:TOOL1191 ;
  skos:member inst:TOOL1199 ;
  skos:member inst:TOOL1204 ;
  skos:member inst:TOOL1214 ;
  skos:member inst:TOOL1215 ;
  skos:member inst:TOOL1216 ;
  skos:member inst:TOOL1235 ;
  skos:member inst:TOOL1249 ;
  skos:member inst:TOOL1252 ;
  skos:member inst:TOOL1253 ;
  skos:member inst:TOOL1259 ;
  skos:member inst:TOOL1260 ;
  skos:member inst:TOOL1261 ;
  skos:member inst:TOOL1272 ;
  skos:member inst:TOOL1274 ;
  skos:member inst:TOOL1285 ;
  skos:member inst:TOOL1304 ;
  skos:member inst:TOOL1326 ;
  skos:member inst:TOOL1339 ;
  skos:member inst:TOOL1371 ;
  skos:member inst:TOOL1372 ;
  skos:member inst:TOOL1373 ;
  skos:member inst:TOOL1374 ;
  skos:member inst:TOOL1375 ;
  skos:member inst:TOOL1376 ;
  skos:member inst:TOOL1378 ;
  skos:member inst:TOOL1379 ;
  skos:member inst:TOOL1405 ;
  skos:member inst:TOOL1413 ;
  skos:member inst:TOOL1414 ;
  skos:member inst:TOOL1415 ;
  skos:member inst:TOOL1416 ;
  skos:member inst:TOOL1417 ;
  skos:member inst:TOOL1454 ;
  skos:member inst:TOOL1455 ;
  skos:member inst:TOOL1462 ;
  skos:member inst:TOOL1463 ;
  skos:member inst:TOOL1464 ;
  skos:member inst:TOOL1465 ;
  skos:member inst:TOOL1466 ;
  skos:member inst:TOOL1467 ;
  skos:member inst:TOOL1468 ;
  skos:member inst:TOOL1469 ;
  skos:member inst:TOOL1477 ;
  skos:member inst:TOOL1478 ;
  skos:member inst:TOOL1480 ;
  skos:member inst:TOOL1485 ;
  skos:member inst:TOOL1486 ;
  skos:member inst:TOOL1487 ;
  skos:member inst:TOOL1527 ;
  skos:member inst:TOOL1533 ;
  skos:member inst:TOOL1535 ;
  skos:member inst:TOOL1536 ;
  skos:member inst:TOOL1537 ;
  skos:member inst:TOOL1560 ;
  skos:member inst:TOOL1574 ;
  skos:member inst:TOOL1575 ;
  skos:member inst:TOOL1576 ;
  skos:member inst:TOOL1644 ;
  skos:member inst:TOOL1654 ;
  skos:member inst:TOOL1668 ;
  skos:member inst:TOOL1703 ;
  skos:member inst:TOOLZZZ ;
  skos:notation "SDN:L19::SDNKG17" ;
  skos:note "accepted"@en ;
  skos:prefLabel "sensor_model"@en ;
.
sdnc:ICAT01
  rdf:type skos:Concept ;
  dcterm:date "2008-01-10 13:02:59.0" ;
  dcterm:identifier "SDN:L21::ICAT01" ;
  pav:authoredOn "2008-01-10 13:02:59.0" ;
  pav:hasCurrentVersion <http://vocab.nerc.ac.uk/collection/L21/current/ICAT01/1> ;
  owl:versionInfo "1" ;
  skos:altLabel "SeaDataNet sample collector categories"@en ;
  skos:altLabel "sample collectors"@en ;
  skos:definition "Categories used in the SeaDataNet project to classify devices that collect any type of physical sample."@en ;
  skos:narrower <http://vocab.nerc.ac.uk/collection/L05/current/11> ;
  skos:narrower <http://vocab.nerc.ac.uk/collection/L05/current/12> ;
  skos:narrower <http://vocab.nerc.ac.uk/collection/L05/current/13> ;
  skos:narrower <http://vocab.nerc.ac.uk/collection/L05/current/14> ;
  skos:narrower <http://vocab.nerc.ac.uk/collection/L05/current/182> ;
  skos:narrower <http://vocab.nerc.ac.uk/collection/L05/current/21> ;
  skos:narrower <http://vocab.nerc.ac.uk/collection/L05/current/22> ;
  skos:narrower <http://vocab.nerc.ac.uk/collection/L05/current/23> ;
  skos:narrower <http://vocab.nerc.ac.uk/collection/L05/current/24> ;
  skos:narrower <http://vocab.nerc.ac.uk/collection/L05/current/30> ;
  skos:narrower <http://vocab.nerc.ac.uk/collection/L05/current/31> ;
  skos:narrower <http://vocab.nerc.ac.uk/collection/L05/current/32> ;
  skos:narrower <http://vocab.nerc.ac.uk/collection/L05/current/33> ;
  skos:narrower <http://vocab.nerc.ac.uk/collection/L05/current/391> ;
  skos:narrower <http://vocab.nerc.ac.uk/collection/L05/current/392> ;
  skos:narrower <http://vocab.nerc.ac.uk/collection/L05/current/50> ;
  skos:narrower <http://vocab.nerc.ac.uk/collection/L05/current/51> ;
  skos:narrower <http://vocab.nerc.ac.uk/collection/L05/current/52> ;
  skos:narrower <http://vocab.nerc.ac.uk/collection/L05/current/53> ;
  skos:narrower <http://vocab.nerc.ac.uk/collection/L05/current/54> ;
  skos:narrower <http://vocab.nerc.ac.uk/collection/L05/current/55> ;
  skos:narrower <http://vocab.nerc.ac.uk/collection/L05/current/56> ;
  skos:narrower <http://vocab.nerc.ac.uk/collection/L05/current/57> ;
  skos:narrower <http://vocab.nerc.ac.uk/collection/L05/current/58> ;
  skos:narrower <http://vocab.nerc.ac.uk/collection/L05/current/59> ;
  skos:narrower <http://vocab.nerc.ac.uk/collection/L05/current/60> ;
  skos:narrower <http://vocab.nerc.ac.uk/collection/L05/current/61> ;
  skos:narrower <http://vocab.nerc.ac.uk/collection/L05/current/62> ;
  skos:narrower <http://vocab.nerc.ac.uk/collection/L05/current/63> ;
  skos:narrower <http://vocab.nerc.ac.uk/collection/L05/current/64> ;
  skos:narrower <http://vocab.nerc.ac.uk/collection/L05/current/65> ;
  skos:narrower <http://vocab.nerc.ac.uk/collection/L05/current/66> ;
  skos:narrower <http://vocab.nerc.ac.uk/collection/L05/current/67> ;
  skos:narrower <http://vocab.nerc.ac.uk/collection/L05/current/68> ;
  skos:narrower <http://vocab.nerc.ac.uk/collection/L05/current/69> ;
  skos:narrower <http://vocab.nerc.ac.uk/collection/L05/current/70> ;
  skos:narrower <http://vocab.nerc.ac.uk/collection/L05/current/71> ;
  skos:narrower <http://vocab.nerc.ac.uk/collection/L05/current/72> ;
  skos:narrower <http://vocab.nerc.ac.uk/collection/L05/current/90> ;
  skos:narrower <http://vocab.nerc.ac.uk/collection/L05/current/999> ;
  skos:narrower sdev:TFSAMP ;
  skos:notation "SDN:L21::ICAT01" ;
  skos:note "accepted"@en ;
  skos:prefLabel "Sample collection instrument"@en ;
  skos:topConceptOf <http://w3id.org/def/samplecollectioninstrument/conceptscheme> ;
.
sdnc:collection
  rdf:type skos:Collection ;
  dcterm:alternative "Device category types" ;
  dcterm:creator "SeaDataNet" ;
  dcterm:date "2012-07-17 02:00:03.0" ;
  dcterm:description "High-level classification of devices based on function and mode of deployment." ;
  dcterm:license <https://creativecommons.org/licenses/by/4.0> ;
  dcterm:publisher "Natural Environment Research Council" ;
  dcterm:title "SeaDataNet device category types" ;
  grg:RE_RegisterManager "British Oceanographic Data Centre" ;
  grg:RE_RegisterOwner "SeaDataNet" ;
  rdfs:comment "Governance for vocabularies used in the EU SeaDataNet project implemented as consultation between BODC and the members of the SeaDataNet Technical Task Team" ;
  owl:versionInfo "5" ;
  skos:altLabel "Device category types" ;
  skos:member sdnc:ICAT01 ;
  skos:prefLabel "SeaDataNet device category types" ;
.
inst:NETT0001
  rdf:type skos:Concept ;
  dcterm:date "2012-05-11 10:27:07.0" ;
  dcterm:identifier "SDN:L22::NETT0001" ;
  pav:hasCurrentVersion <http://vocab.nerc.ac.uk/collection/L22/current/NETT0001/2> ;
  pav:hasVersion <http://vocab.nerc.ac.uk/collection/L22/current/NETT0001/1> ;
  owl:versionInfo "2" ;
  skos:altLabel "Adriatic plankton sampler"@en ;
  skos:broader <http://vocab.nerc.ac.uk/collection/L05/current/22> ;
  skos:definition "Construction is a 50 cm diameter cylindrical sampler sent to depth with the cylinder net (0.25 mm mesh) closed and upside down (cod-end facing upward). A messenger releases the bottom margin of cylinder allowing it to drop open (115 cm length) and at the same time closing half circle doors. A second messenger releases the first support bridle and the sampler turns right side up. Sampler collects about 250 litres of water [Wiebe and Benfield 2003 Plate 11 A]."@en ;
  skos:inScheme <http://vocab.nerc.ac.uk/scheme/SDNDEV/current> ;
  skos:notation "SDN:L22::NETT0001" ;
  skos:note "accepted"@en ;
  skos:prefLabel "Adriatic plankton sampler - Krsinic (1990)"@en ;
.
inst:NETT0002
  rdf:type skos:Concept ;
  dcterm:date "2011-10-21 14:18:49.0" ;
  dcterm:identifier "SDN:L22::NETT0002" ;
  pav:hasCurrentVersion <http://vocab.nerc.ac.uk/collection/L22/current/NETT0002/1> ;
  owl:versionInfo "1" ;
  skos:altLabel "Apstein HSS"@en ;
  skos:broader <http://vocab.nerc.ac.uk/collection/L05/current/67> ;
  skos:definition "Construction is a cylindrical tube with ~2 cm diameter mouth opening expanding to 4 cm diameter in the main body with a filtering surface at the rear.  Overall length ~20 cm [Wiebe and Benfield 2003 Plate 13 A]."@en ;
  skos:inScheme <http://vocab.nerc.ac.uk/scheme/SDNDEV/current> ;
  skos:notation "SDN:L22::NETT0002" ;
  skos:note "accepted"@en ;
  skos:prefLabel "High-speed sampler - Apstein (1906)"@en ;
.
inst:NETT0003
  rdf:type skos:Concept ;
  dcterm:date "2016-04-05 11:49:20.0" ;
  dcterm:identifier "SDN:L22::NETT0003" ;
  pav:hasCurrentVersion <http://vocab.nerc.ac.uk/collection/L22/current/NETT0003/4> ;
  pav:hasVersion <http://vocab.nerc.ac.uk/collection/L22/current/NETT0003/1> ;
  pav:hasVersion <http://vocab.nerc.ac.uk/collection/L22/current/NETT0003/2> ;
  pav:hasVersion <http://vocab.nerc.ac.uk/collection/L22/current/NETT0003/3> ;
  owl:versionInfo "4" ;
  skos:altLabel "Apstein net as in Apstein (1896); Dakin (1908)"@en ;
  skos:broader <http://vocab.nerc.ac.uk/collection/L05/current/22> ;
  skos:definition "Plankton net described as the Apstein net (Apstein 1896; Dakin 1908) [Wiebe & Benfield (2003)]; designed with single circular mouth piece with reducing cone; with measurements:opening diameter (metre)=0.14, non-filtering cone mouth piece length (metre)=0.2, net mouth diameter (metre)=0.4; with opening area (square metre)=0.0154; with total filtering net length (metre)=1; with filtering net shape conical; with additional features: not specified; with mesh size (millimetre)=0.076 (No. 20 silk); and equipped with optional closing mouth mechanism."@en ;
  skos:inScheme <http://vocab.nerc.ac.uk/scheme/SDNDEV/current> ;
  skos:notation "SDN:L22::NETT0003" ;
  skos:note "accepted"@en ;
  skos:prefLabel "Apstein net as described by  Apstein (1896); Dakin (1908)"@en ;
.
inst:NETT0005
  rdf:type skos:Concept ;
  dcterm:date "2011-10-21 14:18:49.0" ;
  dcterm:identifier "SDN:L22::NETT0005" ;
  pav:hasCurrentVersion <http://vocab.nerc.ac.uk/collection/L22/current/NETT0005/1> ;
  owl:versionInfo "1" ;
  skos:altLabel "Automatic high-speed plankton sampler"@en ;
  skos:broader <http://vocab.nerc.ac.uk/collection/L05/current/67> ;
  skos:broader <http://vocab.nerc.ac.uk/collection/L05/current/68> ;
  skos:definition "A sampler that has a series of 21 nets attached to the bottom of rectangular \"trap doors\" which are sequentially closed by means of a cam/screw assembly driven by a ships log (propellor).  Each net is about 6.35 cm long and made of nylon cloth with 23.6 meshes per cm.  The body of the device is 29.2 cm tall x 14 cm wide x 114 cm long not including the side fins. The aperture is 1.9 cm x 1.9 cm  Effective sampling speeds 5 to 11 knots and sample length is 1 to 20 cm."@en ;
  skos:inScheme <http://vocab.nerc.ac.uk/scheme/SDNDEV/current> ;
  skos:notation "SDN:L22::NETT0005" ;
  skos:note "accepted"@en ;
  skos:prefLabel "Automatic high-speed plankton sampler - Williamson (1962, 1963)"@en ;
.
inst:NETT0006
  rdf:type skos:Concept ;
  dcterm:date "2011-10-21 14:18:49.0" ;
  dcterm:identifier "SDN:L22::NETT0006" ;
  pav:hasCurrentVersion <http://vocab.nerc.ac.uk/collection/L22/current/NETT0006/1> ;
  owl:versionInfo "1" ;
  skos:altLabel "Barnes net"@en ;
  skos:broader <http://vocab.nerc.ac.uk/collection/L05/current/22> ;
  skos:definition "Construction is a hemispherical metal cowling mounted in front of a net ring with an opening sized so that a closing lid can be accommodated when the net is open. A Nansen messenger closing mechanism is used to release the spring loaded closing lid which pivots over the net mouth. No dimensions given for net size or mesh [Wiebe and Benfield 2003 Plate 8 C]."@en ;
  skos:inScheme <http://vocab.nerc.ac.uk/scheme/SDNDEV/current> ;
  skos:notation "SDN:L22::NETT0006" ;
  skos:note "accepted"@en ;
  skos:prefLabel "Closing net - Barnes (1953)"@en ;
.
inst:NETT0009
  rdf:type skos:Concept ;
  dcterm:date "2011-10-21 14:18:49.0" ;
  dcterm:identifier "SDN:L22::NETT0009" ;
  pav:hasCurrentVersion <http://vocab.nerc.ac.uk/collection/L22/current/NETT0009/1> ;
  owl:versionInfo "1" ;
  skos:altLabel "Bongo-style net"@en ;
  skos:broader <http://vocab.nerc.ac.uk/collection/L05/current/22> ;
  skos:definition "An open pair of 50 cm diameter circular net hoops were mounted on each end of a 150 cm wide cross-strut which was attached to a towing cable.  Nets were attached to the bottom of the hoops and their cod-ends were attached to a spreader bar which was also attached to the wire. The nets were lowered to a maximum depth to haul and then during the haul back to the surface, a messenger was used to close the nets either by releasing the hoops so that they turned 90 degrees or by releasing the nets which fell back and were pursed by throttling lines attached to the cross-strut. A non-opening/closing variant of this net is known as the CalVET net [Wiebe and Benfield 2003 Plate 10 A]."@en ;
  skos:inScheme <http://vocab.nerc.ac.uk/scheme/SDNDEV/current> ;
  skos:notation "SDN:L22::NETT0009" ;
  skos:note "accepted"@en ;
  skos:prefLabel "Bongo-style vertical closing net  - Brown (1975)"@en ;
.
inst:NETT0010
  rdf:type skos:Concept ;
  dcterm:date "2011-10-21 14:18:49.0" ;
  dcterm:identifier "SDN:L22::NETT0010" ;
  pav:hasCurrentVersion <http://vocab.nerc.ac.uk/collection/L22/current/NETT0010/1> ;
  owl:versionInfo "1" ;
  skos:altLabel "Modified Bongo opening-closing net"@en ;
  skos:broader <http://vocab.nerc.ac.uk/collection/L05/current/22> ;
  skos:definition "A 75 cm diameter reinforced ring held to the wire by the same method as the Octagon Net. The net had a double messenger release mechanism with the first messenger releasing a dacron cloth door blocking the net mouth and the second one releasing the net."@en ;
  skos:inScheme <http://vocab.nerc.ac.uk/scheme/SDNDEV/current> ;
  skos:notation "SDN:L22::NETT0010" ;
  skos:note "accepted"@en ;
  skos:prefLabel "Modified opening-closing Bongo net - Sameoto and Jaroszynski (1976)"@en ;
.
inst:NETT0012
  rdf:type skos:Concept ;
  dcterm:date "2011-10-21 14:18:49.0" ;
  dcterm:identifier "SDN:L22::NETT0012" ;
  pav:hasCurrentVersion <http://vocab.nerc.ac.uk/collection/L22/current/NETT0012/1> ;
  owl:versionInfo "1" ;
  skos:altLabel "Booby-II net"@en ;
  skos:broader <http://vocab.nerc.ac.uk/collection/L05/current/69> ;
  skos:definition "Construction is a wooden frame 63 cm wide x 16.5 cm tall x 121 cm long with a pair of Otter board fins extending down 58.5 cm below the top.  Styrofoam plastic used for floatation.  Inside the wooden frame is a metal framework to support a 63 cm x 20 cm rectangular net 100 cm long (number 54 nylon grit gauze). Towed at 1 to 3 kts from the bow of a vessel with bridle attached to the forward side of the frame so that it rides out away from the vessel [Wiebe and Benfield 2003 Plate 20 B]."@en ;
  skos:inScheme <http://vocab.nerc.ac.uk/scheme/SDNDEV/current> ;
  skos:notation "SDN:L22::NETT0012" ;
  skos:note "accepted"@en ;
  skos:prefLabel "Booby-II neuston net - Bieri and Newbury (1966)"@en ;
.
inst:NETT0016
  rdf:type skos:Concept ;
  dcterm:date "2011-10-21 14:18:49.0" ;
  dcterm:identifier "SDN:L22::NETT0016" ;
  pav:hasCurrentVersion <http://vocab.nerc.ac.uk/collection/L22/current/NETT0016/1> ;
  owl:versionInfo "1" ;
  skos:altLabel "CalCOFI net"@en ;
  skos:broader <http://vocab.nerc.ac.uk/collection/L05/current/22> ;
  skos:definition "A 100 cm diameter ring net about 5 m in length with No. 30 xxx grit gauze (a grade of silk bolting cloth). Netting changed to 505 micron Nitex mesh and then to 333 micron mesh [Wiebe and Benfield 2003 Plate 2 C]."@en ;
  skos:inScheme <http://vocab.nerc.ac.uk/scheme/SDNDEV/current> ;
  skos:notation "SDN:L22::NETT0016" ;
  skos:note "accepted"@en ;
  skos:prefLabel "CalCOFI net - Ahlstrom (1948)"@en ;
.
inst:NETT0019
  rdf:type skos:Concept ;
  dcterm:date "2011-10-21 14:18:49.0" ;
  dcterm:identifier "SDN:L22::NETT0019" ;
  pav:hasCurrentVersion <http://vocab.nerc.ac.uk/collection/L22/current/NETT0019/1> ;
  owl:versionInfo "1" ;
  skos:altLabel "Chun-Peterson net"@en ;
  skos:broader <http://vocab.nerc.ac.uk/collection/L05/current/22> ;
  skos:definition "A vertical net lowered closed with propellor-activated opening and closing."@en ;
  skos:inScheme <http://vocab.nerc.ac.uk/scheme/SDNDEV/current> ;
  skos:notation "SDN:L22::NETT0019" ;
  skos:note "accepted"@en ;
  skos:prefLabel "Chun-Peterson net - Chun (1888, 1903)"@en ;
.
inst:NETT0020
  rdf:type skos:Concept ;
  dcterm:date "2011-10-21 14:18:49.0" ;
  dcterm:identifier "SDN:L22::NETT0020" ;
  pav:hasCurrentVersion <http://vocab.nerc.ac.uk/collection/L22/current/NETT0020/1> ;
  owl:versionInfo "1" ;
  skos:altLabel "Clarke Jet Net HSS"@en ;
  skos:broader <http://vocab.nerc.ac.uk/collection/L05/current/67> ;
  skos:definition "Construction is a 12 cm diameter mouth opening with an overall length of 125 cm. Uses nylon netting with 0.44 mm mesh. Towing speeds up to 10.5 knots [Wiebe and Benfield 2003 Plate 18 E]."@en ;
  skos:inScheme <http://vocab.nerc.ac.uk/scheme/SDNDEV/current> ;
  skos:notation "SDN:L22::NETT0020" ;
  skos:note "accepted"@en ;
  skos:prefLabel "Clarke Jet Net high-speed plankton sampler - Clarke (1964)"@en ;
.
inst:NETT0022
  rdf:type skos:Concept ;
  dcterm:date "2011-10-21 14:18:49.0" ;
  dcterm:identifier "SDN:L22::NETT0022" ;
  pav:hasCurrentVersion <http://vocab.nerc.ac.uk/collection/L22/current/NETT0022/1> ;
  owl:versionInfo "1" ;
  skos:altLabel "Enzhofer and Hume CMT"@en ;
  skos:broader <http://vocab.nerc.ac.uk/collection/L05/current/23> ;
  skos:definition "Construction is a 300 cm x 700 cm rectangular mouth opening with net  1800 cm in length. The net is made from five sets of mesh with coarse mesh at the front and fine mesh at the back (600 cm of 10.2 cm mesh, 400 cm of 5.1 cm mesh, 300 cm of 1.9 cm mesh, 300 cm of 1.3 cm mesh and 200 cm of 0.3 cm mesh). There are two towing cables: one for the top spreader bar and one for the bottom. Each cable goes to separate winch. The net is lowered with tension on bottom spreader so that it is closed. Tension is then transferred to the top spreader to open the net. Tension again taken by lower spreader to close net [Wiebe and Benfield 2003 Plate 12 B]."@en ;
  skos:inScheme <http://vocab.nerc.ac.uk/scheme/SDNDEV/current> ;
  skos:notation "SDN:L22::NETT0022" ;
  skos:note "accepted"@en ;
  skos:prefLabel "Closing midwater trawl - Enzenhofer and Hume (1989)"@en ;
.
inst:NETT0023
  rdf:type skos:Concept ;
  dcterm:date "2011-10-21 14:18:49.0" ;
  dcterm:identifier "SDN:L22::NETT0023" ;
  pav:hasCurrentVersion <http://vocab.nerc.ac.uk/collection/L22/current/NETT0023/1> ;
  owl:versionInfo "1" ;
  skos:altLabel "Hart net"@en ;
  skos:broader <http://vocab.nerc.ac.uk/collection/L05/current/22> ;
  skos:definition "A rod of wood or pipe is outfitted with a combination wire clamp and closing release at the top and a pair of snap hooks at the bottom, one to secure the device to the wire and one to secure the bottom portion of the net. Attached to the rod is a net with a bridle which inserts into the release latch. Midway along the pipe is a second snap hook which is attached to the mid section of the net. Multiples of these units may be attached to the wire at various depth intervals as the wire is lowered vertically into the water.  Plankton collections are made as the nets are hauled up until a messenger hitting the release lets the bridle go, thus closing the net [Wiebe and Benfield 2003 Plate 5 B]."@en ;
  skos:inScheme <http://vocab.nerc.ac.uk/scheme/SDNDEV/current> ;
  skos:notation "SDN:L22::NETT0023" ;
  skos:note "accepted"@en ;
  skos:prefLabel "Closing Net - Hart (1935)"@en ;
.
inst:NETT0024
  rdf:type skos:Concept ;
  dcterm:date "2011-10-21 14:18:49.0" ;
  dcterm:identifier "SDN:L22::NETT0024" ;
  pav:hasCurrentVersion <http://vocab.nerc.ac.uk/collection/L22/current/NETT0024/1> ;
  owl:versionInfo "1" ;
  skos:altLabel "Motoda cod-end sampler"@en ;
  skos:broader <http://vocab.nerc.ac.uk/collection/L05/current/22> ;
  skos:definition "Construction is a 15.5 cm diameter mouth opening and 35.5 cm long body attached to 57 cm diameter net 200 cm long with bolting cloth 42.5 meshes per inch in upper 120 cm and 56.5 meshes per inch in lower 80 cm [Wiebe and Benfield 2003 Plate 25 A]."@en ;
  skos:inScheme <http://vocab.nerc.ac.uk/scheme/SDNDEV/current> ;
  skos:notation "SDN:L22::NETT0024" ;
  skos:note "accepted"@en ;
  skos:prefLabel "Cod-end sampler - Motoda (1953)"@en ;
.
inst:NETT0026
  rdf:type skos:Concept ;
  dcterm:date "2011-10-21 14:18:49.0" ;
  dcterm:identifier "SDN:L22::NETT0026" ;
  pav:hasCurrentVersion <http://vocab.nerc.ac.uk/collection/L22/current/NETT0026/1> ;
  owl:versionInfo "1" ;
  skos:altLabel "CPR"@en ;
  skos:broader <http://vocab.nerc.ac.uk/collection/L05/current/21> ;
  skos:definition "Construction is a 1.27 cm on side square mouth opening (originally 10.1 cm diameter) high-speed (12 to 17 knots) towed body collecting plankton on gauze (22.9 cm wide and 23.6 meshes per cm) rolls. The body is 50 cm wide x 50 cm tall x 100 cm long.  A propellor drives the rollers winding up the gauze.  The system is normally towed at 10 m depth at speeds up to 20 ktnos [Wiebe and Benfield 2003 Plate 19 A, B]."@en ;
  skos:inScheme <http://vocab.nerc.ac.uk/scheme/SDNDEV/current> ;
  skos:notation "SDN:L22::NETT0026" ;
  skos:note "accepted"@en ;
  skos:prefLabel "Continuous Plankton Recorder - Hardy (1926, 1936); Glover (1962)"@en ;
.
inst:NETT0027
  rdf:type skos:Concept ;
  dcterm:date "2011-10-21 14:18:49.0" ;
  dcterm:identifier "SDN:L22::NETT0027" ;
  pav:hasCurrentVersion <http://vocab.nerc.ac.uk/collection/L22/current/NETT0027/1> ;
  owl:versionInfo "1" ;
  skos:altLabel "Modified David neuston net"@en ;
  skos:broader <http://vocab.nerc.ac.uk/collection/L05/current/69> ;
  skos:definition "A pair of vertically stacked nets with 30 cm x 15 cm rectangular mouth opening and 0.3 or 0.5 mm mesh [Wiebe and Benfield 2003 Plate 21 B]."@en ;
  skos:inScheme <http://vocab.nerc.ac.uk/scheme/SDNDEV/current> ;
  skos:notation "SDN:L22::NETT0027" ;
  skos:note "accepted"@en ;
  skos:prefLabel "Modified David neuston net - Hempel and Weikert (1972)"@en ;
.
inst:NETT0030
  rdf:type skos:Concept ;
  dcterm:date "2011-10-21 14:18:49.0" ;
  dcterm:identifier "SDN:L22::NETT0030" ;
  pav:hasCurrentVersion <http://vocab.nerc.ac.uk/collection/L22/current/NETT0030/1> ;
  owl:versionInfo "1" ;
  skos:altLabel "Wishner Deep-Tow net system"@en ;
  skos:broader <http://vocab.nerc.ac.uk/collection/L05/current/22> ;
  skos:broader <http://vocab.nerc.ac.uk/collection/L05/current/68> ;
  skos:definition "Three rectangular mouth opening nets ~30 cm wide x 44 cm tall and 130 cm long mounted on a metal framework attached to the bottom of the Deep-Tow Instrument . The unobstructed nets were opened/closed by surface command transmitted via conducting cable to a release mechanism [Wiebe and Benfield 2003 Plate 24 A]."@en ;
  skos:inScheme <http://vocab.nerc.ac.uk/scheme/SDNDEV/current> ;
  skos:notation "SDN:L22::NETT0030" ;
  skos:note "accepted"@en ;
  skos:prefLabel "Deep-Tow net system - Wishner (1980)"@en ;
.
inst:NETT0031
  rdf:type skos:Concept ;
  dcterm:date "2011-10-21 14:18:49.0" ;
  dcterm:identifier "SDN:L22::NETT0031" ;
  pav:hasCurrentVersion <http://vocab.nerc.ac.uk/collection/L22/current/NETT0031/1> ;
  owl:versionInfo "1" ;
  skos:altLabel "Emery diver tow net"@en ;
  skos:broader <http://vocab.nerc.ac.uk/collection/L05/current/22> ;
  skos:definition "A 30 cm diameter ring net with 0.183 mm mesh towed by diver."@en ;
  skos:inScheme <http://vocab.nerc.ac.uk/scheme/SDNDEV/current> ;
  skos:notation "SDN:L22::NETT0031" ;
  skos:note "accepted"@en ;
  skos:prefLabel "Diver tow net - Emery (1968)"@en ;
.
inst:NETT0032
  rdf:type skos:Concept ;
  dcterm:date "2011-10-21 14:18:49.0" ;
  dcterm:identifier "SDN:L22::NETT0032" ;
  pav:hasCurrentVersion <http://vocab.nerc.ac.uk/collection/L22/current/NETT0032/1> ;
  owl:versionInfo "1" ;
  skos:altLabel "Porter diver-pushed net"@en ;
  skos:broader <http://vocab.nerc.ac.uk/collection/L05/current/22> ;
  skos:definition "A 50 cm diameter ring net 200 cm long with 0.12 mm mesh pushed by a diver."@en ;
  skos:inScheme <http://vocab.nerc.ac.uk/scheme/SDNDEV/current> ;
  skos:notation "SDN:L22::NETT0032" ;
  skos:note "accepted"@en ;
  skos:prefLabel "Diver-pushed net - Porter (1973)"@en ;
.
inst:NETT0034
  rdf:type skos:Concept ;
  dcterm:date "2011-10-21 14:18:49.0" ;
  dcterm:identifier "SDN:L22::NETT0034" ;
  pav:hasCurrentVersion <http://vocab.nerc.ac.uk/collection/L22/current/NETT0034/1> ;
  owl:versionInfo "1" ;
  skos:altLabel "DSRV Alvin Net-1"@en ;
  skos:broader <http://vocab.nerc.ac.uk/collection/L05/current/22> ;
  skos:definition "A pair of nets were mounted onto the front of DSRV Alvin for collecting planktobenthos at great depths. The mouth openings were D-shaped and hinged so that on descent and ascent of the submersible, the nets could be turned back away from the flow and would not filter. The Alvin arm was used by the pilot to open and close the net.  The nets had 0.233 mm mesh [Wiebe and Benfield 2003 Plate 23 D]."@en ;
  skos:inScheme <http://vocab.nerc.ac.uk/scheme/SDNDEV/current> ;
  skos:notation "SDN:L22::NETT0034" ;
  skos:note "accepted"@en ;
  skos:prefLabel "Deep Submergence Rescue Vehicle Alvin Net-1 - Grice and Huelsemann (1970)"@en ;
.
inst:NETT0035
  rdf:type skos:Concept ;
  dcterm:date "2011-10-21 14:18:49.0" ;
  dcterm:identifier "SDN:L22::NETT0035" ;
  pav:hasCurrentVersion <http://vocab.nerc.ac.uk/collection/L22/current/NETT0035/1> ;
  owl:versionInfo "1" ;
  skos:altLabel "DSRV Alvin Net-2"@en ;
  skos:broader <http://vocab.nerc.ac.uk/collection/L05/current/22> ;
  skos:definition "A pair of nets were attached to a pair of rectangular frames 61 cm wide x 31 cm tall which each had a metal door hinged at the top.  The Alvin arm was  used by the pilot to open and close the door.  The nets were positioned about 20 cm above the bottom. The nets had 0.239 mm mesh. Normal pushing speed was 1 knot [Wiebe and Benfield 2003 Plate 23 E]."@en ;
  skos:inScheme <http://vocab.nerc.ac.uk/scheme/SDNDEV/current> ;
  skos:notation "SDN:L22::NETT0035" ;
  skos:note "accepted"@en ;
  skos:prefLabel "Deep Submergence Rescue Vehicle Alvin Net-2 - Grice (1972)"@en ;
.
inst:NETT0036
  rdf:type skos:Concept ;
  dcterm:date "2011-10-21 14:18:49.0" ;
  dcterm:identifier "SDN:L22::NETT0036" ;
  pav:hasCurrentVersion <http://vocab.nerc.ac.uk/collection/L22/current/NETT0036/1> ;
  owl:versionInfo "1" ;
  skos:altLabel "English umbrella net"@en ;
  skos:broader <http://vocab.nerc.ac.uk/collection/L05/current/22> ;
  skos:definition "A rectangular net 200 cm on a side and 300 cm long made from 0.22 mm nylon mesh is designed to fit through a hole in an ice flow closed, and open once underneath. A messenger is used to close the mouth opening at a specific depth prior to retrieval though the ice [Wiebe and Benfield 2003 Plate 11 C]."@en ;
  skos:inScheme <http://vocab.nerc.ac.uk/scheme/SDNDEV/current> ;
  skos:notation "SDN:L22::NETT0036" ;
  skos:note "accepted"@en ;
  skos:prefLabel "English umbrella net - Macaulay and Daly (1987)"@en ;
.
inst:NETT0039
  rdf:type skos:Concept ;
  dcterm:date "2011-10-21 14:18:49.0" ;
  dcterm:identifier "SDN:L22::NETT0039" ;
  pav:hasCurrentVersion <http://vocab.nerc.ac.uk/collection/L22/current/NETT0039/1> ;
  owl:versionInfo "1" ;
  skos:altLabel "Russell epi-benthic plankton net"@en ;
  skos:broader <http://vocab.nerc.ac.uk/collection/L05/current/22> ;
  skos:broader <http://vocab.nerc.ac.uk/collection/L05/current/61> ;
  skos:definition "Construction is 122 cm wide x 30 cm tall rectangular mouth with a 240 cm length net made of stramin. The net is mounted in an Agassiz trawl frame [Wiebe and Benfield 2003 Plate 22 B]."@en ;
  skos:inScheme <http://vocab.nerc.ac.uk/scheme/SDNDEV/current> ;
  skos:notation "SDN:L22::NETT0039" ;
  skos:note "accepted"@en ;
  skos:prefLabel "Epi-benthic plankton net - Russell (1928)"@en ;
.
inst:NETT0040
  rdf:type skos:Concept ;
  dcterm:date "2011-10-21 14:18:49.0" ;
  dcterm:identifier "SDN:L22::NETT0040" ;
  pav:hasCurrentVersion <http://vocab.nerc.ac.uk/collection/L22/current/NETT0040/1> ;
  owl:versionInfo "1" ;
  skos:altLabel "Bossanyi epi-benthic plankton sampler"@en ;
  skos:broader <http://vocab.nerc.ac.uk/collection/L05/current/22> ;
  skos:broader <http://vocab.nerc.ac.uk/collection/L05/current/24> ;
  skos:definition "Approximately 91 cm x 61 cm rectangular mouth with net about 213 cm long. Netting with 15.7 meshes per cm. Able of open/close mouth opening [Wiebe and Benfield 2003 Plate 22 C]."@en ;
  skos:inScheme <http://vocab.nerc.ac.uk/scheme/SDNDEV/current> ;
  skos:notation "SDN:L22::NETT0040" ;
  skos:note "accepted"@en ;
  skos:prefLabel "Epi-benthic plankton sampler - Bossanyi (1951)"@en ;
.
inst:NETT0041
  rdf:type skos:Concept ;
  dcterm:date "2011-10-21 14:18:49.0" ;
  dcterm:identifier "SDN:L22::NETT0041" ;
  pav:hasCurrentVersion <http://vocab.nerc.ac.uk/collection/L22/current/NETT0041/1> ;
  owl:versionInfo "1" ;
  skos:altLabel "Clutter epi-benthic plankton sampler"@en ;
  skos:broader <http://vocab.nerc.ac.uk/collection/L05/current/22> ;
  skos:broader <http://vocab.nerc.ac.uk/collection/L05/current/24> ;
  skos:definition "Construction is a 32cm x 32 cm rectangular mouth opening net attached to a metal box frame work which was 37 cm tall x 37 cm wide x 30 cm long. The net was about 30 cm long had 0.333 mm nylon mesh. The system was lowered to the seafloor where an anchor attached to the net frame by a spool of line became fixed. The net was towed at ~1.5 knots away from the anchor until the line was fully extended whereupon it triggered a choke rope closing the net. Distance covered by the sampler was about 10 m. A scaled up version with 70.1 cm x 70.1 cm mouth opening also described [Wiebe and Benfield 2003 Plate 23 A]."@en ;
  skos:inScheme <http://vocab.nerc.ac.uk/scheme/SDNDEV/current> ;
  skos:notation "SDN:L22::NETT0041" ;
  skos:note "accepted"@en ;
  skos:prefLabel "Epi-benthic plankton sampler - Clutter (1965)"@en ;
.
inst:NETT0042
  rdf:type skos:Concept ;
  dcterm:date "2011-10-21 14:18:49.0" ;
  dcterm:identifier "SDN:L22::NETT0042" ;
  pav:hasCurrentVersion <http://vocab.nerc.ac.uk/collection/L22/current/NETT0042/1> ;
  owl:versionInfo "1" ;
  skos:altLabel "Wickstead epi-benthic sled"@en ;
  skos:broader <http://vocab.nerc.ac.uk/collection/L05/current/22> ;
  skos:broader <http://vocab.nerc.ac.uk/collection/L05/current/24> ;
  skos:definition "Construction is a 61 cm x 30 cm rectangular mouth opening : length of net or mesh size not given [Wiebe and Benfield 2003 Plate 22 D]."@en ;
  skos:inScheme <http://vocab.nerc.ac.uk/scheme/SDNDEV/current> ;
  skos:notation "SDN:L22::NETT0042" ;
  skos:note "accepted"@en ;
  skos:prefLabel "Mechanically opening-closing epi-benthic plankton sled - Wickstead (1953)"@en ;
.
inst:NETT0043
  rdf:type skos:Concept ;
  dcterm:date "2011-10-21 14:18:49.0" ;
  dcterm:identifier "SDN:L22::NETT0043" ;
  pav:hasCurrentVersion <http://vocab.nerc.ac.uk/collection/L22/current/NETT0043/1> ;
  owl:versionInfo "1" ;
  skos:altLabel "Foxton two-chamber cod-end"@en ;
  skos:broader <http://vocab.nerc.ac.uk/collection/L05/current/23> ;
  skos:definition "A modification to the IKMT to allow pressure actuated depth separated collections by a two-part cod end [Wiebe and Benfield 2003 Plate 25 D]."@en ;
  skos:inScheme <http://vocab.nerc.ac.uk/scheme/SDNDEV/current> ;
  skos:notation "SDN:L22::NETT0043" ;
  skos:note "accepted"@en ;
  skos:prefLabel "Foxton two-chamber cod-end - Currie (1962) Foston (1963)"@en ;
.
inst:NETT0044
  rdf:type skos:Concept ;
  dcterm:date "2011-10-21 14:18:49.0" ;
  dcterm:identifier "SDN:L22::NETT0044" ;
  pav:hasCurrentVersion <http://vocab.nerc.ac.uk/collection/L22/current/NETT0044/1> ;
  owl:versionInfo "1" ;
  skos:altLabel "Heron free-fall plankton net"@en ;
  skos:broader <http://vocab.nerc.ac.uk/collection/L05/current/22> ;
  skos:definition "A modified WP2 cylinder-cone closing net (mesh not specified) which is allowed to free-fall and then is strangled shut and retrieved.  [Wiebe and Benfield 2003 Plate 10C]"@en ;
  skos:inScheme <http://vocab.nerc.ac.uk/scheme/SDNDEV/current> ;
  skos:notation "SDN:L22::NETT0044" ;
  skos:note "accepted"@en ;
  skos:prefLabel "Free-fall plankton net - Heron (1982)"@en ;
.
inst:NETT0045
  rdf:type skos:Concept ;
  dcterm:date "2011-10-21 14:18:49.0" ;
  dcterm:identifier "SDN:L22::NETT0045" ;
  pav:hasCurrentVersion <http://vocab.nerc.ac.uk/collection/L22/current/NETT0045/1> ;
  owl:versionInfo "1" ;
  skos:altLabel "Kozasa zooplankton sampler"@en ;
  skos:broader <http://vocab.nerc.ac.uk/collection/L05/current/22> ;
  skos:definition "Construction is a double-gimballed frame 100 cm tall x 65.5 cm wide supporting a ring net 30 cm in diameter. A bridle is attached to the top of the frame and a weight to the bottom so the net mouth is free of obstructions.   No description of net length or mesh size given."@en ;
  skos:inScheme <http://vocab.nerc.ac.uk/scheme/SDNDEV/current> ;
  skos:notation "SDN:L22::NETT0045" ;
  skos:note "accepted"@en ;
  skos:prefLabel "Gimbal-ring zooplankton sampler - Kozasa (1984)"@en ;
.
inst:NETT0047
  rdf:type skos:Concept ;
  dcterm:date "2011-10-21 14:18:49.0" ;
  dcterm:identifier "SDN:L22::NETT0047" ;
  pav:hasCurrentVersion <http://vocab.nerc.ac.uk/collection/L22/current/NETT0047/1> ;
  owl:versionInfo "1" ;
  skos:altLabel "Gulf II HSS"@en ;
  skos:broader <http://vocab.nerc.ac.uk/collection/L05/current/21> ;
  skos:definition "A shipboard pump drew water from near the keel of the vessel which was delivered to a circular pan divided into 8 parts each with a filter to catch the plankton. The  sampling interval for a filter was 1 hour. Filters (#1 bolting silk) were replaced every 8 hours.  This system was developed as a substitute for the Continuous Plankton Recorder."@en ;
  skos:inScheme <http://vocab.nerc.ac.uk/scheme/SDNDEV/current> ;
  skos:notation "SDN:L22::NETT0047" ;
  skos:note "accepted"@en ;
  skos:prefLabel "Gulf II high-speed sampler - Collier (1957)"@en ;
.
inst:NETT0052
  rdf:type skos:Concept ;
  dcterm:date "2011-10-21 14:18:49.0" ;
  dcterm:identifier "SDN:L22::NETT0052" ;
  pav:hasCurrentVersion <http://vocab.nerc.ac.uk/collection/L22/current/NETT0052/1> ;
  owl:versionInfo "1" ;
  skos:altLabel "Hempel modified Gulf III HSS (HAI)"@en ;
  skos:broader <http://vocab.nerc.ac.uk/collection/L05/current/67> ;
  skos:definition "Construction comprises an entrance of 18 cm diameter and a net mesh of 0.4mm. Towed at 6 knots."@en ;
  skos:inScheme <http://vocab.nerc.ac.uk/scheme/SDNDEV/current> ;
  skos:notation "SDN:L22::NETT0052" ;
  skos:note "accepted"@en ;
  skos:prefLabel "Modified Gulf III high-speed sampler - Hempel (1960)"@en ;
.
inst:NETT0053
  rdf:type skos:Concept ;
  dcterm:date "2011-10-21 14:18:49.0" ;
  dcterm:identifier "SDN:L22::NETT0053" ;
  pav:hasCurrentVersion <http://vocab.nerc.ac.uk/collection/L22/current/NETT0053/1> ;
  owl:versionInfo "1" ;
  skos:altLabel "Miller modified Hardy Plankton Sampler"@en ;
  skos:broader <http://vocab.nerc.ac.uk/collection/L05/current/67> ;
  skos:definition "This is a small high-speed sampler (modified from that described by Glover) with 10.1cm diameter aperture opening on a body tube 14 cm internal diameter and a 61cm overall length. Attached to the back of the tube is a 91 cm long nylon net of three meshes (0.947 mm, 0.526 mm, and 0.264 mm). Multiple units used on the towing wire at speeds of 7 to 8 knots with a multiplane kit otter depressor on bottom of wire [Wiebe and Benfield 2003 Plate 14 B]."@en ;
  skos:inScheme <http://vocab.nerc.ac.uk/scheme/SDNDEV/current> ;
  skos:notation "SDN:L22::NETT0053" ;
  skos:note "accepted"@en ;
  skos:prefLabel "Modified small Hardy Plankton Sampler - Miller (1961)"@en ;
.
inst:NETT0054
  rdf:type skos:Concept ;
  dcterm:date "2011-10-21 14:18:49.0" ;
  dcterm:identifier "SDN:L22::NETT0054" ;
  pav:hasCurrentVersion <http://vocab.nerc.ac.uk/collection/L22/current/NETT0054/1> ;
  owl:versionInfo "1" ;
  skos:altLabel "Hensen egg net"@en ;
  skos:broader <http://vocab.nerc.ac.uk/collection/L05/current/22> ;
  skos:definition "Construction is a 38 cm diameter mouth (40 cm long conical mouth piece); 100 cm diameter conical net mouth. 144 cm long net of No. 20 silk [Wiebe and Benfield 2003 Plate 1 A, B)"@en ;
  skos:inScheme <http://vocab.nerc.ac.uk/scheme/SDNDEV/current> ;
  skos:notation "SDN:L22::NETT0054" ;
  skos:note "accepted"@en ;
  skos:prefLabel "Hensen egg net - Hensen (1887); Jenkins (1901); Wimpenny (1937)"@en ;
.
inst:NETT0055
  rdf:type skos:Concept ;
  dcterm:date "2011-10-21 14:18:49.0" ;
  dcterm:identifier "SDN:L22::NETT0055" ;
  pav:hasCurrentVersion <http://vocab.nerc.ac.uk/collection/L22/current/NETT0055/1> ;
  owl:versionInfo "1" ;
  skos:altLabel "Smith HSS"@en ;
  skos:broader <http://vocab.nerc.ac.uk/collection/L05/current/67> ;
  skos:definition "Construction comprises a 2.54 cm diameter mouth expanding to 5.08 cm (brass), cylindrical net 5.08 cm and 25.4 cm long made of No. 56xxx grit gauze, and a bucket. Towed at 9 knots."@en ;
  skos:inScheme <http://vocab.nerc.ac.uk/scheme/SDNDEV/current> ;
  skos:notation "SDN:L22::NETT0055" ;
  skos:note "accepted"@en ;
  skos:prefLabel "High-speed sampler - Smith and Ahlstrom (1948)"@en ;
.
inst:NETT0056
  rdf:type skos:Concept ;
  dcterm:date "2011-10-21 14:18:49.0" ;
  dcterm:identifier "SDN:L22::NETT0056" ;
  pav:hasCurrentVersion <http://vocab.nerc.ac.uk/collection/L22/current/NETT0056/1> ;
  owl:versionInfo "1" ;
  skos:altLabel "Pierce HSS"@en ;
  skos:broader <http://vocab.nerc.ac.uk/collection/L05/current/67> ;
  skos:definition "Construction comprises a 7 cm mouth opening of front cone which was 16.5 cm long.  17.8 cm diameter cylinder body which was 25.4 cm long. 7 cm conical coarse silk net 16.5 cm long with small jar cod end."@en ;
  skos:inScheme <http://vocab.nerc.ac.uk/scheme/SDNDEV/current> ;
  skos:notation "SDN:L22::NETT0056" ;
  skos:note "accepted"@en ;
  skos:prefLabel "High-speed plankton sampler - Pierce (1937)"@en ;
.
inst:NETT0057
  rdf:type skos:Concept ;
  dcterm:date "2011-10-21 14:18:49.0" ;
  dcterm:identifier "SDN:L22::NETT0057" ;
  pav:hasCurrentVersion <http://vocab.nerc.ac.uk/collection/L22/current/NETT0057/1> ;
  owl:versionInfo "1" ;
  skos:altLabel "Erdmann HSS"@en ;
  skos:broader <http://vocab.nerc.ac.uk/collection/L05/current/67> ;
  skos:definition "Construction comprises a ~4.5 cm diameter mouth expanding to 12 cm with overall length of 64 cm.  Has an opening/closing mechanism [Wiebe and Benfield 2003 Plate 14 D]."@en ;
  skos:inScheme <http://vocab.nerc.ac.uk/scheme/SDNDEV/current> ;
  skos:notation "SDN:L22::NETT0057" ;
  skos:note "accepted"@en ;
  skos:prefLabel "High-speed sampler - Erdmann (1937)"@en ;
.
inst:NETT0058
  rdf:type skos:Concept ;
  dcterm:date "2011-10-21 14:18:49.0" ;
  dcterm:identifier "SDN:L22::NETT0058" ;
  pav:hasCurrentVersion <http://vocab.nerc.ac.uk/collection/L22/current/NETT0058/1> ;
  owl:versionInfo "1" ;
  skos:altLabel "Fry high-speed metal plankton net"@en ;
  skos:broader <http://vocab.nerc.ac.uk/collection/L05/current/67> ;
  skos:definition "Construction comprises a 10.2 cm diameter mouth opening expanding to 25.4 cm followed by a mesh cone (15.7 meshes per cm) and a cod end. Overall length 152 cm. Towed with 3 part chain bridle at speeds up to 10 knots [Wiebe and Benfield 2003 Plate 14 C]."@en ;
  skos:inScheme <http://vocab.nerc.ac.uk/scheme/SDNDEV/current> ;
  skos:notation "SDN:L22::NETT0058" ;
  skos:note "accepted"@en ;
  skos:prefLabel "High-speed metal plankton net - Fry (1937)"@en ;
.
inst:NETT0059
  rdf:type skos:Concept ;
  dcterm:date "2011-10-21 14:18:49.0" ;
  dcterm:identifier "SDN:L22::NETT0059" ;
  pav:hasCurrentVersion <http://vocab.nerc.ac.uk/collection/L22/current/NETT0059/1> ;
  owl:versionInfo "1" ;
  skos:altLabel "Cassie high-speed net model I"@en ;
  skos:broader <http://vocab.nerc.ac.uk/collection/L05/current/67> ;
  skos:definition "A brass cylinder 6 cm diameter and 6 cm long with bridle attachment lugs that had a 180 cm bolting cloth net (16 or 30 meshes per cm) attached to the back [Wiebe and Benfield 2003 Plate 18 A ]."@en ;
  skos:inScheme <http://vocab.nerc.ac.uk/scheme/SDNDEV/current> ;
  skos:notation "SDN:L22::NETT0059" ;
  skos:note "accepted"@en ;
  skos:prefLabel "High-speed net model I - Cassie (1956)"@en ;
.
inst:NETT0060
  rdf:type skos:Concept ;
  dcterm:date "2011-10-21 14:18:49.0" ;
  dcterm:identifier "SDN:L22::NETT0060" ;
  pav:hasCurrentVersion <http://vocab.nerc.ac.uk/collection/L22/current/NETT0060/1> ;
  owl:versionInfo "1" ;
  skos:altLabel "Cassie high-speed net model II"@en ;
  skos:broader <http://vocab.nerc.ac.uk/collection/L05/current/67> ;
  skos:definition "Same as the model 1 (6cm diameter 6cm long brass cylinder with 180 cm net) except the system was shorter (90 cm) and the net made out of brass gauze with 16 meshes per cm and two metal rods (struts) connected the brass cylinder to the cod end bucket."@en ;
  skos:inScheme <http://vocab.nerc.ac.uk/scheme/SDNDEV/current> ;
  skos:notation "SDN:L22::NETT0060" ;
  skos:note "accepted"@en ;
  skos:prefLabel "High-Speed net model II - Cassie (1956)"@en ;
.
inst:NETT0061
  rdf:type skos:Concept ;
  dcterm:date "2011-10-21 14:18:49.0" ;
  dcterm:identifier "SDN:L22::NETT0061" ;
  pav:hasCurrentVersion <http://vocab.nerc.ac.uk/collection/L22/current/NETT0061/1> ;
  owl:versionInfo "1" ;
  skos:altLabel "Cassie high-speed net model III"@en ;
  skos:broader <http://vocab.nerc.ac.uk/collection/L05/current/67> ;
  skos:definition "Same as model 2 (6cm diameter 6cm long brass cylinder with 90 cm net) except shorter again (60 cm) and four metal rods (struts) connected the brass cylinder to the cod end bucket."@en ;
  skos:inScheme <http://vocab.nerc.ac.uk/scheme/SDNDEV/current> ;
  skos:notation "SDN:L22::NETT0061" ;
  skos:note "accepted"@en ;
  skos:prefLabel "High-speed net model III - Cassie (1956)"@en ;
.
inst:NETT0062
  rdf:type skos:Concept ;
  dcterm:date "2011-10-21 14:18:49.0" ;
  dcterm:identifier "SDN:L22::NETT0062" ;
  pav:hasCurrentVersion <http://vocab.nerc.ac.uk/collection/L22/current/NETT0062/1> ;
  owl:versionInfo "1" ;
  skos:altLabel "Cassie high-speed net"@en ;
  skos:broader <http://vocab.nerc.ac.uk/collection/L05/current/67> ;
  skos:definition "A combination of model 1, model 2 and model 3 nets  towed from the stern of the vessel at ~ 8 knots on a 40 m tow line."@en ;
  skos:inScheme <http://vocab.nerc.ac.uk/scheme/SDNDEV/current> ;
  skos:notation "SDN:L22::NETT0062" ;
  skos:note "accepted"@en ;
  skos:prefLabel "High-speed net - Cassie (1956)"@en ;
.
inst:NETT0063
  rdf:type skos:Concept ;
  dcterm:date "2011-10-21 14:18:49.0" ;
  dcterm:identifier "SDN:L22::NETT0063" ;
  pav:hasCurrentVersion <http://vocab.nerc.ac.uk/collection/L22/current/NETT0063/1> ;
  owl:versionInfo "1" ;
  skos:altLabel "Gauld high-speed tow net"@en ;
  skos:broader <http://vocab.nerc.ac.uk/collection/L05/current/67> ;
  skos:definition "A 46 cm diameter mouth opening with 15 cm long calico collar, 94 cm long silk net (10.2 meshes per cm), and 12 cm diameter x 17cm long sleeve with ring sewn in at end. The tail of the net is flipped inward and bridles attached to the ring are attached to the front of the net.  A three-part bridle tows the net at speeds up to 7 knots. Design taken from Sheard [Wiebe and Benfield 2003 Plate 15 A]."@en ;
  skos:inScheme <http://vocab.nerc.ac.uk/scheme/SDNDEV/current> ;
  skos:notation "SDN:L22::NETT0063" ;
  skos:note "accepted"@en ;
  skos:prefLabel "High-speed tow net - Gauld and Beganal (1951)"@en ;
.
inst:NETT0065
  rdf:type skos:Concept ;
  dcterm:date "2011-10-21 14:18:49.0" ;
  dcterm:identifier "SDN:L22::NETT0065" ;
  pav:hasCurrentVersion <http://vocab.nerc.ac.uk/collection/L22/current/NETT0065/1> ;
  owl:versionInfo "1" ;
  skos:altLabel "Motoda HSS"@en ;
  skos:broader <http://vocab.nerc.ac.uk/collection/L05/current/67> ;
  skos:definition "Body is 10 cm diameter and 100 cm in length. Tapered nose with two 2 cm openings. Body of cylinder has multiple sections 1.5 cm diameter x 18 cm long to store samples.  Equipped with depth/flowmeter. Collects samples at ~ 8 knots."@en ;
  skos:inScheme <http://vocab.nerc.ac.uk/scheme/SDNDEV/current> ;
  skos:notation "SDN:L22::NETT0065" ;
  skos:note "accepted"@en ;
  skos:prefLabel "High-speed successive plankton sampler - Motoda (1953)"@en ;
.
inst:NETT0066
  rdf:type skos:Concept ;
  dcterm:date "2017-08-10 12:37:04.0" ;
  dcterm:identifier "SDN:L22::NETT0066" ;
  pav:hasCurrentVersion <http://vocab.nerc.ac.uk/collection/L22/current/NETT0066/2> ;
  pav:hasVersion <http://vocab.nerc.ac.uk/collection/L22/current/NETT0066/1> ;
  owl:versionInfo "2" ;
  skos:altLabel "Zacharias HSS"@en ;
  skos:broader <http://vocab.nerc.ac.uk/collection/L05/current/67> ;
  skos:definition "A cylindrical tube similar to Apstein's with ~3 cm diameter mouth opening expanding to 8 cm diameter main body with baffles for different towing speeds and a filtering surface at the rear. Overall length 42 cm [Wiebe and Benfield 2003 Plate 13 B]."@en ;
  skos:inScheme <http://vocab.nerc.ac.uk/scheme/SDNDEV/current> ;
  skos:notation "SDN:L22::NETT0066" ;
  skos:note "accepted"@en ;
  skos:prefLabel "High-speed sampler - Zacharias (1907)"@en ;
.
inst:NETT0067
  rdf:type skos:Concept ;
  dcterm:date "2011-10-21 14:18:49.0" ;
  dcterm:identifier "SDN:L22::NETT0067" ;
  pav:hasCurrentVersion <http://vocab.nerc.ac.uk/collection/L22/current/NETT0067/1> ;
  owl:versionInfo "1" ;
  skos:altLabel "Monti HSS"@en ;
  skos:broader <http://vocab.nerc.ac.uk/collection/L05/current/67> ;
  skos:definition "A cylindrical tube modified from Zacharias with a 3-4 cm diameter mouth opening expanding to 10-12 cm diameter main body and a filtering cone leading to a stopcock at the rear.  Overall length 50 cm [Wiebe and Benfield 2003 Plate 13 C]."@en ;
  skos:inScheme <http://vocab.nerc.ac.uk/scheme/SDNDEV/current> ;
  skos:notation "SDN:L22::NETT0067" ;
  skos:note "accepted"@en ;
  skos:prefLabel "High speed-sampler - Monti (1910)"@en ;
.
inst:NETT0068
  rdf:type skos:Concept ;
  dcterm:date "2011-10-21 14:18:49.0" ;
  dcterm:identifier "SDN:L22::NETT0068" ;
  pav:hasCurrentVersion <http://vocab.nerc.ac.uk/collection/L22/current/NETT0068/1> ;
  owl:versionInfo "1" ;
  skos:altLabel "Porche HSS"@en ;
  skos:broader <http://vocab.nerc.ac.uk/collection/L05/current/67> ;
  skos:definition "Comprises 4 nets and one intake.  The nets rotate into the water flow position to collect a sample. Instrument reference is in French."@en ;
  skos:inScheme <http://vocab.nerc.ac.uk/scheme/SDNDEV/current> ;
  skos:notation "SDN:L22::NETT0068" ;
  skos:note "accepted"@en ;
  skos:prefLabel "High-speed multiple sampler - Porche (1978)"@en ;
.
inst:NETT0071
  rdf:type skos:Concept ;
  dcterm:date "2011-10-21 14:18:49.0" ;
  dcterm:identifier "SDN:L22::NETT0071" ;
  pav:hasCurrentVersion <http://vocab.nerc.ac.uk/collection/L22/current/NETT0071/1> ;
  owl:versionInfo "1" ;
  skos:altLabel "IKMT"@en ;
  skos:broader <http://vocab.nerc.ac.uk/collection/L05/current/23> ;
  skos:definition "A trawl with a pentagonal mouth opening and a dihedral depressor vane as part of the mouth opening. The original IKMTs were 10 foot (304 cm), and 15 foot (457 cm) at the mouth. The 10 foot IKMT net was 31 feet (9.45 m) in length [Wiebe and Benfield 2003 Plate 3 D]."@en ;
  skos:inScheme <http://vocab.nerc.ac.uk/scheme/SDNDEV/current> ;
  skos:notation "SDN:L22::NETT0071" ;
  skos:note "accepted"@en ;
  skos:prefLabel "Isaacs-Kidd Midwater Trawl  - Isaacs and Kidd (1953)"@en ;
.
inst:NETT0072
  rdf:type skos:Concept ;
  dcterm:date "2011-10-21 14:18:49.0" ;
  dcterm:identifier "SDN:L22::NETT0072" ;
  pav:hasCurrentVersion <http://vocab.nerc.ac.uk/collection/L22/current/NETT0072/1> ;
  owl:versionInfo "1" ;
  skos:altLabel "Pearcy modified IKMT"@en ;
  skos:broader <http://vocab.nerc.ac.uk/collection/L05/current/23> ;
  skos:broader <http://vocab.nerc.ac.uk/collection/L05/current/68> ;
  skos:definition "A 1.8 m IKMT fitted with a scaled down version of the Be MPS with 3 nets attached to the back of the trawl.  A pressure-release system controls the opening/closing of the cod-end nets [Wiebe and Benfield 2003 Plate 26 B]."@en ;
  skos:inScheme <http://vocab.nerc.ac.uk/scheme/SDNDEV/current> ;
  skos:notation "SDN:L22::NETT0072" ;
  skos:note "accepted"@en ;
  skos:prefLabel "Modified Isaacs-Kidd Midwater Trawl with MPS cod-end - Pearcy and Hubbard (1964)"@en ;
.
inst:NETT0073
  rdf:type skos:Concept ;
  dcterm:date "2011-10-21 14:18:49.0" ;
  dcterm:identifier "SDN:L22::NETT0073" ;
  pav:hasCurrentVersion <http://vocab.nerc.ac.uk/collection/L22/current/NETT0073/1> ;
  owl:versionInfo "1" ;
  skos:altLabel "Brown modified IKMT"@en ;
  skos:broader <http://vocab.nerc.ac.uk/collection/L05/current/23> ;
  skos:broader <http://vocab.nerc.ac.uk/collection/L05/current/68> ;
  skos:definition "An IKMT was outfitted with a flap of material that extended from the net mouth to the back end of the net and a 3-stage cod end.  At the start of a haul the flap was down and animals collect in stage 1 of the cod end. A timer released the flap which rode to the top of the net and animals collected in the stage II cod end.  A second timer release caused the stage II cod end to be pursed and it was replaced with the stage III cod end."@en ;
  skos:inScheme <http://vocab.nerc.ac.uk/scheme/SDNDEV/current> ;
  skos:notation "SDN:L22::NETT0073" ;
  skos:note "accepted"@en ;
  skos:prefLabel "Modified opening-closing Isaacs-Kidd Midwater Trawl - Brown (1975)"@en ;
.
inst:NETT0074
  rdf:type skos:Concept ;
  dcterm:date "2011-10-21 14:18:49.0" ;
  dcterm:identifier "SDN:L22::NETT0074" ;
  pav:hasCurrentVersion <http://vocab.nerc.ac.uk/collection/L22/current/NETT0074/1> ;
  owl:versionInfo "1" ;
  skos:altLabel "ICES standard net"@en ;
  skos:broader <http://vocab.nerc.ac.uk/collection/L05/current/22> ;
  skos:definition "Net has 50 cm diameter mouth with 60 cm cylindrical portion of 1 cm mesh,  200 cm conical section of silk (No. 25 or No 3).  This net is used for both vertical and horizontal closing tows (based on the Nansen net). A unique way to avoid ship motion described using two davits and a counter balancing weight [Wiebe and Benfield 2003 Plate 1 D]."@en ;
  skos:inScheme <http://vocab.nerc.ac.uk/scheme/SDNDEV/current> ;
  skos:notation "SDN:L22::NETT0074" ;
  skos:note "accepted"@en ;
  skos:prefLabel "International Council for the Exploration of the Seas standard net - Ostenfeld and Jespersen  (1924)"@en ;
.
inst:NETT0075
  rdf:type skos:Concept ;
  dcterm:date "2011-10-21 14:18:49.0" ;
  dcterm:identifier "SDN:L22::NETT0075" ;
  pav:hasCurrentVersion <http://vocab.nerc.ac.uk/collection/L22/current/NETT0075/1> ;
  owl:versionInfo "1" ;
  skos:altLabel "IOS net"@en ;
  skos:broader <http://vocab.nerc.ac.uk/collection/L05/current/22> ;
  skos:definition "Net has a 113 cm diameter mouth with 3 cylinder sections 70 cm (12.5 mm mesh), 30 cm (sail cloth, and 100 cm (0.330 mm nylon mesh) and a conical section 300 cm (0.333 mm mesh). No closing mechanism is used in standard haul. Flowmeter use is recommended.  It was based on the Discovery N 100 net.  Used during the UK NIO Indian Ocean Expedition of the 1960s [Wiebe and Benfield 2003 Plate 1 G]."@en ;
  skos:inScheme <http://vocab.nerc.ac.uk/scheme/SDNDEV/current> ;
  skos:notation "SDN:L22::NETT0075" ;
  skos:note "accepted"@en ;
  skos:prefLabel "Indian Ocean standard net - Currie (1963)"@en ;
.
inst:NETT0077
  rdf:type skos:Concept ;
  dcterm:date "2011-10-21 14:18:49.0" ;
  dcterm:identifier "SDN:L22::NETT0077" ;
  pav:hasCurrentVersion <http://vocab.nerc.ac.uk/collection/L22/current/NETT0077/1> ;
  owl:versionInfo "1" ;
  skos:altLabel "Aksnes modified Juday net"@en ;
  skos:broader <http://vocab.nerc.ac.uk/collection/L05/current/22> ;
  skos:definition "A pair of Juday nets with 40 cm diameter mouth openings were mounted on a frame 50 cm apart. Mesh of nets 0.18 mm. Designed to be towed vertically."@en ;
  skos:inScheme <http://vocab.nerc.ac.uk/scheme/SDNDEV/current> ;
  skos:notation "SDN:L22::NETT0077" ;
  skos:note "accepted"@en ;
  skos:prefLabel "Modified Juday net - Aksnes and Magnesen (1983)"@en ;
.
inst:NETT0078
  rdf:type skos:Concept ;
  dcterm:date "2011-10-21 14:18:49.0" ;
  dcterm:identifier "SDN:L22::NETT0078" ;
  pav:hasCurrentVersion <http://vocab.nerc.ac.uk/collection/L22/current/NETT0078/1> ;
  owl:versionInfo "1" ;
  skos:altLabel "Juday net"@en ;
  skos:broader <http://vocab.nerc.ac.uk/collection/L05/current/22> ;
  skos:definition "Net has a 25 cm diameter mouth opening with 33 cm long canvas cone expanding to 30 cm diameter, followed by a conical net 70 cm long made of No 20 silk bolting cloth [Wiebe and Benfield 2003 Plate 1 C]. A closing net with simple messenger release is also described: this has a 12 cm diameter mouth opening with 40 cm long canvas cone expanding to 17 cm, followed by a 47 cm long conical net with the same mesh."@en ;
  skos:inScheme <http://vocab.nerc.ac.uk/scheme/SDNDEV/current> ;
  skos:notation "SDN:L22::NETT0078" ;
  skos:note "accepted"@en ;
  skos:prefLabel "Juday net - Juday (1916)"@en ;
.
inst:NETT0079
  rdf:type skos:Concept ;
  dcterm:date "2011-10-21 14:18:49.0" ;
  dcterm:identifier "SDN:L22::NETT0079" ;
  pav:hasCurrentVersion <http://vocab.nerc.ac.uk/collection/L22/current/NETT0079/1> ;
  owl:versionInfo "1" ;
  skos:altLabel "Clayton modified Juday net."@en ;
  skos:broader <http://vocab.nerc.ac.uk/collection/L05/current/22> ;
  skos:definition "A net designed to avoid surface contamination of the sample. Construction is a 75 cm diameter cylinder (120 cm length) and cone (290 cm length), net (Nitex mesh size not given) with a cylinder skirt 380 cm long to enclose the net mesh.  The net ring and netting are enclosed in nylon utility cloth and tied with a release line that is pulled free after the net is underwater.  A messenger used to close net [Wiebe and Benfield 2003 Plate 7 B, C]."@en ;
  skos:inScheme <http://vocab.nerc.ac.uk/scheme/SDNDEV/current> ;
  skos:notation "SDN:L22::NETT0079" ;
  skos:note "accepted"@en ;
  skos:prefLabel "Modified Juday net  - Clayton and Pavlou (1978)"@en ;
.
inst:NETT0080
  rdf:type skos:Concept ;
  dcterm:date "2011-10-21 14:18:49.0" ;
  dcterm:identifier "SDN:L22::NETT0080" ;
  pav:hasCurrentVersion <http://vocab.nerc.ac.uk/collection/L22/current/NETT0080/1> ;
  owl:versionInfo "1" ;
  skos:altLabel "Kitahara"@en ;
  skos:broader <http://vocab.nerc.ac.uk/collection/L05/current/22> ;
  skos:definition "Net has a 24 cm diameter mouth opening for head piece and 45 cm diameter conical net 80 cm long. A Hensen style net (KT)"@en ;
  skos:inScheme <http://vocab.nerc.ac.uk/scheme/SDNDEV/current> ;
  skos:notation "SDN:L22::NETT0080" ;
  skos:note "accepted"@en ;
  skos:prefLabel "Kitahara - Nakai (1962)"@en ;
.
inst:NETT0090
  rdf:type skos:Concept ;
  dcterm:date "2011-10-21 14:18:49.0" ;
  dcterm:identifier "SDN:L22::NETT0090" ;
  pav:hasCurrentVersion <http://vocab.nerc.ac.uk/collection/L22/current/NETT0090/1> ;
  owl:versionInfo "1" ;
  skos:altLabel "Maruchi nets"@en ;
  skos:broader <http://vocab.nerc.ac.uk/collection/L05/current/22> ;
  skos:definition "Construction comprises a 130 cm diameter mouth opening with 450 cm long net. There were a series of variants MCA-MCE."@en ;
  skos:inScheme <http://vocab.nerc.ac.uk/scheme/SDNDEV/current> ;
  skos:notation "SDN:L22::NETT0090" ;
  skos:note "accepted"@en ;
  skos:prefLabel "Maruchi conical nets - Nakai (1962)"@en ;
.
inst:NETT0091
  rdf:type skos:Concept ;
  dcterm:date "2011-10-21 14:18:49.0" ;
  dcterm:identifier "SDN:L22::NETT0091" ;
  pav:hasCurrentVersion <http://vocab.nerc.ac.uk/collection/L22/current/NETT0091/1> ;
  owl:versionInfo "1" ;
  skos:altLabel "Marudai"@en ;
  skos:broader <http://vocab.nerc.ac.uk/collection/L05/current/22> ;
  skos:definition "Construction comprises a 250 cm diameter mouth opening with 800 cm long net.  A series of variants designed to sample megaplankton and nekton (MDA, MDB, PMD)"@en ;
  skos:inScheme <http://vocab.nerc.ac.uk/scheme/SDNDEV/current> ;
  skos:notation "SDN:L22::NETT0091" ;
  skos:note "accepted"@en ;
  skos:prefLabel "Marudai - Nakai (1962)"@en ;
.
inst:NETT0092
  rdf:type skos:Concept ;
  dcterm:date "2011-10-21 14:18:49.0" ;
  dcterm:identifier "SDN:L22::NETT0092" ;
  pav:hasCurrentVersion <http://vocab.nerc.ac.uk/collection/L22/current/NETT0092/1> ;
  owl:versionInfo "1" ;
  skos:altLabel "Marunaka"@en ;
  skos:broader <http://vocab.nerc.ac.uk/collection/L05/current/22> ;
  skos:definition "Has a 60 cm diameter mouth opening  cylinder/cone design. Cylinder coarse mesh (3.3 cm) 33 cm long.  Conical portion silk net 150 cm long. Can accommodate flowmeter. Sometimes rigged as Nansen closing net. Variants listed as MNA, MNB."@en ;
  skos:inScheme <http://vocab.nerc.ac.uk/scheme/SDNDEV/current> ;
  skos:notation "SDN:L22::NETT0092" ;
  skos:note "accepted"@en ;
  skos:prefLabel "Marunaka - Nakai (1962)"@en ;
.
inst:NETT0095
  rdf:type skos:Concept ;
  dcterm:date "2011-10-21 14:18:49.0" ;
  dcterm:identifier "SDN:L22::NETT0095" ;
  pav:hasCurrentVersion <http://vocab.nerc.ac.uk/collection/L22/current/NETT0095/1> ;
  owl:versionInfo "1" ;
  skos:altLabel "Fowler midwater net"@en ;
  skos:broader <http://vocab.nerc.ac.uk/collection/L05/current/22> ;
  skos:definition "A 11.4 cm x 11.4 cm rectangular net mouth frame which was hinged at the central axis.  It was equipped with a silk net ( 9.8 or 15.7 meshes per cm) which was enclosed by a similar net made from mosquito netting. This net was sent down closed, opened by a messenger and closed by a second one.  Designed for vertical towing."@en ;
  skos:inScheme <http://vocab.nerc.ac.uk/scheme/SDNDEV/current> ;
  skos:notation "SDN:L22::NETT0095" ;
  skos:note "accepted"@en ;
  skos:prefLabel "Midwater net - Fowler (1898)"@en ;
.
inst:NETT0096
  rdf:type skos:Concept ;
  dcterm:date "2011-10-21 14:18:49.0" ;
  dcterm:identifier "SDN:L22::NETT0096" ;
  pav:hasCurrentVersion <http://vocab.nerc.ac.uk/collection/L22/current/NETT0096/1> ;
  owl:versionInfo "1" ;
  skos:altLabel "Zaitsev MNT"@en ;
  skos:broader <http://vocab.nerc.ac.uk/collection/L05/current/69> ;
  skos:definition "Construction is an elliptical metal frame 100 cm wide x 50 cm tall with a net 400 cm long made of netting with Nos. 21-23 meshes. Two plastic foam floats (25 cm x 12 cm x 8 cm) are attached to each side of the net frame. The net is towed in a circle at about 4 knots."@en ;
  skos:inScheme <http://vocab.nerc.ac.uk/scheme/SDNDEV/current> ;
  skos:notation "SDN:L22::NETT0096" ;
  skos:note "accepted"@en ;
  skos:prefLabel "Midwater neuston trawl - Zaitsev (1970)"@en ;
.
inst:NETT0098
  rdf:type skos:Concept ;
  dcterm:date "2011-10-21 14:18:49.0" ;
  dcterm:identifier "SDN:L22::NETT0098" ;
  pav:hasCurrentVersion <http://vocab.nerc.ac.uk/collection/L22/current/NETT0098/1> ;
  owl:versionInfo "1" ;
  skos:altLabel "Weikert modified MPS"@en ;
  skos:broader <http://vocab.nerc.ac.uk/collection/L05/current/22> ;
  skos:broader <http://vocab.nerc.ac.uk/collection/L05/current/68> ;
  skos:definition "A modified version of the Be MPS net with a rectangular sampler box 50 cm x 50 cm on a side and 60 cm deep equipped with 5 nets (0.3 mm mesh) each 250 cm long.  Nets are opened and closed electronically through conducting cable and pressure is monitored. No flowmeter used [Wiebe and Benfield 2003 Plate 31 A, B]."@en ;
  skos:inScheme <http://vocab.nerc.ac.uk/scheme/SDNDEV/current> ;
  skos:notation "SDN:L22::NETT0098" ;
  skos:note "accepted"@en ;
  skos:prefLabel "Modified Multiple Plankton Sampler - Weikert and John (1981)"@en ;
.
inst:NETT0100
  rdf:type skos:Concept ;
  dcterm:date "2011-10-21 14:18:49.0" ;
  dcterm:identifier "SDN:L22::NETT0100" ;
  pav:hasCurrentVersion <http://vocab.nerc.ac.uk/collection/L22/current/NETT0100/1> ;
  owl:versionInfo "1" ;
  skos:altLabel "MTD horizontal net"@en ;
  skos:broader <http://vocab.nerc.ac.uk/collection/L05/current/22> ;
  skos:definition "Comprises a 56 cm diameter cylinder (80 cm length and cone (110 cm length) net mounted on wire with a triangular framework so that up to 10 can be towed simultaneously. Has a closing system that inverts the forward portion of the net and draws mid-net section tight. A flowmeter can provide approximate volumes filtered. Mesh size not given [Wiebe and Benfield 2003 Plate 8 D]."@en ;
  skos:inScheme <http://vocab.nerc.ac.uk/scheme/SDNDEV/current> ;
  skos:notation "SDN:L22::NETT0100" ;
  skos:note "accepted"@en ;
  skos:prefLabel "MTD horizontal net - Motoda (1971)"@en ;
.
inst:NETT0102
  rdf:type skos:Concept ;
  dcterm:date "2011-10-21 14:18:49.0" ;
  dcterm:identifier "SDN:L22::NETT0102" ;
  pav:hasCurrentVersion <http://vocab.nerc.ac.uk/collection/L22/current/NETT0102/1> ;
  owl:versionInfo "1" ;
  skos:altLabel "N100"@en ;
  skos:broader <http://vocab.nerc.ac.uk/collection/L05/current/22> ;
  skos:definition "Cylinder-cone net structure. The cylinder is 100 cm diameter  by 107 cm long with a 1.27 cm mesh. The cone has two sections one 107 cm long with 4 mm mesh, and the other 213 cm long with 5.9 meshes per cm or stramin."@en ;
  skos:inScheme <http://vocab.nerc.ac.uk/scheme/SDNDEV/current> ;
  skos:notation "SDN:L22::NETT0102" ;
  skos:note "accepted"@en ;
  skos:prefLabel "N100 - Kemp et al. (1929); Marr (1938)"@en ;
.
inst:NETT0103
  rdf:type skos:Concept ;
  dcterm:date "2011-10-21 14:18:49.0" ;
  dcterm:identifier "SDN:L22::NETT0103" ;
  pav:hasCurrentVersion <http://vocab.nerc.ac.uk/collection/L22/current/NETT0103/1> ;
  owl:versionInfo "1" ;
  skos:altLabel "N200"@en ;
  skos:broader <http://vocab.nerc.ac.uk/collection/L05/current/22> ;
  skos:definition "Cylinder-cone net structure. The cylinder is 200 cm diameter by 213 cm long with a 2.54 cm mesh 213 cm long. The cone has two sections one 198 cm long with 7 mm mesh, and the other 396 cm long with 4 mm mesh."@en ;
  skos:inScheme <http://vocab.nerc.ac.uk/scheme/SDNDEV/current> ;
  skos:notation "SDN:L22::NETT0103" ;
  skos:note "accepted"@en ;
  skos:prefLabel "N200 - Kemp et al. (1929); Marr (1938)"@en ;
.
inst:NETT0104
  rdf:type skos:Concept ;
  dcterm:date "2011-10-21 14:18:49.0" ;
  dcterm:identifier "SDN:L22::NETT0104" ;
  pav:hasCurrentVersion <http://vocab.nerc.ac.uk/collection/L22/current/NETT0104/1> ;
  owl:versionInfo "1" ;
  skos:altLabel "N450"@en ;
  skos:broader <http://vocab.nerc.ac.uk/collection/L05/current/22> ;
  skos:definition "Cylinder-cone net structure with four sections. The cylinder is 450cm diameter by 457 cm long with a 3.8 cm mesh. The cone is  1371 cm long with three equal length sections with 1.27 cm mesh, 0.7 cm mesh, and 0.7 cm mesh with 0.4 cm mesh liner respectively. Used either as open net or with a messenger device that closed the net about half way back to the cod end while still allowing the net ring to tow normally.  Depth recording instrument used on the net."@en ;
  skos:inScheme <http://vocab.nerc.ac.uk/scheme/SDNDEV/current> ;
  skos:notation "SDN:L22::NETT0104" ;
  skos:note "accepted"@en ;
  skos:prefLabel "N450 - Kemp et al. (1929); Marr (1938)"@en ;
.
inst:NETT0105
  rdf:type skos:Concept ;
  dcterm:date "2011-10-21 14:18:49.0" ;
  dcterm:identifier "SDN:L22::NETT0105" ;
  pav:hasCurrentVersion <http://vocab.nerc.ac.uk/collection/L22/current/NETT0105/1> ;
  owl:versionInfo "1" ;
  skos:altLabel "N50"@en ;
  skos:broader <http://vocab.nerc.ac.uk/collection/L05/current/22> ;
  skos:definition "Cylinder-cone net structure. The cylinder is 50 cm diameter by 66 cm long made of canvas. The cone is 65 cm long made of silk netting of 78 meshes /cm."@en ;
  skos:inScheme <http://vocab.nerc.ac.uk/scheme/SDNDEV/current> ;
  skos:notation "SDN:L22::NETT0105" ;
  skos:note "accepted"@en ;
  skos:prefLabel "N50 - Kemp et al. (1929); Marr (1938)"@en ;
.
inst:NETT0106
  rdf:type skos:Concept ;
  dcterm:date "2011-10-21 14:18:49.0" ;
  dcterm:identifier "SDN:L22::NETT0106" ;
  pav:hasCurrentVersion <http://vocab.nerc.ac.uk/collection/L22/current/NETT0106/1> ;
  owl:versionInfo "1" ;
  skos:altLabel "N70"@en ;
  skos:broader <http://vocab.nerc.ac.uk/collection/L05/current/22> ;
  skos:definition "Cylinder-cone net structure. The cylinder is 70 cm diameter by 53 cm long with  0.64 cm mesh.  The cone has two sections: one 96.5 cm long with 15.74 threads per cm, and the other 134.6 cm long with 29.1 threads per cm."@en ;
  skos:inScheme <http://vocab.nerc.ac.uk/scheme/SDNDEV/current> ;
  skos:notation "SDN:L22::NETT0106" ;
  skos:note "accepted"@en ;
  skos:prefLabel "N70 - Kemp et al. (1929)"@en ;
.
inst:NETT0108
  rdf:type skos:Concept ;
  dcterm:date "2011-10-21 14:18:49.0" ;
  dcterm:identifier "SDN:L22::NETT0108" ;
  pav:hasCurrentVersion <http://vocab.nerc.ac.uk/collection/L22/current/NETT0108/1> ;
  owl:versionInfo "1" ;
  skos:altLabel "Discovery net"@en ;
  skos:broader <http://vocab.nerc.ac.uk/collection/L05/current/22> ;
  skos:definition "A version of the Nansen net with a 70 cm diameter mouth opening with 3 nearly cylindrical net sections and a final conical section. Section 1 with .63 cm mesh, section 2 canvas for closing rope, section 3 made of silk with 40 meshes per inch (15.7 meshes per 1 cm), and  section 4 made of silk with 74 meshes per inch (29.1 meshes per 1 cm)"@en ;
  skos:inScheme <http://vocab.nerc.ac.uk/scheme/SDNDEV/current> ;
  skos:notation "SDN:L22::NETT0108" ;
  skos:note "accepted"@en ;
  skos:prefLabel "Discovery net N70 V net - Currie and Foxton (1956)"@en ;
.
inst:NETT0109
  rdf:type skos:Concept ;
  dcterm:date "2011-10-21 14:18:49.0" ;
  dcterm:identifier "SDN:L22::NETT0109" ;
  pav:hasCurrentVersion <http://vocab.nerc.ac.uk/collection/L22/current/NETT0109/1> ;
  owl:versionInfo "1" ;
  skos:altLabel "Nackthai net"@en ;
  skos:broader <http://vocab.nerc.ac.uk/collection/L05/current/67> ;
  skos:definition "A modified Gulf V sampler with a 20 cm diameter nose cone aperture expanding to 38 cm diameter over length of 53 cm. Attached to back of cone is a net 120 cm long.  Frame work in which net supported 45 cm x 45 cm x 190 cm long. Overall length 143 cm. A comparison was made between the Hai and the Nackthai samplers which showed the Nackthai filtered more water and caught significantly more plankton and fish a result attributed to its non-encased net [Wiebe and Benfield 2003 Plate 16 E]."@en ;
  skos:inScheme <http://vocab.nerc.ac.uk/scheme/SDNDEV/current> ;
  skos:notation "SDN:L22::NETT0109" ;
  skos:note "accepted"@en ;
  skos:prefLabel "Nackthai net - Nellen and Hempel (1969)"@en ;
.
inst:NETT0111
  rdf:type skos:Concept ;
  dcterm:date "2011-10-21 14:18:49.0" ;
  dcterm:identifier "SDN:L22::NETT0111" ;
  pav:hasCurrentVersion <http://vocab.nerc.ac.uk/collection/L22/current/NETT0111/1> ;
  owl:versionInfo "1" ;
  skos:altLabel "Ellertsen neuston net"@en ;
  skos:broader <http://vocab.nerc.ac.uk/collection/L05/current/69> ;
  skos:definition "Six stacked nets two with 10 cm tall x 25 cm wide rectangular mouth opening and four with 20 cm tall x 25 cm wide mouths. Nets 100 cm long made of 0.2 mm nylon mesh. Pontoons made of fiberglass covered Styrofoam 10 x 15 x 100 cm. A flowmeter can be used [Wiebe and Benfield 2003 Plate 21 C]."@en ;
  skos:inScheme <http://vocab.nerc.ac.uk/scheme/SDNDEV/current> ;
  skos:notation "SDN:L22::NETT0111" ;
  skos:note "accepted"@en ;
  skos:prefLabel "Neuston net - Ellertsen (1977)"@en ;
.
inst:NETT0112
  rdf:type skos:Concept ;
  dcterm:date "2011-10-21 14:18:49.0" ;
  dcterm:identifier "SDN:L22::NETT0112" ;
  pav:hasCurrentVersion <http://vocab.nerc.ac.uk/collection/L22/current/NETT0112/1> ;
  owl:versionInfo "1" ;
  skos:altLabel "Sconfietti neuston net"@en ;
  skos:broader <http://vocab.nerc.ac.uk/collection/L05/current/69> ;
  skos:definition "A 40 cm diameter net (60 cm long) is attached at the front and rear to a polyurethane float by rods extending down below the float with the top of net about 12 cm below the surface.  [Wiebe and Benfield 2003 Plate 20 F]"@en ;
  skos:inScheme <http://vocab.nerc.ac.uk/scheme/SDNDEV/current> ;
  skos:notation "SDN:L22::NETT0112" ;
  skos:note "accepted"@en ;
  skos:prefLabel "Neuston net - Sconfietti and Cantonati (1990)"@en ;
.
inst:NETT0113
  rdf:type skos:Concept ;
  dcterm:date "2011-10-21 14:18:49.0" ;
  dcterm:identifier "SDN:L22::NETT0113" ;
  pav:hasCurrentVersion <http://vocab.nerc.ac.uk/collection/L22/current/NETT0113/1> ;
  owl:versionInfo "1" ;
  skos:altLabel "David neuston net"@en ;
  skos:broader <http://vocab.nerc.ac.uk/collection/L05/current/69> ;
  skos:definition "Has a 30 cm x 15 cm rectangular mouth opening with a net 365 cm in length (21.3 meshes to cm). Normally towed at 5-6 knots [Wiebe and Benfield 2003 Plate 20 D]."@en ;
  skos:inScheme <http://vocab.nerc.ac.uk/scheme/SDNDEV/current> ;
  skos:notation "SDN:L22::NETT0113" ;
  skos:note "accepted"@en ;
  skos:prefLabel "Neuston net - David (1965)"@en ;
.
inst:NETT0114
  rdf:type skos:Concept ;
  dcterm:date "2011-10-21 14:18:49.0" ;
  dcterm:identifier "SDN:L22::NETT0114" ;
  pav:hasCurrentVersion <http://vocab.nerc.ac.uk/collection/L22/current/NETT0114/1> ;
  owl:versionInfo "1" ;
  skos:altLabel "Zaitsev neuston net"@en ;
  skos:broader <http://vocab.nerc.ac.uk/collection/L05/current/69> ;
  skos:definition "Has a 60cm x 20 cm rectangular mouth aperture with a net 250 cm long with plastic foam floats 20 cm x 10 cm x 4 cm attached to sides of metal net frame.  Used from drifting or anchored vessel [Wiebe and Benfield 2003 Plate 20 A]."@en ;
  skos:inScheme <http://vocab.nerc.ac.uk/scheme/SDNDEV/current> ;
  skos:notation "SDN:L22::NETT0114" ;
  skos:note "accepted"@en ;
  skos:prefLabel "Neuston net - Zaitsev (1959, 1970)"@en ;
.
inst:NETT0115
  rdf:type skos:Concept ;
  dcterm:date "2011-10-21 14:18:49.0" ;
  dcterm:identifier "SDN:L22::NETT0115" ;
  pav:hasCurrentVersion <http://vocab.nerc.ac.uk/collection/L22/current/NETT0115/1> ;
  owl:versionInfo "1" ;
  skos:altLabel "Schram neuston net"@en ;
  skos:broader <http://vocab.nerc.ac.uk/collection/L05/current/69> ;
  skos:definition "Neuston sampling system with three nets having a 60x20 cm rectangular mouth and 250 cm long."@en ;
  skos:inScheme <http://vocab.nerc.ac.uk/scheme/SDNDEV/current> ;
  skos:notation "SDN:L22::NETT0115" ;
  skos:note "accepted"@en ;
  skos:prefLabel "Mini-neuston net - Schram et al. (1981)"@en ;
.
inst:NETT0116
  rdf:type skos:Concept ;
  dcterm:date "2011-10-21 14:18:49.0" ;
  dcterm:identifier "SDN:L22::NETT0116" ;
  pav:hasCurrentVersion <http://vocab.nerc.ac.uk/collection/L22/current/NETT0116/1> ;
  owl:versionInfo "1" ;
  skos:altLabel "Willis neuston net"@en ;
  skos:broader <http://vocab.nerc.ac.uk/collection/L05/current/69> ;
  skos:definition "Has a 17.8 cm x 3.8 cm rectangular mouth opening of net 67.3 cm long (netting nylon with 78.7 meshes/cm).  Normally towed while ship drifting at 1 knot [Wiebe and Benfield 2003 Plate 20 C]."@en ;
  skos:inScheme <http://vocab.nerc.ac.uk/scheme/SDNDEV/current> ;
  skos:notation "SDN:L22::NETT0116" ;
  skos:note "accepted"@en ;
  skos:prefLabel "Neuston net - Willis (1963)"@en ;
.
inst:NETT0118
  rdf:type skos:Concept ;
  dcterm:date "2014-11-12 11:29:50.0" ;
  dcterm:identifier "SDN:L22::NETT0118" ;
  pav:hasCurrentVersion <http://vocab.nerc.ac.uk/collection/L22/current/NETT0118/2> ;
  pav:hasVersion <http://vocab.nerc.ac.uk/collection/L22/current/NETT0118/1> ;
  owl:versionInfo "2" ;
  skos:altLabel "Sameoto neuston sampler"@en ;
  skos:broader <http://vocab.nerc.ac.uk/collection/L05/current/69> ;
  skos:definition "Has a 102 cm x 102 cm square mouth opening aluminium box frame 152 cm long equipped with foam floatation on top, a pair of fins on the side, and a fin on the bottom.  Attached to the back is a net 104 cm x 104 cm at the mouth and 927 cm long made from 0.308 mm nylon mesh. A two-part towing bridle was attached to one side and the sampler kited out away from the side of the vessel beyond the ships wake. Towing speeds 8 to 11 knots [Wiebe and Benfield 2003 Plate 20 E]."@en ;
  skos:inScheme <http://vocab.nerc.ac.uk/scheme/SDNDEV/current> ;
  skos:notation "SDN:L22::NETT0118" ;
  skos:note "accepted"@en ;
  skos:prefLabel "Neuston sampler - Sameoto and Jaroszynski (1969)"@en ;
.
inst:NETT0122
  rdf:type skos:Concept ;
  dcterm:date "2011-10-21 14:18:49.0" ;
  dcterm:identifier "SDN:L22::NETT0122" ;
  pav:hasCurrentVersion <http://vocab.nerc.ac.uk/collection/L22/current/NETT0122/1> ;
  owl:versionInfo "1" ;
  skos:altLabel "NorPac net"@en ;
  skos:broader <http://vocab.nerc.ac.uk/collection/L05/current/22> ;
  skos:definition "Has a 45 cm mouth diameter with a conical net length of 180 cm (mesh 0.33 mm - GG54) [Wiebe and Benfield 2003 Plate 1 F]."@en ;
  skos:inScheme <http://vocab.nerc.ac.uk/scheme/SDNDEV/current> ;
  skos:notation "SDN:L22::NETT0122" ;
  skos:note "accepted"@en ;
  skos:prefLabel "North Pacific standard net  - Motoda (1957)"@en ;
.
inst:NETT0124
  rdf:type skos:Concept ;
  dcterm:date "2011-10-21 14:18:49.0" ;
  dcterm:identifier "SDN:L22::NETT0124" ;
  pav:hasCurrentVersion <http://vocab.nerc.ac.uk/collection/L22/current/NETT0124/1> ;
  owl:versionInfo "1" ;
  skos:altLabel "N-series nets"@en ;
  skos:broader <http://vocab.nerc.ac.uk/collection/L05/current/22> ;
  skos:definition "Cylinder-cone nets of varying sizes that were used in conjunction and towed either vertically, horizontally or obliquely depending upon size. All could be closed. N50 and N70  were similar in size and mesh to Hjort net [Wiebe and Benfield 2003 Plate 1 E].  Grouping term for N50, N70, N100, N200 and N450 nets."@en ;
  skos:inScheme <http://vocab.nerc.ac.uk/scheme/SDNDEV/current> ;
  skos:notation "SDN:L22::NETT0124" ;
  skos:note "accepted"@en ;
  skos:prefLabel "N-series (N50, N70, N100, N200, N450) nets - Kemp et al. (1929); Marr (1938)"@en ;
.
inst:NETT0125
  rdf:type skos:Concept ;
  dcterm:date "2011-10-21 14:18:49.0" ;
  dcterm:identifier "SDN:L22::NETT0125" ;
  pav:hasCurrentVersion <http://vocab.nerc.ac.uk/collection/L22/current/NETT0125/1> ;
  owl:versionInfo "1" ;
  skos:altLabel "Sameoto octagon net"@en ;
  skos:broader <http://vocab.nerc.ac.uk/collection/L05/current/22> ;
  skos:broader <http://vocab.nerc.ac.uk/collection/L05/current/67> ;
  skos:definition "Has a 75 cm diameter iron channel octagon mouth opening which was attached to the towing wire with stainless steel snap swivels and held from sliding down by a stop on the wire. Used with a net made of 1 mm nylon mesh and towed at speeds up to 7 knots [Wiebe and Benfield 2003 Plate 3 C]."@en ;
  skos:inScheme <http://vocab.nerc.ac.uk/scheme/SDNDEV/current> ;
  skos:notation "SDN:L22::NETT0125" ;
  skos:note "accepted"@en ;
  skos:prefLabel "Octagon net - Sameoto and Jaroszynski (1976)"@en ;
.
inst:NETT0126
  rdf:type skos:Concept ;
  dcterm:date "2011-10-21 14:18:49.0" ;
  dcterm:identifier "SDN:L22::NETT0126" ;
  pav:hasCurrentVersion <http://vocab.nerc.ac.uk/collection/L22/current/NETT0126/1> ;
  owl:versionInfo "1" ;
  skos:altLabel "Bourdillon mechanism"@en ;
  skos:broader <http://vocab.nerc.ac.uk/collection/L05/current/22> ;
  skos:definition "A double messenger system to allow a ring net to be sent down closed, opened at depth, and then closed again by a second messenger [Wiebe and Benfield 2003 Plate 7 A]"@en ;
  skos:inScheme <http://vocab.nerc.ac.uk/scheme/SDNDEV/current> ;
  skos:notation "SDN:L22::NETT0126" ;
  skos:note "accepted"@en ;
  skos:prefLabel "Opening-closing mechanism for plankton nets - Bourdillon et al. (1978)"@en ;
.
inst:NETT0127
  rdf:type skos:Concept ;
  dcterm:date "2011-10-21 14:18:49.0" ;
  dcterm:identifier "SDN:L22::NETT0127" ;
  pav:hasCurrentVersion <http://vocab.nerc.ac.uk/collection/L22/current/NETT0127/1> ;
  owl:versionInfo "1" ;
  skos:altLabel "Hoyle opening-closing net"@en ;
  skos:broader <http://vocab.nerc.ac.uk/collection/L05/current/22> ;
  skos:definition "A 61 cm diameter conical net (muslin or silk). No other dimensions given. Proposed electrical activation to open/close net [Wiebe and Benfield 2003 Plate 5 C]."@en ;
  skos:inScheme <http://vocab.nerc.ac.uk/scheme/SDNDEV/current> ;
  skos:notation "SDN:L22::NETT0127" ;
  skos:note "accepted"@en ;
  skos:prefLabel "Opening-closing net - Hoyle (1889)"@en ;
.
inst:NETT0128
  rdf:type skos:Concept ;
  dcterm:date "2011-10-21 14:18:49.0" ;
  dcterm:identifier "SDN:L22::NETT0128" ;
  pav:hasCurrentVersion <http://vocab.nerc.ac.uk/collection/L22/current/NETT0128/1> ;
  owl:versionInfo "1" ;
  skos:altLabel "Leavitt opening-closing net"@en ;
  skos:broader <http://vocab.nerc.ac.uk/collection/L05/current/22> ;
  skos:definition "100, 150, and 200 cm diameter nets made of scrim, silk, and stramin respectively. Net dimensions not given [Wiebe and Benfield 2003 Plate 6 A]."@en ;
  skos:inScheme <http://vocab.nerc.ac.uk/scheme/SDNDEV/current> ;
  skos:notation "SDN:L22::NETT0128" ;
  skos:note "accepted"@en ;
  skos:prefLabel "Opening-closing net system  - Leavitt (1935, 1938)"@en ;
.
inst:NETT0129
  rdf:type skos:Concept ;
  dcterm:date "2011-10-21 14:18:49.0" ;
  dcterm:identifier "SDN:L22::NETT0129" ;
  pav:hasCurrentVersion <http://vocab.nerc.ac.uk/collection/L22/current/NETT0129/1> ;
  owl:versionInfo "1" ;
  skos:altLabel "Bigelow opening-closing net"@en ;
  skos:broader <http://vocab.nerc.ac.uk/collection/L05/current/22> ;
  skos:definition "A hinged ring to which a net with 75 cm diameter mouth was attached. System sent down with ring closed and opened with a messenger. A second messenger released the ring and a draw-string closed the net off."@en ;
  skos:inScheme <http://vocab.nerc.ac.uk/scheme/SDNDEV/current> ;
  skos:notation "SDN:L22::NETT0129" ;
  skos:note "accepted"@en ;
  skos:prefLabel "Horizontal opening-closing net - Bigelow (1913)"@en ;
.
inst:NETT0131
  rdf:type skos:Concept ;
  dcterm:date "2011-10-21 14:18:49.0" ;
  dcterm:identifier "SDN:L22::NETT0131" ;
  pav:hasCurrentVersion <http://vocab.nerc.ac.uk/collection/L22/current/NETT0131/1> ;
  owl:versionInfo "1" ;
  skos:altLabel "ORI nets"@en ;
  skos:broader <http://vocab.nerc.ac.uk/collection/L05/current/22> ;
  skos:definition "Generic term for 160 cm cylinder-cone nets equipped for a Motoda double releasing mechanism."@en ;
  skos:inScheme <http://vocab.nerc.ac.uk/scheme/SDNDEV/current> ;
  skos:notation "SDN:L22::NETT0131" ;
  skos:note "accepted"@en ;
  skos:prefLabel "ORI nets - Omori (1965)"@en ;
.
inst:NETT0132
  rdf:type skos:Concept ;
  dcterm:date "2011-10-21 14:18:49.0" ;
  dcterm:identifier "SDN:L22::NETT0132" ;
  pav:hasCurrentVersion <http://vocab.nerc.ac.uk/collection/L22/current/NETT0132/1> ;
  owl:versionInfo "1" ;
  skos:altLabel "ORI-200 net"@en ;
  skos:broader <http://vocab.nerc.ac.uk/collection/L05/current/22> ;
  skos:definition "Has a 160 cm diameter mouth opening with 2x70 cm long cylinder sections plus 2 conical sections 450 cm. All 1.97 mm mesh. Equipped for a Motoda double releasing mechanism."@en ;
  skos:inScheme <http://vocab.nerc.ac.uk/scheme/SDNDEV/current> ;
  skos:notation "SDN:L22::NETT0132" ;
  skos:note "accepted"@en ;
  skos:prefLabel "ORI-200 - Omori (1965)"@en ;
.
inst:NETT0133
  rdf:type skos:Concept ;
  dcterm:date "2011-10-21 14:18:49.0" ;
  dcterm:identifier "SDN:L22::NETT0133" ;
  pav:hasCurrentVersion <http://vocab.nerc.ac.uk/collection/L22/current/NETT0133/1> ;
  owl:versionInfo "1" ;
  skos:altLabel "ORI-C net"@en ;
  skos:broader <http://vocab.nerc.ac.uk/collection/L05/current/22> ;
  skos:definition "Has a 160 cm diameter mouth opening with 2x70 cm long cylinder sections made of 1.97 mm mesh and sail cloth plus 2 conical sections 450 cm (1.97 mm mesh) and 150 cm (.33 mm mesh). Equipped for a Motoda double releasing mechanism."@en ;
  skos:inScheme <http://vocab.nerc.ac.uk/scheme/SDNDEV/current> ;
  skos:notation "SDN:L22::NETT0133" ;
  skos:note "accepted"@en ;
  skos:prefLabel "ORI-C - Omori (1965)"@en ;
.
inst:NETT0134
  rdf:type skos:Concept ;
  dcterm:date "2011-10-21 14:18:49.0" ;
  dcterm:identifier "SDN:L22::NETT0134" ;
  pav:hasCurrentVersion <http://vocab.nerc.ac.uk/collection/L22/current/NETT0134/1> ;
  owl:versionInfo "1" ;
  skos:altLabel "ORI-VMPS"@en ;
  skos:broader <http://vocab.nerc.ac.uk/collection/L05/current/22> ;
  skos:broader <http://vocab.nerc.ac.uk/collection/L05/current/68> ;
  skos:definition "Has a 100 cm x 100 cm rectangular mouth opening multiple net system that can be equipped with 4 to 10 nets 510 cm long with 0.33 mm nylon mesh.  Nets are opened/closed by surface commands down transmitted via conduction cable to an underwater unit [Wiebe and Benfield 2003 Plate 31 C]."@en ;
  skos:inScheme <http://vocab.nerc.ac.uk/scheme/SDNDEV/current> ;
  skos:notation "SDN:L22::NETT0134" ;
  skos:note "accepted"@en ;
  skos:prefLabel "Ocean Research Institute Vertical Muliple Plankton Sampler - Terazaki (1991)"@en ;
.
inst:NETT0135
  rdf:type skos:Concept ;
  dcterm:date "2011-10-21 14:18:49.0" ;
  dcterm:identifier "SDN:L22::NETT0135" ;
  pav:hasCurrentVersion <http://vocab.nerc.ac.uk/collection/L22/current/NETT0135/1> ;
  owl:versionInfo "1" ;
  skos:altLabel "Parachute net"@en ;
  skos:broader <http://vocab.nerc.ac.uk/collection/L05/current/22> ;
  skos:definition "This has a 275 cm diameter parachute opening tapering over a distance of 350 cm to a 100 cm diameter mosquito netting net.  Free fall to bottom with concrete weights, released by salt block dissolution, and floated backwards to surface with gasoline float [Wiebe and Benfield 2003 Plate 11 B]."@en ;
  skos:inScheme <http://vocab.nerc.ac.uk/scheme/SDNDEV/current> ;
  skos:notation "SDN:L22::NETT0135" ;
  skos:note "accepted"@en ;
  skos:prefLabel "Parachute net - Wheeler (1941)"@en ;
.
inst:NETT0136
  rdf:type skos:Concept ;
  dcterm:date "2011-10-21 14:18:49.0" ;
  dcterm:identifier "SDN:L22::NETT0136" ;
  pav:hasCurrentVersion <http://vocab.nerc.ac.uk/collection/L22/current/NETT0136/1> ;
  owl:versionInfo "1" ;
  skos:altLabel "Henderson MPI"@en ;
  skos:broader <http://vocab.nerc.ac.uk/collection/L05/current/22> ;
  skos:definition "This indicator had a body length of 33 cm, a diameter of 3.8 cm, an aperture diameter of 1.27 cm, a filter disc of 2.54 cm in diameter and was towed at about 2 knots [Wiebe and Benfield 2003 Plate 13 F]."@en ;
  skos:inScheme <http://vocab.nerc.ac.uk/scheme/SDNDEV/current> ;
  skos:notation "SDN:L22::NETT0136" ;
  skos:note "accepted"@en ;
  skos:prefLabel "Miniature Plankton Indicator  - Henderson et al. (1936); Glover (1953)"@en ;
.
inst:NETT0137
  rdf:type skos:Concept ;
  dcterm:date "2011-10-21 14:18:49.0" ;
  dcterm:identifier "SDN:L22::NETT0137" ;
  pav:hasCurrentVersion <http://vocab.nerc.ac.uk/collection/L22/current/NETT0137/1> ;
  owl:versionInfo "1" ;
  skos:altLabel "Johannes plankton net"@en ;
  skos:broader <http://vocab.nerc.ac.uk/collection/L05/current/22> ;
  skos:definition "A pair of 50 cm diameter nets made from number 10 gauze were mounted side by side in a rectangular frame with an extender rod to support the net cod ends horizontally .  The nets and frame were attached 100 cm above the bottom to a wire extending from an anchor stand to a surface float. The nets were free to rotate so that they always faced into the flow [Wiebe and Benfield 2003 Plate 24 B]."@en ;
  skos:inScheme <http://vocab.nerc.ac.uk/scheme/SDNDEV/current> ;
  skos:notation "SDN:L22::NETT0137" ;
  skos:note "accepted"@en ;
  skos:prefLabel "Fixed in-current plankton net - Johannes et al (1970)"@en ;
.
inst:NETT0138
  rdf:type skos:Concept ;
  dcterm:date "2011-10-21 14:18:49.0" ;
  dcterm:identifier "SDN:L22::NETT0138" ;
  pav:hasCurrentVersion <http://vocab.nerc.ac.uk/collection/L22/current/NETT0138/1> ;
  owl:versionInfo "1" ;
  skos:altLabel "Murphy plankton purse seine"@en ;
  skos:broader <http://vocab.nerc.ac.uk/collection/L05/current/22> ;
  skos:definition "A miniature purse seine 3048 cm long x 640 cm tall with netting of 0.333 mm nylon mesh [Wiebe and Benfield 2003 Plate 12 C]."@en ;
  skos:inScheme <http://vocab.nerc.ac.uk/scheme/SDNDEV/current> ;
  skos:notation "SDN:L22::NETT0138" ;
  skos:note "accepted"@en ;
  skos:prefLabel "Plankton purse seine  - Murphy and Clutter (1972)"@en ;
.
inst:NETT0139
  rdf:type skos:Concept ;
  dcterm:date "2011-10-21 14:18:49.0" ;
  dcterm:identifier "SDN:L22::NETT0139" ;
  pav:hasCurrentVersion <http://vocab.nerc.ac.uk/collection/L22/current/NETT0139/1> ;
  owl:versionInfo "1" ;
  skos:altLabel "Glover plankton sampler"@en ;
  skos:broader <http://vocab.nerc.ac.uk/collection/L05/current/67> ;
  skos:definition "This is a small high-speed sampler (similar to the Hardy Standard Plankton Indicator and the Miniature Plankton Indicator) with a 1.9 cm diameter aperture opening, 3.2 cm diameter internal net and 8.9 cm long, and a 30.5 cm overall length [Wiebe and Benfield 2003 Plate 14 A]."@en ;
  skos:inScheme <http://vocab.nerc.ac.uk/scheme/SDNDEV/current> ;
  skos:notation "SDN:L22::NETT0139" ;
  skos:note "accepted"@en ;
  skos:prefLabel "Small plankton sampler - Glover (1953)"@en ;
.
inst:NETT0140
  rdf:type skos:Concept ;
  dcterm:date "2011-10-21 14:18:49.0" ;
  dcterm:identifier "SDN:L22::NETT0140" ;
  pav:hasCurrentVersion <http://vocab.nerc.ac.uk/collection/L22/current/NETT0140/1> ;
  owl:versionInfo "1" ;
  skos:altLabel "Plankton-Bar"@en ;
  skos:broader <http://vocab.nerc.ac.uk/collection/L05/current/22> ;
  skos:definition "A device for continuously sampling plankton from several depths simultaneously using a combination of ~18 cm diameter nets with 38 meshes per cm and a pumping system.  Five nets with equidistant spacing on a towing wire were normally used [Wiebe and Benfield 2003 Plate 11 D]."@en ;
  skos:inScheme <http://vocab.nerc.ac.uk/scheme/SDNDEV/current> ;
  skos:notation "SDN:L22::NETT0140" ;
  skos:note "accepted"@en ;
  skos:prefLabel "Plankton-Bar - Tonolli (1951)"@en ;
.
inst:NETT0141
  rdf:type skos:Concept ;
  dcterm:date "2011-10-21 14:18:49.0" ;
  dcterm:identifier "SDN:L22::NETT0141" ;
  pav:hasCurrentVersion <http://vocab.nerc.ac.uk/collection/L22/current/NETT0141/1> ;
  owl:versionInfo "1" ;
  skos:altLabel "Beauchamp planktonbenthos dredge"@en ;
  skos:broader <http://vocab.nerc.ac.uk/collection/L05/current/22> ;
  skos:broader <http://vocab.nerc.ac.uk/collection/L05/current/24> ;
  skos:definition "A simple pair of U-shaped runners were connected by two cross struts which supported a net which collected animals living  just above the bottom. No opening/closing mechanism was present."@en ;
  skos:inScheme <http://vocab.nerc.ac.uk/scheme/SDNDEV/current> ;
  skos:notation "SDN:L22::NETT0141" ;
  skos:note "accepted"@en ;
  skos:prefLabel "Planktonbenthos dredge - Beauchamp (1932)"@en ;
.
inst:NETT0142
  rdf:type skos:Concept ;
  dcterm:date "2011-10-21 14:18:49.0" ;
  dcterm:identifier "SDN:L22::NETT0142" ;
  pav:hasCurrentVersion <http://vocab.nerc.ac.uk/collection/L22/current/NETT0142/1> ;
  owl:versionInfo "1" ;
  skos:altLabel "Hensen planktonbenthos sampler"@en ;
  skos:broader <http://vocab.nerc.ac.uk/collection/L05/current/22> ;
  skos:broader <http://vocab.nerc.ac.uk/collection/L05/current/24> ;
  skos:definition "An eight wheeled carriage-like sled with a net mounted in between the third and fourth pairs of wheels. [Wiebe and Benfield 2003 Plate 22 A]"@en ;
  skos:inScheme <http://vocab.nerc.ac.uk/scheme/SDNDEV/current> ;
  skos:notation "SDN:L22::NETT0142" ;
  skos:note "accepted"@en ;
  skos:prefLabel "Planktonbenthos sampler - Hensen (1895)"@en ;
.
inst:NETT0143
  rdf:type skos:Concept ;
  dcterm:date "2011-10-21 14:18:49.0" ;
  dcterm:identifier "SDN:L22::NETT0143" ;
  pav:hasCurrentVersion <http://vocab.nerc.ac.uk/collection/L22/current/NETT0143/1> ;
  owl:versionInfo "1" ;
  skos:altLabel "Hovekamp-Daly plummet net"@en ;
  skos:broader <http://vocab.nerc.ac.uk/collection/L05/current/22> ;
  skos:definition "Construction has a 100 cm diameter mouth with a lead weighted net ring and net with 0.571 mm mesh. For downward collecting, the net was lowered by the cod-end to a pre-determined depth and a messenger used to release the cod-end attachment and draw tight a choke collar near the mouth of the net [Wiebe and Benfield 2003 Plate 9 D]."@en ;
  skos:inScheme <http://vocab.nerc.ac.uk/scheme/SDNDEV/current> ;
  skos:notation "SDN:L22::NETT0143" ;
  skos:note "accepted"@en ;
  skos:prefLabel "Plummet net - Hovekamp ; Daly [personal communication to Wiebe and Benfield]"@en ;
.
inst:NETT0144
  rdf:type skos:Concept ;
  dcterm:date "2011-10-21 14:18:49.0" ;
  dcterm:identifier "SDN:L22::NETT0144" ;
  pav:hasCurrentVersion <http://vocab.nerc.ac.uk/collection/L22/current/NETT0144/1> ;
  owl:versionInfo "1" ;
  skos:altLabel "Hovekamp-Daly plummet net type II"@en ;
  skos:broader <http://vocab.nerc.ac.uk/collection/L05/current/22> ;
  skos:definition "A downward-fishing, vertical, closing plummet net with a 1-m2 rectangular mouth opening with a net that is attached to two bars that run along a pair of net bar glides along parallel sides.  A double messenger system is used to opened the net as it falls to depth and to close it as it reaches the bottom of the haul.  The net ~ 180 cm in length has been used with a variety of mesh sizes; 0.163 mm, 0.560 mm, and 1600 mm Nitex.  According to Daly [personal communication], the first messenger releases a bridle attached to the opening net bar under tension from a shock cord.  The second messenger releases two bridles, one attached to the back of the net frame and the other attached to the closing net bar.  The net frame assumes a vertical position, allowing the second net bar to fall, closing the net, and retrieval is begun."@en ;
  skos:inScheme <http://vocab.nerc.ac.uk/scheme/SDNDEV/current> ;
  skos:notation "SDN:L22::NETT0144" ;
  skos:note "accepted"@en ;
  skos:prefLabel "Plummet net type II - Hovekamp (1989) and Daly [personal communication to Wiebe and Benfield]"@en ;
.
inst:NETT0145
  rdf:type skos:Concept ;
  dcterm:date "2011-10-21 14:18:49.0" ;
  dcterm:identifier "SDN:L22::NETT0145" ;
  pav:hasCurrentVersion <http://vocab.nerc.ac.uk/collection/L22/current/NETT0145/1> ;
  owl:versionInfo "1" ;
  skos:altLabel "Zaitsev PNS"@en ;
  skos:broader <http://vocab.nerc.ac.uk/collection/L05/current/69> ;
  skos:definition "A five-stage sampling frame with a height of 100 cm and width of 60 cm in which five 60cm x 20 cm rectangular mouth aperture nets are stacked. Nets and frame flotation similar to that described by Zaitsev . Used from drifting or anchored vessel."@en ;
  skos:inScheme <http://vocab.nerc.ac.uk/scheme/SDNDEV/current> ;
  skos:notation "SDN:L22::NETT0145" ;
  skos:note "accepted"@en ;
  skos:prefLabel "PNS neuston net - Zaitsev (1961, 1970)"@en ;
.
inst:NETT0147
  rdf:type skos:Concept ;
  dcterm:date "2011-10-21 14:18:49.0" ;
  dcterm:identifier "SDN:L22::NETT0147" ;
  pav:hasCurrentVersion <http://vocab.nerc.ac.uk/collection/L22/current/NETT0147/1> ;
  owl:versionInfo "1" ;
  skos:altLabel "Reeve Net"@en ;
  skos:broader <http://vocab.nerc.ac.uk/collection/L05/current/22> ;
  skos:definition "A very large acrylic cylindrical cod end (30 litres) attached to a simple ring net or a paired net system (with 75 cm diameter nets) to collect fragile gelatinous animals (with 17-litre cod ends). Also describes a pressure activated mechanism to enable the nets to float up the wire to the surface without being affected by the motion of the vessel [Wiebe and Benfield 2003 Plate 3 E, F]."@en ;
  skos:inScheme <http://vocab.nerc.ac.uk/scheme/SDNDEV/current> ;
  skos:notation "SDN:L22::NETT0147" ;
  skos:note "accepted"@en ;
  skos:prefLabel "Reeve net - Reeve (1981)"@en ;
.
inst:NETT0150
  rdf:type skos:Concept ;
  dcterm:date "2011-10-21 14:18:49.0" ;
  dcterm:identifier "SDN:L22::NETT0150" ;
  pav:hasCurrentVersion <http://vocab.nerc.ac.uk/collection/L22/current/NETT0150/1> ;
  owl:versionInfo "1" ;
  skos:altLabel "RMT 8"@en ;
  skos:broader <http://vocab.nerc.ac.uk/collection/L05/current/23> ;
  skos:definition "A 283 cm x 400 cm rectangular flexible mouth opening with 5 mm mesh net 1188 cm long. Net mouth is opened and closed acoustically. Pinger used to determine depth."@en ;
  skos:inScheme <http://vocab.nerc.ac.uk/scheme/SDNDEV/current> ;
  skos:notation "SDN:L22::NETT0150" ;
  skos:note "accepted"@en ;
  skos:prefLabel "Tucker-style opening-closing Rectangular Midwater Trawl 8 - Clarke (1969)"@en ;
.
inst:NETT0151
  rdf:type skos:Concept ;
  dcterm:date "2011-10-21 14:18:49.0" ;
  dcterm:identifier "SDN:L22::NETT0151" ;
  pav:hasCurrentVersion <http://vocab.nerc.ac.uk/collection/L22/current/NETT0151/1> ;
  owl:versionInfo "1" ;
  skos:altLabel "Scotia net"@en ;
  skos:broader <http://vocab.nerc.ac.uk/collection/L05/current/22> ;
  skos:definition "Essentially like the Nansen net (construction has a 35 to 100 cm net diameter 50 cm cylindrical portion of canvas; 150 cm long conical section of silk)."@en ;
  skos:inScheme <http://vocab.nerc.ac.uk/scheme/SDNDEV/current> ;
  skos:notation "SDN:L22::NETT0151" ;
  skos:note "accepted"@en ;
  skos:prefLabel "Scotia closing plankton net - Bruce (1904)"@en ;
.
inst:NETT0153
  rdf:type skos:Concept ;
  dcterm:date "2011-10-21 14:18:49.0" ;
  dcterm:identifier "SDN:L22::NETT0153" ;
  pav:hasCurrentVersion <http://vocab.nerc.ac.uk/collection/L22/current/NETT0153/1> ;
  owl:versionInfo "1" ;
  skos:altLabel "Kofoid self-closing net"@en ;
  skos:broader <http://vocab.nerc.ac.uk/collection/L05/current/22> ;
  skos:definition "Has a 37 cm net diameter. Conical silk bolting cloth net (nos. 12 to 20) about 200 cm long.  Two hinged jaws in the mouth of the net swing forward and downward. Each is activated by a messenger to open then close the net mouth. Used at the end to a cable for horizontal/oblique towing [Wiebe and Benfield 2003 Plate 5D]."@en ;
  skos:inScheme <http://vocab.nerc.ac.uk/scheme/SDNDEV/current> ;
  skos:notation "SDN:L22::NETT0153" ;
  skos:note "accepted"@en ;
  skos:prefLabel "Horizontal self-closing net - Kofoid (1911, 1911, 1912)"@en ;
.
inst:NETT0154
  rdf:type skos:Concept ;
  dcterm:date "2011-10-21 14:18:49.0" ;
  dcterm:identifier "SDN:L22::NETT0154" ;
  pav:hasCurrentVersion <http://vocab.nerc.ac.uk/collection/L22/current/NETT0154/1> ;
  owl:versionInfo "1" ;
  skos:altLabel "Standard Plankton Indicator HSS"@en ;
  skos:broader <http://vocab.nerc.ac.uk/collection/L05/current/67> ;
  skos:definition "Originally had a 10.1 cm diameter mouth opening expanding to 17.8 cm diameter main body. Overall length 91.4 cm.  In modified form with 3.8 cm diameter aperture opening, 7.6 cm diameter filter disc, 56 cm overall length, and with depressor and stabilizing fins.  Normal towing speed 8 knots [Wiebe and Benfield 2003 Plate 13 D,E]."@en ;
  skos:inScheme <http://vocab.nerc.ac.uk/scheme/SDNDEV/current> ;
  skos:notation "SDN:L22::NETT0154" ;
  skos:note "accepted"@en ;
  skos:prefLabel "Standard Plankton Indicator high-speed sampler - Hardy (1926, 1936); Glover (1953)"@en ;
.
inst:NETT0155
  rdf:type skos:Concept ;
  dcterm:date "2011-10-21 14:18:49.0" ;
  dcterm:identifier "SDN:L22::NETT0155" ;
  pav:hasCurrentVersion <http://vocab.nerc.ac.uk/collection/L22/current/NETT0155/1> ;
  owl:versionInfo "1" ;
  skos:altLabel "Ishida streamer sampler"@en ;
  skos:broader <http://vocab.nerc.ac.uk/collection/L05/current/22> ;
  skos:definition "A 45 cm diameter mouth opening with a closing door and a metal cylinder 45 cm long to which is attached a net of 5 meters length.  The sampler sinks with closing door open flushing the net. When halted attached line lifted, the door closes and end of net is closed capturing a 600 litre sample [Wiebe and Benfield 2003 Plate 10 E]."@en ;
  skos:inScheme <http://vocab.nerc.ac.uk/scheme/SDNDEV/current> ;
  skos:notation "SDN:L22::NETT0155" ;
  skos:note "accepted"@en ;
  skos:prefLabel "Streamer Plankton sampler - Ishida (1963, 1964)"@en ;
.
inst:NETT0161
  rdf:type skos:Concept ;
  dcterm:date "2011-10-21 14:18:49.0" ;
  dcterm:identifier "SDN:L22::NETT0161" ;
  pav:hasCurrentVersion <http://vocab.nerc.ac.uk/collection/L22/current/NETT0161/1> ;
  owl:versionInfo "1" ;
  skos:altLabel "Tucker Trawl"@en ;
  skos:broader <http://vocab.nerc.ac.uk/collection/L05/current/23> ;
  skos:definition "Has a  183 cm x 183 cm flexible rectangular net mouth. 914 cm long net with 1.8 cm streched mesh for first 457 cm and 1.3 cm mesh for last 457 cm. 152 cm of coarse plankton or muslin netting lined the end of the net. System equipped with mechanical time/depth recorder [Wiebe and Benfield 2003 Plate 4 A, B]."@en ;
  skos:inScheme <http://vocab.nerc.ac.uk/scheme/SDNDEV/current> ;
  skos:notation "SDN:L22::NETT0161" ;
  skos:note "accepted"@en ;
  skos:prefLabel "Tucker Trawl - Tucker (1951)"@en ;
.
inst:NETT0162
  rdf:type skos:Concept ;
  dcterm:date "2011-10-21 14:18:49.0" ;
  dcterm:identifier "SDN:L22::NETT0162" ;
  pav:hasCurrentVersion <http://vocab.nerc.ac.uk/collection/L22/current/NETT0162/1> ;
  owl:versionInfo "1" ;
  skos:altLabel "Davis modified Tucker Trawl"@en ;
  skos:broader <http://vocab.nerc.ac.uk/collection/L05/current/23> ;
  skos:definition "Modification used timing clocks to open and close the Tucker trawl mouth.  Net design modified from that described by Tucker so that first 500 cm of the net mesh was 1.1 cm Marlon netting and last 200 cm was 0.33 mm nylon mesh.  A depth-telemetering pinger used to monitor net depth during tow and a depth-time recorder used to make alternate record [Wiebe and Benfield 2003 Plate 9 E]."@en ;
  skos:inScheme <http://vocab.nerc.ac.uk/scheme/SDNDEV/current> ;
  skos:notation "SDN:L22::NETT0162" ;
  skos:note "accepted"@en ;
  skos:prefLabel "Opening-closing Tucker Trawl  - Davis and Barham (1969)"@en ;
.
inst:NETT0163
  rdf:type skos:Concept ;
  dcterm:date "2011-10-21 14:18:49.0" ;
  dcterm:identifier "SDN:L22::NETT0163" ;
  pav:hasCurrentVersion <http://vocab.nerc.ac.uk/collection/L22/current/NETT0163/1> ;
  owl:versionInfo "1" ;
  skos:altLabel "Umbrella net"@en ;
  skos:broader <http://vocab.nerc.ac.uk/collection/L05/current/22> ;
  skos:definition "A pair of nets attached to an umbrella-like support.  The system was deployed down a 12 cm ice hole and expanded below the undersurface of the ice. A circular motion caused the nets to scrap the undersurface of the ice and collect organisms in the water just below it. There was no flow meter or a description of the net specifications."@en ;
  skos:inScheme <http://vocab.nerc.ac.uk/scheme/SDNDEV/current> ;
  skos:notation "SDN:L22::NETT0163" ;
  skos:note "accepted"@en ;
  skos:prefLabel "Umbrella net - Rakusa-Suszczewski (1972)"@en ;
.
inst:NETT0164
  rdf:type skos:Concept ;
  dcterm:date "2011-10-21 14:18:49.0" ;
  dcterm:identifier "SDN:L22::NETT0164" ;
  pav:hasCurrentVersion <http://vocab.nerc.ac.uk/collection/L22/current/NETT0164/1> ;
  owl:versionInfo "1" ;
  skos:altLabel "Nansen net system"@en ;
  skos:broader <http://vocab.nerc.ac.uk/collection/L05/current/22> ;
  skos:definition "Construction has a 35 to 100 cm net diameter (but up to 300 cm for Murray and Hjort Expedition of 1910); 50 cm cylindrical portion of canvas; 150 cm long conical section of silk (no size given) [Wiebe and Benfield 2003 Plate 5 A]."@en ;
  skos:inScheme <http://vocab.nerc.ac.uk/scheme/SDNDEV/current> ;
  skos:notation "SDN:L22::NETT0164" ;
  skos:note "accepted"@en ;
  skos:prefLabel "Vertical and horizontal closing nets with flow meter - Nansen (1915)"@en ;
.
inst:NETT0165
  rdf:type skos:Concept ;
  dcterm:date "2011-10-21 14:18:49.0" ;
  dcterm:identifier "SDN:L22::NETT0165" ;
  pav:hasCurrentVersion <http://vocab.nerc.ac.uk/collection/L22/current/NETT0165/1> ;
  owl:versionInfo "1" ;
  skos:altLabel "VHSS"@en ;
  skos:broader <http://vocab.nerc.ac.uk/collection/L05/current/67> ;
  skos:definition "Rectangular mouth opening. Closed like a Juday net. Used No. 38 silk. Speeds up to 2.8 m/sec (5+ knots)"@en ;
  skos:inScheme <http://vocab.nerc.ac.uk/scheme/SDNDEV/current> ;
  skos:notation "SDN:L22::NETT0165" ;
  skos:note "accepted"@en ;
  skos:prefLabel "Vertical high-speed plankton net - Jaschnov (1961)"@en ;
.
inst:NETT0166
  rdf:type skos:Concept ;
  dcterm:date "2011-10-21 14:18:49.0" ;
  dcterm:identifier "SDN:L22::NETT0166" ;
  pav:hasCurrentVersion <http://vocab.nerc.ac.uk/collection/L22/current/NETT0166/1> ;
  owl:versionInfo "1" ;
  skos:altLabel "Kim modified Deep-Tow net system"@en ;
  skos:broader <http://vocab.nerc.ac.uk/collection/L05/current/22> ;
  skos:broader <http://vocab.nerc.ac.uk/collection/L05/current/68> ;
  skos:definition "Three rectangular mouth opening nets ~30 cm wide x 44 cm tall and 130 cm long mounted on a metal framework attached to the front instrument basket of DSRV Alvin. Sequential opening and closing of the nets done by the pilot using the manipulator arm."@en ;
  skos:inScheme <http://vocab.nerc.ac.uk/scheme/SDNDEV/current> ;
  skos:notation "SDN:L22::NETT0166" ;
  skos:note "accepted"@en ;
  skos:prefLabel "Wishner Deep-Tow net system adapted for use on Alvin - Kim and Mullineaux (1998)"@en ;
.
inst:NETT0167
  rdf:type skos:Concept ;
  dcterm:date "2011-10-21 14:18:49.0" ;
  dcterm:identifier "SDN:L22::NETT0167" ;
  pav:hasCurrentVersion <http://vocab.nerc.ac.uk/collection/L22/current/NETT0167/1> ;
  owl:versionInfo "1" ;
  skos:altLabel "Wollaston net"@en ;
  skos:broader <http://vocab.nerc.ac.uk/collection/L05/current/22> ;
  skos:definition "A 55 cm net opening diameter 34 cm long made of canvas; 25 cm diameter conical section 68 cm long made of silk netting (no size given).  [Wiebe and Benfield 2003 Plate 10 B]."@en ;
  skos:inScheme <http://vocab.nerc.ac.uk/scheme/SDNDEV/current> ;
  skos:notation "SDN:L22::NETT0167" ;
  skos:note "accepted"@en ;
  skos:prefLabel "Wollaston pop-down net - Buchanan-Wollaston (1911)"@en ;
.
inst:NETT0169
  rdf:type skos:Concept ;
  dcterm:date "2011-10-21 14:18:49.0" ;
  dcterm:identifier "SDN:L22::NETT0169" ;
  pav:hasCurrentVersion <http://vocab.nerc.ac.uk/collection/L22/current/NETT0169/1> ;
  owl:versionInfo "1" ;
  skos:altLabel "ORI-33 net"@en ;
  skos:broader <http://vocab.nerc.ac.uk/collection/L05/current/22> ;
  skos:definition "Has a 160 cm diameter mouth opening with 2x70 cm long cylinder sections plus 2 conical sections 450 cm. All GG 54 silk netting. Equipped for a Motoda double releasing mechanism."@en ;
  skos:inScheme <http://vocab.nerc.ac.uk/scheme/SDNDEV/current> ;
  skos:notation "SDN:L22::NETT0169" ;
  skos:note "accepted"@en ;
  skos:prefLabel "ORI-33 - Omori (1965)"@en ;
.
inst:NETT0171
  rdf:type skos:Concept ;
  dcterm:date "2012-09-25 14:08:12.0" ;
  dcterm:identifier "SDN:L22::NETT0171" ;
  pav:hasCurrentVersion <http://vocab.nerc.ac.uk/collection/L22/current/NETT0171/1> ;
  owl:versionInfo "1" ;
  skos:altLabel "OCEAN MKI"@en ;
  skos:broader <http://vocab.nerc.ac.uk/collection/L05/current/22> ;
  skos:definition "An oceanographic sampler designed to be towed behind a vessel. The sampler includes 4 nets which are controlled by acoustic signals from the towing ship. The system can be fitted with live codend buckets or codend bags. This version of the sampler has been supserseded."@en ;
  skos:inScheme <http://vocab.nerc.ac.uk/scheme/SDNDEV/current> ;
  skos:notation "SDN:L22::NETT0171" ;
  skos:note "accepted"@en ;
  skos:prefLabel "Marine Scotland Opening Closing Environmental Acoustic Net MKI"@en ;
.
inst:NETT0173
  rdf:type skos:Concept ;
  dcterm:date "2012-10-12 14:13:09.0" ;
  dcterm:identifier "SDN:L22::NETT0173" ;
  pav:hasCurrentVersion <http://vocab.nerc.ac.uk/collection/L22/current/NETT0173/1> ;
  owl:versionInfo "1" ;
  skos:altLabel "Plankton pump sampler"@en ;
  skos:broader <http://vocab.nerc.ac.uk/collection/L05/current/22> ;
  skos:definition "An in situ pump and net system for collecting plankton samples. Water is pumped at approximately 1.2 m^3 per minute through a mesh, and samples are collected in the net cod end. The device was used on research cruises in the late 1990s."@en ;
  skos:inScheme <http://vocab.nerc.ac.uk/scheme/SDNDEV/current> ;
  skos:notation "SDN:L22::NETT0173" ;
  skos:note "accepted"@en ;
  skos:prefLabel "Plankton pump sampler"@en ;
.
inst:NETT0174
  rdf:type skos:Concept ;
  dcterm:date "2014-09-12 17:20:07.0" ;
  dcterm:identifier "SDN:L22::NETT0174" ;
  pav:hasCurrentVersion <http://vocab.nerc.ac.uk/collection/L22/current/NETT0174/1> ;
  owl:versionInfo "1" ;
  skos:altLabel "KC Denmark 25 cm small plankton net"@en ;
  skos:broader <http://vocab.nerc.ac.uk/collection/L05/current/22> ;
  skos:definition "Construction has an upper cylindrical net made of strong Beaver Nylon with a diameter of 25 cm and a length of 15 cm. Below is a conical mesh net bag made of Monodur Nytal (Nylon) and is 40 cm deep.  The net is ended with a 35 ml or 80 ml (fitted with mesh windows) sample cylinder."@en ;
  skos:inScheme <http://vocab.nerc.ac.uk/scheme/SDNDEV/current> ;
  skos:notation "SDN:L22::NETT0174" ;
  skos:note "accepted"@en ;
  skos:prefLabel "KC Denmark AS small plankton net"@en ;
  skos:related <http://vocab.nerc.ac.uk/collection/B75/current/ORG00909> ;
.
inst:NETT0175
  rdf:type skos:Concept ;
  dcterm:date "2014-09-12 17:20:07.0" ;
  dcterm:identifier "SDN:L22::NETT0175" ;
  pav:hasCurrentVersion <http://vocab.nerc.ac.uk/collection/L22/current/NETT0175/1> ;
  owl:versionInfo "1" ;
  skos:altLabel "Lindahl sampling hose"@en ;
  skos:broader <http://vocab.nerc.ac.uk/collection/L05/current/30> ;
  skos:definition "A rubber hose (material may vary) comprising length sections which integrate water samples from selected depth intervals. The division of the hose is adapted as needed. The hose inner diameter is >12 mm. The hose end is weighted. The hose is slowly lowered into the water (20 m/min). The top valve is closed when the hose has reached maximum depth. Sections are sequentially closed with valves as they appear during ascent. A full description is available in https://www.bodc.ac.uk/data/documents/nodb/pdf/Lindahl_1986.pdf."@en ;
  skos:inScheme <http://vocab.nerc.ac.uk/scheme/SDNDEV/current> ;
  skos:notation "SDN:L22::NETT0175" ;
  skos:note "accepted"@en ;
  skos:prefLabel "Lindahl dividable phytoplankton sampling hose"@en ;
.
inst:NETT0176
  rdf:type skos:Concept ;
  dcterm:date "2018-01-09 13:29:51.0" ;
  dcterm:identifier "SDN:L22::NETT0176" ;
  pav:hasCurrentVersion <http://vocab.nerc.ac.uk/collection/L22/current/NETT0176/1> ;
  owl:versionInfo "1" ;
  skos:altLabel "Bongo"@en ;
  skos:broader <http://vocab.nerc.ac.uk/collection/L05/current/22> ;
  skos:definition "A generic term for a plankton net designed with double circular (ring, hoop or drum) mouth pieces; with further specifications either unknown or described elsewhere in the supporting metadata."@en ;
  skos:inScheme <http://vocab.nerc.ac.uk/scheme/SDNDEV/current> ;
  skos:notation "SDN:L22::NETT0176" ;
  skos:note "accepted"@en ;
  skos:prefLabel "Bongo net"@en ;
.
inst:NETT0177
  rdf:type skos:Concept ;
  dcterm:date "2018-01-09 13:29:51.0" ;
  dcterm:identifier "SDN:L22::NETT0177" ;
  pav:hasCurrentVersion <http://vocab.nerc.ac.uk/collection/L22/current/NETT0177/1> ;
  owl:versionInfo "1" ;
  skos:altLabel "Manta trawl"@en ;
  skos:broader <http://vocab.nerc.ac.uk/collection/L05/current/22> ;
  skos:broader <http://vocab.nerc.ac.uk/collection/L05/current/69> ;
  skos:definition "A generic term for a net system designed for sampling the surface of the ocean. Based on the original design by Brown and Cheng 1981, it has a single rectangular mouth piece and a pair of wings that ride the sea surface; further specifications are either unknown or described elsewhere in the supporting metadata."@en ;
  skos:inScheme <http://vocab.nerc.ac.uk/scheme/SDNDEV/current> ;
  skos:notation "SDN:L22::NETT0177" ;
  skos:note "accepted"@en ;
  skos:prefLabel "Manta net"@en ;
.
inst:NETT0178
  rdf:type skos:Concept ;
  dcterm:date "2018-01-30 16:59:47.0" ;
  dcterm:identifier "SDN:L22::NETT0178" ;
  pav:hasCurrentVersion <http://vocab.nerc.ac.uk/collection/L22/current/NETT0178/1> ;
  owl:versionInfo "1" ;
  skos:altLabel "BAS RMT1"@en ;
  skos:broader <http://vocab.nerc.ac.uk/collection/L05/current/23> ;
  skos:definition "A British Antarctic Survey-built pelagic trawl system, mainly used to catch zooplankton. The RMT system is operated in combination with the down-wire net monitor, a custom-built electronic system that enables two-way communications between the net and controllers aboard the ship. The net has a mouth opening of 1 m^2."@en ;
  skos:inScheme <http://vocab.nerc.ac.uk/scheme/SDNDEV/current> ;
  skos:notation "SDN:L22::NETT0178" ;
  skos:note "accepted"@en ;
  skos:prefLabel "British Antarctic Survey Rectangular Midwater Trawl 1"@en ;
  skos:related <http://vocab.nerc.ac.uk/collection/B75/current/ORG0015> ;
.
inst:NETT0179
  rdf:type skos:Concept ;
  dcterm:date "2018-01-30 16:59:47.0" ;
  dcterm:identifier "SDN:L22::NETT0179" ;
  pav:hasCurrentVersion <http://vocab.nerc.ac.uk/collection/L22/current/NETT0179/1> ;
  owl:versionInfo "1" ;
  skos:altLabel "BAS RMT1+8"@en ;
  skos:broader <http://vocab.nerc.ac.uk/collection/L05/current/23> ;
  skos:broader <http://vocab.nerc.ac.uk/collection/L05/current/68> ;
  skos:definition "A British Antarctic Survey-built pelagic trawl system, composed of a combination of RMT1 and RMT8 nets. The RMT1 net is best suited to catch zooplankton, while the RMT8 net is used to catch krill. The RMT system is operated in combination with the down-wire net monitor, a custom-built electronic system that enables two-way communications between the net and controllers aboard the ship. The nets have mouth openings of 1 m^2 (RMT1) and 8 m^2 (RMT8)."@en ;
  skos:inScheme <http://vocab.nerc.ac.uk/scheme/SDNDEV/current> ;
  skos:notation "SDN:L22::NETT0179" ;
  skos:note "accepted"@en ;
  skos:prefLabel "British Antarctic Survey Rectangular Midwater Trawl 1+8"@en ;
  skos:related <http://vocab.nerc.ac.uk/collection/B75/current/ORG0015> ;
.
inst:NETT0180
  rdf:type skos:Concept ;
  dcterm:date "2018-01-30 16:59:47.0" ;
  dcterm:identifier "SDN:L22::NETT0180" ;
  pav:hasCurrentVersion <http://vocab.nerc.ac.uk/collection/L22/current/NETT0180/1> ;
  owl:versionInfo "1" ;
  skos:altLabel "BAS RMT8"@en ;
  skos:broader <http://vocab.nerc.ac.uk/collection/L05/current/23> ;
  skos:definition "A British Antarctic Survey-built pelagic trawl system, mainly used to catch krill. The RMT system is operated in combination with the down-wire net monitor, a custom-built electronic system that enables two-way communications between the net and controllers aboard the ship. The net has a mouth opening of 8 m^2."@en ;
  skos:inScheme <http://vocab.nerc.ac.uk/scheme/SDNDEV/current> ;
  skos:notation "SDN:L22::NETT0180" ;
  skos:note "accepted"@en ;
  skos:prefLabel "British Antarctic Survey Rectangular Midwater Trawl 8"@en ;
  skos:related <http://vocab.nerc.ac.uk/collection/B75/current/ORG0015> ;
.
inst:NETT0181
  rdf:type skos:Concept ;
  dcterm:date "2018-01-30 16:59:47.0" ;
  dcterm:identifier "SDN:L22::NETT0181" ;
  pav:hasCurrentVersion <http://vocab.nerc.ac.uk/collection/L22/current/NETT0181/1> ;
  owl:versionInfo "1" ;
  skos:altLabel "BAS RMT25"@en ;
  skos:broader <http://vocab.nerc.ac.uk/collection/L05/current/23> ;
  skos:definition "A British Antarctic Survey-built pelagic trawl system, best suited to catch fish. For targeted sampling in specific swarms or water layers, two nets can be used independently. The RMT system is operated in combination with the down-wire net monitor, a custom-built electronic system that enables two-way communications between the net and controllers aboard the ship. The net has a mouth opening of 25 m^2, and weighs around 1000 kg."@en ;
  skos:inScheme <http://vocab.nerc.ac.uk/scheme/SDNDEV/current> ;
  skos:notation "SDN:L22::NETT0181" ;
  skos:note "accepted"@en ;
  skos:prefLabel "British Antarctic Survey Rectangular Midwater Trawl 25"@en ;
  skos:related <http://vocab.nerc.ac.uk/collection/B75/current/ORG0015> ;
.
inst:NETT0182
  rdf:type skos:Concept ;
  dcterm:date "2018-01-30 16:59:47.0" ;
  dcterm:identifier "SDN:L22::NETT0182" ;
  pav:hasCurrentVersion <http://vocab.nerc.ac.uk/collection/L22/current/NETT0182/1> ;
  owl:versionInfo "1" ;
  skos:altLabel "BAS EBS"@en ;
  skos:broader <http://vocab.nerc.ac.uk/collection/L05/current/24> ;
  skos:definition "A British Antarctic Survey-built sledge, designed to be towed along the seabed to stir up the top layer of sediment and collect organisms living just above the seafloor. The EBS has a stainless steel metal frame with two nets built in, and two doors at the front, which are operated by a mechanical leaver to ensure accurate sampling."@en ;
  skos:inScheme <http://vocab.nerc.ac.uk/scheme/SDNDEV/current> ;
  skos:notation "SDN:L22::NETT0182" ;
  skos:note "accepted"@en ;
  skos:prefLabel "British Antarctic Survey Epi-benthic Sledge"@en ;
  skos:related <http://vocab.nerc.ac.uk/collection/B75/current/ORG0015> ;
.
inst:NETT0183
  rdf:type skos:Concept ;
  dcterm:date "2018-01-30 16:59:47.0" ;
  dcterm:identifier "SDN:L22::NETT0183" ;
  pav:hasCurrentVersion <http://vocab.nerc.ac.uk/collection/L22/current/NETT0183/1> ;
  owl:versionInfo "1" ;
  skos:altLabel "RBOT"@en ;
  skos:broader <http://vocab.nerc.ac.uk/collection/L05/current/61> ;
  skos:definition "A cone-shaped net kept opened horizontally by two otter boards, and vertically by floats on the upper edge (floatline) and weights on the groundrope. The groundrope is also equipped with bobbins to prevent the leading margin of the trawl from being damaged; on particularly rough grounds, special rock hopper gears are used. Codend mesh size varies depending on species of fish sampled. The net is connected to the ship by a steel cable."@en ;
  skos:inScheme <http://vocab.nerc.ac.uk/scheme/SDNDEV/current> ;
  skos:notation "SDN:L22::NETT0183" ;
  skos:note "accepted"@en ;
  skos:prefLabel "Rough Bottom Otter Trawl"@en ;
.
inst:NETT0184
  rdf:type skos:Concept ;
  dcterm:date "2018-01-30 16:59:47.0" ;
  dcterm:identifier "SDN:L22::NETT0184" ;
  pav:hasCurrentVersion <http://vocab.nerc.ac.uk/collection/L22/current/NETT0184/1> ;
  owl:versionInfo "1" ;
  skos:altLabel "BAS CPR"@en ;
  skos:broader <http://vocab.nerc.ac.uk/collection/L05/current/21> ;
  skos:definition "A British Antarctic Survey-built plankton sampling instrument, designed to be towed from a ship at a depth of approximately 10 m. Water passes through the CPR, and plankton are filtered onto a slow-moving band of silk with a mesh size of 270 um, covered by a second band of silk."@en ;
  skos:inScheme <http://vocab.nerc.ac.uk/scheme/SDNDEV/current> ;
  skos:notation "SDN:L22::NETT0184" ;
  skos:note "accepted"@en ;
  skos:prefLabel "British Antarctic Survey Continuous Plankton Recorder"@en ;
  skos:related <http://vocab.nerc.ac.uk/collection/B75/current/ORG0015> ;
.
inst:NETT0186
  rdf:type skos:Concept ;
  dcterm:date "2018-01-30 16:59:47.0" ;
  dcterm:identifier "SDN:L22::NETT0186" ;
  pav:hasCurrentVersion <http://vocab.nerc.ac.uk/collection/L22/current/NETT0186/1> ;
  owl:versionInfo "1" ;
  skos:altLabel "Rauschert dredge"@en ;
  skos:broader <http://vocab.nerc.ac.uk/collection/L05/current/24> ;
  skos:definition "A fine-mesh dredge composed of a symmetrical metal frame attached to two nets: an inner one with mesh size of 500 um, and an outer one to protect it, with mesh size of 10 mm. This dredge was designed by Dr. Martin Rauschert (Alfred Wegener Institute Helmholtz Centre for Polar and Marine Research) to collect organisms that live on the seabed."@en ;
  skos:inScheme <http://vocab.nerc.ac.uk/scheme/SDNDEV/current> ;
  skos:notation "SDN:L22::NETT0186" ;
  skos:note "accepted"@en ;
  skos:prefLabel "Rauschert dredge"@en ;
  skos:related <http://vocab.nerc.ac.uk/collection/B75/current/ORG00144> ;
.
inst:NETT0188
  rdf:type skos:Concept ;
  dcterm:date "2018-10-04 10:12:44.0" ;
  dcterm:identifier "SDN:L22::NETT0188" ;
  pav:hasCurrentVersion <http://vocab.nerc.ac.uk/collection/L22/current/NETT0188/1> ;
  owl:versionInfo "1" ;
  skos:altLabel "BAS NEMO net"@en ;
  skos:broader <http://vocab.nerc.ac.uk/collection/L05/current/69> ;
  skos:definition "A HydroBios microplastic sampling net of mesh size 0.3 mm mounted in a neuston sledge. The 70 cm x 40 cm rectangular net mouth is equipped with a flowmeter. A modified design comprises of two microplastic nets, a 0.1mm mesh size net outside of a 0.3mm mesh size net. The system is designed for sea surface sampling in the maximum sea state of Beaufort 5."@en ;
  skos:inScheme <http://vocab.nerc.ac.uk/scheme/SDNDEV/current> ;
  skos:notation "SDN:L22::NETT0188" ;
  skos:note "accepted"@en ;
  skos:prefLabel "British Antarctic Survey NEuston MOdified {NEMO} microplastics net"@en ;
  skos:related <http://vocab.nerc.ac.uk/collection/B75/current/ORG0015> ;
.
inst:NETT0189
  rdf:type skos:Concept ;
  dcterm:date "2018-12-04 10:13:26.0" ;
  dcterm:identifier "SDN:L22::NETT0189" ;
  pav:hasCurrentVersion <http://vocab.nerc.ac.uk/collection/L22/current/NETT0189/1> ;
  owl:versionInfo "1" ;
  skos:altLabel "HypBenthos sledge"@en ;
  skos:broader <http://vocab.nerc.ac.uk/collection/L05/current/24> ;
  skos:definition "A benthic sledge used for sampling benthic organisms that live just above the sediment (hyperbenthos). They are typically designed to measure the lower 1 m of the water column and normally consist of a heavy, metal frame with two or more nets on top of each other that are 0.5 or 1 mm mesh size. They are equipped with an opening-closing device to prevent contamination with organisms from the upper water column and are towed from a large vessel such as a research ship. Most variations incorporate some space between the bottom and the nets, so the nets float in the water column and don't catch any sediment."@en ;
  skos:inScheme <http://vocab.nerc.ac.uk/scheme/SDNDEV/current> ;
  skos:notation "SDN:L22::NETT0189" ;
  skos:note "accepted"@en ;
  skos:prefLabel "Unspecified hyperbenthic sledge"@en ;
  skos:related <http://vocab.nerc.ac.uk/collection/B75/current/UNSPEC> ;
.
inst:NETT0190
  rdf:type skos:Concept ;
  dcterm:date "2019-12-02 09:02:24.0" ;
  dcterm:identifier "SDN:L22::NETT0190" ;
  pav:hasCurrentVersion <http://vocab.nerc.ac.uk/collection/L22/current/NETT0190/1> ;
  owl:versionInfo "1" ;
  skos:altLabel "Natlst dredge"@en ;
  skos:broader <http://vocab.nerc.ac.uk/collection/L05/current/24> ;
  skos:broader <http://vocab.nerc.ac.uk/collection/L05/current/60> ;
  skos:definition "An instrument designed for the collection of benthic organisms and bottom material on a variety of grounds. It consists of a rectangular dredge frame, two dredge arms and a triangular mesh net, usually about half as deep as it is wide. The dredge frame varies in length, depending on the size of the towing vessel: 300-380 mm for small boats; 450-600 mm for larger boats; and 750-1300 mm for trawlers. Typically, one dredge arm is attached directly to the tow rope, while the other is attached by a weak link, such as twine, to release the dredge should it become stuck on the seabed. The collection net may be lined with an inner bag of non-impervious material for the collection of sediment."@en ;
  skos:inScheme <http://vocab.nerc.ac.uk/scheme/SDNDEV/current> ;
  skos:notation "SDN:L22::NETT0190" ;
  skos:note "accepted"@en ;
  skos:prefLabel "Unspecified naturalists {rectangular} dredge"@en ;
  skos:related <http://vocab.nerc.ac.uk/collection/B75/current/UNSPEC> ;
  skos:related <http://vocab.nerc.ac.uk/collection/L35/current/MAN0002> ;
.
inst:NETT0191
  rdf:type skos:Concept ;
  dcterm:date "2019-12-10 09:27:08.0" ;
  dcterm:identifier "SDN:L22::NETT0191" ;
  pav:hasCurrentVersion <http://vocab.nerc.ac.uk/collection/L22/current/NETT0191/1> ;
  owl:versionInfo "1" ;
  skos:altLabel "41 x 91cm blade dredge"@en ;
  skos:broader <http://vocab.nerc.ac.uk/collection/L05/current/24> ;
  skos:definition "A towed box dredge where the make and manufacturer are unknown. The dredge is a box-shape and extracts fauna by means of a blade that is 41cm deep and 91cm wide. Typically, hydraulic dredges fluidise the sand immediately ahead and then extracts fauna from the substrate using a blade that protrudes into the sediment. The forward movement of the dredge blade through the fluidised sand lifts the biota and backwards into a collecting vessel."@en ;
  skos:inScheme <http://vocab.nerc.ac.uk/scheme/SDNDEV/current> ;
  skos:notation "SDN:L22::NETT0191" ;
  skos:note "accepted"@en ;
  skos:prefLabel "Unknown 41 x 91 cm hydraulic blade dredge"@en ;
  skos:related <http://vocab.nerc.ac.uk/collection/B75/current/UNSPEC> ;
  skos:related <http://vocab.nerc.ac.uk/collection/L35/current/MAN0002> ;
.
inst:NETT0192
  rdf:type skos:Concept ;
  dcterm:date "2019-12-10 09:27:08.0" ;
  dcterm:identifier "SDN:L22::NETT0192" ;
  pav:hasCurrentVersion <http://vocab.nerc.ac.uk/collection/L22/current/NETT0192/1> ;
  owl:versionInfo "1" ;
  skos:altLabel "UMBSM blade dredge"@en ;
  skos:broader <http://vocab.nerc.ac.uk/collection/L05/current/24> ;
  skos:definition "A hydraulic (water-jet) dredge designed to collect epifauna and infauna from the water-sediment surface. The dredge consists of a 0.39-m wide hollow tooth, which penetrates the sea bed to a depth of 0.34 m. Sea water is delivered to the dredge from a pump by means of a hose. A steel box (0.17 m x 0.77 m x 0.53 m) of 4 cm x 1.5 cm diamond-pattern mesh extended behind the dredge mouth to retain the catch."@en ;
  skos:inScheme <http://vocab.nerc.ac.uk/scheme/SDNDEV/current> ;
  skos:notation "SDN:L22::NETT0192" ;
  skos:note "accepted"@en ;
  skos:prefLabel "University Marine Biological Station Millport hydraulic blade dredge"@en ;
  skos:related <http://vocab.nerc.ac.uk/collection/B75/current/ORG00115> ;
  skos:related <http://vocab.nerc.ac.uk/collection/L35/current/MAN0058> ;
.
inst:NETT0193
  rdf:type skos:Concept ;
  dcterm:date "2020-03-09 19:18:14.0" ;
  dcterm:identifier "SDN:L22::NETT0193" ;
  pav:hasCurrentVersion <http://vocab.nerc.ac.uk/collection/L22/current/NETT0193/1> ;
  owl:versionInfo "1" ;
  skos:altLabel "OTSB"@en ;
  skos:broader <http://vocab.nerc.ac.uk/collection/L05/current/61> ;
  skos:definition "A funnel-shaped net designed to trap organisms at its closed-end while being trawled along the seafloor. It is composed of a non-fixed wide mouth attached to the main wire and held open horizontally by an otter board at each side; a tickler chain is mounted across the lower edge of the net to keep it in contact with the ground, whereas a float fixed to the top of the net ensures its vertical spread. Typically, a semi-balloon otter trawl has a mouth size of approximately 2m x 8.5m; the net has a fine mash and it is mounted to a head rope of maximum 14m in length. This type of trawl is ideal for deep-water sampling of megafauna near the seafloor, mostly for conducting species diversity, abundance and biomass studies. The semi-balloon otter trawl is also known as OTSB, OTSB 14 and Marinovitch Trawl. Ref: Methods for the Study of Marine Benthos, fourth edition by WILEY Blackwell."@en ;
  skos:inScheme <http://vocab.nerc.ac.uk/scheme/SDNDEV/current> ;
  skos:narrower inst:NETT0194 ;
  skos:notation "SDN:L22::NETT0193" ;
  skos:note "accepted"@en ;
  skos:prefLabel "Semi-Balloon Otter Trawl"@en ;
  skos:related <http://vocab.nerc.ac.uk/collection/B75/current/UNSPEC> ;
  skos:related <http://vocab.nerc.ac.uk/collection/L35/current/MAN0002> ;
.
inst:NETT0194
  rdf:type skos:Concept ;
  dcterm:date "2020-05-19 08:57:18.0" ;
  dcterm:identifier "SDN:L22::NETT0194" ;
  pav:hasCurrentVersion <http://vocab.nerc.ac.uk/collection/L22/current/NETT0194/2> ;
  pav:hasVersion <http://vocab.nerc.ac.uk/collection/L22/current/NETT0194/1> ;
  owl:versionInfo "2" ;
  skos:altLabel "OTSB14"@en ;
  skos:broader <http://vocab.nerc.ac.uk/collection/L05/current/61> ;
  skos:broader inst:NETT0193 ;
  skos:definition "The semi-balloon trawl (OTSB14), complete with \"V\" doors was originally obtained from the Marinovich Trawl Company (Biloxi, Mississippi, USA). It was constructed of 4.4 cm stretch mesh body and 3.7 cm mesh intermediate and cod end, with a 1.3 cm inner liner in the cod end. Buoyancy on the headline was provided by one centrally placed glass sphere having a positive buoyancy of 5 kg. Twenty three 13 x 15 cm plastic mud rollers were spaced evenly along the footrope (17 m), with three loops of 6 mm chain in between each set. A pair of sweep lines on each side separated the \"V\" doors by 7 m from the wing ends of the net. The height of the wing ends between headline and footrope was 1.5 m. The doors, each measuring 1.5 x 1 m and weighing 180 kg; were connected by bridles 50 m in length, through a swivel to the single trawl warp. Reference: Merrett, N.R. and Marshall, N.B., 1980. Observations on the ecology of deep-sea bottom-living fishes collected off northwest Africa (08 deg–27 deg N). Progress in Oceanography, 9(4), 185-244. Doi: 10.1016/0079-6611(80)90002-6."@en ;
  skos:inScheme <http://vocab.nerc.ac.uk/scheme/SDNDEV/current> ;
  skos:notation "SDN:L22::NETT0194" ;
  skos:note "accepted"@en ;
  skos:prefLabel "Semi-Balloon Otter Trawl (14 m headrope; single-warp operation) - Merrett and Marshall (1980)"@en ;
  skos:related <http://vocab.nerc.ac.uk/collection/B75/current/UNSPEC> ;
  skos:related <http://vocab.nerc.ac.uk/collection/L35/current/MAN0002> ;
.
inst:NETT0195
  rdf:type skos:Concept ;
  dcterm:date "2020-09-01 16:16:42.0" ;
  dcterm:identifier "SDN:L22::NETT0195" ;
  pav:hasCurrentVersion <http://vocab.nerc.ac.uk/collection/L22/current/NETT0195/1> ;
  owl:versionInfo "1" ;
  skos:altLabel "Epifaunal trawl"@en ;
  skos:broader <http://vocab.nerc.ac.uk/collection/L05/current/61> ;
  skos:definition "A small trawl net designed to sample species living on or near the seabed whilst being towed over the seafloor. Its mouth or opening has dimensions of 30 x 18 cm, and the total length of the net is 37 cm. The net has a mesh size of 1 mm."@en ;
  skos:inScheme <http://vocab.nerc.ac.uk/scheme/SDNDEV/current> ;
  skos:notation "SDN:L22::NETT0195" ;
  skos:note "accepted"@en ;
  skos:prefLabel "Unspecified epifaunal trawl"@en ;
  skos:related <http://vocab.nerc.ac.uk/collection/B75/current/UNSPEC> ;
  skos:related <http://vocab.nerc.ac.uk/collection/L35/current/MAN0001> ;
.
inst:NETT0196
  rdf:type skos:Concept ;
  dcterm:date "2021-04-14 10:20:17.0" ;
  dcterm:identifier "SDN:L22::NETT0196" ;
  pav:hasCurrentVersion <http://vocab.nerc.ac.uk/collection/L22/current/NETT0196/1> ;
  owl:versionInfo "1" ;
  skos:altLabel "MBA Channel Hunter Box Trawl"@en ;
  skos:broader <http://vocab.nerc.ac.uk/collection/L05/current/61> ;
  skos:definition "A type of trawl that is made up of four panels of netting, a top panel, a lower panel and two side panels with these four panels carried down to a four-panel cod-end. Usually used to catch fish. The headline length is 15m, the foot rope length is 20m, it has a diamond mesh with mesh size 80mm, the cod end mesh size is 80mm, and the cod end liner mesh size 20mm. The headline is fitted with 13 x 8-inch diameter plastic floats. The net is held open by a pair of Vee doors. The total net length (from headline midpoint to cod end) is 16m."@en ;
  skos:inScheme <http://vocab.nerc.ac.uk/scheme/SDNDEV/current> ;
  skos:notation "SDN:L22::NETT0196" ;
  skos:note "accepted"@en ;
  skos:prefLabel "Marine Biological Association Channel Hunter Box Trawl"@en ;
  skos:related <http://vocab.nerc.ac.uk/collection/B75/current/ORG00074> ;
  skos:related <http://vocab.nerc.ac.uk/collection/L35/current/MAN0001> ;
.
inst:NETT0197
  rdf:type skos:Concept ;
  dcterm:date "2021-04-14 10:20:17.0" ;
  dcterm:identifier "SDN:L22::NETT0197" ;
  pav:hasCurrentVersion <http://vocab.nerc.ac.uk/collection/L22/current/NETT0197/1> ;
  owl:versionInfo "1" ;
  skos:altLabel "MBA Small Otter Trawl"@en ;
  skos:broader <http://vocab.nerc.ac.uk/collection/L05/current/61> ;
  skos:definition "A type of trawl net designed to be dragged behind a research vessel along the sea bottom or the pelagic zone. The otter trawl is mainly used to catch roundfish living above the sea bottom. The headline length is 15m, the foot rope length is 17.5m, it has diamond mesh with mesh size 80mm, the cod end mesh size is 80mm. Cod end cover (when used) has a mesh size of 5mm. The headline is fitted with 9 plastic floats (2 x 8-inch diameter and 7 x 6-inch diameter). The net is held open by a pair of plastic Vee doors. The total net length (from headline midpoint to cod end) is 11.5m."@en ;
  skos:inScheme <http://vocab.nerc.ac.uk/scheme/SDNDEV/current> ;
  skos:notation "SDN:L22::NETT0197" ;
  skos:note "accepted"@en ;
  skos:prefLabel "Marine Biological Association Small Otter Trawl"@en ;
  skos:related <http://vocab.nerc.ac.uk/collection/B75/current/ORG00074> ;
  skos:related <http://vocab.nerc.ac.uk/collection/L35/current/MAN0001> ;
.
inst:NETT0198
  rdf:type skos:Concept ;
  dcterm:date "2021-04-14 10:20:17.0" ;
  dcterm:identifier "SDN:L22::NETT0198" ;
  pav:hasCurrentVersion <http://vocab.nerc.ac.uk/collection/L22/current/NETT0198/1> ;
  owl:versionInfo "1" ;
  skos:altLabel "MBA Modified Small Otter Trawl"@en ;
  skos:broader <http://vocab.nerc.ac.uk/collection/L05/current/61> ;
  skos:definition "A type of trawl net designed to be dragged behind a research vessel along the sea bottom or the pelagic zone. The otter trawl is mainly used to catch roundfish living above the sea bottom. The headline length is 15m, the foot rope length is 17.5m, it has diamond mesh with mesh size 80mm, the cod end mesh size is 80mm. Cod end cover (when used) has a mesh size of 5mm. The headline is fitted with 9 plastic floats (2 x 8-inch diameter and 7 x 6-inch diameter). The net is held open by a pair of metal Vee doors, each weighing 150kg. The total net length (from headline midpoint to cod end) is 11.5m."@en ;
  skos:inScheme <http://vocab.nerc.ac.uk/scheme/SDNDEV/current> ;
  skos:notation "SDN:L22::NETT0198" ;
  skos:note "accepted"@en ;
  skos:prefLabel "Marine Biological Association Modified Small Otter Trawl"@en ;
  skos:related <http://vocab.nerc.ac.uk/collection/B75/current/ORG00074> ;
  skos:related <http://vocab.nerc.ac.uk/collection/L35/current/MAN0001> ;
.
inst:NETT0199
  rdf:type skos:Concept ;
  dcterm:date "2021-11-16 09:18:10.0" ;
  dcterm:identifier "SDN:L22::NETT0199" ;
  pav:hasCurrentVersion <http://vocab.nerc.ac.uk/collection/L22/current/NETT0199/1> ;
  owl:versionInfo "1" ;
  skos:altLabel "AMT 18 plankton net"@en ;
  skos:broader <http://vocab.nerc.ac.uk/collection/L05/current/22> ;
  skos:definition "Construction is 3 conical nets with mesh sizes 180, 100 and 40 um. Each net comprises an 18 cm mouth opening using a plastic inverted cone to reduce the diameter from approx. 40 cm to 18 cm. The nets were conical with an outer diameter of approx. 40 cm and a closed cod-end design."@en ;
  skos:inScheme <http://vocab.nerc.ac.uk/scheme/SDNDEV/current> ;
  skos:notation "SDN:L22::NETT0199" ;
  skos:note "accepted"@en ;
  skos:prefLabel "Custom 3 x 18 cm mouth opening x 40 cm diameter conical nets plankton net - AMT 18 (2008)"@en ;
  skos:related <http://vocab.nerc.ac.uk/collection/B75/current/UNSPEC> ;
  skos:related <http://vocab.nerc.ac.uk/collection/L35/current/MAN0002> ;
.
inst:NETT0200
  rdf:type skos:Concept ;
  dcterm:date "2022-02-22 17:09:18.0" ;
  dcterm:identifier "SDN:L22::NETT0200" ;
  pav:hasCurrentVersion <http://vocab.nerc.ac.uk/collection/L22/current/NETT0200/1> ;
  owl:versionInfo "1" ;
  skos:altLabel "Hydro-Bios RingTrawl CalCOFI net"@en ;
  skos:broader <http://vocab.nerc.ac.uk/collection/L05/current/22> ;
  skos:definition "An oceanographic plankton net based on the California Cooperative Oceanic Fisheries Investigations (CalCOFI) design. It is designed for quantitative sampling of larger volumes of water during horizontal or oblique tows. Typically the net is lowered to a set depth and towed obliquely at a 45 degrees to the surface at a constant speed. The net may also be used for horizontal and flat-angled oblique tows. It features a 100 cm diameter stainless steel ring, equipped with a 4 meter long net bag, and is designed to operate in conjunction with a 22 kg V-Fin depressor to create negative lift. The sample is concentrated inside a removable plastic net bucket with side window (covered with sieve gauze). A Mechanical Flow Meter can also be fixed in the net to measure the filtered water volume. Standard mesh size is 500 um, and the net opening area is 0.7854 m-2."@en ;
  skos:inScheme <http://vocab.nerc.ac.uk/scheme/SDNDEV/current> ;
  skos:notation "SDN:L22::NETT0200" ;
  skos:note "accepted"@en ;
  skos:prefLabel "Hydro-Bios RingTrawl (CalCOFI) net"@en ;
  skos:related <http://vocab.nerc.ac.uk/collection/B75/current/ORG00761> ;
  skos:related <http://vocab.nerc.ac.uk/collection/L35/current/MAN0198> ;
.
inst:NETT0201
  rdf:type skos:Concept ;
  dcterm:date "2022-09-30 12:45:04.0" ;
  dcterm:identifier "SDN:L22::NETT0201" ;
  pav:hasCurrentVersion <http://vocab.nerc.ac.uk/collection/L22/current/NETT0201/1> ;
  owl:versionInfo "1" ;
  skos:altLabel "ICES MIK Ringnet"@en ;
  skos:broader <http://vocab.nerc.ac.uk/collection/L05/current/22> ;
  skos:definition "A plankton net composing of a rigid 2 m diameter ring frame mounted to a nylon gauze conical net. It is designed for sampling of larval herring and other similar species between 2 and 3 cm in length. The design was used for the sampling of fish larvae during the North Sea International Bottom Survey Trawl in 1977 (first quarter). Additional features include a codend bucket, a pair of 10 m bridles for towing, a depressor (approximately 25 kg or more) with 3 m bridles, a flowmeter for filtered volume determination and a depth gauge for monitoring net depth. The net iteself is 13m long and of 1.6 mm pore. In the last metre of net, a 500 um net is inserted. The net is designed for oblique haul profiles at a maximum tow depth of 100 m."@en ;
  skos:inScheme <http://vocab.nerc.ac.uk/scheme/SDNDEV/current> ;
  skos:notation "SDN:L22::NETT0201" ;
  skos:note "accepted"@en ;
  skos:prefLabel "ICES MIK Midwater Ringnet"@en ;
  skos:related <http://vocab.nerc.ac.uk/collection/B75/current/ORG01989> ;
  skos:related <http://vocab.nerc.ac.uk/collection/L35/current/MAN0233> ;
.
inst:NETT0202
  rdf:type skos:Concept ;
  dcterm:date "2022-10-04 10:24:29.0" ;
  dcterm:identifier "SDN:L22::NETT0202" ;
  pav:hasCurrentVersion <http://vocab.nerc.ac.uk/collection/L22/current/NETT0202/1> ;
  owl:versionInfo "1" ;
  skos:altLabel "Ifremer mesopelagos net"@en ;
  skos:broader <http://vocab.nerc.ac.uk/collection/L05/current/22> ;
  skos:definition "A plankton net composing of an 8.4 m diameter rectangular frame mounted to a 12.6 m net, with an opening mouth area of 50 m squared. It is used to determine the composition of zooplankton and micronekton layers, and it can harvest samples of micronektonic fauna (fish, molluscs, crustaceans, jellyfish) of 1 to 30 cm long, as well as large mesozooplankton. The net itself features varying mesh sizes throughout its length; mesh size at the mouth is 30 mm and gradually reduces to 4 mm at the cod end. Designed for oblique-horizontal or oblique tows at trawl speeds of2 to 4 knots."@en ;
  skos:inScheme <http://vocab.nerc.ac.uk/scheme/SDNDEV/current> ;
  skos:notation "SDN:L22::NETT0202" ;
  skos:note "accepted"@en ;
  skos:prefLabel "Ifremer mesopelagos net"@en ;
  skos:related <http://vocab.nerc.ac.uk/collection/B75/current/ORG00749> ;
  skos:related <http://vocab.nerc.ac.uk/collection/L35/current/MAN0232> ;
.
inst:TOOL000X
  rdf:type skos:Concept ;
  dcterm:date "2017-03-22 11:14:12.0" ;
  dcterm:identifier "SDN:L22::TOOL000X" ;
  pav:hasCurrentVersion <http://vocab.nerc.ac.uk/collection/L22/current/TOOL000X/1> ;
  owl:versionInfo "1" ;
  skos:altLabel "inapplicable"@en ;
  skos:broader <http://vocab.nerc.ac.uk/collection/L05/current/182> ;
  skos:definition "There is no appropriate value. To be used in cases where metadata elements cannot be set null due to schema constraints."@en ;
  skos:inScheme <http://vocab.nerc.ac.uk/scheme/SDNDEV/current> ;
  skos:notation "SDN:L22::TOOL000X" ;
  skos:note "accepted"@en ;
  skos:prefLabel "inapplicable"@en ;
.
inst:TOOL0235
  rdf:type skos:Concept ;
  dcterm:date "2010-05-18 16:10:58.0" ;
  dcterm:identifier "SDN:L22::TOOL0235" ;
  pav:hasCurrentVersion <http://vocab.nerc.ac.uk/collection/L22/current/TOOL0235/1> ;
  owl:versionInfo "1" ;
  skos:altLabel "Bottle"@en ;
  skos:broader <http://vocab.nerc.ac.uk/collection/L05/current/30> ;
  skos:definition "A generic term for a device for the collection of a water sample from a pre-determined depth in a water body. The device is positioned at the desired depth where it is closed and sealed by some form of command from the surface."@en ;
  skos:inScheme <http://vocab.nerc.ac.uk/scheme/SDNDEV/current> ;
  skos:notation "SDN:L22::TOOL0235" ;
  skos:note "accepted"@en ;
  skos:prefLabel "Water bottle"@en ;
  skos:related <http://vocab.nerc.ac.uk/collection/B75/current/ORG00001> ;
.
inst:TOOL0236
  rdf:type skos:Concept ;
  dcterm:date "2010-11-18 12:39:41.0" ;
  dcterm:identifier "SDN:L22::TOOL0236" ;
  pav:hasCurrentVersion <http://vocab.nerc.ac.uk/collection/L22/current/TOOL0236/2> ;
  pav:hasVersion <http://vocab.nerc.ac.uk/collection/L22/current/TOOL0236/1> ;
  owl:versionInfo "2" ;
  skos:altLabel "NIO bottle"@en ;
  skos:broader <http://vocab.nerc.ac.uk/collection/L05/current/30> ;
  skos:definition "A 1.35 litre plastic water bottle designed by the National Institute of Oceanography. It is deployed clamped to a cable and triggered by a weight sliding down the cable. When triggered the bottle rotates through 180 degrees which simultaneously closes the valves and fires any reversing thermometers mounted on the bottle."@en ;
  skos:inScheme <http://vocab.nerc.ac.uk/scheme/SDNDEV/current> ;
  skos:notation "SDN:L22::TOOL0236" ;
  skos:note "accepted"@en ;
  skos:prefLabel "National Institute of Oceanography plastic reversing water bottle"@en ;
  skos:related <http://vocab.nerc.ac.uk/collection/B75/current/ORG00288> ;
.
inst:TOOL0248
  rdf:type skos:Concept ;
  dcterm:date "2010-11-18 12:39:41.0" ;
  dcterm:identifier "SDN:L22::TOOL0248" ;
  pav:hasCurrentVersion <http://vocab.nerc.ac.uk/collection/L22/current/TOOL0248/2> ;
  pav:hasVersion <http://vocab.nerc.ac.uk/collection/L22/current/TOOL0248/1> ;
  owl:versionInfo "2" ;
  skos:altLabel "Nansen bottle"@en ;
  skos:broader <http://vocab.nerc.ac.uk/collection/L05/current/30> ;
  skos:definition "Metal or plastic insulated bottles with an approximate capacity of 1-2 litres designed for deployment on a cable, sealed by with a spring-loaded valve when triggered by dropping a weight down the cable. It was designed to recover an uncontaminated sample from depth within 0.01C of its in-situ temperature. The design is an improvement by Petterson in collaboration with Nansen on an original design by Nansen. Both designs are commonly known as Nansen bottles."@en ;
  skos:inScheme <http://vocab.nerc.ac.uk/scheme/SDNDEV/current> ;
  skos:notation "SDN:L22::TOOL0248" ;
  skos:note "accepted"@en ;
  skos:prefLabel "Nansen-Petterson water bottle"@en ;
  skos:related <http://vocab.nerc.ac.uk/collection/B75/current/ORG00001> ;
.
inst:TOOL0381
  rdf:type skos:Concept ;
  dcterm:date "2011-03-14 15:22:43.0" ;
  dcterm:identifier "SDN:L22::TOOL0381" ;
  pav:hasCurrentVersion <http://vocab.nerc.ac.uk/collection/L22/current/TOOL0381/1> ;
  owl:versionInfo "1" ;
  skos:altLabel "Aqua Monitor Water Sampler"@en ;
  skos:broader <http://vocab.nerc.ac.uk/collection/L05/current/30> ;
  skos:definition "A programmable water sampler that can collect up to 48 discrete water samples of up to 1000ml each and may be programmed for time series sampling or for operation in \"slave\" mode within a system. Samples are collected using a syringe mechanism and stored in gas impermeable bags within protective enclosures.The sampler can be deployed on moorings, towed-vehicle systems, ROV or AUV platforms, and can be used for applications such as phytoplankton, nutrients, salinity and suspended sediment measurements."@en ;
  skos:inScheme <http://vocab.nerc.ac.uk/scheme/SDNDEV/current> ;
  skos:notation "SDN:L22::TOOL0381" ;
  skos:note "accepted"@en ;
  skos:prefLabel "EnviroTech LLC Aqua Monitor Smart Water Sampler"@en ;
  skos:related <http://vocab.nerc.ac.uk/collection/B75/current/ORG00387> ;
.
inst:TOOL0412
  rdf:type skos:Concept ;
  dcterm:date "2012-06-22 13:43:26.0" ;
  dcterm:identifier "SDN:L22::TOOL0412" ;
  pav:hasCurrentVersion <http://vocab.nerc.ac.uk/collection/L22/current/TOOL0412/2> ;
  pav:hasVersion <http://vocab.nerc.ac.uk/collection/L22/current/TOOL0412/1> ;
  owl:versionInfo "2" ;
  skos:altLabel "Niskin bottle"@en ;
  skos:broader <http://vocab.nerc.ac.uk/collection/L05/current/30> ;
  skos:definition "A plastic free-flushing water sampling bottle with a capacity of 1.7-30 litres. It has caps with rubber seals at each end joined by a plastic-coated metal spring or elastic cord running through the interior of the bottle. It is deployed with the caps held open against the spring by plastic lanyards. When the bottle reaches the desired depth the lanyards are released by a pressure-actuated switch, command signal or messenger weight and the caps are forced shut and sealed. Bottles may be deployed singly clamped to a wire or in groups of up to 48 on a rosette. Reversing thermometers may be attached to a spring-loaded disk that rotates through 180 degrees on bottle closure."@en ;
  skos:inScheme <http://vocab.nerc.ac.uk/scheme/SDNDEV/current> ;
  skos:notation "SDN:L22::TOOL0412" ;
  skos:note "accepted"@en ;
  skos:prefLabel "Niskin bottle"@en ;
  skos:related <http://vocab.nerc.ac.uk/collection/B75/current/ORG00001> ;
.
inst:TOOL0413
  rdf:type skos:Concept ;
  dcterm:date "2011-08-05 09:08:32.0" ;
  dcterm:identifier "SDN:L22::TOOL0413" ;
  pav:hasCurrentVersion <http://vocab.nerc.ac.uk/collection/L22/current/TOOL0413/1> ;
  owl:versionInfo "1" ;
  skos:altLabel "Non-toxic supply"@en ;
  skos:broader <http://vocab.nerc.ac.uk/collection/L05/current/31> ;
  skos:definition "A source of uncontaminated near-surface (commonly 3 to 7 m) seawater pumped continuously to shipboard laboratories on research vessels. There is typically a temperature sensor near the intake (known as the hull temperature) to provide measurements that are as close as possible to the ambient water temperature. The flow from the supply is typically directed through continuously logged sensors such as a thermosalinograph and a fluorometer. Water samples are often collected from the non-toxic supply. The system is also referred to as the underway supply."@en ;
  skos:inScheme <http://vocab.nerc.ac.uk/scheme/SDNDEV/current> ;
  skos:notation "SDN:L22::TOOL0413" ;
  skos:note "accepted"@en ;
  skos:prefLabel "Non-toxic sea water supply"@en ;
  skos:related <http://vocab.nerc.ac.uk/collection/B75/current/ORG00001> ;
.
inst:TOOL0418
  rdf:type skos:Concept ;
  dcterm:date "2012-06-22 13:49:29.0" ;
  dcterm:identifier "SDN:L22::TOOL0418" ;
  pav:hasCurrentVersion <http://vocab.nerc.ac.uk/collection/L22/current/TOOL0418/2> ;
  pav:hasVersion <http://vocab.nerc.ac.uk/collection/L22/current/TOOL0418/1> ;
  owl:versionInfo "2" ;
  skos:altLabel "Teflon-coated Niskin"@en ;
  skos:broader <http://vocab.nerc.ac.uk/collection/L05/current/30> ;
  skos:definition "A teflon-coated free-flushing water sampling bottle with a capacity of 1.7-30 litres. It has caps with rubber seals at each end joined by a latex cord running through the interior of the bottle. It is deployed with the caps held open against the latex cord by plastic lanyards. When the bottle reaches the desired depth the lanyards are released by a pressure-actuated switch, command signal or messenger weight and the caps are forced shut and sealed. Bottles may be deployed singly clamped to a wire or in groups of up to 48 on a rosette. Reversing thermometers may be attached to a spring-loaded disk that rotates through 180 degrees on bottle closure. These bottles are specifically designed to minimise metal contamination when sampling trace metals."@en ;
  skos:inScheme <http://vocab.nerc.ac.uk/scheme/SDNDEV/current> ;
  skos:notation "SDN:L22::TOOL0418" ;
  skos:note "accepted"@en ;
  skos:prefLabel "Teflon-coated Niskin bottle"@en ;
  skos:related <http://vocab.nerc.ac.uk/collection/B75/current/ORG00001> ;
.
inst:TOOL0427
  rdf:type skos:Concept ;
  dcterm:date "2022-08-30 15:10:01.0" ;
  dcterm:identifier "SDN:L22::TOOL0427" ;
  pav:hasCurrentVersion <http://vocab.nerc.ac.uk/collection/L22/current/TOOL0427/2> ;
  pav:hasVersion <http://vocab.nerc.ac.uk/collection/L22/current/TOOL0427/1> ;
  owl:versionInfo "2" ;
  skos:altLabel "Levered Niskin Bottle"@en ;
  skos:broader <http://vocab.nerc.ac.uk/collection/L05/current/30> ;
  skos:definition "A plastic free-flushing water sampling bottle with a typical capacity between 1.7 and 30 litres. It has caps with rubber seals at each end and is deployed with the caps held open by externally mounted stainless steel springs. Unlike the standard Niskin design, this bottle does not feature an internal lanyard, and is thus recommended for applications where a completely clear sample chamber is critical. When the bottle reaches the desired depth it is closed by messenger when serially attached to hydrocable or by remote command when attached to sampling rosette."@en ;
  skos:inScheme <http://vocab.nerc.ac.uk/scheme/SDNDEV/current> ;
  skos:notation "SDN:L22::TOOL0427" ;
  skos:note "accepted"@en ;
  skos:prefLabel "Lever Action Niskin Bottle"@en ;
  skos:related <http://vocab.nerc.ac.uk/collection/B75/current/ORG00001> ;
.
inst:TOOL0472
  rdf:type skos:Concept ;
  dcterm:date "2012-02-21 16:06:42.0" ;
  dcterm:identifier "SDN:L22::TOOL0472" ;
  pav:hasCurrentVersion <http://vocab.nerc.ac.uk/collection/L22/current/TOOL0472/1> ;
  owl:versionInfo "1" ;
  skos:altLabel "Bowers and Connelly Mega Corer"@en ;
  skos:broader <http://vocab.nerc.ac.uk/collection/L05/current/51> ;
  skos:definition "A sediment corer which collects relatively undisturbed sea-floor sediment samples including an intact sediment-water interface and overlying supernatant water. The Mega Corer holds 12 tubes, each 600 mm in length, allowing collection of sediment cores up to 400 mm long. It has a hydrostatic damping system which is used to slow down the penetration rate and to remove the typical bow wave. Corer deployment rates are in the region of 1 metre per second on the descent, and at any speed on retrieval as the samples are sealed top and bottom. The core tubing can be manufactured from acrylic, poly carbonate or stainless steel. The instrument was designed by Bowers and Connelly and is now manufactured by OSIL."@en ;
  skos:inScheme <http://vocab.nerc.ac.uk/scheme/SDNDEV/current> ;
  skos:notation "SDN:L22::TOOL0472" ;
  skos:note "accepted"@en ;
  skos:prefLabel "Bowers and Connelly Mega Corer"@en ;
  skos:related <http://vocab.nerc.ac.uk/collection/B75/current/ORG00411> ;
.
inst:TOOL0501
  rdf:type skos:Concept ;
  dcterm:date "2012-06-21 16:09:48.0" ;
  dcterm:identifier "SDN:L22::TOOL0501" ;
  pav:hasCurrentVersion <http://vocab.nerc.ac.uk/collection/L22/current/TOOL0501/1> ;
  owl:versionInfo "1" ;
  skos:altLabel "ARIES water sample bottle"@en ;
  skos:broader <http://vocab.nerc.ac.uk/collection/L05/current/30> ;
  skos:definition "A custom made water sampling bottle designed to fit on the ARIES net rosette sampler. The bottle comprises a free-flooding tube with hinged sealing lids at each end. The lids of each tube are connected by an internal length of silicone elastic. Prior to sampling the lids are held open by pins slotted into pivoting levers. When sampling is complete for one bottle the levels at each end of the next tube in the carousel are simultaneously turned by a rotating arm, thus releasing the lids and closing the tube. Each tube is 40 cm long and has an external diameter of 42 mm and a capacity of 250 ml."@en ;
  skos:inScheme <http://vocab.nerc.ac.uk/scheme/SDNDEV/current> ;
  skos:notation "SDN:L22::TOOL0501" ;
  skos:note "accepted"@en ;
  skos:prefLabel "Autosampling and Recording Instrumental Environmental Sampler rosette water bottle"@en ;
  skos:related <http://vocab.nerc.ac.uk/collection/B75/current/ORG00013> ;
.
inst:TOOL0502
  rdf:type skos:Concept ;
  dcterm:date "2012-06-21 16:09:48.0" ;
  dcterm:identifier "SDN:L22::TOOL0502" ;
  pav:hasCurrentVersion <http://vocab.nerc.ac.uk/collection/L22/current/TOOL0502/1> ;
  owl:versionInfo "1" ;
  skos:altLabel "Van Dorn water sampler"@en ;
  skos:broader <http://vocab.nerc.ac.uk/collection/L05/current/30> ;
  skos:definition "A free-flushing water sample bottle comprising a cylinder (polycarbonate, acrylic or PVC) with a stopper at each end. The bottle is closed by means of a messenger from the surface releasing the tension on a latex band and thus pulling the two stoppers firmly into place. A thermometer can be mounted inside the bottle. One or more bottles can be lowered on a line to allow sampling at a single or multiple depth levels. Van Dorn samplers are suitable for for physical (temperature), chemical and biological sampling in shallow to very deep water. Bottles are typically lowered vertically through the water column although a horizontal version is available for sampling near the seabed or at thermoclines or chemoclines. Because of the lack of metal parts the bottles are suitable for trace metal sampling, although the blue polyurethane seal used in the Alpha version may leach mercury. The Beta version uses white ASA plastic seals that do not leach mercury but are less durable."@en ;
  skos:inScheme <http://vocab.nerc.ac.uk/scheme/SDNDEV/current> ;
  skos:notation "SDN:L22::TOOL0502" ;
  skos:note "accepted"@en ;
  skos:prefLabel "Van Dorn water sampler"@en ;
  skos:related <http://vocab.nerc.ac.uk/collection/B75/current/ORG00001> ;
.
inst:TOOL0503
  rdf:type skos:Concept ;
  dcterm:date "2012-06-21 16:09:48.0" ;
  dcterm:identifier "SDN:L22::TOOL0503" ;
  pav:hasCurrentVersion <http://vocab.nerc.ac.uk/collection/L22/current/TOOL0503/1> ;
  owl:versionInfo "1" ;
  skos:altLabel "PRISTINE sampler"@en ;
  skos:broader <http://vocab.nerc.ac.uk/collection/L05/current/30> ;
  skos:definition "Ultraclean water sampler developed by the Royal Netherlands Institute For Sea Research (NIOZ) for the GEOTRACES Program. Individual sample bottles have a capacity of 27 litres and include butterfly valves that ensure bottles are closed when passing through the ocean surface and reopen subsurface. Teflon valves for subsampling at the base of bottles ensure drainage of settling particulates. Samplers are deployed with a Kevlar hydrowire cable with internal signal cables. A single bottle may be used (e.g. during small boat work) or an array of bottles may be mounted on a frame for shipboard CTD work. Trip mechanisms range from a weighted messenger to trip wires or hydraulics for rosette sampling."@en ;
  skos:inScheme <http://vocab.nerc.ac.uk/scheme/SDNDEV/current> ;
  skos:notation "SDN:L22::TOOL0503" ;
  skos:note "accepted"@en ;
  skos:prefLabel "NIOZ PRISTINE ultraclean water sampler"@en ;
  skos:related <http://vocab.nerc.ac.uk/collection/B75/current/ORG00239> ;
.
inst:TOOL0504
  rdf:type skos:Concept ;
  dcterm:date "2012-06-21 16:09:48.0" ;
  dcterm:identifier "SDN:L22::TOOL0504" ;
  pav:hasCurrentVersion <http://vocab.nerc.ac.uk/collection/L22/current/TOOL0504/1> ;
  owl:versionInfo "1" ;
  skos:altLabel "Carboy"@en ;
  skos:broader <http://vocab.nerc.ac.uk/collection/L05/current/30> ;
  skos:definition "A rigid container made of material such as glass or high density plastic with a typical capacity of 20 to 60 litres. A carboy is typically used to store or transport liquids."@en ;
  skos:inScheme <http://vocab.nerc.ac.uk/scheme/SDNDEV/current> ;
  skos:notation "SDN:L22::TOOL0504" ;
  skos:note "accepted"@en ;
  skos:prefLabel "Carboy"@en ;
  skos:related <http://vocab.nerc.ac.uk/collection/B75/current/ORG00001> ;
.
inst:TOOL0505
  rdf:type skos:Concept ;
  dcterm:date "2012-06-21 16:09:48.0" ;
  dcterm:identifier "SDN:L22::TOOL0505" ;
  pav:hasCurrentVersion <http://vocab.nerc.ac.uk/collection/L22/current/TOOL0505/1> ;
  owl:versionInfo "1" ;
  skos:altLabel "Knudsen bottle"@en ;
  skos:broader <http://vocab.nerc.ac.uk/collection/L05/current/30> ;
  skos:definition "A frameless reversing water bottle with reversing thermometers that is used to collect water samples. The bottom of the bottle is clamped to a wire and the top of the bottle is held to the wire by a catch. It has independent hinged lids at each end which are held open against an internal spring when the bottle is deployed. Once the bottle has reached the target depth a messenger is dropped down the wire and hits the catch. The lids close and the bottle falls through 180deg, pivoting on the bottom clamp. This action reversed the thermometers, which are housed in a frame attached to the bottle."@en ;
  skos:inScheme <http://vocab.nerc.ac.uk/scheme/SDNDEV/current> ;
  skos:notation "SDN:L22::TOOL0505" ;
  skos:note "accepted"@en ;
  skos:prefLabel "Knudsen reversing water bottle"@en ;
  skos:related <http://vocab.nerc.ac.uk/collection/B75/current/ORG00001> ;
.
inst:TOOL0506
  rdf:type skos:Concept ;
  dcterm:date "2012-06-21 16:09:48.0" ;
  dcterm:identifier "SDN:L22::TOOL0506" ;
  pav:hasCurrentVersion <http://vocab.nerc.ac.uk/collection/L22/current/TOOL0506/1> ;
  owl:versionInfo "1" ;
  skos:altLabel "GO-FLO bottle"@en ;
  skos:broader <http://vocab.nerc.ac.uk/collection/L05/current/30> ;
  skos:definition "A plastic free-flushing water sampling bottle with a capacity of 1.7-100 litres. The tube is composed of PVC and has ball valves with Viton and silicone seals at each end joined by an external latex spring and nylon and Kevlar lanyards. It is closed when deployed then opens automatically (hydrostatic pressure activated) at approximately 10 m and flushes until closed. When the bottle reaches the desired depth the lanyards are released by a pressure-actuated switch, command signal or messenger weight and the caps are forced shut and sealed. Bottles may be deployed singly clamped to a wire or in groups on a rosette. A reversing thermometer assembly may be attached to the bottle. When extracting water from the bottle, inert gas can be injected into the bottle to force the sample out of the sampling valve. The GO-FLO sampler avoids sample contamination at the surface, internal spring contamination, loss of sample on deck (internal seals), and exchange of water from different depths."@en ;
  skos:inScheme <http://vocab.nerc.ac.uk/scheme/SDNDEV/current> ;
  skos:notation "SDN:L22::TOOL0506" ;
  skos:note "accepted"@en ;
  skos:prefLabel "General Oceanics GO-FLO water sampler"@en ;
  skos:related <http://vocab.nerc.ac.uk/collection/B75/current/ORG00617> ;
.
inst:TOOL0508
  rdf:type skos:Concept ;
  dcterm:date "2012-06-22 15:36:10.0" ;
  dcterm:identifier "SDN:L22::TOOL0508" ;
  pav:hasCurrentVersion <http://vocab.nerc.ac.uk/collection/L22/current/TOOL0508/1> ;
  owl:versionInfo "1" ;
  skos:altLabel "Friedinger bottle"@en ;
  skos:broader <http://vocab.nerc.ac.uk/collection/L05/current/30> ;
  skos:definition "A free flushing sample bottle of 1-5 litre capacity comprising a glass, metal or plastic tube with a hinged lid at each end. The bottle is deployed on a wire with the lids held open. When the bottle reaches the target depth a weighted messenger is sent down the wire and releases the lids, sealing the sample in the bottle. The bottle was designed by H Friedinger (Lucerne, Switzerland) to collect water samples for plankton analysis."@en ;
  skos:inScheme <http://vocab.nerc.ac.uk/scheme/SDNDEV/current> ;
  skos:notation "SDN:L22::TOOL0508" ;
  skos:note "accepted"@en ;
  skos:prefLabel "Friedinger bottle water sampler"@en ;
  skos:related <http://vocab.nerc.ac.uk/collection/B75/current/ORG00001> ;
.
inst:TOOL0535
  rdf:type skos:Concept ;
  dcterm:date "2012-09-25 14:01:15.0" ;
  dcterm:identifier "SDN:L22::TOOL0535" ;
  pav:hasCurrentVersion <http://vocab.nerc.ac.uk/collection/L22/current/TOOL0535/1> ;
  owl:versionInfo "1" ;
  skos:altLabel "OCEAN water sample bottle"@en ;
  skos:broader <http://vocab.nerc.ac.uk/collection/L05/current/30> ;
  skos:definition "A custom made water sampling bottle designed to fit on the OCEAN sampler. The bottle comprises a free-flooding tube with a capacity of 0.5 litres. The bottle closes when a net sample is collected. Bottle firing is pre-programmed using a computer prior to deployment of the sampler."@en ;
  skos:inScheme <http://vocab.nerc.ac.uk/scheme/SDNDEV/current> ;
  skos:notation "SDN:L22::TOOL0535" ;
  skos:note "accepted"@en ;
  skos:prefLabel "Marine Scotland Opening Closing Environmental Acoustic Net water bottle"@en ;
  skos:related <http://vocab.nerc.ac.uk/collection/B75/current/ORG00013> ;
.
inst:TOOL0536
  rdf:type skos:Concept ;
  dcterm:date "2012-09-25 16:03:31.0" ;
  dcterm:identifier "SDN:L22::TOOL0536" ;
  pav:hasCurrentVersion <http://vocab.nerc.ac.uk/collection/L22/current/TOOL0536/1> ;
  owl:versionInfo "1" ;
  skos:altLabel "Bucket"@en ;
  skos:broader <http://vocab.nerc.ac.uk/collection/L05/current/30> ;
  skos:definition "Typically a watertight, vertical cylinder or truncated cone, with an open top and a flat bottom. Usually attached to a semicircular handle."@en ;
  skos:inScheme <http://vocab.nerc.ac.uk/scheme/SDNDEV/current> ;
  skos:notation "SDN:L22::TOOL0536" ;
  skos:note "accepted"@en ;
  skos:prefLabel "Bucket"@en ;
  skos:related <http://vocab.nerc.ac.uk/collection/B75/current/ORG00001> ;
.
inst:TOOL0537
  rdf:type skos:Concept ;
  dcterm:date "2012-09-25 16:03:31.0" ;
  dcterm:identifier "SDN:L22::TOOL0537" ;
  pav:hasCurrentVersion <http://vocab.nerc.ac.uk/collection/L22/current/TOOL0537/1> ;
  owl:versionInfo "1" ;
  skos:altLabel "Winchester bottle"@en ;
  skos:broader <http://vocab.nerc.ac.uk/collection/L05/current/30> ;
  skos:definition "A strong, heavy bottle typically made of brown glass (to filter out UV light) but may also be made of plastics. A range of capacities is available. Also known as a Boston round bottle."@en ;
  skos:inScheme <http://vocab.nerc.ac.uk/scheme/SDNDEV/current> ;
  skos:notation "SDN:L22::TOOL0537" ;
  skos:note "accepted"@en ;
  skos:prefLabel "Winchester bottle"@en ;
  skos:related <http://vocab.nerc.ac.uk/collection/B75/current/ORG00001> ;
.
inst:TOOL0538
  rdf:type skos:Concept ;
  dcterm:date "2012-09-25 16:03:31.0" ;
  dcterm:identifier "SDN:L22::TOOL0538" ;
  pav:hasCurrentVersion <http://vocab.nerc.ac.uk/collection/L22/current/TOOL0538/1> ;
  owl:versionInfo "1" ;
  skos:altLabel "NOEX bottle"@en ;
  skos:broader <http://vocab.nerc.ac.uk/collection/L05/current/30> ;
  skos:definition "Water bottle designed for oceanographic sampling. The bottle comprises a plastic tube with caps at each end and is deployed with the caps held open, then closed at the target depth. Multiple bottles can be deployed on a CTD frame rosette. Bottle capacity is variable, but normally several litres. The bottle was developed by Technicap in the 1990s but has been superseded by more recent models. There is no known source of support available for this sampler."@en ;
  skos:inScheme <http://vocab.nerc.ac.uk/scheme/SDNDEV/current> ;
  skos:notation "SDN:L22::TOOL0538" ;
  skos:note "accepted"@en ;
  skos:prefLabel "Technicap NOEX bottle"@en ;
  skos:related <http://vocab.nerc.ac.uk/collection/B75/current/ORG00001> ;
.
inst:TOOL0539
  rdf:type skos:Concept ;
  dcterm:date "2012-10-12 09:11:26.0" ;
  dcterm:identifier "SDN:L22::TOOL0539" ;
  pav:hasCurrentVersion <http://vocab.nerc.ac.uk/collection/L22/current/TOOL0539/2> ;
  pav:hasVersion <http://vocab.nerc.ac.uk/collection/L22/current/TOOL0539/1> ;
  owl:versionInfo "2" ;
  skos:altLabel "Flygt pump"@en ;
  skos:broader <http://vocab.nerc.ac.uk/collection/L05/current/31> ;
  skos:definition "Submersible electrical pump designed for continuous pumping of water. It incorporates an impeller, allowing large volumes of water to be pumped quickly. Flygt pumps were used by institutes such as the then Institute of Marine Environmental Research (now Plymouth Marine Laboratory) for oceanographic sampling in the 1970s. This allowed continuous monitoring of water properties as well as the collection of discrete samples from the pump outflow."@en ;
  skos:inScheme <http://vocab.nerc.ac.uk/scheme/SDNDEV/current> ;
  skos:notation "SDN:L22::TOOL0539" ;
  skos:note "accepted"@en ;
  skos:prefLabel "Flygt pump"@en ;
  skos:related <http://vocab.nerc.ac.uk/collection/B75/current/ORG00001> ;
.
inst:TOOL0540
  rdf:type skos:Concept ;
  dcterm:date "2012-09-25 16:03:31.0" ;
  dcterm:identifier "SDN:L22::TOOL0540" ;
  pav:hasCurrentVersion <http://vocab.nerc.ac.uk/collection/L22/current/TOOL0540/1> ;
  owl:versionInfo "1" ;
  skos:altLabel "NIO bottle"@en ;
  skos:broader <http://vocab.nerc.ac.uk/collection/L05/current/30> ;
  skos:definition "A plastic free-flushing water sampling bottle designed for oceanographic sampling. It has valves at each end, which are held open on deployment. When the bottle reaches the desired depth the valves are released and sealed. A reversing thermometer may be mounted on the bottle. The bottle inverts on closure, triggering the thermometer. A sampling spigot is positioned at the base of the bottle. The bottle was designed in the 1970s by Francis E. Pierce, Dennis I. Gaunt, and Richard Dobson at what was  then the National Institute of Oceanography, UK (a predecessor of the National Oceanography Centre)."@en ;
  skos:inScheme <http://vocab.nerc.ac.uk/scheme/SDNDEV/current> ;
  skos:notation "SDN:L22::TOOL0540" ;
  skos:note "accepted"@en ;
  skos:prefLabel "National Institute of Oceanography water sampling bottle"@en ;
  skos:related <http://vocab.nerc.ac.uk/collection/B75/current/ORG00001> ;
.
inst:TOOL0541
  rdf:type skos:Concept ;
  dcterm:date "2012-09-26 16:33:22.0" ;
  dcterm:identifier "SDN:L22::TOOL0541" ;
  pav:hasCurrentVersion <http://vocab.nerc.ac.uk/collection/L22/current/TOOL0541/1> ;
  owl:versionInfo "1" ;
  skos:altLabel "UEA rainwater sampler"@en ;
  skos:broader <http://vocab.nerc.ac.uk/collection/L05/current/14> ;
  skos:definition "A rainwater sampler comprising a 40 cm diameter polypropylene plastic funnel feeding into a low density polyethylene (LDPE) bottle."@en ;
  skos:inScheme <http://vocab.nerc.ac.uk/scheme/SDNDEV/current> ;
  skos:notation "SDN:L22::TOOL0541" ;
  skos:note "accepted"@en ;
  skos:prefLabel "University of East Anglia rainwater sampler"@en ;
  skos:related <http://vocab.nerc.ac.uk/collection/B75/current/ORG00024> ;
.
inst:TOOL0542
  rdf:type skos:Concept ;
  dcterm:date "2012-09-26 16:33:22.0" ;
  dcterm:identifier "SDN:L22::TOOL0542" ;
  pav:hasCurrentVersion <http://vocab.nerc.ac.uk/collection/L22/current/TOOL0542/1> ;
  owl:versionInfo "1" ;
  skos:altLabel "Polypropylene 10L bottle"@en ;
  skos:broader <http://vocab.nerc.ac.uk/collection/L05/current/30> ;
  skos:definition "Polypropylene plastic bottle with 10 litre capacity used for surface sampling from small boats during OMEX and LOIS RACS projects in the 1990s."@en ;
  skos:inScheme <http://vocab.nerc.ac.uk/scheme/SDNDEV/current> ;
  skos:notation "SDN:L22::TOOL0542" ;
  skos:note "accepted"@en ;
  skos:prefLabel "Polypropylene 10L surface sample bottle"@en ;
  skos:related <http://vocab.nerc.ac.uk/collection/B75/current/ORG00001> ;
.
inst:TOOL0543
  rdf:type skos:Concept ;
  dcterm:date "2012-09-26 16:33:22.0" ;
  dcterm:identifier "SDN:L22::TOOL0543" ;
  pav:hasCurrentVersion <http://vocab.nerc.ac.uk/collection/L22/current/TOOL0543/1> ;
  owl:versionInfo "1" ;
  skos:altLabel "Transparent sample bottle"@en ;
  skos:broader <http://vocab.nerc.ac.uk/collection/L05/current/30> ;
  skos:definition "Sampling bottle of unknown material that posseses the physical property of allowing the transmission of light with little or no intereference."@en ;
  skos:inScheme <http://vocab.nerc.ac.uk/scheme/SDNDEV/current> ;
  skos:notation "SDN:L22::TOOL0543" ;
  skos:note "accepted"@en ;
  skos:prefLabel "Transparent sample bottle"@en ;
  skos:related <http://vocab.nerc.ac.uk/collection/B75/current/ORG00001> ;
.
inst:TOOL0544
  rdf:type skos:Concept ;
  dcterm:date "2012-09-26 16:33:22.0" ;
  dcterm:identifier "SDN:L22::TOOL0544" ;
  pav:hasCurrentVersion <http://vocab.nerc.ac.uk/collection/L22/current/TOOL0544/1> ;
  owl:versionInfo "1" ;
  skos:altLabel "Electropolished canister"@en ;
  skos:broader <http://vocab.nerc.ac.uk/collection/L05/current/11> ;
  skos:definition "Metal sampling container of unknown make and capacity that has been smoothed by electropolishing (also known as electrochemical or electrolytic polishing). Suitable for the collection of high pressure air samples."@en ;
  skos:inScheme <http://vocab.nerc.ac.uk/scheme/SDNDEV/current> ;
  skos:notation "SDN:L22::TOOL0544" ;
  skos:note "accepted"@en ;
  skos:prefLabel "Electropolished air sample canister"@en ;
  skos:related <http://vocab.nerc.ac.uk/collection/B75/current/ORG00001> ;
.
inst:TOOL0545
  rdf:type skos:Concept ;
  dcterm:date "2012-09-26 16:33:22.0" ;
  dcterm:identifier "SDN:L22::TOOL0545" ;
  pav:hasCurrentVersion <http://vocab.nerc.ac.uk/collection/L22/current/TOOL0545/1> ;
  owl:versionInfo "1" ;
  skos:altLabel "Stainless steel canister"@en ;
  skos:broader <http://vocab.nerc.ac.uk/collection/L05/current/11> ;
  skos:definition "Stainless steel sampling container suitable for the collection of high pressure air samples. The container has a capacity of several litres."@en ;
  skos:inScheme <http://vocab.nerc.ac.uk/scheme/SDNDEV/current> ;
  skos:notation "SDN:L22::TOOL0545" ;
  skos:note "accepted"@en ;
  skos:prefLabel "Stainless steel air sample canister"@en ;
  skos:related <http://vocab.nerc.ac.uk/collection/B75/current/ORG00001> ;
.
inst:TOOL0546
  rdf:type skos:Concept ;
  dcterm:date "2012-09-26 16:33:22.0" ;
  dcterm:identifier "SDN:L22::TOOL0546" ;
  pav:hasCurrentVersion <http://vocab.nerc.ac.uk/collection/L22/current/TOOL0546/1> ;
  owl:versionInfo "1" ;
  skos:altLabel "PML Interfacial Sampler"@en ;
  skos:broader <http://vocab.nerc.ac.uk/collection/L05/current/30> ;
  skos:definition "A sampler comprising a frame fitted with 10 horizontal syringe-type 4 litre water bottles. An electronic control cylinder, mounted in the top of the frame, is programmed to release the bottle pistons once the frame has settled on the seabed and disturbed sediment has had time to disperse. The release of the piston draws in a sample and, at completion of the piston stroke, a mechanism is triggered to close the bottle inlet."@en ;
  skos:inScheme <http://vocab.nerc.ac.uk/scheme/SDNDEV/current> ;
  skos:notation "SDN:L22::TOOL0546" ;
  skos:note "accepted"@en ;
  skos:prefLabel "Plymouth Marine Laboratory Interfacial Sampler"@en ;
  skos:related <http://vocab.nerc.ac.uk/collection/B75/current/ORG00023> ;
.
inst:TOOL0547
  rdf:type skos:Concept ;
  dcterm:date "2012-09-26 16:33:22.0" ;
  dcterm:identifier "SDN:L22::TOOL0547" ;
  pav:hasCurrentVersion <http://vocab.nerc.ac.uk/collection/L22/current/TOOL0547/1> ;
  owl:versionInfo "1" ;
  skos:altLabel "Lancs Uni syringe sampler"@en ;
  skos:broader <http://vocab.nerc.ac.uk/collection/L05/current/30> ;
  skos:definition "A water sample collection system comprising a peristaltic pump attached to a syringe, allowing near-surface samples to be gathered without introducing oxygen (a closed system)."@en ;
  skos:inScheme <http://vocab.nerc.ac.uk/scheme/SDNDEV/current> ;
  skos:notation "SDN:L22::TOOL0547" ;
  skos:note "accepted"@en ;
  skos:prefLabel "Lancaster University syringe water sampler"@en ;
  skos:related <http://vocab.nerc.ac.uk/collection/B75/current/ORG00068> ;
.
inst:TOOL0548
  rdf:type skos:Concept ;
  dcterm:date "2012-09-26 16:33:22.0" ;
  dcterm:identifier "SDN:L22::TOOL0548" ;
  pav:hasCurrentVersion <http://vocab.nerc.ac.uk/collection/L22/current/TOOL0548/1> ;
  owl:versionInfo "1" ;
  skos:altLabel "PML NSSD"@en ;
  skos:broader <http://vocab.nerc.ac.uk/collection/L05/current/30> ;
  skos:definition "A water sample collection system comprising a flotation ring supporting a central vertical spar that carries a 8 sampling bottles, of which the upper 5 are vertically spaced at 20 cm intervals and the lower 3 at approximately 30 cm intervals. The spar also carries an array of thermistors spaced at logarithmic intervals between a few mm below the surface to approximately 2 m depth. Atop the spar is a control system which continuously logs the thermistor data. The device is deployed from a vessel and allowed to drift away on a tether with a conductive core. Thermistor data are transmitted up the cable to a host computer on board the ship, while the control system allows for the remote firing of the sampling bottles by the host computer."@en ;
  skos:inScheme <http://vocab.nerc.ac.uk/scheme/SDNDEV/current> ;
  skos:notation "SDN:L22::TOOL0548" ;
  skos:note "accepted"@en ;
  skos:prefLabel "Plymouth Marine Laboratory Near-Surface Sampling Device"@en ;
  skos:related <http://vocab.nerc.ac.uk/collection/B75/current/ORG00023> ;
.
inst:TOOL0550
  rdf:type skos:Concept ;
  dcterm:date "2012-09-26 16:33:22.0" ;
  dcterm:identifier "SDN:L22::TOOL0550" ;
  pav:hasCurrentVersion <http://vocab.nerc.ac.uk/collection/L22/current/TOOL0550/1> ;
  owl:versionInfo "1" ;
  skos:altLabel "UEA LVAS"@en ;
  skos:broader <http://vocab.nerc.ac.uk/collection/L05/current/13> ;
  skos:definition "An atmospheric sampler that pumps air through a series of filters to collect samples for off-line analysis of aerosol and gas-phase constituents. Air samples are drawn into a sheltered housing, and through a PTFE filter, which collect samples of particulate material. The air is then drawn through a pair of oxalic acid-impregnated paper filters, which trap gas-phase components. The pump is chosen to produce a flow rate of approximately 50 litres per minute. Inline flow meters between the filter set and the pump determine the volume of air sampled."@en ;
  skos:inScheme <http://vocab.nerc.ac.uk/scheme/SDNDEV/current> ;
  skos:notation "SDN:L22::TOOL0550" ;
  skos:note "accepted"@en ;
  skos:prefLabel "University of East Anglia Low Volume Air Sampler"@en ;
  skos:related <http://vocab.nerc.ac.uk/collection/B75/current/ORG00024> ;
.
inst:TOOL0551
  rdf:type skos:Concept ;
  dcterm:date "2012-09-26 16:33:22.0" ;
  dcterm:identifier "SDN:L22::TOOL0551" ;
  pav:hasCurrentVersion <http://vocab.nerc.ac.uk/collection/L22/current/TOOL0551/1> ;
  owl:versionInfo "1" ;
  skos:altLabel "HVAS"@en ;
  skos:broader <http://vocab.nerc.ac.uk/collection/L05/current/13> ;
  skos:definition "An atmospheric sampler that pumps air through a series of filters and traps to collect samples for off-line analysis of aerosol and gas-phase constituents. Air samples are drawn into a sheltered housing, and through one or more aerosol filters, which collect samples of particulate material. Successive aerosol filters may have smaller pore sizes to collect size fractionated aerosol samples. The air may then be drawn through one or more gas-phase filters or traps, such as reagent-soaked filter papers, reagent-filled impingers, or resin (polymer) traps. Flow meters between the filter set and the pump determine the volume of air sampled."@en ;
  skos:inScheme <http://vocab.nerc.ac.uk/scheme/SDNDEV/current> ;
  skos:notation "SDN:L22::TOOL0551" ;
  skos:note "accepted"@en ;
  skos:prefLabel "High Volume Air Sampler"@en ;
  skos:related <http://vocab.nerc.ac.uk/collection/B75/current/ORG00001> ;
.
inst:TOOL0552
  rdf:type skos:Concept ;
  dcterm:date "2012-09-26 17:11:56.0" ;
  dcterm:identifier "SDN:L22::TOOL0552" ;
  pav:hasCurrentVersion <http://vocab.nerc.ac.uk/collection/L22/current/TOOL0552/1> ;
  owl:versionInfo "1" ;
  skos:altLabel "Nereides 300l bottle"@en ;
  skos:broader <http://vocab.nerc.ac.uk/collection/L05/current/30> ;
  skos:definition "A 300 litre capacity sampling bottle designed for oceanographic sampling. The bottle was closed by a messenger. It was used during the OMEX project in the 1990s."@en ;
  skos:inScheme <http://vocab.nerc.ac.uk/scheme/SDNDEV/current> ;
  skos:notation "SDN:L22::TOOL0552" ;
  skos:note "accepted"@en ;
  skos:prefLabel "Nereides 300l sample bottle"@en ;
  skos:related <http://vocab.nerc.ac.uk/collection/B75/current/ORG00633> ;
.
inst:TOOL0553
  rdf:type skos:Concept ;
  dcterm:date "2012-11-15 10:40:15.0" ;
  dcterm:identifier "SDN:L22::TOOL0553" ;
  pav:hasCurrentVersion <http://vocab.nerc.ac.uk/collection/L22/current/TOOL0553/3> ;
  pav:hasVersion <http://vocab.nerc.ac.uk/collection/L22/current/TOOL0553/1> ;
  pav:hasVersion <http://vocab.nerc.ac.uk/collection/L22/current/TOOL0553/2> ;
  owl:versionInfo "3" ;
  skos:altLabel "DGT trace metal sampler"@en ;
  skos:broader sdev:TFSAMP ;
  skos:definition "A device designed to measure concentrations of dissolved metal species in water. It comprises a plastic casing that contains a Chelex resin impregnated in a hydrogel to accumulate metals. The resin layer is overlain by a diffusive layer of hydrogel and a filter. Ions diffuse through the filter and diffusive layer to reach the resin layer, thereby establishing a constant concentration gradient in the diffusive layer that allows the quantitative measurement of labile species in solution through laboratory analysis."@en ;
  skos:inScheme <http://vocab.nerc.ac.uk/scheme/SDNDEV/current> ;
  skos:notation "SDN:L22::TOOL0553" ;
  skos:note "accepted"@en ;
  skos:prefLabel "DGT Research Diffusive Gradients in Thin Films trace metal sampler"@en ;
  skos:related <http://vocab.nerc.ac.uk/collection/B75/current/ORG00634> ;
.
inst:TOOL0554
  rdf:type skos:Concept ;
  dcterm:date "2012-09-28 09:56:09.0" ;
  dcterm:identifier "SDN:L22::TOOL0554" ;
  pav:hasCurrentVersion <http://vocab.nerc.ac.uk/collection/L22/current/TOOL0554/1> ;
  owl:versionInfo "1" ;
  skos:altLabel "UMA 4-stage CCI"@en ;
  skos:broader <http://vocab.nerc.ac.uk/collection/L05/current/13> ;
  skos:definition "An aerosol sampler modelled on the Harvard Compact Cascade Impactor. Sample air is accelerated through an orifice towards a collector plate, which deflects the airflow around it. Particles too large to follow the streamlines impact on the plate. The air stream, now with the largest particles removed, proceeds to the subsequent impactor stages, each tuned to collect successively smaller particles. The four stages collect particles in the following size categories: greater than 9.9 um; 5.3-9.9 um; 1.0-5.3 um; 0.16-1.0 um."@en ;
  skos:inScheme <http://vocab.nerc.ac.uk/scheme/SDNDEV/current> ;
  skos:notation "SDN:L22::TOOL0554" ;
  skos:note "accepted"@en ;
  skos:prefLabel "University of Manchester 4-stage Compact Cascade Impactor"@en ;
  skos:related <http://vocab.nerc.ac.uk/collection/B75/current/ORG00123> ;
.
inst:TOOL0555
  rdf:type skos:Concept ;
  dcterm:date "2012-09-28 14:08:54.0" ;
  dcterm:identifier "SDN:L22::TOOL0555" ;
  pav:hasCurrentVersion <http://vocab.nerc.ac.uk/collection/L22/current/TOOL0555/1> ;
  owl:versionInfo "1" ;
  skos:altLabel "NOC torpedo towfish"@en ;
  skos:broader <http://vocab.nerc.ac.uk/collection/L05/current/31> ;
  skos:definition "An epoxy resin-coated steel torpedo-shaped object designed to be towed alongside a moving ship at speeds of 1-12 knots. A teflon-lined tube runs through the centre of the fish and is connected to a pump on board the ship. Stabilising fins at the rear of the fish ensure that the sampling hose points forwards and that the fish maintains a roughly constant depth. The system is typically used for continuous, underway, clean sampling (e.g., trace metal studies) of near-surface waters."@en ;
  skos:inScheme <http://vocab.nerc.ac.uk/scheme/SDNDEV/current> ;
  skos:notation "SDN:L22::TOOL0555" ;
  skos:note "accepted"@en ;
  skos:prefLabel "National Oceanography Centre torpedo towfish water sampler"@en ;
  skos:related <http://vocab.nerc.ac.uk/collection/B75/current/ORG00009> ;
.
inst:TOOL0556
  rdf:type skos:Concept ;
  dcterm:date "2012-09-28 14:08:54.0" ;
  dcterm:identifier "SDN:L22::TOOL0556" ;
  pav:hasCurrentVersion <http://vocab.nerc.ac.uk/collection/L22/current/TOOL0556/1> ;
  owl:versionInfo "1" ;
  skos:altLabel "Glass bottle and bung"@en ;
  skos:broader <http://vocab.nerc.ac.uk/collection/L05/current/30> ;
  skos:definition "Glass bottle of unknown capacity used for manual water sampling. The bottle was sealed with a bung attached to a rope. The system was used for near-surface sampling during the Marine and Freshwater Microbial Biodiversity project for sampling in Priest Pot."@en ;
  skos:inScheme <http://vocab.nerc.ac.uk/scheme/SDNDEV/current> ;
  skos:notation "SDN:L22::TOOL0556" ;
  skos:note "accepted"@en ;
  skos:prefLabel "Glass bottle and bung water sampler"@en ;
  skos:related <http://vocab.nerc.ac.uk/collection/B75/current/ORG00001> ;
.
inst:TOOL0557
  rdf:type skos:Concept ;
  dcterm:date "2012-10-04 11:59:23.0" ;
  dcterm:identifier "SDN:L22::TOOL0557" ;
  pav:hasCurrentVersion <http://vocab.nerc.ac.uk/collection/L22/current/TOOL0557/2> ;
  pav:hasVersion <http://vocab.nerc.ac.uk/collection/L22/current/TOOL0557/1> ;
  owl:versionInfo "2" ;
  skos:altLabel "ISOMAP-UK manual sampler"@en ;
  skos:broader <http://vocab.nerc.ac.uk/collection/L05/current/30> ;
  skos:definition "Manual water sample collection system used during the RAPID ISOMAP-UK project. It comprises a sample container attached to the end of an extendable pole marked with target depths. The container is fitted with a sealing plug attached to a long cord. Samples are obtained by lowering the pole (or just the container for surface samples) vertically into the water. At the required depth the cord is pulled, thereby removing the plug and filling the container. After 30 seconds the container is brought slowly to the surface and the sample transfered to a storage bottle."@en ;
  skos:inScheme <http://vocab.nerc.ac.uk/scheme/SDNDEV/current> ;
  skos:notation "SDN:L22::TOOL0557" ;
  skos:note "accepted"@en ;
  skos:prefLabel "RAPID ISOMAP-UK manual water sampler"@en ;
  skos:related <http://vocab.nerc.ac.uk/collection/B75/current/ORG00001> ;
.
inst:TOOL0561
  rdf:type skos:Concept ;
  dcterm:date "2012-10-17 15:58:06.0" ;
  dcterm:identifier "SDN:L22::TOOL0561" ;
  pav:hasCurrentVersion <http://vocab.nerc.ac.uk/collection/L22/current/TOOL0561/2> ;
  pav:hasVersion <http://vocab.nerc.ac.uk/collection/L22/current/TOOL0561/1> ;
  owl:versionInfo "2" ;
  skos:altLabel "Clean pumped sea water supply"@en ;
  skos:broader <http://vocab.nerc.ac.uk/collection/L05/current/31> ;
  skos:definition "The system comprises a precision echosounder (PES) fish attached to a clean, reinforced tube (typically composed of braided PVC). The fish is designed to be towed alongside a moving ship at a depth of 1-3m and water is drawn through the system by a clean pump. The tube usually leads to a clean laboratory on board the vessel, inside which samples are drawn for analysis. The system is typically used for continuous, underway, clean sampling (e.g., trace metal studies) of near-surface waters."@en ;
  skos:inScheme <http://vocab.nerc.ac.uk/scheme/SDNDEV/current> ;
  skos:notation "SDN:L22::TOOL0561" ;
  skos:note "accepted"@en ;
  skos:prefLabel "Clean pumped sea water supply"@en ;
  skos:related <http://vocab.nerc.ac.uk/collection/B75/current/ORG00001> ;
.
inst:TOOL0562
  rdf:type skos:Concept ;
  dcterm:date "2012-10-15 14:57:16.0" ;
  dcterm:identifier "SDN:L22::TOOL0562" ;
  pav:hasCurrentVersion <http://vocab.nerc.ac.uk/collection/L22/current/TOOL0562/1> ;
  owl:versionInfo "1" ;
  skos:altLabel "IFM clean pumped sea water supply"@en ;
  skos:broader <http://vocab.nerc.ac.uk/collection/L05/current/31> ;
  skos:definition "A system designed for continuous, underway, clean sampling of near-surface waters. A hollow stainless steel shaft holding a high density polyethylene (HDPE) tube is submerged beneath a vessel through a hole in the hull. The inlet head is located 1.7 m below the keel and features a sieve-like Teflon cap. Water is pumped from the inlet through a serial ball-valve panel from which it can be directed to different sampling facilities. Flow is maintained by chemically inert double membrane pump driven by compressed air. HDPE tubing is used throughout the system and the valves are composed of polypropylene and Teflon, thereby ensuring that the sampled water remains clean and suitable for trace metal analyses. The system was developed by what was then the Institut fur Meereskunde at Kiel University."@en ;
  skos:inScheme <http://vocab.nerc.ac.uk/scheme/SDNDEV/current> ;
  skos:notation "SDN:L22::TOOL0562" ;
  skos:note "accepted"@en ;
  skos:prefLabel "IFM Kiel clean pumped sea water supply"@en ;
  skos:related <http://vocab.nerc.ac.uk/collection/B75/current/ORG00204> ;
.
inst:TOOL0563
  rdf:type skos:Concept ;
  dcterm:date "2012-10-15 14:57:16.0" ;
  dcterm:identifier "SDN:L22::TOOL0563" ;
  pav:hasCurrentVersion <http://vocab.nerc.ac.uk/collection/L22/current/TOOL0563/1> ;
  owl:versionInfo "1" ;
  skos:altLabel "Cyclonic separation sampler"@en ;
  skos:broader <http://vocab.nerc.ac.uk/collection/L05/current/58> ;
  skos:definition "A device designed to remove particulates from an air, gas or liquid stream through vortex separation. A high speed rotating flow is established within a vertical cylindrical or conical container, where the stream to be separated is fed in the top (wide) end, flows helically around the container to the bottom (narrow) end and then exits the cyclone in a straight stream through the centre and out the top. Instead of following the flow of the stream, the inertia of large (dense) particles causes them to hit the sides of the container and fall to the bottom, where they can be removed. The cyclone geometry and flow rate define a cut point, which is the size of the particle that will be removed from the stream with 50% efficiency. Larger particles will be removed with a greater efficiency and smaller particles with a lower efficiency. The sampler may be used in series with filters designed to collect different target particles."@en ;
  skos:inScheme <http://vocab.nerc.ac.uk/scheme/SDNDEV/current> ;
  skos:notation "SDN:L22::TOOL0563" ;
  skos:note "accepted"@en ;
  skos:prefLabel "Cyclonic separation sampler"@en ;
  skos:related <http://vocab.nerc.ac.uk/collection/B75/current/ORG00001> ;
.
inst:TOOL0571
  rdf:type skos:Concept ;
  dcterm:date "2012-11-15 09:32:51.0" ;
  dcterm:identifier "SDN:L22::TOOL0571" ;
  pav:hasCurrentVersion <http://vocab.nerc.ac.uk/collection/L22/current/TOOL0571/1> ;
  owl:versionInfo "1" ;
  skos:altLabel "Copper pipe air sampler"@en ;
  skos:broader <http://vocab.nerc.ac.uk/collection/L05/current/58> ;
  skos:definition "Copper tubing leading directly from the least contaminated part of a ship to an analytical instrument. Air is drawn through the pipe by the instrument."@en ;
  skos:inScheme <http://vocab.nerc.ac.uk/scheme/SDNDEV/current> ;
  skos:notation "SDN:L22::TOOL0571" ;
  skos:note "accepted"@en ;
  skos:prefLabel "Copper pipe air sampler"@en ;
  skos:related <http://vocab.nerc.ac.uk/collection/B75/current/ORG00001> ;
.
inst:TOOL0573
  rdf:type skos:Concept ;
  dcterm:date "2012-11-28 14:15:26.0" ;
  dcterm:identifier "SDN:L22::TOOL0573" ;
  pav:hasCurrentVersion <http://vocab.nerc.ac.uk/collection/L22/current/TOOL0573/1> ;
  owl:versionInfo "1" ;
  skos:altLabel "Teflon PFA manifold air sampler"@en ;
  skos:broader <http://vocab.nerc.ac.uk/collection/L05/current/58> ;
  skos:definition "Teflon PFA manifold leading directly from the least contaminated part of a ship to a clean metal bellows pump. Air is drawn through the tube by the pump at a flow rate of 30 litres/min and a subsample is fed into an analytical instrument."@en ;
  skos:inScheme <http://vocab.nerc.ac.uk/scheme/SDNDEV/current> ;
  skos:notation "SDN:L22::TOOL0573" ;
  skos:note "accepted"@en ;
  skos:prefLabel "Teflon PFA manifold air sampler"@en ;
  skos:related <http://vocab.nerc.ac.uk/collection/B75/current/ORG00001> ;
.
inst:TOOL0588
  rdf:type skos:Concept ;
  dcterm:date "2013-01-15 15:43:48.0" ;
  dcterm:identifier "SDN:L22::TOOL0588" ;
  pav:hasCurrentVersion <http://vocab.nerc.ac.uk/collection/L22/current/TOOL0588/1> ;
  owl:versionInfo "1" ;
  skos:altLabel "Tedlar bag"@en ;
  skos:broader <http://vocab.nerc.ac.uk/collection/L05/current/11> ;
  skos:definition "A generic term for atmospheric sampling bags manufactured from Tedlar (DuPont trade name for the chemically inert plastic polyvinyl fluoride) film, fitted with a polypropylene or stainless steel valve and available with capacities ranging from 1-100 litres.  Samples are taken by either pumping air into the bag or evacuating the bag and opening the valve at the sampling site. Filled bags are connected directly to measuring equipment for analysis. Bags are available from several manufactureres and suppliers"@en ;
  skos:inScheme <http://vocab.nerc.ac.uk/scheme/SDNDEV/current> ;
  skos:notation "SDN:L22::TOOL0588" ;
  skos:note "accepted"@en ;
  skos:prefLabel "Tedlar atmospheric sampling bag"@en ;
  skos:related <http://vocab.nerc.ac.uk/collection/B75/current/ORG00001> ;
.
inst:TOOL0651
  rdf:type skos:Concept ;
  dcterm:date "2013-11-19 09:51:15.0" ;
  dcterm:identifier "SDN:L22::TOOL0651" ;
  pav:hasCurrentVersion <http://vocab.nerc.ac.uk/collection/L22/current/TOOL0651/2> ;
  pav:hasVersion <http://vocab.nerc.ac.uk/collection/L22/current/TOOL0651/1> ;
  owl:versionInfo "2" ;
  skos:altLabel "Beam trawl"@en ;
  skos:broader <http://vocab.nerc.ac.uk/collection/L05/current/62> ;
  skos:definition "A net that is held open by a solid wooden or metal beam, attached to plates at the ends that act as runners over the seabed. The beam can vary in length from 2-12m. A chain mat may be fitted to the beam to increase seabed disturbance. The net is towed on the seabed and the resulting disturbance causes fish and shellfish to swim up and get caught in the net."@en ;
  skos:inScheme <http://vocab.nerc.ac.uk/scheme/SDNDEV/current> ;
  skos:notation "SDN:L22::TOOL0651" ;
  skos:note "accepted"@en ;
  skos:prefLabel "Unknown beam trawl"@en ;
.
inst:TOOL0652
  rdf:type skos:Concept ;
  dcterm:date "2013-11-19 10:00:04.0" ;
  dcterm:identifier "SDN:L22::TOOL0652" ;
  pav:hasCurrentVersion <http://vocab.nerc.ac.uk/collection/L22/current/TOOL0652/1> ;
  owl:versionInfo "1" ;
  skos:altLabel "CEFAS 4m beam trawl"@en ;
  skos:broader <http://vocab.nerc.ac.uk/collection/L05/current/62> ;
  skos:definition "This is the standard net used by the CEFAS fisheries laboratory for beam trawl surveys in UK coastal waters. The net is held open by a 4m (measured inside the end plates) metal beam with a chain mat attached to the beam to increase seabed disturbance. 75mm cod ends were optionally fitted with 40mm liners. Post-1991 80mm (post-1991) cod ends were always fitted with 40mm liners."@en ;
  skos:inScheme <http://vocab.nerc.ac.uk/scheme/SDNDEV/current> ;
  skos:notation "SDN:L22::TOOL0652" ;
  skos:note "accepted"@en ;
  skos:prefLabel "CEFAS 4m survey beam trawl"@en ;
.
inst:TOOL0653
  rdf:type skos:Concept ;
  dcterm:date "2013-11-26 08:11:24.0" ;
  dcterm:identifier "SDN:L22::TOOL0653" ;
  pav:hasCurrentVersion <http://vocab.nerc.ac.uk/collection/L22/current/TOOL0653/2> ;
  pav:hasVersion <http://vocab.nerc.ac.uk/collection/L22/current/TOOL0653/1> ;
  owl:versionInfo "2" ;
  skos:altLabel "Van Veen grab"@en ;
  skos:broader <http://vocab.nerc.ac.uk/collection/L05/current/50> ;
  skos:definition "A simple clam-shell sediment grab penetrating approximately 20cm with a typical sampling area of 0.1m2 (but grab sizes can vary). On descent two levers with buckets at their ends are spread like open scissors that unlock on hitting the seabed. When pulled upwards the two buckets close and grab a sample. This is subject to more disturbance than by Craib or box corers."@en ;
  skos:inScheme <http://vocab.nerc.ac.uk/scheme/SDNDEV/current> ;
  skos:notation "SDN:L22::TOOL0653" ;
  skos:note "accepted"@en ;
  skos:prefLabel "Van Veen grab"@en ;
.
inst:TOOL0660
  rdf:type skos:Concept ;
  dcterm:date "2014-01-28 11:01:06.0" ;
  dcterm:identifier "SDN:L22::TOOL0660" ;
  pav:hasCurrentVersion <http://vocab.nerc.ac.uk/collection/L22/current/TOOL0660/2> ;
  pav:hasVersion <http://vocab.nerc.ac.uk/collection/L22/current/TOOL0660/1> ;
  owl:versionInfo "2" ;
  skos:altLabel "OSIL MSC"@en ;
  skos:broader <http://vocab.nerc.ac.uk/collection/L05/current/30> ;
  skos:definition "The Marine Snow Catcher is a large volume water bottle designed to collect Marine Snow particles. The water transport through the device during the descent is controlled through two large diameter terminal apertures constructed to reduce turbulence. The device is usually rested upright after recovery to allow the marine particles to sink to the bottom, after which, the overlying water is slowly drained off via a tap. The bottom section of the water bottle is detachable allowing recovery of the marine snow."@en ;
  skos:inScheme <http://vocab.nerc.ac.uk/scheme/SDNDEV/current> ;
  skos:notation "SDN:L22::TOOL0660" ;
  skos:note "accepted"@en ;
  skos:prefLabel "OSIL Marine Snow Catcher"@en ;
  skos:related <http://vocab.nerc.ac.uk/collection/B75/current/ORG00411> ;
.
inst:TOOL0784
  rdf:type skos:Concept ;
  dcterm:date "2014-08-28 09:27:27.0" ;
  dcterm:identifier "SDN:L22::TOOL0784" ;
  pav:hasCurrentVersion <http://vocab.nerc.ac.uk/collection/L22/current/TOOL0784/1> ;
  owl:versionInfo "1" ;
  skos:altLabel "SMBA multicorer"@en ;
  skos:broader <http://vocab.nerc.ac.uk/collection/L05/current/51> ;
  skos:definition "A corer designed at SMBA (current name Scottish Association for Marine Science) that collects multiple undisturbed samples of the upper sediment, flocculent material and overlying water. This is achieved by a hydraulically-damped controlled descent of the open core liners once the frame has landed on the seabed. Rubber seals at the top and bottom of the core liner prevent sample loss during recovery. The outer framework supports weighted arrays of polycarbonate liners (4 split liners of 10cm internal diameter and 8 split liners of 6 cm internal diameter) hanging from a water-filled dashpot."@en ;
  skos:inScheme <http://vocab.nerc.ac.uk/scheme/SDNDEV/current> ;
  skos:notation "SDN:L22::TOOL0784" ;
  skos:note "accepted"@en ;
  skos:prefLabel "Barnett-Watson multiple corer"@en ;
  skos:related <http://vocab.nerc.ac.uk/collection/B75/current/ORG00005> ;
.
inst:TOOL0785
  rdf:type skos:Concept ;
  dcterm:date "2014-09-01 08:06:25.0" ;
  dcterm:identifier "SDN:L22::TOOL0785" ;
  pav:hasCurrentVersion <http://vocab.nerc.ac.uk/collection/L22/current/TOOL0785/1> ;
  owl:versionInfo "1" ;
  skos:altLabel "PARFLUX Mark78H-21"@en ;
  skos:broader <http://vocab.nerc.ac.uk/collection/L05/current/33> ;
  skos:definition "A sediment trap designed for mid-water mooring deployment (maximum depth 6500m) with a conical collector passing settled particles into one of a set of bottles mounted in a carousel. The bottles are changed after a user-selected period of time.  An optional wet sample particle divider may be fitted to divide wet specimens into 5-10 equal parts. Compass/tilt and pressure sensors may also be fitted.  This model carries 21 bottles (250 or 500 ml) and is 1.64m tall and 0.91m diameter."@en ;
  skos:inScheme <http://vocab.nerc.ac.uk/scheme/SDNDEV/current> ;
  skos:notation "SDN:L22::TOOL0785" ;
  skos:note "accepted"@en ;
  skos:prefLabel "McLane PARFLUX Mark78H-21 Sediment Traps"@en ;
  skos:related <http://vocab.nerc.ac.uk/collection/B75/current/ORG00996> ;
.
inst:TOOL0786
  rdf:type skos:Concept ;
  dcterm:date "2014-09-01 08:07:46.0" ;
  dcterm:identifier "SDN:L22::TOOL0786" ;
  pav:hasCurrentVersion <http://vocab.nerc.ac.uk/collection/L22/current/TOOL0786/1> ;
  owl:versionInfo "1" ;
  skos:altLabel "PARFLUX Mark78HW-13"@en ;
  skos:broader <http://vocab.nerc.ac.uk/collection/L05/current/33> ;
  skos:definition "A sediment trap designed for mid-water mooring deployment (maximum depth 6500m) with a conical collector passing settled particles into one of a set of bottles mounted in a carousel. The bottles are changed after a user-selected period of time.  An optional wet sample particle divider may be fitted to divide wet specimens into 5-10 equal parts. Compass/tilt and pressure sensors may also be fitted. This model carries 13 wide bottles (250 or 500 ml) and is 1.64m tall and 0.91m diameter."@en ;
  skos:inScheme <http://vocab.nerc.ac.uk/scheme/SDNDEV/current> ;
  skos:notation "SDN:L22::TOOL0786" ;
  skos:note "accepted"@en ;
  skos:prefLabel "McLane PARFLUX Mark78HW-13 Sediment Traps"@en ;
  skos:related <http://vocab.nerc.ac.uk/collection/B75/current/ORG00996> ;
.
inst:TOOL0787
  rdf:type skos:Concept ;
  dcterm:date "2014-09-01 08:09:10.0" ;
  dcterm:identifier "SDN:L22::TOOL0787" ;
  pav:hasCurrentVersion <http://vocab.nerc.ac.uk/collection/L22/current/TOOL0787/1> ;
  owl:versionInfo "1" ;
  skos:altLabel "PARFLUX Mark8-13"@en ;
  skos:broader <http://vocab.nerc.ac.uk/collection/L05/current/33> ;
  skos:definition "A sediment trap designed for mid-water mooring deployment (maximum depth 6500m) with a conical collector passing settled particles into one of a set of bottles mounted in a carousel. The bottles are changed after a user-selected period of time.  An optional wet sample particle divider may be fitted to divide wet specimens into 5-10 equal parts. Compass/tilt and pressure sensors may also be fitted. This model carries 13 bottles (250 or 500 ml) and is 1.16m tall and 0.66m diameter. The reduced size eases handling at sea."@en ;
  skos:inScheme <http://vocab.nerc.ac.uk/scheme/SDNDEV/current> ;
  skos:notation "SDN:L22::TOOL0787" ;
  skos:note "accepted"@en ;
  skos:prefLabel "McLane PARFLUX Mark8-13"@en ;
  skos:related <http://vocab.nerc.ac.uk/collection/B75/current/ORG00996> ;
.
inst:TOOL0788
  rdf:type skos:Concept ;
  dcterm:date "2014-09-12 17:20:07.0" ;
  dcterm:identifier "SDN:L22::TOOL0788" ;
  pav:hasCurrentVersion <http://vocab.nerc.ac.uk/collection/L22/current/TOOL0788/1> ;
  owl:versionInfo "1" ;
  skos:altLabel "Gunther grab"@en ;
  skos:broader <http://vocab.nerc.ac.uk/collection/L05/current/50> ;
  skos:definition "A light sediment grab, 12.5 cm wide and weighing 1kg. The grab is equipped with 8kg weights and nylon gauze sacks (0.5mm mesh size) for the sediment storage. The surface of the grab is 270 cm squared. Note that sizes and depths may vary. A full description is available in https://www.bodc.ac.uk/data/documents/nodb/pdf/Gunther_1963.pdf."@en ;
  skos:inScheme <http://vocab.nerc.ac.uk/scheme/SDNDEV/current> ;
  skos:notation "SDN:L22::TOOL0788" ;
  skos:note "accepted"@en ;
  skos:prefLabel "Gunther grab"@en ;
.
inst:TOOL0806
  rdf:type skos:Concept ;
  dcterm:date "2014-11-12 11:31:22.0" ;
  dcterm:identifier "SDN:L22::TOOL0806" ;
  pav:hasCurrentVersion <http://vocab.nerc.ac.uk/collection/L22/current/TOOL0806/2> ;
  pav:hasVersion <http://vocab.nerc.ac.uk/collection/L22/current/TOOL0806/1> ;
  owl:versionInfo "2" ;
  skos:altLabel "NIOZ 15cm PVC corer"@en ;
  skos:broader <http://vocab.nerc.ac.uk/collection/L05/current/51> ;
  skos:definition "A manual sediment corer produced by NIOZ for sampling sediments exposed at low tide. It comprises a 1m-long PVC tube with a diameter of 15 cm (core area 0.0175 m2) that has a closure the top. It is manually pushed approximately 25 cm into the sediment, the top is closed and then it is pulled out complete with the sediment sample."@en ;
  skos:inScheme <http://vocab.nerc.ac.uk/scheme/SDNDEV/current> ;
  skos:notation "SDN:L22::TOOL0806" ;
  skos:note "accepted"@en ;
  skos:prefLabel "NIOZ PVC 15cm manual sediment corer"@en ;
  skos:related <http://vocab.nerc.ac.uk/collection/B75/current/ORG00239> ;
.
inst:TOOL0807
  rdf:type skos:Concept ;
  dcterm:date "2014-11-12 11:31:22.0" ;
  dcterm:identifier "SDN:L22::TOOL0807" ;
  pav:hasCurrentVersion <http://vocab.nerc.ac.uk/collection/L22/current/TOOL0807/3> ;
  pav:hasVersion <http://vocab.nerc.ac.uk/collection/L22/current/TOOL0807/1> ;
  pav:hasVersion <http://vocab.nerc.ac.uk/collection/L22/current/TOOL0807/2> ;
  owl:versionInfo "3" ;
  skos:altLabel "NIOZ 10.5cm steel corer"@en ;
  skos:broader <http://vocab.nerc.ac.uk/collection/L05/current/51> ;
  skos:definition "A manual sediment corer produced by NIOZ for sampling sediments in shallow waters from a small boat.  It comprises a 10.5cm diameter (core area 0.009 m2) steel core with a closure at the top attached to a 2m aluminium pole. It is manually pushed approximately 25 cm into the sediment, the top is closed and then it is pulled out complete with the sediment sample."@en ;
  skos:inScheme <http://vocab.nerc.ac.uk/scheme/SDNDEV/current> ;
  skos:notation "SDN:L22::TOOL0807" ;
  skos:note "accepted"@en ;
  skos:prefLabel "NIOZ Steel 10.5cm manual sediment corer"@en ;
  skos:related <http://vocab.nerc.ac.uk/collection/B75/current/ORG00239> ;
.
inst:TOOL0817
  rdf:type skos:Concept ;
  dcterm:date "2015-01-09 14:18:23.0" ;
  dcterm:identifier "SDN:L22::TOOL0817" ;
  pav:hasCurrentVersion <http://vocab.nerc.ac.uk/collection/L22/current/TOOL0817/1> ;
  owl:versionInfo "1" ;
  skos:altLabel "Quadrat"@en ;
  skos:broader <http://vocab.nerc.ac.uk/collection/L05/current/59> ;
  skos:definition "A square or rectangular rigid frame of known area, often home-made, that is placed on the substrate to be sampled to mark a fixed area for sampling flora or fauna."@en ;
  skos:inScheme <http://vocab.nerc.ac.uk/scheme/SDNDEV/current> ;
  skos:notation "SDN:L22::TOOL0817" ;
  skos:note "accepted"@en ;
  skos:prefLabel "Quadrat"@en ;
  skos:related <http://vocab.nerc.ac.uk/collection/B75/current/ORG00001> ;
.
inst:TOOL0818
  rdf:type skos:Concept ;
  dcterm:date "2015-01-09 14:18:23.0" ;
  dcterm:identifier "SDN:L22::TOOL0818" ;
  pav:hasCurrentVersion <http://vocab.nerc.ac.uk/collection/L22/current/TOOL0818/1> ;
  owl:versionInfo "1" ;
  skos:altLabel "Point quadrat"@en ;
  skos:broader <http://vocab.nerc.ac.uk/collection/L05/current/59> ;
  skos:definition "A square or rectangular rigid frame of known area, often home-made, with a series of needles or nails at set distances throughout the quadrat. When placed on the substrate to be sampled the quadrat marks a fixed area and the needles or nails mark fixed sampling points within that area."@en ;
  skos:inScheme <http://vocab.nerc.ac.uk/scheme/SDNDEV/current> ;
  skos:notation "SDN:L22::TOOL0818" ;
  skos:note "accepted"@en ;
  skos:prefLabel "Point quadrat"@en ;
  skos:related <http://vocab.nerc.ac.uk/collection/B75/current/ORG00001> ;
.
inst:TOOL0819
  rdf:type skos:Concept ;
  dcterm:date "2015-01-09 14:18:23.0" ;
  dcterm:identifier "SDN:L22::TOOL0819" ;
  pav:hasCurrentVersion <http://vocab.nerc.ac.uk/collection/L22/current/TOOL0819/1> ;
  owl:versionInfo "1" ;
  skos:altLabel "Gridded quadrat"@en ;
  skos:broader <http://vocab.nerc.ac.uk/collection/L05/current/59> ;
  skos:definition "A square or rectangular rigid frame of known area, often home-made, with the total area divided into sub-areas by a graticule made up of threads or wires connecting opposite sides of the quadrat spaced at equal intervals. It is placed on the substrate to mark a fixed area for sampling flora or fauna. The subdivision by the graticule increases the accuracy of coverage estimates."@en ;
  skos:inScheme <http://vocab.nerc.ac.uk/scheme/SDNDEV/current> ;
  skos:notation "SDN:L22::TOOL0819" ;
  skos:note "accepted"@en ;
  skos:prefLabel "Gridded quadrat"@en ;
  skos:related <http://vocab.nerc.ac.uk/collection/B75/current/ORG00001> ;
.
inst:TOOL0828
  rdf:type skos:Concept ;
  dcterm:date "2015-01-29 11:24:26.0" ;
  dcterm:identifier "SDN:L22::TOOL0828" ;
  pav:hasCurrentVersion <http://vocab.nerc.ac.uk/collection/L22/current/TOOL0828/1> ;
  owl:versionInfo "1" ;
  skos:altLabel "MPI PCTD water sampler"@en ;
  skos:broader <http://vocab.nerc.ac.uk/collection/L05/current/30> ;
  skos:definition "Free falling system developed by MPI which allows for high resolution sampling of gradients in the water column, as well as sampling large amounts of water without contact with the atmosphere. When the system in at the water surface, the pump is initiated and after at least 10 minutes, water sampling begins. The water sampling has a delay of a few minutes, depending on tube length. Samples can be taken every 1 to 2 seconds."@en ;
  skos:inScheme <http://vocab.nerc.ac.uk/scheme/SDNDEV/current> ;
  skos:notation "SDN:L22::TOOL0828" ;
  skos:note "accepted"@en ;
  skos:prefLabel "Max Planck Institute Pump CTD water sampler"@en ;
  skos:related <http://vocab.nerc.ac.uk/collection/B75/current/ORG00159> ;
.
inst:TOOL0843
  rdf:type skos:Concept ;
  dcterm:date "2015-04-20 15:44:53.0" ;
  dcterm:identifier "SDN:L22::TOOL0843" ;
  pav:hasCurrentVersion <http://vocab.nerc.ac.uk/collection/L22/current/TOOL0843/1> ;
  owl:versionInfo "1" ;
  skos:altLabel "HiVol3000 air sampler"@en ;
  skos:broader <http://vocab.nerc.ac.uk/collection/L05/current/58> ;
  skos:definition "High volume particulate matter air sampler that can perform remote unattended sampling of PM10, PM2.5 or TSP alongside basic meteorological parameters. The air-borne suspended particles are drawn through an inlet hood and collected on a pre-weighed filter over a pre-determined period. After sampling, the filter is removed and re-weighed to determine the concentration of particulate matter. Two other models measure organic compounds using different filter types (PUF- poly-urethane foam and XAD- hydrophobic polyaromatic resin)."@en ;
  skos:inScheme <http://vocab.nerc.ac.uk/scheme/SDNDEV/current> ;
  skos:notation "SDN:L22::TOOL0843" ;
  skos:note "accepted"@en ;
  skos:prefLabel "Ecotech HiVol3000 air sampler"@en ;
  skos:related <http://vocab.nerc.ac.uk/collection/B75/current/ORG00952> ;
.
inst:TOOL0917
  rdf:type skos:Concept ;
  dcterm:date "2015-07-23 11:23:25.0" ;
  dcterm:identifier "SDN:L22::TOOL0917" ;
  pav:hasCurrentVersion <http://vocab.nerc.ac.uk/collection/L22/current/TOOL0917/1> ;
  owl:versionInfo "1" ;
  skos:altLabel "Peterson IRS Trap"@en ;
  skos:broader <http://vocab.nerc.ac.uk/collection/L05/current/33> ;
  skos:definition "This is a sediment trap designed to eliminate sediment flux sample contamination by free-swimming organisms using an indented rotating sphere (IRS) valve within the trap. The trap has three components: a particle accumulator, the IRS valve and a sample accumulator. The particle collector is either cylindrical with a diameter of 15-17cm or conical with a 70cm mouth. The IRS valve comprises an acrylic outer cylinder, a slightly smaller diameter PVC sphere with small indentations over part of its surface and a sealing collar. The sphere is periodically (an hour to a day depending sedimentation rates) slowly (1 rpm) rotated on an axis perpendicular to the vertical axis of the cylinder transferring material accumulated in its surface indentations to the sample accumulator. The sample accumulator is either a central funnel feeding a single cup or a skewed funnel feeding multiple cups on a carousel. The trap is deployed closed with a buoyant lid held in place by a burn wire to prevent contamination."@en ;
  skos:inScheme <http://vocab.nerc.ac.uk/scheme/SDNDEV/current> ;
  skos:notation "SDN:L22::TOOL0917" ;
  skos:note "accepted"@en ;
  skos:prefLabel "Peterson Indented Rotating Sphere Sediment Trap"@en ;
.
inst:TOOL0939
  rdf:type skos:Concept ;
  dcterm:date "2015-09-01 07:50:17.0" ;
  dcterm:identifier "SDN:L22::TOOL0939" ;
  pav:hasCurrentVersion <http://vocab.nerc.ac.uk/collection/L22/current/TOOL0939/1> ;
  owl:versionInfo "1" ;
  skos:altLabel "McLane RAS-500 sampler"@en ;
  skos:broader <http://vocab.nerc.ac.uk/collection/L05/current/30> ;
  skos:definition "A deep water or coastal time series water sampler that collects samples for biological, dissolved major and minor nutrient, dissolved trace metal, or dissolved organic carbon analyses. It collects 48 500ml samples of ambient water and suspended material in Tedlar bags, isolating the samples for subsequent laboratory analysis following a user defined sampling schedule. RAS systems can optionally be fitted with in-line pre-filters and an external temperature sensor. Deployment data with a report of sample event conditions is stored to non-volatile EEPROM. Further information is available at http://www.mclanelabs.com/master_page/product-type/samplers/remote-access-sampler."@en ;
  skos:inScheme <http://vocab.nerc.ac.uk/scheme/SDNDEV/current> ;
  skos:notation "SDN:L22::TOOL0939" ;
  skos:note "accepted"@en ;
  skos:prefLabel "McLane RAS-500 remote-access sampler"@en ;
  skos:related <http://vocab.nerc.ac.uk/collection/B75/current/ORG00996> ;
.
inst:TOOL0940
  rdf:type skos:Concept ;
  dcterm:date "2015-09-01 07:51:29.0" ;
  dcterm:identifier "SDN:L22::TOOL0940" ;
  pav:hasCurrentVersion <http://vocab.nerc.ac.uk/collection/L22/current/TOOL0940/1> ;
  owl:versionInfo "1" ;
  skos:altLabel "McLane RAS-100 sampler"@en ;
  skos:broader <http://vocab.nerc.ac.uk/collection/L05/current/30> ;
  skos:definition "A deep water or coastal time series water sampler that collects samples for biological, dissolved major and minor nutrient, dissolved trace metal, or dissolved organic carbon analyses. It collects 48 100ml samples of ambient water and suspended material in Tedlar bags, isolating the samples for subsequent laboratory analysis following a user defined sampling schedule. RAS systems can optionally be fitted with in-line pre-filters and an external temperature sensor. Deployment data with a report of sample event conditions is stored to non-volatile EEPROM. Further information is available at http://www.mclanelabs.com/master_page/product-type/samplers/remote-access-sampler."@en ;
  skos:inScheme <http://vocab.nerc.ac.uk/scheme/SDNDEV/current> ;
  skos:notation "SDN:L22::TOOL0940" ;
  skos:note "accepted"@en ;
  skos:prefLabel "McLane RAS-100 remote-access sampler"@en ;
  skos:related <http://vocab.nerc.ac.uk/collection/B75/current/ORG00996> ;
.
inst:TOOL0960
  rdf:type skos:Concept ;
  dcterm:date "2015-12-16 16:57:05.0" ;
  dcterm:identifier "SDN:L22::TOOL0960" ;
  pav:hasCurrentVersion <http://vocab.nerc.ac.uk/collection/L22/current/TOOL0960/1> ;
  owl:versionInfo "1" ;
  skos:altLabel "Hamon grab"@en ;
  skos:broader <http://vocab.nerc.ac.uk/collection/L05/current/50> ;
  skos:definition "The Hamon grab is used for obtaining samples in coarse sediment, as well as for sampling benthic infauna. It has a typical sampling area of 0.25 m2 (0.2 m2 - 0.29 m2) and a penetration depth up to 30 cm. This grab consists of a rectangular (but sometimes triangular) frame forming a stable support for a sampling bucket attached to a pivoted arm. On reaching the seabed, tension in the wire is released which causes the sampling bucket to pivot through 90 degrees pushing seabed sediment into the bucket. The bucket locates onto an inclined rubber-covered steel plate, sealing it completely. Weights are attached to the grab to minimize the lateral movement of the supporting frame during sample collection."@en ;
  skos:inScheme <http://vocab.nerc.ac.uk/scheme/SDNDEV/current> ;
  skos:notation "SDN:L22::TOOL0960" ;
  skos:note "accepted"@en ;
  skos:prefLabel "Hamon grab"@en ;
.
inst:TOOL0961
  rdf:type skos:Concept ;
  dcterm:date "2015-12-16 16:57:05.0" ;
  dcterm:identifier "SDN:L22::TOOL0961" ;
  pav:hasCurrentVersion <http://vocab.nerc.ac.uk/collection/L22/current/TOOL0961/1> ;
  owl:versionInfo "1" ;
  skos:altLabel "Mini-Hamon grab"@en ;
  skos:broader <http://vocab.nerc.ac.uk/collection/L05/current/50> ;
  skos:definition "The Mini-Hamon Grab was introduced by CEFAS and is used for obtaining samples in coarse sediment, as well as for sampling benthic infauna. The standard Hamon Grab comprises of a stainless steel box shaped sampling scoop mounted in a rectangular (but sometimes triangular) frame. It is a mini version of the standard Hamon Grab, with a typical sampling area of 0.1 m2 and a penetration depth up to 20 cm. It often has a longer than standard tooth bar fitted compared with the standard Hamon Grab."@en ;
  skos:inScheme <http://vocab.nerc.ac.uk/scheme/SDNDEV/current> ;
  skos:notation "SDN:L22::TOOL0961" ;
  skos:note "accepted"@en ;
  skos:prefLabel "Mini-Hamon grab"@en ;
  skos:related <http://vocab.nerc.ac.uk/collection/B75/current/ORG00008> ;
.
inst:TOOL0962
  rdf:type skos:Concept ;
  dcterm:date "2015-12-16 16:57:05.0" ;
  dcterm:identifier "SDN:L22::TOOL0962" ;
  pav:hasCurrentVersion <http://vocab.nerc.ac.uk/collection/L22/current/TOOL0962/1> ;
  owl:versionInfo "1" ;
  skos:altLabel "Smith-McIntyre grab"@en ;
  skos:broader <http://vocab.nerc.ac.uk/collection/L05/current/50> ;
  skos:definition "This grab was designed to operate under difficult conditions in the open sea. It has a typical sampling area of 0.1 m2 and a penetration depth up to 30 cm. This grab is mounted on a stainless steel frame suspended from a pair of lowering cables (bridles) attached to the bucket arms. Springs activated by a trigger mechanism, released when the foot plates come into contact with the ocean floor, force the bucket jaws into the sediment in order to collect the sample. Safety features have been fitted to the grab to prevent the tripping mechanism from being triggered prematurely."@en ;
  skos:inScheme <http://vocab.nerc.ac.uk/scheme/SDNDEV/current> ;
  skos:notation "SDN:L22::TOOL0962" ;
  skos:note "accepted"@en ;
  skos:prefLabel "Smith-McIntyre grab"@en ;
.
inst:TOOL0963
  rdf:type skos:Concept ;
  dcterm:date "2015-12-16 16:57:05.0" ;
  dcterm:identifier "SDN:L22::TOOL0963" ;
  pav:hasCurrentVersion <http://vocab.nerc.ac.uk/collection/L22/current/TOOL0963/1> ;
  owl:versionInfo "1" ;
  skos:altLabel "Day grab"@en ;
  skos:broader <http://vocab.nerc.ac.uk/collection/L05/current/50> ;
  skos:definition "The Day grab is regarded as a valuable alternative to the Smith-McIntyre grab. It has a typical sampling area of 0.1 m2 and a typical penetration depth of up to 15 cm. It has a frame to keep the grab level on the sea bed, and two trigger plates for actuating the release, but no springs to force the hinged buckets into the bottom. Penetration of the sediment is assisted by the weight of the grab, of sometimes with addition lead weights."@en ;
  skos:inScheme <http://vocab.nerc.ac.uk/scheme/SDNDEV/current> ;
  skos:notation "SDN:L22::TOOL0963" ;
  skos:note "accepted"@en ;
  skos:prefLabel "Day grab"@en ;
.
inst:TOOL0978
  rdf:type skos:Concept ;
  dcterm:date "2016-04-04 14:47:13.0" ;
  dcterm:identifier "SDN:L22::TOOL0978" ;
  pav:hasCurrentVersion <http://vocab.nerc.ac.uk/collection/L22/current/TOOL0978/1> ;
  owl:versionInfo "1" ;
  skos:altLabel "Apstein"@en ;
  skos:broader <http://vocab.nerc.ac.uk/collection/L05/current/22> ;
  skos:definition "Plankton net described as Apstein-style ring net based on Apstein (1896); a small ring net designed with single circular mouth piece with optional reducing cone; with conical filtering net shape; and equipped with optional closing mechanism."@en ;
  skos:inScheme <http://vocab.nerc.ac.uk/scheme/SDNDEV/current> ;
  skos:notation "SDN:L22::TOOL0978" ;
  skos:note "accepted"@en ;
  skos:prefLabel "Apstein-style ring net"@en ;
.
inst:TOOL0979
  rdf:type skos:Concept ;
  dcterm:date "2016-04-04 14:47:13.0" ;
  dcterm:identifier "SDN:L22::TOOL0979" ;
  pav:hasCurrentVersion <http://vocab.nerc.ac.uk/collection/L22/current/TOOL0979/1> ;
  owl:versionInfo "1" ;
  skos:altLabel "WP2"@en ;
  skos:broader <http://vocab.nerc.ac.uk/collection/L05/current/22> ;
  skos:definition "Plankton net described as WP-2 net adapted from UNESCO Working Party 2 (1968); designed with single circular (ring or hoop) mouth piece with measurements: diameter (metre)=0.57; with opening area (square metre)=0.25; with total filtering net length (metre)=not specified; with filtering net shape cylindrical-conical; with additional features: filtration ratio (ratio of mesh aperture to mouth area) of at least 6:1; with mesh size (millimetre)=0.2 as a standard but may vary; and equipped with optional closing mechanism."@en ;
  skos:inScheme <http://vocab.nerc.ac.uk/scheme/SDNDEV/current> ;
  skos:notation "SDN:L22::TOOL0979" ;
  skos:note "accepted"@en ;
  skos:prefLabel "WP-2 net"@en ;
.
inst:TOOL0980
  rdf:type skos:Concept ;
  dcterm:date "2016-04-04 14:47:13.0" ;
  dcterm:identifier "SDN:L22::TOOL0980" ;
  pav:hasCurrentVersion <http://vocab.nerc.ac.uk/collection/L22/current/TOOL0980/1> ;
  owl:versionInfo "1" ;
  skos:altLabel "WP2-style"@en ;
  skos:broader <http://vocab.nerc.ac.uk/collection/L05/current/22> ;
  skos:definition "Plankton net described as WP-2-style net; designed with single circular mouth piece; with filtering net shape cylindrical-conical; with further specifications either unknown or described elsewhere in the supporting metadata."@en ;
  skos:inScheme <http://vocab.nerc.ac.uk/scheme/SDNDEV/current> ;
  skos:notation "SDN:L22::TOOL0980" ;
  skos:note "accepted"@en ;
  skos:prefLabel "WP-2-style net"@en ;
.
inst:TOOL0981
  rdf:type skos:Concept ;
  dcterm:date "2016-04-04 14:47:13.0" ;
  dcterm:identifier "SDN:L22::TOOL0981" ;
  pav:hasCurrentVersion <http://vocab.nerc.ac.uk/collection/L22/current/TOOL0981/1> ;
  owl:versionInfo "1" ;
  skos:altLabel "Hand net"@en ;
  skos:broader <http://vocab.nerc.ac.uk/collection/L05/current/22> ;
  skos:definition "Plankton net described as an hand-held plankton net; designed with single mouth piece with specifications with specifications unknown or available elsewhere in the supporting metadata; with additional features: qualitative sampling gear operated like a butterfly net either by SCUBA divers or from the side of a fixed dock or a small vessel; net size, shape, colour and mesh size may vary."@en ;
  skos:inScheme <http://vocab.nerc.ac.uk/scheme/SDNDEV/current> ;
  skos:notation "SDN:L22::TOOL0981" ;
  skos:note "accepted"@en ;
  skos:prefLabel "Hand-held plankton net"@en ;
.
inst:TOOL0982
  rdf:type skos:Concept ;
  dcterm:date "2016-04-04 14:47:13.0" ;
  dcterm:identifier "SDN:L22::TOOL0982" ;
  pav:hasCurrentVersion <http://vocab.nerc.ac.uk/collection/L22/current/TOOL0982/1> ;
  owl:versionInfo "1" ;
  skos:altLabel "WP2 Bongo"@en ;
  skos:broader <http://vocab.nerc.ac.uk/collection/L05/current/22> ;
  skos:definition "Plankton net described as PML twin WP-2 Bongo net; designed with double circular (ring or hoop) mouth piece with measurements: diameter (metre)=0.60; with opening area (square metre)=0.26; with total filtering net length (metre)=not specified; with filtering net shape cylindrical-conical; with additional features: not specified; with mesh size (millimetre)=0.2; and equipped with NO closing mechanism."@en ;
  skos:inScheme <http://vocab.nerc.ac.uk/scheme/SDNDEV/current> ;
  skos:notation "SDN:L22::TOOL0982" ;
  skos:note "accepted"@en ;
  skos:prefLabel "Plymouth Marine Laboratory twin WP-2 Bongo net"@en ;
  skos:related <http://vocab.nerc.ac.uk/collection/B75/current/ORG00733> ;
.
inst:TOOL0983
  rdf:type skos:Concept ;
  dcterm:date "2016-04-04 14:47:13.0" ;
  dcterm:identifier "SDN:L22::TOOL0983" ;
  pav:hasCurrentVersion <http://vocab.nerc.ac.uk/collection/L22/current/TOOL0983/1> ;
  owl:versionInfo "1" ;
  skos:altLabel "Bongo 63-um"@en ;
  skos:broader <http://vocab.nerc.ac.uk/collection/L05/current/22> ;
  skos:definition "Plankton net described as 63 micron Bongo net as used during e.g. the UK Marine Productivity (MarProd) programme for work on Oithona copepods; designed with double circular (ring) mouth piece with measurements: diameter (metre)=0.36; with opening area (square metre)=0.102; with total filtering net length (metre)=2; with filtering net shape conical; with additional features: cod-end diameter=0.085 m; with mesh size (millimetre)=0.063; and equipped with NO closing mechanism."@en ;
  skos:inScheme <http://vocab.nerc.ac.uk/scheme/SDNDEV/current> ;
  skos:notation "SDN:L22::TOOL0983" ;
  skos:note "accepted"@en ;
  skos:prefLabel "Plymouth Marine Laboratory 63-um Bongo net"@en ;
  skos:related <http://vocab.nerc.ac.uk/collection/B75/current/ORG00733> ;
.
inst:TOOL0984
  rdf:type skos:Concept ;
  dcterm:date "2016-04-04 14:47:13.0" ;
  dcterm:identifier "SDN:L22::TOOL0984" ;
  pav:hasCurrentVersion <http://vocab.nerc.ac.uk/collection/L22/current/TOOL0984/1> ;
  owl:versionInfo "1" ;
  skos:altLabel "Bongo 95+200-um"@en ;
  skos:broader <http://vocab.nerc.ac.uk/collection/L05/current/22> ;
  skos:definition "Plankton net described as University of Aberdeen 95+200 micron size-resolving Bongo net; designed with double circular (drum) mouth piece with measurements: diameter (metre)=0.30; with opening area (square metre)=0.071; with total filtering net length (metre)=2; with filtering net shape cylindrical-conical; with additional features: net collar length=0.25 m, cylinder section length=1 m, conical section length=1 m, cod-end diameter=0.080 m; with mesh size (millimetre)=0.095 and 0.200; and equipped with NO closing mechanism."@en ;
  skos:inScheme <http://vocab.nerc.ac.uk/scheme/SDNDEV/current> ;
  skos:notation "SDN:L22::TOOL0984" ;
  skos:note "accepted"@en ;
  skos:prefLabel "University of Aberdeen size-resolving Bongo net"@en ;
  skos:related <http://vocab.nerc.ac.uk/collection/B75/current/ORG00733> ;
.
inst:TOOL0985
  rdf:type skos:Concept ;
  dcterm:date "2016-04-04 14:47:13.0" ;
  dcterm:identifier "SDN:L22::TOOL0985" ;
  pav:hasCurrentVersion <http://vocab.nerc.ac.uk/collection/L22/current/TOOL0985/1> ;
  owl:versionInfo "1" ;
  skos:altLabel "DMIKT"@en ;
  skos:broader <http://vocab.nerc.ac.uk/collection/L05/current/23> ;
  skos:broader <http://vocab.nerc.ac.uk/collection/L05/current/68> ;
  skos:definition "Pelagic trawl net described as Dual Methot Trawl net ; designed with single rectangular mouth piece with measurements: not specified; with opening area (square metre)=1.5; with total filtering net length (metre)=not specified; with filtering net shape conical; with additional features: dual-net system; with mesh size (millimetre)=1.5; and equipped with an opening-closing mechanism."@en ;
  skos:inScheme <http://vocab.nerc.ac.uk/scheme/SDNDEV/current> ;
  skos:notation "SDN:L22::TOOL0985" ;
  skos:note "accepted"@en ;
  skos:prefLabel "Dual Methot Isaacs-Kidd Trawl net"@en ;
  skos:related <http://vocab.nerc.ac.uk/collection/B75/current/ORG00013> ;
.
inst:TOOL0986
  rdf:type skos:Concept ;
  dcterm:date "2016-04-04 14:47:13.0" ;
  dcterm:identifier "SDN:L22::TOOL0986" ;
  pav:hasCurrentVersion <http://vocab.nerc.ac.uk/collection/L22/current/TOOL0986/1> ;
  owl:versionInfo "1" ;
  skos:altLabel "ARIES pup-net"@en ;
  skos:broader <http://vocab.nerc.ac.uk/collection/L05/current/22> ;
  skos:definition "Plankton net described as one of typically two simple conical ring nets attached by bungee to either side of the ARIES net sampler frame to collect integrated samples; designed with single circular mouth piece with measurements: diameter (metre)=0.14; with opening area (square metre)=0.015; with total filtering net length (metre)=1.47; with filtering net shape conical; with mesh size (millimetre)=not specified; and equipped with NO closing mechanism."@en ;
  skos:inScheme <http://vocab.nerc.ac.uk/scheme/SDNDEV/current> ;
  skos:notation "SDN:L22::TOOL0986" ;
  skos:note "accepted"@en ;
  skos:prefLabel "ARIES pup net"@en ;
  skos:related <http://vocab.nerc.ac.uk/collection/B75/current/ORG00013> ;
.
inst:TOOL0987
  rdf:type skos:Concept ;
  dcterm:date "2016-04-04 14:47:13.0" ;
  dcterm:identifier "SDN:L22::TOOL0987" ;
  pav:hasCurrentVersion <http://vocab.nerc.ac.uk/collection/L22/current/TOOL0987/1> ;
  owl:versionInfo "1" ;
  skos:altLabel "OCEAN pup-net"@en ;
  skos:broader <http://vocab.nerc.ac.uk/collection/L05/current/22> ;
  skos:definition "Plankton net described as one of typically two simple conical ring nets attached by bungee to either side of the OCEAN sampler frame to collect integrated samples; designed with single circular mouth piece with measurements: diameter (metre)=0.14; with opening area (square metre)=0.015; with total filtering net length (metre)=1.47; with filtering net shape conical; with mesh size (millimetre)=not specified; and equipped with NO closing mechanism."@en ;
  skos:inScheme <http://vocab.nerc.ac.uk/scheme/SDNDEV/current> ;
  skos:notation "SDN:L22::TOOL0987" ;
  skos:note "accepted"@en ;
  skos:prefLabel "OCEAN sampler pup net"@en ;
  skos:related <http://vocab.nerc.ac.uk/collection/B75/current/ORG00013> ;
.
inst:TOOL0988
  rdf:type skos:Concept ;
  dcterm:date "2016-04-04 14:47:13.0" ;
  dcterm:identifier "SDN:L22::TOOL0988" ;
  pav:hasCurrentVersion <http://vocab.nerc.ac.uk/collection/L22/current/TOOL0988/1> ;
  owl:versionInfo "1" ;
  skos:altLabel "Metre net"@en ;
  skos:broader <http://vocab.nerc.ac.uk/collection/L05/current/22> ;
  skos:definition "Plankton net described as 1-metre ring net; designed with single circular (ring) mouth piece with measurements: mouth diameter (metre)=1; with opening area (square metre)=0.8; with total filtering net length (metre)=not specified; with filtering net shape conical; with additional features: can be used for qualitative sampling or the capture of live animals or quantitative sampling if used with flowmeter; with mesh size (millimetre)=0.333 as a standard but may vary; and equipped with NO closing mechanism."@en ;
  skos:inScheme <http://vocab.nerc.ac.uk/scheme/SDNDEV/current> ;
  skos:notation "SDN:L22::TOOL0988" ;
  skos:note "accepted"@en ;
  skos:prefLabel "1-metre ring net"@en ;
.
inst:TOOL0989
  rdf:type skos:Concept ;
  dcterm:date "2016-04-04 14:47:13.0" ;
  dcterm:identifier "SDN:L22::TOOL0989" ;
  pav:hasCurrentVersion <http://vocab.nerc.ac.uk/collection/L22/current/TOOL0989/1> ;
  owl:versionInfo "1" ;
  skos:altLabel "0.5-m net"@en ;
  skos:broader <http://vocab.nerc.ac.uk/collection/L05/current/22> ;
  skos:definition "Plankton net described as 0.5-m ring net; designed with single circular (ring) mouth piece with measurements: mouth diameter (metre)=0.5; with opening area (square metre)=0.2; with total filtering net length (metre)=not specified; with filtering net shape conical; with additional features: can be used for qualitative sampling or the capture of live animals or quantitative sampling if used with flowmeter; with mesh size (millimetre)=0.2 to 0.5 but may vary; and equipped with NO closing mechanism."@en ;
  skos:inScheme <http://vocab.nerc.ac.uk/scheme/SDNDEV/current> ;
  skos:notation "SDN:L22::TOOL0989" ;
  skos:note "accepted"@en ;
  skos:prefLabel "Half-metre ring net"@en ;
.
inst:TOOL0990
  rdf:type skos:Concept ;
  dcterm:date "2016-04-04 14:47:13.0" ;
  dcterm:identifier "SDN:L22::TOOL0990" ;
  pav:hasCurrentVersion <http://vocab.nerc.ac.uk/collection/L22/current/TOOL0990/1> ;
  owl:versionInfo "1" ;
  skos:altLabel "N113"@en ;
  skos:broader <http://vocab.nerc.ac.uk/collection/L05/current/22> ;
  skos:definition "Plankton net described as N113 (modified Indian Ocean standard net) - Foxton (1969); designed with single cylindrical mouth piece with measurements: mouth diameter (metre)=1.13, cylindrical non-filtering mouth section length (m)=1, upper cylindrical filtering section length (m)= 1, lower conical filtering section length (m)=3; with opening area (square metre)=1; with total filtering net length (metre)=4; with filtering net shape cylindrical-conical; with additional features: not specified; with mesh size (millimetre)=0.33; and equipped with a catch dividing bucket."@en ;
  skos:inScheme <http://vocab.nerc.ac.uk/scheme/SDNDEV/current> ;
  skos:notation "SDN:L22::TOOL0990" ;
  skos:note "accepted"@en ;
  skos:prefLabel "N113 (modified Indian Ocean standard net) - Foxton (1969)"@en ;
  skos:related <http://vocab.nerc.ac.uk/collection/B75/current/ORG00009> ;
.
inst:TOOL0991
  rdf:type skos:Concept ;
  dcterm:date "2016-04-04 14:47:13.0" ;
  dcterm:identifier "SDN:L22::TOOL0991" ;
  pav:hasCurrentVersion <http://vocab.nerc.ac.uk/collection/L22/current/TOOL0991/1> ;
  owl:versionInfo "1" ;
  skos:altLabel "Agassiz 3.5m"@en ;
  skos:broader <http://vocab.nerc.ac.uk/collection/L05/current/61> ;
  skos:definition "Demersal trawl net described as 3.5m Agassiz trawl sampler; designed with single rectangular mouth piece with measurements: mouth opening width (metre)=3.5, mouth opening height (metre)=1; with opening area (square metre)=3.5; with total filtering net length (metre)=not specified; with filtering net shape conical; with additional features: not specified; with mesh size (millimetre)=10; and equipped with closing mouth mechanism."@en ;
  skos:inScheme <http://vocab.nerc.ac.uk/scheme/SDNDEV/current> ;
  skos:notation "SDN:L22::TOOL0991" ;
  skos:note "accepted"@en ;
  skos:prefLabel "Agassiz 3.5m trawl sampler"@en ;
  skos:related <http://vocab.nerc.ac.uk/collection/B75/current/ORG00239> ;
.
inst:TOOL0992
  rdf:type skos:Concept ;
  dcterm:date "2016-04-04 14:47:13.0" ;
  dcterm:identifier "SDN:L22::TOOL0992" ;
  pav:hasCurrentVersion <http://vocab.nerc.ac.uk/collection/L22/current/TOOL0992/1> ;
  owl:versionInfo "1" ;
  skos:altLabel "F-Net"@en ;
  skos:broader <http://vocab.nerc.ac.uk/collection/L05/current/22> ;
  skos:definition "The foredeck (also fore-deck) net was designed by Doug Bone (Gear Development, British Antarctic Survey) in 1980. It has a square net mouth of 1 square metre area and is fitted with a 5 millimetre mesh tapering over 3 metre to a solid conical cod end. The foredeck net is towed from the hydrolic crane at a depth near to the sea surface."@en ;
  skos:inScheme <http://vocab.nerc.ac.uk/scheme/SDNDEV/current> ;
  skos:notation "SDN:L22::TOOL0992" ;
  skos:note "accepted"@en ;
  skos:prefLabel "British Antarctic Survey Foredeck Net"@en ;
  skos:related <http://vocab.nerc.ac.uk/collection/B75/current/ORG0015> ;
.
inst:TOOL0993
  rdf:type skos:Concept ;
  dcterm:date "2016-04-04 14:47:13.0" ;
  dcterm:identifier "SDN:L22::TOOL0993" ;
  pav:hasCurrentVersion <http://vocab.nerc.ac.uk/collection/L22/current/TOOL0993/1> ;
  owl:versionInfo "1" ;
  skos:altLabel "BAS motion-compensated Bongo"@en ;
  skos:broader <http://vocab.nerc.ac.uk/collection/L05/current/22> ;
  skos:definition "A British Antarctic Survey-built motion compensated Bongo net. It has two nets with different mesh sizes (100 um and 200 um) deployed at the same time to collect plankton samples. No open or closing is required. The motion compensation unit has a spring mechanism to maintain the net at a steady speed by increasing or decreasing the length of the wire depending on the ships movements and catches plankton in much better conditions."@en ;
  skos:inScheme <http://vocab.nerc.ac.uk/scheme/SDNDEV/current> ;
  skos:notation "SDN:L22::TOOL0993" ;
  skos:note "accepted"@en ;
  skos:prefLabel "British Antarctic Survey Motion Compensated Bongo Net"@en ;
  skos:related <http://vocab.nerc.ac.uk/collection/B75/current/ORG0015> ;
.
inst:TOOL0994
  rdf:type skos:Concept ;
  dcterm:date "2016-04-04 14:47:13.0" ;
  dcterm:identifier "SDN:L22::TOOL0994" ;
  pav:hasCurrentVersion <http://vocab.nerc.ac.uk/collection/L22/current/TOOL0994/1> ;
  owl:versionInfo "1" ;
  skos:altLabel "BAS mini-Bongo"@en ;
  skos:broader <http://vocab.nerc.ac.uk/collection/L05/current/22> ;
  skos:definition "A British Antarctic Survey-built small and light version of a Bongo net, the Mini-Bongo can be deployed from smaller boats with small winches. It is mainly used to catch small Zooplankton in good condition in depth up to about 100m."@en ;
  skos:inScheme <http://vocab.nerc.ac.uk/scheme/SDNDEV/current> ;
  skos:notation "SDN:L22::TOOL0994" ;
  skos:note "accepted"@en ;
  skos:prefLabel "British Antarctic Survey Mini-Bongo net"@en ;
  skos:related <http://vocab.nerc.ac.uk/collection/B75/current/ORG0015> ;
.
inst:TOOL0995
  rdf:type skos:Concept ;
  dcterm:date "2022-05-13 08:17:25.0" ;
  dcterm:identifier "SDN:L22::TOOL0995" ;
  pav:hasCurrentVersion <http://vocab.nerc.ac.uk/collection/L22/current/TOOL0995/2> ;
  pav:hasVersion <http://vocab.nerc.ac.uk/collection/L22/current/TOOL0995/1> ;
  owl:versionInfo "2" ;
  skos:altLabel "BAS towed Bongo"@en ;
  skos:broader <http://vocab.nerc.ac.uk/collection/L05/current/22> ;
  skos:definition "A British Antarctic Survey-built bongo net used to collect plankton samples while being towed behind the ship; collects samples from targeted water depths or strata."@en ;
  skos:inScheme <http://vocab.nerc.ac.uk/scheme/SDNDEV/current> ;
  skos:notation "SDN:L22::TOOL0995" ;
  skos:note "accepted"@en ;
  skos:prefLabel "British Antarctic Survey Towed Bongo Net"@en ;
  skos:related <http://vocab.nerc.ac.uk/collection/B75/current/ORG0015> ;
.
inst:TOOL0996
  rdf:type skos:Concept ;
  dcterm:date "2016-04-04 14:47:13.0" ;
  dcterm:identifier "SDN:L22::TOOL0996" ;
  pav:hasCurrentVersion <http://vocab.nerc.ac.uk/collection/L22/current/TOOL0996/1> ;
  owl:versionInfo "1" ;
  skos:altLabel "BAS N70"@en ;
  skos:broader <http://vocab.nerc.ac.uk/collection/L05/current/22> ;
  skos:definition "A British Antarctic Survey-rebuilt version of the Nansen N70 net as described in Ward et al. 2012 used to collect zooplankton samples."@en ;
  skos:inScheme <http://vocab.nerc.ac.uk/scheme/SDNDEV/current> ;
  skos:notation "SDN:L22::TOOL0996" ;
  skos:note "accepted"@en ;
  skos:prefLabel "British Antarctic Survey N70 Plankton Net"@en ;
  skos:related <http://vocab.nerc.ac.uk/collection/B75/current/ORG0015> ;
.
inst:TOOL0997
  rdf:type skos:Concept ;
  dcterm:date "2016-04-05 10:34:08.0" ;
  dcterm:identifier "SDN:L22::TOOL0997" ;
  pav:hasCurrentVersion <http://vocab.nerc.ac.uk/collection/L22/current/TOOL0997/1> ;
  owl:versionInfo "1" ;
  skos:altLabel "MARMAP 20-cm Bongo"@en ;
  skos:broader <http://vocab.nerc.ac.uk/collection/L05/current/22> ;
  skos:definition "Plankton net described as 20-cm MARMAP Bongo Net [Posgay and Marak (1980)]; designed with double cylindrical (hoop) mouth piece with measurements: diameter (metre)=0.20, length (metre)=0.28; with opening area (square metre)=0.031; with total filtering net length (metre)=1.58; with filtering net shape cylindrical-conical; with additional features: cylinder section length=1.07 m, conical section length=0.51 m; with mesh size (millimetre)=0.1 to 0.5 but usually 0.333; and equipped with NO closing mechanism."@en ;
  skos:inScheme <http://vocab.nerc.ac.uk/scheme/SDNDEV/current> ;
  skos:notation "SDN:L22::TOOL0997" ;
  skos:note "accepted"@en ;
  skos:prefLabel "MARMAP 20-cm Bongo net"@en ;
.
inst:TOOL1012
  rdf:type skos:Concept ;
  dcterm:date "2016-07-19 12:17:11.0" ;
  dcterm:identifier "SDN:L22::TOOL1012" ;
  pav:hasCurrentVersion <http://vocab.nerc.ac.uk/collection/L22/current/TOOL1012/1> ;
  owl:versionInfo "1" ;
  skos:altLabel "PFA pipe air sampler"@en ;
  skos:broader <http://vocab.nerc.ac.uk/collection/L05/current/58> ;
  skos:definition "Perfluoroalkoxy tubbing leading directly from the least contaminated part of a ship to an analytical instrument. Air is drawn through the pipe by the instrument."@en ;
  skos:inScheme <http://vocab.nerc.ac.uk/scheme/SDNDEV/current> ;
  skos:notation "SDN:L22::TOOL1012" ;
  skos:note "accepted"@en ;
  skos:prefLabel "Perfluoroalkoxy pipe air sampler"@en ;
  skos:related <http://vocab.nerc.ac.uk/collection/B75/current/ORG00001> ;
.
inst:TOOL1135
  rdf:type skos:Concept ;
  dcterm:date "2017-06-14 16:49:46.0" ;
  dcterm:identifier "SDN:L22::TOOL1135" ;
  pav:hasCurrentVersion <http://vocab.nerc.ac.uk/collection/L22/current/TOOL1135/1> ;
  owl:versionInfo "1" ;
  skos:altLabel "KPZ GMBH pump"@en ;
  skos:broader <http://vocab.nerc.ac.uk/collection/L05/current/31> ;
  skos:definition "A submersible pump that can be used for multiple applications where large volumes of water are required."@en ;
  skos:inScheme <http://vocab.nerc.ac.uk/scheme/SDNDEV/current> ;
  skos:notation "SDN:L22::TOOL1135" ;
  skos:note "accepted"@en ;
  skos:prefLabel "Kompressoren-Pumpen-Zentrale GMBH pump"@en ;
  skos:related <http://vocab.nerc.ac.uk/collection/B75/current/ORG01052> ;
.
inst:TOOL1165
  rdf:type skos:Concept ;
  dcterm:date "2017-11-06 15:37:36.0" ;
  dcterm:identifier "SDN:L22::TOOL1165" ;
  pav:hasCurrentVersion <http://vocab.nerc.ac.uk/collection/L22/current/TOOL1165/1> ;
  owl:versionInfo "1" ;
  skos:altLabel "Marine Institute Slurp Sampler"@en ;
  skos:broader <http://vocab.nerc.ac.uk/collection/L05/current/24> ;
  skos:definition "The slurp sampler is a manipulator designed by the Marine Institute for use on Remotely Operated Vehicle (ROV) systems to sample live coral. The 75 mm slurp gun uses a vacuum suction mechanism to collect samples into a single chamber container."@en ;
  skos:inScheme <http://vocab.nerc.ac.uk/scheme/SDNDEV/current> ;
  skos:notation "SDN:L22::TOOL1165" ;
  skos:note "accepted"@en ;
  skos:prefLabel "Marine Institute Slurp Sampler"@en ;
  skos:related <http://vocab.nerc.ac.uk/collection/B75/current/ORG00164> ;
.
inst:TOOL1166
  rdf:type skos:Concept ;
  dcterm:date "2017-11-06 15:37:36.0" ;
  dcterm:identifier "SDN:L22::TOOL1166" ;
  pav:hasCurrentVersion <http://vocab.nerc.ac.uk/collection/L22/current/TOOL1166/1> ;
  owl:versionInfo "1" ;
  skos:altLabel "ORION 7P and 7R Manipulators"@en ;
  skos:broader <http://vocab.nerc.ac.uk/collection/L05/current/24> ;
  skos:definition "The ORION 7 manipulators are seven-function manipulator systems designed for use on light and medium class Remotely Operated Vehicles (ROVs). The manipulators have a standard depth rating of 6545 dbar, allowing  the manipulators to be used on a wide range of ROVs, and can be configured to be either position-controlled or rate-controlled. The ORION 7 models can also be configured for extended reach, which adds 318 mm to the arm's length. The ORION manipulators were produced by FMC Technologies who have since merged with Technip to form TechnipFMC."@en ;
  skos:inScheme <http://vocab.nerc.ac.uk/scheme/SDNDEV/current> ;
  skos:notation "SDN:L22::TOOL1166" ;
  skos:note "accepted"@en ;
  skos:prefLabel "FMC Technologies Schilling Robotics ORION 7P and 7R Manipulators"@en ;
  skos:related <http://vocab.nerc.ac.uk/collection/B75/current/ORG01093> ;
.
inst:TOOL1169
  rdf:type skos:Concept ;
  dcterm:date "2017-11-23 13:03:21.0" ;
  dcterm:identifier "SDN:L22::TOOL1169" ;
  pav:hasCurrentVersion <http://vocab.nerc.ac.uk/collection/L22/current/TOOL1169/1> ;
  owl:versionInfo "1" ;
  skos:altLabel "BAS LG pist"@en ;
  skos:broader <http://vocab.nerc.ac.uk/collection/L05/current/51> ;
  skos:definition "Long Piston Corer (LPC) developed by BAS in collaboration with Marine Project Developments of Hull, originally trialled in 1992. Piston corers use heavy tubes which are plunged into the seafloor to extract samples of mud sediment. A piston inside the tube allows scientists to capture the longest possible samples. The corer can collect undisturbed marine sediment cores with barrel lengths of up to 30m."@en ;
  skos:inScheme <http://vocab.nerc.ac.uk/scheme/SDNDEV/current> ;
  skos:notation "SDN:L22::TOOL1169" ;
  skos:note "accepted"@en ;
  skos:prefLabel "British Antarctic Survey (long) piston corer"@en ;
  skos:related <http://vocab.nerc.ac.uk/collection/B75/current/ORG0015> ;
.
inst:TOOL1170
  rdf:type skos:Concept ;
  dcterm:date "2017-11-23 13:03:21.0" ;
  dcterm:identifier "SDN:L22::TOOL1170" ;
  pav:hasCurrentVersion <http://vocab.nerc.ac.uk/collection/L22/current/TOOL1170/1> ;
  owl:versionInfo "1" ;
  skos:altLabel "BAS Wax"@en ;
  skos:broader <http://vocab.nerc.ac.uk/collection/L05/current/53> ;
  skos:definition "BAS built rock chipper (also known as a wax corer) collects samples of volcanic rock. The head of the chipper is wax filled so that when the corer is lowered and free falls to the seabed, it splinters the rock and collects samples of rocks in the wax."@en ;
  skos:inScheme <http://vocab.nerc.ac.uk/scheme/SDNDEV/current> ;
  skos:notation "SDN:L22::TOOL1170" ;
  skos:note "accepted"@en ;
  skos:prefLabel "British Antarctic Survey rock chipper"@en ;
  skos:related <http://vocab.nerc.ac.uk/collection/B75/current/ORG0015> ;
.
inst:TOOL1171
  rdf:type skos:Concept ;
  dcterm:date "2017-11-23 13:03:21.0" ;
  dcterm:identifier "SDN:L22::TOOL1171" ;
  pav:hasCurrentVersion <http://vocab.nerc.ac.uk/collection/L22/current/TOOL1171/1> ;
  owl:versionInfo "1" ;
  skos:altLabel "BGS VC1 6m"@en ;
  skos:broader <http://vocab.nerc.ac.uk/collection/L05/current/51> ;
  skos:definition "British Geological Survey (BGS) VC1 Vibrocorer is an upgraded 6m system. It is used for collecting soft and unconsolidated sediment. Sediments are collected in a plastic liner tube within a core barrel driven by a one-tonne weight and vibrator motor (hence the name vibrocorer) mounted at the top of the rig. Guillotine closure below the core barrel during recovery of the equipment aids in core retention during operations. It is capable of collecting sediment in up to 6000m of water."@en ;
  skos:inScheme <http://vocab.nerc.ac.uk/scheme/SDNDEV/current> ;
  skos:notation "SDN:L22::TOOL1171" ;
  skos:note "accepted"@en ;
  skos:prefLabel "British Geological Survey VC1 6m vibrocorer"@en ;
  skos:related <http://vocab.nerc.ac.uk/collection/B75/current/ORG00086> ;
.
inst:TOOL1172
  rdf:type skos:Concept ;
  dcterm:date "2017-11-23 13:03:21.0" ;
  dcterm:identifier "SDN:L22::TOOL1172" ;
  pav:hasCurrentVersion <http://vocab.nerc.ac.uk/collection/L22/current/TOOL1172/1> ;
  owl:versionInfo "1" ;
  skos:altLabel "BGS RD1 5m"@en ;
  skos:broader <http://vocab.nerc.ac.uk/collection/L05/current/51> ;
  skos:broader <http://vocab.nerc.ac.uk/collection/L05/current/53> ;
  skos:definition "A combined rockdrill and vibrocorer system developed by BGS. It has been used to sample offshore and deep water material. The system is capable of collecting hard rock (5m maximum) and soft sediment (6 m maximum)."@en ;
  skos:inScheme <http://vocab.nerc.ac.uk/scheme/SDNDEV/current> ;
  skos:notation "SDN:L22::TOOL1172" ;
  skos:note "accepted"@en ;
  skos:prefLabel "British Geological Survey RD1 5m (combined) rockdrill and vibrocorer"@en ;
  skos:related <http://vocab.nerc.ac.uk/collection/B75/current/ORG00086> ;
.
inst:TOOL1173
  rdf:type skos:Concept ;
  dcterm:date "2017-11-23 13:03:21.0" ;
  dcterm:identifier "SDN:L22::TOOL1173" ;
  pav:hasCurrentVersion <http://vocab.nerc.ac.uk/collection/L22/current/TOOL1173/1> ;
  owl:versionInfo "1" ;
  skos:altLabel "Duncan Ass. Box"@en ;
  skos:broader <http://vocab.nerc.ac.uk/collection/L05/current/51> ;
  skos:definition "A Duncan and Associates box corer where the model is unknown. It is fitted with a 300 mm X 300 mm X 955-975 mm high cabinet box. It is capable of collecting oceanographic sediments up to 5000 m."@en ;
  skos:inScheme <http://vocab.nerc.ac.uk/scheme/SDNDEV/current> ;
  skos:notation "SDN:L22::TOOL1173" ;
  skos:note "accepted"@en ;
  skos:prefLabel "Duncan and Associates unknown box corer"@en ;
  skos:related <http://vocab.nerc.ac.uk/collection/B75/current/ORG01106> ;
.
inst:TOOL1174
  rdf:type skos:Concept ;
  dcterm:date "2017-11-23 13:03:21.0" ;
  dcterm:identifier "SDN:L22::TOOL1174" ;
  pav:hasCurrentVersion <http://vocab.nerc.ac.uk/collection/L22/current/TOOL1174/1> ;
  owl:versionInfo "1" ;
  skos:altLabel "Duncan Ass. Grav"@en ;
  skos:broader <http://vocab.nerc.ac.uk/collection/L05/current/51> ;
  skos:definition "A marine sediment corer. It uses the pull of gravity to penetrate the seabed with a core barrel to collect samples. Manufactured in mild steel with varying corer barrel lengths between 1m and 6m, and a range of barrel diameters. These can also be adapted to be used as Piston corers and supplied with stainless steel releaser mechanisms."@en ;
  skos:inScheme <http://vocab.nerc.ac.uk/scheme/SDNDEV/current> ;
  skos:notation "SDN:L22::TOOL1174" ;
  skos:note "accepted"@en ;
  skos:prefLabel "Duncan and Associates gravity corer"@en ;
  skos:related <http://vocab.nerc.ac.uk/collection/B75/current/ORG01106> ;
.
inst:TOOL1175
  rdf:type skos:Concept ;
  dcterm:date "2017-11-23 13:03:21.0" ;
  dcterm:identifier "SDN:L22::TOOL1175" ;
  pav:hasCurrentVersion <http://vocab.nerc.ac.uk/collection/L22/current/TOOL1175/1> ;
  owl:versionInfo "1" ;
  skos:altLabel "NMF Grav"@en ;
  skos:broader <http://vocab.nerc.ac.uk/collection/L05/current/51> ;
  skos:definition "A marine sediment corer. The corer consists of a weight with steel tube sections attached to it. The end of the corer is fitted with a tapered cutter section and a catcher to retain the sample. Sample tubes are fitted with a clear polycarbonate liner with diameter of 63.5mm. To collect a core sample, the corer is lowered down to the seabed on the end of a wire, stopping a set distance above. It is then lowered at a set speed into the sediment to obtain the sample, before being raised to the surface, it is dismantled and the polycarbonate core liner encasing the sample is removed. The weight can vary between 100kg to 1000kg. Depending on the size of the sample tube, the corer is capable of collecting sediments between 1-4 m in length."@en ;
  skos:inScheme <http://vocab.nerc.ac.uk/scheme/SDNDEV/current> ;
  skos:notation "SDN:L22::TOOL1175" ;
  skos:note "accepted"@en ;
  skos:prefLabel "National Marine Facilities gravity corer"@en ;
  skos:related <http://vocab.nerc.ac.uk/collection/B75/current/ORG00125> ;
.
inst:TOOL1176
  rdf:type skos:Concept ;
  dcterm:date "2017-11-23 13:03:21.0" ;
  dcterm:identifier "SDN:L22::TOOL1176" ;
  pav:hasCurrentVersion <http://vocab.nerc.ac.uk/collection/L22/current/TOOL1176/1> ;
  owl:versionInfo "1" ;
  skos:altLabel "NMF Piston"@en ;
  skos:broader <http://vocab.nerc.ac.uk/collection/L05/current/51> ;
  skos:definition "A marine piston corer part of the UK National Marine Equipment Pool (NMEP). The corer consists of a weight fitted with steel sample tubes. A PVC liner tube is fitted the full-length core barrel. A piston is fitted inside the PVC liner and is attached to a wire, which runs inside the corer barrel, through a hole in the centre of the weight and is attached to the main deployment wire. The corer is lowered on a wire to the seabed and a trigger system causes the core barrel to free fall into the sediment to collect samples. The action of the piston reduces internal friction allowing long cores to be collected. Core samples of 90mm and 110mm diameter can be taken. Up to five sections of 5.4 metre-long barrels can be fitted depending on the type of sediment being sampled."@en ;
  skos:inScheme <http://vocab.nerc.ac.uk/scheme/SDNDEV/current> ;
  skos:notation "SDN:L22::TOOL1176" ;
  skos:note "accepted"@en ;
  skos:prefLabel "National Marine Facilities piston corer"@en ;
  skos:related <http://vocab.nerc.ac.uk/collection/B75/current/ORG00125> ;
.
inst:TOOL1177
  rdf:type skos:Concept ;
  dcterm:date "2017-11-23 13:03:21.0" ;
  dcterm:identifier "SDN:L22::TOOL1177" ;
  pav:hasCurrentVersion <http://vocab.nerc.ac.uk/collection/L22/current/TOOL1177/1> ;
  owl:versionInfo "1" ;
  skos:altLabel "UnSpec Box"@en ;
  skos:broader <http://vocab.nerc.ac.uk/collection/L05/current/51> ;
  skos:definition "A marine geological tool that recovers undisturbed soft surface sediments. It is designed for minimum disturbance of the sediment surface by bow wave effects. Traditionally, it consists of a weighted stem fitted to a square sampling box. The corer is lowered vertically until it impacts with the seabed. At this point the instrument is triggered by a trip as the main coring stem passes through its frame. While pulling the corer out of the sediment a spade swings underneath the sample to prevent loss. When hauled back on board, the spade is under the box."@en ;
  skos:inScheme <http://vocab.nerc.ac.uk/scheme/SDNDEV/current> ;
  skos:notation "SDN:L22::TOOL1177" ;
  skos:note "accepted"@en ;
  skos:prefLabel "Unspecified box corer"@en ;
  skos:related <http://vocab.nerc.ac.uk/collection/B75/current/ORG00001> ;
.
inst:TOOL1178
  rdf:type skos:Concept ;
  dcterm:date "2017-11-23 13:03:21.0" ;
  dcterm:identifier "SDN:L22::TOOL1178" ;
  pav:hasCurrentVersion <http://vocab.nerc.ac.uk/collection/L22/current/TOOL1178/1> ;
  owl:versionInfo "1" ;
  skos:altLabel "UnSpec Trigger"@en ;
  skos:broader <http://vocab.nerc.ac.uk/collection/L05/current/51> ;
  skos:definition "A trigger corer is a marine geological coring device used as part of the trigger system which allows a piston corer to free fall and collect cores. These trigger cores are often analysed by scientists."@en ;
  skos:inScheme <http://vocab.nerc.ac.uk/scheme/SDNDEV/current> ;
  skos:notation "SDN:L22::TOOL1178" ;
  skos:note "accepted"@en ;
  skos:prefLabel "Unspecified trigger corer"@en ;
  skos:related <http://vocab.nerc.ac.uk/collection/B75/current/ORG00001> ;
.
inst:TOOL1179
  rdf:type skos:Concept ;
  dcterm:date "2017-11-23 13:03:21.0" ;
  dcterm:identifier "SDN:L22::TOOL1179" ;
  pav:hasCurrentVersion <http://vocab.nerc.ac.uk/collection/L22/current/TOOL1179/1> ;
  owl:versionInfo "1" ;
  skos:altLabel "BAS Grav"@en ;
  skos:broader <http://vocab.nerc.ac.uk/collection/L05/current/51> ;
  skos:definition "Gravity corer built in 2010 by P.Smit, Netherland. It was primarily used in the Paleo - Ice Sheets and Quaternary Sediments Work packages at BAS. The corer uses the pull of gravity to penetrate the seabed with a core barrel to collect samples. Corer can configure 3m, 6m, 9m, and 12m barrels."@en ;
  skos:inScheme <http://vocab.nerc.ac.uk/scheme/SDNDEV/current> ;
  skos:notation "SDN:L22::TOOL1179" ;
  skos:note "accepted"@en ;
  skos:prefLabel "British Antarctic Survey gravity corer"@en ;
  skos:related <http://vocab.nerc.ac.uk/collection/B75/current/ORG0015> ;
.
inst:TOOL1181
  rdf:type skos:Concept ;
  dcterm:date "2017-11-27 16:02:45.0" ;
  dcterm:identifier "SDN:L22::TOOL1181" ;
  pav:hasCurrentVersion <http://vocab.nerc.ac.uk/collection/L22/current/TOOL1181/1> ;
  owl:versionInfo "1" ;
  skos:altLabel "BAS MUDL net"@en ;
  skos:broader <http://vocab.nerc.ac.uk/collection/L05/current/22> ;
  skos:definition "A motion-compensated upwards and downwards looking Bongo net - one facing upwards, one downwards. The instrument is designed for capturing zooplankton moving up and down the water column. It uses a spring mechanism to compensate for the platform's movements, maintaining the net's upward and downward velocity close to steady-state. The system uses sealed cod ends and a time-controlled open/close mechanism. The cod ends need to be pre-filled with water before deployment to avoid implosion."@en ;
  skos:inScheme <http://vocab.nerc.ac.uk/scheme/SDNDEV/current> ;
  skos:notation "SDN:L22::TOOL1181" ;
  skos:note "accepted"@en ;
  skos:prefLabel "BAS MUDL Bongo net"@en ;
  skos:related <http://vocab.nerc.ac.uk/collection/B75/current/ORG0015> ;
.
inst:TOOL1191
  rdf:type skos:Concept ;
  dcterm:date "2018-01-17 13:39:30.0" ;
  dcterm:identifier "SDN:L22::TOOL1191" ;
  pav:hasCurrentVersion <http://vocab.nerc.ac.uk/collection/L22/current/TOOL1191/1> ;
  owl:versionInfo "1" ;
  skos:altLabel "Oktopus MC8-12"@en ;
  skos:broader <http://vocab.nerc.ac.uk/collection/L05/current/51> ;
  skos:definition "An oceanographic sediment core sampling device. Collects multiple cores of undisturbed samples of the upper boundary layers between sea floor and the water column. Consists of a 2.1 m (dia.) x 1.2-1.7 m (H) stainless steel frame and between 8-12 polycarbonate coring tubes (610 mm length). Tube material is optional. The tube diameter used can range between 60-110 mm. The frame can be fitted with external equipment such as cameras and sensors systems. It is capable of full ocean depth deployments and a penetration depth of ca. 300 mm."@en ;
  skos:inScheme <http://vocab.nerc.ac.uk/scheme/SDNDEV/current> ;
  skos:notation "SDN:L22::TOOL1191" ;
  skos:note "accepted"@en ;
  skos:prefLabel "Oktopus MC8-12 multicorer"@en ;
  skos:related <http://vocab.nerc.ac.uk/collection/B75/current/ORG01115> ;
.
inst:TOOL1199
  rdf:type skos:Concept ;
  dcterm:date "2018-01-30 16:59:47.0" ;
  dcterm:identifier "SDN:L22::TOOL1199" ;
  pav:hasCurrentVersion <http://vocab.nerc.ac.uk/collection/L22/current/TOOL1199/1> ;
  owl:versionInfo "1" ;
  skos:altLabel "UnSpec kasten"@en ;
  skos:broader <http://vocab.nerc.ac.uk/collection/L05/current/51> ;
  skos:definition "A marine geological coring device designed to sample large volumes of soft sediments. The kasten corer may come in four different lengths (2 m, 3 m, or 4 m), and uses a stainless steel box with a rectangular section of 15 cm^2 to push into the sediment with the help of a weight on top and a trap at the bottom. To deploy and retrieve the corer, the track and tilt system is used. After retrieval, a removable side of the core barrel can provide immediate access to the sampled sediment. The kasten corer is a variation of the gravity corer."@en ;
  skos:inScheme <http://vocab.nerc.ac.uk/scheme/SDNDEV/current> ;
  skos:notation "SDN:L22::TOOL1199" ;
  skos:note "accepted"@en ;
  skos:prefLabel "Unspecified kasten corer"@en ;
.
inst:TOOL1204
  rdf:type skos:Concept ;
  dcterm:date "2018-01-30 16:59:47.0" ;
  dcterm:identifier "SDN:L22::TOOL1204" ;
  pav:hasCurrentVersion <http://vocab.nerc.ac.uk/collection/L22/current/TOOL1204/1> ;
  owl:versionInfo "1" ;
  skos:altLabel "BX-650"@en ;
  skos:broader <http://vocab.nerc.ac.uk/collection/L05/current/51> ;
  skos:definition "A box corer designed for sediment surface sampling, also referred to as 'MK-III box (spade) corer'. The unit includes a stainless steel sample box of 50 cm x 50 cm in dimension, an automatic door-closing device, a pretrip preventer bar, quick release spade latches, and jacking dolly for mounting and removing sample box and spade. The corer can penetrate to a maximum of 60 cm into the sediment. Its weight is of approximately 740 kg, and its height is 212 cm with a deck footprint of 165 cm x 192 cm."@en ;
  skos:inScheme <http://vocab.nerc.ac.uk/scheme/SDNDEV/current> ;
  skos:notation "SDN:L22::TOOL1204" ;
  skos:note "accepted"@en ;
  skos:prefLabel "BX-650 box corer"@en ;
  skos:related <http://vocab.nerc.ac.uk/collection/B75/current/ORG00738> ;
.
inst:TOOL1214
  rdf:type skos:Concept ;
  dcterm:date "2018-02-27 12:21:14.0" ;
  dcterm:identifier "SDN:L22::TOOL1214" ;
  pav:hasCurrentVersion <http://vocab.nerc.ac.uk/collection/L22/current/TOOL1214/1> ;
  owl:versionInfo "1" ;
  skos:altLabel "Ponar grab"@en ;
  skos:broader <http://vocab.nerc.ac.uk/collection/L05/current/50> ;
  skos:definition "Developed in the mid-1960s (Powers and Robertson 1967), ponar grabs are used to sample coarse or fine, undisturbed sediment from the sea floor. It consists of a pair of weighted, tapered jaws held open by a catch bar across the top of the sampler. On touching the bottom, the tension bar is released, allowing the jaws to move and close. The device is activated by the release of the cable tension on the lifting mechanism when the sampler reaches the sediment. During retrieval, the tension on the cable keeps the jaws closed. It has a pair of metal side plates which prevents the sampler from falling over after the jaws' closure. Its jaws overlap to minimise sample washout during ascent. Depending on the variant (standard or petite), the sampled area can be between approx. 15-23 cm sq. (approx. 1000 - 7250 cubic metres)."@en ;
  skos:inScheme <http://vocab.nerc.ac.uk/scheme/SDNDEV/current> ;
  skos:notation "SDN:L22::TOOL1214" ;
  skos:note "accepted"@en ;
  skos:prefLabel "Unspecified ponar grab"@en ;
.
inst:TOOL1215
  rdf:type skos:Concept ;
  dcterm:date "2018-02-27 12:21:14.0" ;
  dcterm:identifier "SDN:L22::TOOL1215" ;
  pav:hasCurrentVersion <http://vocab.nerc.ac.uk/collection/L22/current/TOOL1215/1> ;
  owl:versionInfo "1" ;
  skos:altLabel "Standard ponar grab"@en ;
  skos:broader <http://vocab.nerc.ac.uk/collection/L05/current/50> ;
  skos:definition "Developed in the mid-1960s (Powers and Robertson 1967), ponar grabs are used to sample coarse or fine, undisturbed sediment from the sea floor. It consists of a pair of weighted, tapered jaws held open by a catch bar across the top of the sampler. On touching the bottom, the tension bar is released, allowing the jaws to move and close. The device is activated by the release of the cable tension on the lifting mechanism when the sampler reaches the sediment. During retrieval, the tension on the cable keeps the jaws closed. It has a pair of metal side plates which prevents the sampler from falling over after the jaws' closure. Its jaws overlap to minimise sample washout during ascent. It is typically used with a winch or crane hoist. The sampled area is approx. 23 cm sq. (approx. 7250 cubic metres)."@en ;
  skos:inScheme <http://vocab.nerc.ac.uk/scheme/SDNDEV/current> ;
  skos:notation "SDN:L22::TOOL1215" ;
  skos:note "accepted"@en ;
  skos:prefLabel "Unspecified Standard ponar grab"@en ;
.
inst:TOOL1216
  rdf:type skos:Concept ;
  dcterm:date "2018-02-27 12:21:14.0" ;
  dcterm:identifier "SDN:L22::TOOL1216" ;
  pav:hasCurrentVersion <http://vocab.nerc.ac.uk/collection/L22/current/TOOL1216/1> ;
  owl:versionInfo "1" ;
  skos:altLabel "Petite ponar grab"@en ;
  skos:broader <http://vocab.nerc.ac.uk/collection/L05/current/50> ;
  skos:definition "Developed in the mid-1960s (Powers and Robertson 1967), ponar grabs are used to sample coarse or fine, undisturbed sediment from the sea floor. It consists of a pair of weighted, tapered jaws held open by a catch bar across the top of the sampler. On touching the bottom, the tension bar is released, allowing the jaws to move and close. The device is activated by the release of the cable tension on the lifting mechanism when the sampler reaches the sediment. During retrieval, the tension on the cable keeps the jaws closed. It has a pair of metal side plates which prevents the sampler from falling over after the jaws' closure. Its jaws overlap to minimise sample washout during ascent. Smaller than the standard ponar grab, it is typically used in hand line operations. The sampled area is approx. 15 cm sq. (approx. 1000 cubic metres)."@en ;
  skos:inScheme <http://vocab.nerc.ac.uk/scheme/SDNDEV/current> ;
  skos:notation "SDN:L22::TOOL1216" ;
  skos:note "accepted"@en ;
  skos:prefLabel "Unspecified Petite ponar grab"@en ;
.
inst:TOOL1235
  rdf:type skos:Concept ;
  dcterm:date "2018-05-04 16:14:17.0" ;
  dcterm:identifier "SDN:L22::TOOL1235" ;
  pav:hasCurrentVersion <http://vocab.nerc.ac.uk/collection/L22/current/TOOL1235/1> ;
  owl:versionInfo "1" ;
  skos:altLabel "Vibrocorer"@en ;
  skos:broader <http://vocab.nerc.ac.uk/collection/L05/current/51> ;
  skos:definition "A corer designed to collect sediment samples from unconsolidated, waterlogged, heterogeneous sediments and soils. Typically, samples are collected in a core tube that is driven into sediment by the force of gravity, enhanced by vibration energy from a viration motor."@en ;
  skos:inScheme <http://vocab.nerc.ac.uk/scheme/SDNDEV/current> ;
  skos:notation "SDN:L22::TOOL1235" ;
  skos:note "accepted"@en ;
  skos:prefLabel "Unspecified vibrocorer"@en ;
.
inst:TOOL1249
  rdf:type skos:Concept ;
  dcterm:date "2018-07-30 16:30:34.0" ;
  dcterm:identifier "SDN:L22::TOOL1249" ;
  pav:hasCurrentVersion <http://vocab.nerc.ac.uk/collection/L22/current/TOOL1249/1> ;
  owl:versionInfo "1" ;
  skos:altLabel "KOVACS ice coring systems"@en ;
  skos:broader <http://vocab.nerc.ac.uk/collection/L05/current/56> ;
  skos:definition "A series of hand auger systems designed for the retrieval of ice cores. Each KOVACS ice coring system includes a light weight core barrel made of a filament composite tube with plastic fitting, an aluminium cutting shoe, heat-treated steel cutting teeth, a stainless steel and aluminium drive head, as well as two extension rods of 1m in length each. Different core diameters and lengths are delivered by the four coring systems available: MARK II (9cm x 1m), MARK III (7.25cm x 1m), MARK V (14cm x 1m), and MARK VI (9cm x 1.5m)."@en ;
  skos:inScheme <http://vocab.nerc.ac.uk/scheme/SDNDEV/current> ;
  skos:notation "SDN:L22::TOOL1249" ;
  skos:note "accepted"@en ;
  skos:prefLabel "KOVACS ice coring systems"@en ;
  skos:related <http://vocab.nerc.ac.uk/collection/B75/current/ORG01152> ;
.
inst:TOOL1252
  rdf:type skos:Concept ;
  dcterm:date "2018-08-02 15:26:57.0" ;
  dcterm:identifier "SDN:L22::TOOL1252" ;
  pav:hasCurrentVersion <http://vocab.nerc.ac.uk/collection/L22/current/TOOL1252/1> ;
  owl:versionInfo "1" ;
  skos:altLabel "UnSpec Agassiz"@en ;
  skos:broader <http://vocab.nerc.ac.uk/collection/L05/current/61> ;
  skos:definition "A sledge composed of a metal frame with a net attached, designed to be towed along the seabed at a maximum of approximately 4000 m depth. Mouth width can vary."@en ;
  skos:inScheme <http://vocab.nerc.ac.uk/scheme/SDNDEV/current> ;
  skos:notation "SDN:L22::TOOL1252" ;
  skos:note "accepted"@en ;
  skos:prefLabel "Unspecified Agassiz trawl"@en ;
.
inst:TOOL1253
  rdf:type skos:Concept ;
  dcterm:date "2018-08-02 15:26:57.0" ;
  dcterm:identifier "SDN:L22::TOOL1253" ;
  pav:hasCurrentVersion <http://vocab.nerc.ac.uk/collection/L22/current/TOOL1253/1> ;
  owl:versionInfo "1" ;
  skos:altLabel "UnSpec MSC"@en ;
  skos:broader <http://vocab.nerc.ac.uk/collection/L05/current/30> ;
  skos:definition "A large water bottle (volume of approximately 100 litres) designed to collect marine snow particles. The device is deployed open, and closed at a chosen depth. Once recovered, it is usually rested upright for typically 2 hours, to allow the formation of three distinct carbon pools: suspended, slow-sinking and fast-sinking."@en ;
  skos:inScheme <http://vocab.nerc.ac.uk/scheme/SDNDEV/current> ;
  skos:notation "SDN:L22::TOOL1253" ;
  skos:note "accepted"@en ;
  skos:prefLabel "Unspecified Marine Snow Catcher"@en ;
.
inst:TOOL1259
  rdf:type skos:Concept ;
  dcterm:date "2018-08-02 15:26:57.0" ;
  dcterm:identifier "SDN:L22::TOOL1259" ;
  pav:hasCurrentVersion <http://vocab.nerc.ac.uk/collection/L22/current/TOOL1259/1> ;
  owl:versionInfo "1" ;
  skos:altLabel "UnSpec trammel net"@en ;
  skos:broader <http://vocab.nerc.ac.uk/collection/L05/current/65> ;
  skos:definition "A net consisting of a sheet of fine-meshed net sandwiched between two outer sheets of large-meshed nets. All three net walls are attached to a weighted foot rope and a floating headline, so that they hang vertically in the water. The height of the inner net is double that of the outer nets, so that fish swim through the larger outer net wall and become entangled in the loose pockets of the inner net."@en ;
  skos:inScheme <http://vocab.nerc.ac.uk/scheme/SDNDEV/current> ;
  skos:notation "SDN:L22::TOOL1259" ;
  skos:note "accepted"@en ;
  skos:prefLabel "Unspecified trammel net"@en ;
.
inst:TOOL1260
  rdf:type skos:Concept ;
  dcterm:date "2018-08-02 15:26:57.0" ;
  dcterm:identifier "SDN:L22::TOOL1260" ;
  pav:hasCurrentVersion <http://vocab.nerc.ac.uk/collection/L22/current/TOOL1260/1> ;
  owl:versionInfo "1" ;
  skos:altLabel "UnSpec gravity corer"@en ;
  skos:broader <http://vocab.nerc.ac.uk/collection/L05/current/51> ;
  skos:definition "Marine geological coring device that uses a lead weight system to penetrate the seabed and collect sediment samples."@en ;
  skos:inScheme <http://vocab.nerc.ac.uk/scheme/SDNDEV/current> ;
  skos:notation "SDN:L22::TOOL1260" ;
  skos:note "accepted"@en ;
  skos:prefLabel "Unspecified gravity corer"@en ;
.
inst:TOOL1274
  rdf:type skos:Concept ;
  dcterm:date "2018-08-02 15:26:57.0" ;
  dcterm:identifier "SDN:L22::TOOL1274" ;
  pav:hasCurrentVersion <http://vocab.nerc.ac.uk/collection/L22/current/TOOL1274/1> ;
  owl:versionInfo "1" ;
  skos:altLabel "BAS Net Traps"@en ;
  skos:broader <http://vocab.nerc.ac.uk/collection/L05/current/68> ;
  skos:definition "A pair of nets composed by an upward-looking bongo net, composed by two conjoined rings, and a downward-looking net with lead weights on the net-ring. The net traps are connected to a brass jawed mechanism, which uses brass messengers sent down the wires to sequentially open them at the desired depth, and close them at the end of the sampling period before for recovery. They are designed to catch plankton swimming into them from both directions."@en ;
  skos:inScheme <http://vocab.nerc.ac.uk/scheme/SDNDEV/current> ;
  skos:notation "SDN:L22::TOOL1274" ;
  skos:note "accepted"@en ;
  skos:prefLabel "British Antarctic Survey Net Traps"@en ;
  skos:related <http://vocab.nerc.ac.uk/collection/B75/current/ORG0015> ;
.
inst:TOOL1285
  rdf:type skos:Concept ;
  dcterm:date "2018-09-26 14:55:49.0" ;
  dcterm:identifier "SDN:L22::TOOL1285" ;
  pav:hasCurrentVersion <http://vocab.nerc.ac.uk/collection/L22/current/TOOL1285/1> ;
  owl:versionInfo "1" ;
  skos:altLabel "GEMAX corer"@en ;
  skos:broader <http://vocab.nerc.ac.uk/collection/L05/current/51> ;
  skos:definition "A gravity corer with an internal tube diameter of 90mm, designed for undisturbed sampling of soft sediment from the sea floor. The GEMAX corer is an evolution of the GEMINI corer (itself a development from the Niemistö corer, 1974); both consist of twin steel core barrels, though the GEMAX has a larger core-barrel diameter and an added peeler facility in the slicer unit, implemented to limit sample contamination without loss in sample volume. Optimum penetration of 50-60 cm into the seabed can be achieved in soft muddy sediments at wire speed of 1 m/s and two standard weights."@en ;
  skos:inScheme <http://vocab.nerc.ac.uk/scheme/SDNDEV/current> ;
  skos:notation "SDN:L22::TOOL1285" ;
  skos:note "accepted"@en ;
  skos:prefLabel "GEMAX gravity corer"@en ;
.
inst:TOOL1304
  rdf:type skos:Concept ;
  dcterm:date "2019-01-23 14:03:46.0" ;
  dcterm:identifier "SDN:L22::TOOL1304" ;
  pav:hasCurrentVersion <http://vocab.nerc.ac.uk/collection/L22/current/TOOL1304/1> ;
  owl:versionInfo "1" ;
  skos:altLabel "Technicap PPS 4-3 24S 500ML"@en ;
  skos:broader <http://vocab.nerc.ac.uk/collection/L05/current/33> ;
  skos:definition "A mooring sediment trap designed for long-term continuous deployments. It is used for the determine the flux of settling particles in-situ. It uses a funnel to collect passing settled particles into one of a set of bottles mounted on a carousel. The bottles are changed after a set period of time. It consists of a cylindro-conical funnel (collecting area of 0.05 m2) with a phenolic composite baffle (cell dia. 8 mm) to prevent large objects clogging the system. The trap is fitted with 24 x 500 ml polypropylen sampling bottles. It is capable of 18 month deployments and has a sampling interval of 1 hour - 60 days. It has a maximum operating depth of 1000 m (PETP) or 5000m (Aluminium) or 6000m (Titanium)."@en ;
  skos:inScheme <http://vocab.nerc.ac.uk/scheme/SDNDEV/current> ;
  skos:notation "SDN:L22::TOOL1304" ;
  skos:note "accepted"@en ;
  skos:prefLabel "Technicap PPS 4-3 24S 500ML sediment trap"@en ;
  skos:related <http://vocab.nerc.ac.uk/collection/B75/current/ORG01178> ;
.
inst:TOOL1326
  rdf:type skos:Concept ;
  dcterm:date "2019-04-08 11:18:12.0" ;
  dcterm:identifier "SDN:L22::TOOL1326" ;
  pav:hasCurrentVersion <http://vocab.nerc.ac.uk/collection/L22/current/TOOL1326/1> ;
  owl:versionInfo "1" ;
  skos:altLabel "McLane PPS"@en ;
  skos:broader <http://vocab.nerc.ac.uk/collection/L05/current/30> ;
  skos:definition "An autonomous time-series particulate sampler. It consists of a stainless steel frame, aluminium controller housing, 25-port valve, pump and 24-filter holders containing 47mm 0.7 micron GF/F filters. Individual water samples are collected by user-defined time-series events. The 25 port valve physically isolates samples and pumps samples through the selected filter position before passing through the 50, 125, or 250 ml/min pump. The maximum volume per sample is 10 litres. The data recorded during a deployment includes flow rates, volume pumped, pump feedback, power, temperature and event times. This data is offloaded from the PPS after deployment and used for sample analysis. It is depth-rated to 5,500 m."@en ;
  skos:inScheme <http://vocab.nerc.ac.uk/scheme/SDNDEV/current> ;
  skos:notation "SDN:L22::TOOL1326" ;
  skos:note "accepted"@en ;
  skos:prefLabel "McLane Research Laboratories PPS {Phytoplankton Sampler} water sampler"@en ;
  skos:related <http://vocab.nerc.ac.uk/collection/B75/current/ORG00996> ;
  skos:related <http://vocab.nerc.ac.uk/collection/L35/current/MAN0036> ;
.
inst:TOOL1339
  rdf:type skos:Concept ;
  dcterm:date "2019-07-11 11:45:11.0" ;
  dcterm:identifier "SDN:L22::TOOL1339" ;
  pav:hasCurrentVersion <http://vocab.nerc.ac.uk/collection/L22/current/TOOL1339/1> ;
  owl:versionInfo "1" ;
  skos:altLabel "Cefas water sampler"@en ;
  skos:broader <http://vocab.nerc.ac.uk/collection/L05/current/30> ;
  skos:definition "A programmable water sampler developed in-house, originally designed for use with a Continuous Plankton Recorder (CPR). It can also be deployed on moorings, ROV or AUV platforms and towed-vehicle systems, to determine the species of marine plankton or for capturing marine contaminents. A pump collects up to 16 individual samples into gas-impermeable 250 ml bags, each within protective enclosures, which can be pre-filled with preservative. Sampling can be set-up via a Windows software interface, allowing the user to programme for water samples to be taken at specific times. It also has the capability for remote control sampling through an Iridium satellite interface, allowing remote sampling activation. Each bag fill can be performed either as a one shot operation, or as a repeat fill. The repeat fill feature allows a sample bag to be filled gradually over a period of time, with the amount of fill for each stage being preset through the user interface. Larger sampling bags can also be fitted as necessary. The sampler operates up to approximately 20 m depth, and can pump 100 ml in approximately 90 seconds. Further information can be found at http://www.cefastechnology.co.uk/products/water-sampler/."@en ;
  skos:inScheme <http://vocab.nerc.ac.uk/scheme/SDNDEV/current> ;
  skos:notation "SDN:L22::TOOL1339" ;
  skos:note "accepted"@en ;
  skos:prefLabel "Cefas water sampler"@en ;
  skos:related <http://vocab.nerc.ac.uk/collection/B75/current/ORG00008> ;
  skos:related <http://vocab.nerc.ac.uk/collection/L35/current/MAN0044> ;
.
inst:TOOL1371
  rdf:type skos:Concept ;
  dcterm:date "2019-12-10 09:27:08.0" ;
  dcterm:identifier "SDN:L22::TOOL1371" ;
  pav:hasCurrentVersion <http://vocab.nerc.ac.uk/collection/L22/current/TOOL1371/1> ;
  owl:versionInfo "1" ;
  skos:altLabel "diver suction pump"@en ;
  skos:broader <http://vocab.nerc.ac.uk/collection/L05/current/391> ;
  skos:definition "A generic term for a manually operated instrument that is used to collect sediment via suction. The sampler is operated underwater by divers. The method of suction is unspecified."@en ;
  skos:inScheme <http://vocab.nerc.ac.uk/scheme/SDNDEV/current> ;
  skos:notation "SDN:L22::TOOL1371" ;
  skos:note "accepted"@en ;
  skos:prefLabel "Unspecified diver-operated sediment suction sampler"@en ;
  skos:related <http://vocab.nerc.ac.uk/collection/B75/current/UNSPEC> ;
  skos:related <http://vocab.nerc.ac.uk/collection/L35/current/MAN0001> ;
.
inst:TOOL1372
  rdf:type skos:Concept ;
  dcterm:date "2019-12-10 10:47:35.0" ;
  dcterm:identifier "SDN:L22::TOOL1372" ;
  pav:hasCurrentVersion <http://vocab.nerc.ac.uk/collection/L22/current/TOOL1372/1> ;
  owl:versionInfo "1" ;
  skos:altLabel "diver suction pump - Rostron 1983"@en ;
  skos:broader <http://vocab.nerc.ac.uk/collection/L05/current/391> ;
  skos:definition "A manually operated instrument that is used to collect sediment via suction. The sampler consists of a closed chamber with a detachable lid and screw threads on the inside to facilitate the attachment and detachment of mesh sampling bags. Air is supplied from a compressed air cylinder, fitted with a pressure-reducing valve and connected to the sampler via a short length of reinforced tubing. The sampler is operated underwater by divers."@en ;
  skos:inScheme <http://vocab.nerc.ac.uk/scheme/SDNDEV/current> ;
  skos:notation "SDN:L22::TOOL1372" ;
  skos:note "accepted"@en ;
  skos:prefLabel "Unknown diver-operated sediment suction sampler - Rostron 1983"@en ;
  skos:related <http://vocab.nerc.ac.uk/collection/B75/current/UNSPEC> ;
  skos:related <http://vocab.nerc.ac.uk/collection/L35/current/MAN0002> ;
.
inst:TOOL1373
  rdf:type skos:Concept ;
  dcterm:date "2019-12-10 10:47:35.0" ;
  dcterm:identifier "SDN:L22::TOOL1373" ;
  pav:hasCurrentVersion <http://vocab.nerc.ac.uk/collection/L22/current/TOOL1373/1> ;
  owl:versionInfo "1" ;
  skos:altLabel "steel 1m pipe dredge"@en ;
  skos:broader <http://vocab.nerc.ac.uk/collection/L05/current/60> ;
  skos:definition "A heavy-duty dredge consisting of a steel pipe where the make and model are unknown. The collection pipe is 1m length by 25cm diameter and made of 5mm thick steel. The dredge is towed through the target area collecting material from the bed. The pipe is 1 metre length, 25cm diameter and made of 5mm steel."@en ;
  skos:inScheme <http://vocab.nerc.ac.uk/scheme/SDNDEV/current> ;
  skos:notation "SDN:L22::TOOL1373" ;
  skos:note "accepted"@en ;
  skos:prefLabel "Unknown 1 x 0.25m sediment pipe dredge"@en ;
  skos:related <http://vocab.nerc.ac.uk/collection/B75/current/UNSPEC> ;
  skos:related <http://vocab.nerc.ac.uk/collection/L35/current/MAN0002> ;
.
inst:TOOL1374
  rdf:type skos:Concept ;
  dcterm:date "2019-12-10 10:47:35.0" ;
  dcterm:identifier "SDN:L22::TOOL1374" ;
  pav:hasCurrentVersion <http://vocab.nerc.ac.uk/collection/L22/current/TOOL1374/1> ;
  owl:versionInfo "1" ;
  skos:altLabel "sediment corer"@en ;
  skos:broader <http://vocab.nerc.ac.uk/collection/L05/current/51> ;
  skos:definition "A generic term for a coring device that allows for relatively undisturbed penetration of the sediment. Generally, core samplers consist of a core barrel (a hollow pipe or box) and a core cutter (or cutting head), located at the advancing end of the core barrel to facilitate the sampler's advancement into the sediment. Core catchers are commonly inserted into the cutting head to prevent sample loss during retrieval."@en ;
  skos:inScheme <http://vocab.nerc.ac.uk/scheme/SDNDEV/current> ;
  skos:notation "SDN:L22::TOOL1374" ;
  skos:note "accepted"@en ;
  skos:prefLabel "Unspecified sediment corer"@en ;
  skos:related <http://vocab.nerc.ac.uk/collection/B75/current/UNSPEC> ;
  skos:related <http://vocab.nerc.ac.uk/collection/L35/current/MAN0001> ;
.
inst:TOOL1375
  rdf:type skos:Concept ;
  dcterm:date "2019-12-10 10:47:35.0" ;
  dcterm:identifier "SDN:L22::TOOL1375" ;
  pav:hasCurrentVersion <http://vocab.nerc.ac.uk/collection/L22/current/TOOL1375/1> ;
  owl:versionInfo "1" ;
  skos:altLabel "HAPS corer"@en ;
  skos:broader <http://vocab.nerc.ac.uk/collection/L05/current/51> ;
  skos:definition "A generic term for a HAPS corer. It is a gravity corer that is designed to collect undisturbed sediments from hard and coarse material, such as sand. It typically consists of a triangular frame and a core barrel with tight top valve and core catcher to prevent porewater loss. The frame is weighted to penetrate the sediment but can be equipped with vibrator units to aid penetration."@en ;
  skos:inScheme <http://vocab.nerc.ac.uk/scheme/SDNDEV/current> ;
  skos:notation "SDN:L22::TOOL1375" ;
  skos:note "accepted"@en ;
  skos:prefLabel "Unspecified HAPS corer"@en ;
  skos:related <http://vocab.nerc.ac.uk/collection/B75/current/UNSPEC> ;
  skos:related <http://vocab.nerc.ac.uk/collection/L35/current/MAN0001> ;
.
inst:TOOL1376
  rdf:type skos:Concept ;
  dcterm:date "2019-12-10 10:47:35.0" ;
  dcterm:identifier "SDN:L22::TOOL1376" ;
  pav:hasCurrentVersion <http://vocab.nerc.ac.uk/collection/L22/current/TOOL1376/1> ;
  owl:versionInfo "1" ;
  skos:altLabel "manual corer"@en ;
  skos:broader <http://vocab.nerc.ac.uk/collection/L05/current/51> ;
  skos:definition "A hand-held sediment corer. Consists of a tube that is inserted into the sediment manually by a human operator (e.g. through manual force, hammering, rotating etc.)."@en ;
  skos:inScheme <http://vocab.nerc.ac.uk/scheme/SDNDEV/current> ;
  skos:notation "SDN:L22::TOOL1376" ;
  skos:note "accepted"@en ;
  skos:prefLabel "Unspecified manual sediment corer"@en ;
  skos:related <http://vocab.nerc.ac.uk/collection/B75/current/UNSPEC> ;
  skos:related <http://vocab.nerc.ac.uk/collection/L35/current/MAN0001> ;
.
inst:TOOL1378
  rdf:type skos:Concept ;
  dcterm:date "2019-12-19 09:54:55.0" ;
  dcterm:identifier "SDN:L22::TOOL1378" ;
  pav:hasCurrentVersion <http://vocab.nerc.ac.uk/collection/L22/current/TOOL1378/1> ;
  owl:versionInfo "1" ;
  skos:altLabel "scallop dredge"@en ;
  skos:broader <http://vocab.nerc.ac.uk/collection/L05/current/24> ;
  skos:definition "Rigid structures with a chain mail collecting bag, towed on the seabed to target king scallops. Generally used by towing several dredges side by side behind the vessel (source: seafish.org)."@en ;
  skos:inScheme <http://vocab.nerc.ac.uk/scheme/SDNDEV/current> ;
  skos:notation "SDN:L22::TOOL1378" ;
  skos:note "accepted"@en ;
  skos:prefLabel "Unspecified scallop dredge"@en ;
  skos:related <http://vocab.nerc.ac.uk/collection/B75/current/UNSPEC> ;
  skos:related <http://vocab.nerc.ac.uk/collection/L35/current/MAN0001> ;
.
inst:TOOL1379
  rdf:type skos:Concept ;
  dcterm:date "2019-12-19 09:54:55.0" ;
  dcterm:identifier "SDN:L22::TOOL1379" ;
  pav:hasCurrentVersion <http://vocab.nerc.ac.uk/collection/L22/current/TOOL1379/1> ;
  owl:versionInfo "1" ;
  skos:altLabel "queen scallop dredge"@en ;
  skos:broader <http://vocab.nerc.ac.uk/collection/L05/current/24> ;
  skos:definition "The dredges used to target queen scallops are wider and higher than a traditional scallop dredge. They do not have tooth bar across the front, instead they have either a metal grid, or tickler chains to get the scallops to lift up off the seabed and swim into the dredge. The scallops then fall back into a bag made of metal rings. Some fishermen are replacing the tickler chain and metal grid with a strip of rubber matting across the front of the dredge (source seafish.org)."@en ;
  skos:inScheme <http://vocab.nerc.ac.uk/scheme/SDNDEV/current> ;
  skos:notation "SDN:L22::TOOL1379" ;
  skos:note "accepted"@en ;
  skos:prefLabel "Unspecified queen scallop dredge"@en ;
  skos:related <http://vocab.nerc.ac.uk/collection/B75/current/UNSPEC> ;
  skos:related <http://vocab.nerc.ac.uk/collection/L35/current/MAN0001> ;
.
inst:TOOL1405
  rdf:type skos:Concept ;
  dcterm:date "2020-02-14 10:24:24.0" ;
  dcterm:identifier "SDN:L22::TOOL1405" ;
  pav:hasCurrentVersion <http://vocab.nerc.ac.uk/collection/L22/current/TOOL1405/1> ;
  owl:versionInfo "1" ;
  skos:altLabel "Manual bilge pump"@en ;
  skos:broader <http://vocab.nerc.ac.uk/collection/L05/current/31> ;
  skos:definition "A hand-powered submersible pump that can be used to suck water from the water body for sampling as well as other applications."@en ;
  skos:inScheme <http://vocab.nerc.ac.uk/scheme/SDNDEV/current> ;
  skos:notation "SDN:L22::TOOL1405" ;
  skos:note "accepted"@en ;
  skos:prefLabel "Unknown manual bilge pump"@en ;
  skos:related <http://vocab.nerc.ac.uk/collection/B75/current/UNSPEC> ;
  skos:related <http://vocab.nerc.ac.uk/collection/L35/current/MAN0002> ;
.
inst:TOOL1413
  rdf:type skos:Concept ;
  dcterm:date "2020-04-07 16:24:48.0" ;
  dcterm:identifier "SDN:L22::TOOL1413" ;
  pav:hasCurrentVersion <http://vocab.nerc.ac.uk/collection/L22/current/TOOL1413/1> ;
  owl:versionInfo "1" ;
  skos:altLabel "Lexan plastic panel substrate"@en ;
  skos:broader <http://vocab.nerc.ac.uk/collection/L05/current/392> ;
  skos:definition "An artificial colonisation substrate sometimes referred to as \"colonisation sandwich\", that is made of 6 Lexan plastic sheets separated from each other by spacers. It is used to determine the extent of colonisation and/or the diversity of settled organisms in a marine or artificial environment."@en ;
  skos:inScheme <http://vocab.nerc.ac.uk/scheme/SDNDEV/current> ;
  skos:notation "SDN:L22::TOOL1413" ;
  skos:note "accepted"@en ;
  skos:prefLabel "Custom-made Lexan plastic 6-plate settlement panel"@en ;
  skos:related <http://vocab.nerc.ac.uk/collection/B75/current/UNSPEC> ;
  skos:related <http://vocab.nerc.ac.uk/collection/L35/current/MAN0069> ;
.
inst:TOOL1414
  rdf:type skos:Concept ;
  dcterm:date "2020-04-07 16:24:48.0" ;
  dcterm:identifier "SDN:L22::TOOL1414" ;
  pav:hasCurrentVersion <http://vocab.nerc.ac.uk/collection/L22/current/TOOL1414/1> ;
  owl:versionInfo "1" ;
  skos:altLabel "Grooved PVC half-pipe substrate"@en ;
  skos:broader <http://vocab.nerc.ac.uk/collection/L05/current/392> ;
  skos:definition "An artificial colonisation substrate made from PVC pipe cut length-wise and engraved with lines to roughen its surface. It is used to determine the extent of colonisation and/or the diversity of settled organisms in a marine or artificial environment."@en ;
  skos:inScheme <http://vocab.nerc.ac.uk/scheme/SDNDEV/current> ;
  skos:notation "SDN:L22::TOOL1414" ;
  skos:note "accepted"@en ;
  skos:prefLabel "Custom-made grooved polyvinyl chloride half-pipe"@en ;
  skos:related <http://vocab.nerc.ac.uk/collection/B75/current/UNSPEC> ;
  skos:related <http://vocab.nerc.ac.uk/collection/L35/current/MAN0069> ;
.
inst:TOOL1415
  rdf:type skos:Concept ;
  dcterm:date "2020-04-07 16:24:48.0" ;
  dcterm:identifier "SDN:L22::TOOL1415" ;
  pav:hasCurrentVersion <http://vocab.nerc.ac.uk/collection/L22/current/TOOL1415/1> ;
  owl:versionInfo "1" ;
  skos:altLabel "Ceramic tile substrate"@en ;
  skos:broader <http://vocab.nerc.ac.uk/collection/L05/current/392> ;
  skos:definition "An artificial colonisation substrate made of ceramic tiles. It is used to determine the extent of colonisation and/or the diversity of settled organisms in a marine or artificial environment."@en ;
  skos:inScheme <http://vocab.nerc.ac.uk/scheme/SDNDEV/current> ;
  skos:notation "SDN:L22::TOOL1415" ;
  skos:note "accepted"@en ;
  skos:prefLabel "Custom-made ceramic tile settlement plate"@en ;
  skos:related <http://vocab.nerc.ac.uk/collection/B75/current/UNSPEC> ;
  skos:related <http://vocab.nerc.ac.uk/collection/L35/current/MAN0069> ;
.
inst:TOOL1416
  rdf:type skos:Concept ;
  dcterm:date "2020-04-07 16:24:48.0" ;
  dcterm:identifier "SDN:L22::TOOL1416" ;
  pav:hasCurrentVersion <http://vocab.nerc.ac.uk/collection/L22/current/TOOL1416/1> ;
  owl:versionInfo "1" ;
  skos:altLabel "Scotch-Brite PVC substrate"@en ;
  skos:broader <http://vocab.nerc.ac.uk/collection/L05/current/392> ;
  skos:definition "An artifical colonisation substrate made of a sheet of PVC covered with 3M Scotch-Brite pads of unknown material. It is used to determine the extent of colonisation and/or the diversity of settled organisms in a marine or artificial environment."@en ;
  skos:inScheme <http://vocab.nerc.ac.uk/scheme/SDNDEV/current> ;
  skos:notation "SDN:L22::TOOL1416" ;
  skos:note "accepted"@en ;
  skos:prefLabel "Custom-made 3M Scotch-Brite pad on polyvinyl chloride settlement plate"@en ;
  skos:related <http://vocab.nerc.ac.uk/collection/B75/current/UNSPEC> ;
  skos:related <http://vocab.nerc.ac.uk/collection/L35/current/MAN0069> ;
.
inst:TOOL1417
  rdf:type skos:Concept ;
  dcterm:date "2020-04-07 16:24:48.0" ;
  dcterm:identifier "SDN:L22::TOOL1417" ;
  pav:hasCurrentVersion <http://vocab.nerc.ac.uk/collection/L22/current/TOOL1417/1> ;
  owl:versionInfo "1" ;
  skos:altLabel "Grooved PVC substrate"@en ;
  skos:broader <http://vocab.nerc.ac.uk/collection/L05/current/392> ;
  skos:definition "An artificial colonisation substrate made of a sheet of PVC with engraved lines to roughen its surface. It is used to determine the extent of colonisation and/or the diversity of settled organisms in a marine or artificial environment."@en ;
  skos:inScheme <http://vocab.nerc.ac.uk/scheme/SDNDEV/current> ;
  skos:notation "SDN:L22::TOOL1417" ;
  skos:note "accepted"@en ;
  skos:prefLabel "Custom-made grooved polyvinyl chloride settlement plate"@en ;
  skos:related <http://vocab.nerc.ac.uk/collection/B75/current/UNSPEC> ;
  skos:related <http://vocab.nerc.ac.uk/collection/L35/current/MAN0069> ;
.
inst:TOOL1454
  rdf:type skos:Concept ;
  dcterm:date "2020-05-26 10:03:47.0" ;
  dcterm:identifier "SDN:L22::TOOL1454" ;
  pav:hasCurrentVersion <http://vocab.nerc.ac.uk/collection/L22/current/TOOL1454/1> ;
  owl:versionInfo "1" ;
  skos:altLabel "KUM SedimentTrap14"@en ;
  skos:broader <http://vocab.nerc.ac.uk/collection/L05/current/33> ;
  skos:definition "A device to collect particles in the water column for mooring deployments in the ocean and inland waters. It includes a multi bottle sample collection turntable for 14 samples, 14 sample bottles (400ml) and has a collection area of 0.25m2. Maximum operation: 12 months (or optional 24 months). Maximum operation depth: 3000m."@en ;
  skos:inScheme <http://vocab.nerc.ac.uk/scheme/SDNDEV/current> ;
  skos:notation "SDN:L22::TOOL1454" ;
  skos:note "accepted"@en ;
  skos:prefLabel "K.U.M. K-MT 236 (14 bottles) sediment trap"@en ;
  skos:related <http://vocab.nerc.ac.uk/collection/B75/current/ORG01535> ;
  skos:related <http://vocab.nerc.ac.uk/collection/L35/current/MAN0082> ;
.
inst:TOOL1455
  rdf:type skos:Concept ;
  dcterm:date "2020-05-26 10:03:47.0" ;
  dcterm:identifier "SDN:L22::TOOL1455" ;
  pav:hasCurrentVersion <http://vocab.nerc.ac.uk/collection/L22/current/TOOL1455/1> ;
  owl:versionInfo "1" ;
  skos:altLabel "KUM SedimentTrap21"@en ;
  skos:broader <http://vocab.nerc.ac.uk/collection/L05/current/33> ;
  skos:definition "A device to collect particles in the water column for mooring deployments in the ocean and inland waters. It includes a multi bottle sample collection turntable for 21 samples, 21 sample bottles (400ml) and has a collection area of 0.5m2. Maximum operation: 12 months (or optional 24 months). Maximum operation depth: 6000m."@en ;
  skos:inScheme <http://vocab.nerc.ac.uk/scheme/SDNDEV/current> ;
  skos:notation "SDN:L22::TOOL1455" ;
  skos:note "accepted"@en ;
  skos:prefLabel "K.U.M. K-MT 234 (21 bottles) sediment trap"@en ;
  skos:related <http://vocab.nerc.ac.uk/collection/B75/current/ORG01535> ;
  skos:related <http://vocab.nerc.ac.uk/collection/L35/current/MAN0082> ;
.
inst:TOOL1462
  rdf:type skos:Concept ;
  dcterm:date "2020-05-28 16:46:46.0" ;
  dcterm:identifier "SDN:L22::TOOL1462" ;
  pav:hasCurrentVersion <http://vocab.nerc.ac.uk/collection/L22/current/TOOL1462/1> ;
  owl:versionInfo "1" ;
  skos:altLabel "Gilson dredge"@en ;
  skos:broader <http://vocab.nerc.ac.uk/collection/L05/current/24> ;
  skos:definition "The Gilson dredge consists of a sort of plough and a net behind it. This device is pulled by a research vessel and is mostly used for sampling rough substrates, e.g. sampling of oysters and shells. The Gilson dredge is also suitable for collecting archeological artefacts but not for sampling fish."@en ;
  skos:inScheme <http://vocab.nerc.ac.uk/scheme/SDNDEV/current> ;
  skos:notation "SDN:L22::TOOL1462" ;
  skos:note "accepted"@en ;
  skos:prefLabel "Flanders Marine Institute (VLIZ) Gilson dredge"@en ;
  skos:related <http://vocab.nerc.ac.uk/collection/B75/current/ORG01061> ;
  skos:related <http://vocab.nerc.ac.uk/collection/L35/current/MAN0001> ;
.
inst:TOOL1463
  rdf:type skos:Concept ;
  dcterm:date "2020-05-28 16:52:48.0" ;
  dcterm:identifier "SDN:L22::TOOL1463" ;
  pav:hasCurrentVersion <http://vocab.nerc.ac.uk/collection/L22/current/TOOL1463/2> ;
  pav:hasVersion <http://vocab.nerc.ac.uk/collection/L22/current/TOOL1463/1> ;
  owl:versionInfo "2" ;
  skos:altLabel "HDPE bottle"@en ;
  skos:broader <http://vocab.nerc.ac.uk/collection/L05/current/30> ;
  skos:definition "A High Density Polyethylene (HDPE) water bottle. Used for surface sampling from small boats. HDPE has a somewhat higher chemical resistance than LDPE. HDPE is also somewhat harder and more opaque and it can withstand higher temperatures (120 degrees Celsius for short periods, 110 degrees Celsius continuously)."@en ;
  skos:inScheme <http://vocab.nerc.ac.uk/scheme/SDNDEV/current> ;
  skos:notation "SDN:L22::TOOL1463" ;
  skos:note "accepted"@en ;
  skos:prefLabel "High density polyethylene water bottle"@en ;
  skos:related <http://vocab.nerc.ac.uk/collection/B75/current/UNSPEC> ;
  skos:related <http://vocab.nerc.ac.uk/collection/L35/current/MAN0001> ;
.
inst:TOOL1464
  rdf:type skos:Concept ;
  dcterm:date "2020-05-28 16:46:46.0" ;
  dcterm:identifier "SDN:L22::TOOL1464" ;
  pav:hasCurrentVersion <http://vocab.nerc.ac.uk/collection/L22/current/TOOL1464/1> ;
  owl:versionInfo "1" ;
  skos:altLabel "Teflon bottle"@en ;
  skos:broader <http://vocab.nerc.ac.uk/collection/L05/current/30> ;
  skos:definition "A water sampling bottle made from Teflon, a brand of Polytetrafluoroethylene (PTFE). Used for surface sampling from small boats."@en ;
  skos:inScheme <http://vocab.nerc.ac.uk/scheme/SDNDEV/current> ;
  skos:notation "SDN:L22::TOOL1464" ;
  skos:note "accepted"@en ;
  skos:prefLabel "Teflon water bottle"@en ;
  skos:related <http://vocab.nerc.ac.uk/collection/B75/current/UNSPEC> ;
  skos:related <http://vocab.nerc.ac.uk/collection/L35/current/MAN0001> ;
.
inst:TOOL1465
  rdf:type skos:Concept ;
  dcterm:date "2020-05-28 16:46:46.0" ;
  dcterm:identifier "SDN:L22::TOOL1465" ;
  pav:hasCurrentVersion <http://vocab.nerc.ac.uk/collection/L22/current/TOOL1465/1> ;
  owl:versionInfo "1" ;
  skos:altLabel "Schott bottle"@en ;
  skos:broader <http://vocab.nerc.ac.uk/collection/L05/current/30> ;
  skos:definition "A borosilicate water sampling bottle manufactured by Schott. Used for surface sampling from small boats."@en ;
  skos:inScheme <http://vocab.nerc.ac.uk/scheme/SDNDEV/current> ;
  skos:notation "SDN:L22::TOOL1465" ;
  skos:note "accepted"@en ;
  skos:prefLabel "Schott borosilicate water bottle"@en ;
  skos:related <http://vocab.nerc.ac.uk/collection/B75/current/ORG01552> ;
  skos:related <http://vocab.nerc.ac.uk/collection/L35/current/MAN0084> ;
.
inst:TOOL1466
  rdf:type skos:Concept ;
  dcterm:date "2020-05-28 16:46:46.0" ;
  dcterm:identifier "SDN:L22::TOOL1466" ;
  pav:hasCurrentVersion <http://vocab.nerc.ac.uk/collection/L22/current/TOOL1466/1> ;
  owl:versionInfo "1" ;
  skos:altLabel "Polycarbonate bottle"@en ;
  skos:broader <http://vocab.nerc.ac.uk/collection/L05/current/30> ;
  skos:definition "A polycarbonate water sampling bottle. Used for surface sampling from small boats."@en ;
  skos:inScheme <http://vocab.nerc.ac.uk/scheme/SDNDEV/current> ;
  skos:notation "SDN:L22::TOOL1466" ;
  skos:note "accepted"@en ;
  skos:prefLabel "Polycarbonate water bottle"@en ;
  skos:related <http://vocab.nerc.ac.uk/collection/B75/current/UNSPEC> ;
  skos:related <http://vocab.nerc.ac.uk/collection/L35/current/MAN0001> ;
.
inst:TOOL1467
  rdf:type skos:Concept ;
  dcterm:date "2020-05-28 16:46:46.0" ;
  dcterm:identifier "SDN:L22::TOOL1467" ;
  pav:hasCurrentVersion <http://vocab.nerc.ac.uk/collection/L22/current/TOOL1467/1> ;
  owl:versionInfo "1" ;
  skos:altLabel "Pyrex bottle"@en ;
  skos:broader <http://vocab.nerc.ac.uk/collection/L05/current/30> ;
  skos:definition "A Pyrex water sampling bottle. Used for surface sampling from small boats."@en ;
  skos:inScheme <http://vocab.nerc.ac.uk/scheme/SDNDEV/current> ;
  skos:notation "SDN:L22::TOOL1467" ;
  skos:note "accepted"@en ;
  skos:prefLabel "Pyrex borosilicate water bottle"@en ;
  skos:related <http://vocab.nerc.ac.uk/collection/B75/current/ORG01553> ;
  skos:related <http://vocab.nerc.ac.uk/collection/L35/current/MAN0083> ;
.
inst:TOOL1468
  rdf:type skos:Concept ;
  dcterm:date "2020-06-02 14:50:38.0" ;
  dcterm:identifier "SDN:L22::TOOL1468" ;
  pav:hasCurrentVersion <http://vocab.nerc.ac.uk/collection/L22/current/TOOL1468/1> ;
  owl:versionInfo "1" ;
  skos:altLabel "TNO-NITG Geodoff flush corer"@en ;
  skos:broader <http://vocab.nerc.ac.uk/collection/L05/current/51> ;
  skos:definition "A marine sediment flush corer constructed by the Netherlands Institute of Applied Geosciences (TNO-NITG), later known as Netherlands Organization for Applied Scientific Research (TNO). It is designed to recover sediment cores from the seafloor, and uses the Geodoff counterflush system of sediment core recovery which was first developed by Conrad-Stork BV of Haarlem, Netherlands. The Geodoff flush corer utilises reversed mud flush circulation that permits uninterrupted core recovery in the rotary drilling system. It can drill into seafloor sediments to depths of approximately 20 metres, and can be operated in water depths of approximately 200 m."@en ;
  skos:inScheme <http://vocab.nerc.ac.uk/scheme/SDNDEV/current> ;
  skos:notation "SDN:L22::TOOL1468" ;
  skos:note "accepted"@en ;
  skos:prefLabel "Netherlands Institute for Applied Geosciences (TNO-NITG) Geodoff flush corer"@en ;
  skos:related <http://vocab.nerc.ac.uk/collection/B75/current/ORG01531> ;
  skos:related <http://vocab.nerc.ac.uk/collection/L35/current/MAN0086> ;
.
inst:TOOL1469
  rdf:type skos:Concept ;
  dcterm:date "2020-06-02 14:50:38.0" ;
  dcterm:identifier "SDN:L22::TOOL1469" ;
  pav:hasCurrentVersion <http://vocab.nerc.ac.uk/collection/L22/current/TOOL1469/1> ;
  owl:versionInfo "1" ;
  skos:altLabel "Reineck box corer"@en ;
  skos:broader <http://vocab.nerc.ac.uk/collection/L05/current/51> ;
  skos:definition "A marine geological tool that recovers undisturbed soft surface sediments, based on the design by Hans-Erich Reineck (1963). Also referred to as a 'spade' corer, it is designed for minimum disturbance of the sediment surface by bow wave effects. Traditionally, it consists of a weighted stem fitted to a square sampling box. The corer is lowered vertically until it impacts with the seabed. At this point the instrument is triggered by a trip as the main coring stem passes through its frame. While pulling the corer out of the sediment a spade swings underneath the sample to prevent loss. When hauled back on board, the spade is under the box."@en ;
  skos:inScheme <http://vocab.nerc.ac.uk/scheme/SDNDEV/current> ;
  skos:notation "SDN:L22::TOOL1469" ;
  skos:note "accepted"@en ;
  skos:prefLabel "Unspecified Reineck box corer"@en ;
  skos:related <http://vocab.nerc.ac.uk/collection/B75/current/UNSPEC> ;
  skos:related <http://vocab.nerc.ac.uk/collection/L35/current/MAN0001> ;
.
inst:TOOL1485
  rdf:type skos:Concept ;
  dcterm:date "2022-04-27 16:55:15.0" ;
  dcterm:identifier "SDN:L22::TOOL1485" ;
  pav:hasCurrentVersion <http://vocab.nerc.ac.uk/collection/L22/current/TOOL1485/2> ;
  pav:hasVersion <http://vocab.nerc.ac.uk/collection/L22/current/TOOL1485/1> ;
  owl:versionInfo "2" ;
  skos:altLabel "Geo-Resources Geo-Corer 3000"@en ;
  skos:broader <http://vocab.nerc.ac.uk/collection/L05/current/51> ;
  skos:definition "A high frequency (28 Hz), electrically driven vibrocoring system, with a core barrel length of 3m. It can penetrate fast (thereby enhancing the quality of the core) into all common unconsolidated sediments, including compact sands and stiff clays, and even unconsolidated chalk. The core barrel is made of stainless steel 316, and contains a PVC liner of 106 mm inner diameter and wall thickness of 2 mm. The core barrel is connected to the barrel pivot by two locking bolts - this pivotal connection allows the core barrel to be positioned horizontally for extracting the core liner. Optional pressure-compensated module(for water depths > 150 m)."@en ;
  skos:inScheme <http://vocab.nerc.ac.uk/scheme/SDNDEV/current> ;
  skos:notation "SDN:L22::TOOL1485" ;
  skos:note "accepted"@en ;
  skos:prefLabel "Geo-Resources Geo-Corer 3000 vibrocorer"@en ;
  skos:related <http://vocab.nerc.ac.uk/collection/B75/current/UNSPEC> ;
  skos:related <http://vocab.nerc.ac.uk/collection/L35/current/MAN0094> ;
.
inst:TOOL1486
  rdf:type skos:Concept ;
  dcterm:date "2020-06-30 08:47:51.0" ;
  dcterm:identifier "SDN:L22::TOOL1486" ;
  pav:hasCurrentVersion <http://vocab.nerc.ac.uk/collection/L22/current/TOOL1486/1> ;
  owl:versionInfo "1" ;
  skos:altLabel "Geo-Resources Geo-Corer 6000"@en ;
  skos:broader <http://vocab.nerc.ac.uk/collection/L05/current/51> ;
  skos:definition "A high frequency (28 Hz), electrically driven vibrocoring system, with a core barrel length of 6m. It can penetrate fast (thereby enhancing the quality of the core) into all common unconsolidated sediments, including compact sands and stiff clays, and even unconsolidated chalk. The core barrel is made of stainless steel 316, and contains a PVC liner of 106 mm inner diameter and wall thickness of 2 mm. The core barrel is connected to the barrel pivot by two locking bolts - this pivotal connection allows the core barrel to be positioned horizontally for extracting the core liner."@en ;
  skos:inScheme <http://vocab.nerc.ac.uk/scheme/SDNDEV/current> ;
  skos:notation "SDN:L22::TOOL1486" ;
  skos:note "accepted"@en ;
  skos:prefLabel "Geo-Resources Geo-Corer 6000 vibrocorer"@en ;
  skos:related <http://vocab.nerc.ac.uk/collection/B75/current/UNSPEC> ;
  skos:related <http://vocab.nerc.ac.uk/collection/L35/current/MAN0094> ;
.
inst:TOOL1487
  rdf:type skos:Concept ;
  dcterm:date "2020-06-30 08:47:51.0" ;
  dcterm:identifier "SDN:L22::TOOL1487" ;
  pav:hasCurrentVersion <http://vocab.nerc.ac.uk/collection/L22/current/TOOL1487/1> ;
  owl:versionInfo "1" ;
  skos:altLabel "Duncan Ass. Shipek"@en ;
  skos:broader <http://vocab.nerc.ac.uk/collection/L05/current/50> ;
  skos:definition "A center-pivot sampler designed to sample unconsolidated sediments from soft ooze to hard-packed silts from deep lakes and near offshore. The sampler scoops a sediment sample from the top 10cm of the seabed. It brings up virtually un- disturbed, unwashed samples to the surface from any depth. Its specialty is sampling benthic organisms living at or immediately below the water/bottom interface and sediment containing a significant population of non-sessile forms. When the grab touches the bottom, inertia from a self-contained weight releases a catch and helical springs rotate the inner half cylinder by 180 degrees. After turning, the scoop remains closed by the residual torque of the scoop spring. Because the rotation of the bucket is very rapid, its shear strength is far greater than the sediment strength, thus cutting cleanly, particularly in soft clays, muds, silts and sands. Manufactured in 316 stainless steel with a sampling area of 0.042m sq. There is the option of adding a landing table."@en ;
  skos:inScheme <http://vocab.nerc.ac.uk/scheme/SDNDEV/current> ;
  skos:notation "SDN:L22::TOOL1487" ;
  skos:note "accepted"@en ;
  skos:prefLabel "Duncan and Associates Shipek grab"@en ;
  skos:related <http://vocab.nerc.ac.uk/collection/B75/current/ORG01106> ;
  skos:related <http://vocab.nerc.ac.uk/collection/L35/current/MAN0091> ;
.
inst:TOOL1527
  rdf:type skos:Concept ;
  dcterm:date "2020-08-17 15:04:27.0" ;
  dcterm:identifier "SDN:L22::TOOL1527" ;
  pav:hasCurrentVersion <http://vocab.nerc.ac.uk/collection/L22/current/TOOL1527/1> ;
  owl:versionInfo "1" ;
  skos:altLabel "KC HAPS"@en ;
  skos:broader <http://vocab.nerc.ac.uk/collection/L05/current/51> ;
  skos:definition "A HAPS corer manufactured by KC Denmark A/S. It is a gravity corer that is designed to collect defined, undisturbed samples from hard and soft sediments. It consists of a triangular frame and a core barrel with tight top valve and core catcher to prevent porewater loss. Manufactured from AISI 316 stainless steel with electro polished surface. The sample tube is made of stainless steel (standard) but it can be delivered in transparent polycarbonate as well. In order to stabilize the HAPS in sea swells, and to sample in sandy sediments, weights can be mounted. For harder sediments a vibrator can be added."@en ;
  skos:inScheme <http://vocab.nerc.ac.uk/scheme/SDNDEV/current> ;
  skos:notation "SDN:L22::TOOL1527" ;
  skos:note "accepted"@en ;
  skos:prefLabel "KC Denmark HAPS corer"@en ;
  skos:related <http://vocab.nerc.ac.uk/collection/B75/current/ORG00909> ;
  skos:related <http://vocab.nerc.ac.uk/collection/L35/current/MAN0108> ;
.
inst:TOOL1533
  rdf:type skos:Concept ;
  dcterm:date "2020-09-01 16:16:42.0" ;
  dcterm:identifier "SDN:L22::TOOL1533" ;
  pav:hasCurrentVersion <http://vocab.nerc.ac.uk/collection/L22/current/TOOL1533/1> ;
  owl:versionInfo "1" ;
  skos:altLabel "Van Walt Ekman grab"@en ;
  skos:broader <http://vocab.nerc.ac.uk/collection/L05/current/50> ;
  skos:definition "A stainless steel sediment sampler designed to retrieve soft-sediment samples from rivers, harbours and shallow marine areas. The samples retrieved are semi-disturbed from the surface layers. The grab is lowered using an attached 30 m cable or rod. It has two spring-loaded jaws which are in the open position when lowered. The jaws are closed when a drop-weight is dropped (cable operated) or a button is pressed (rod operated). The jaws overlap once closed to prevent any loss of sample. The Ekman grab can be supplied with a 1.5m rod or cable for use in very shallow water. It has a sample volume of 3.5 litres, weighs 7 kg, and its overall dimensions are 152 x 152 x 152 mm."@en ;
  skos:inScheme <http://vocab.nerc.ac.uk/scheme/SDNDEV/current> ;
  skos:notation "SDN:L22::TOOL1533" ;
  skos:note "accepted"@en ;
  skos:prefLabel "Van Walt Ekman grab"@en ;
  skos:related <http://vocab.nerc.ac.uk/collection/B75/current/ORG01733> ;
  skos:related <http://vocab.nerc.ac.uk/collection/L35/current/MAN0110> ;
.
inst:TOOL1535
  rdf:type skos:Concept ;
  dcterm:date "2020-09-01 16:16:42.0" ;
  dcterm:identifier "SDN:L22::TOOL1535" ;
  pav:hasCurrentVersion <http://vocab.nerc.ac.uk/collection/L22/current/TOOL1535/1> ;
  owl:versionInfo "1" ;
  skos:altLabel "Ocean Ecology Dual Van Veen Grab"@en ;
  skos:broader <http://vocab.nerc.ac.uk/collection/L05/current/50> ;
  skos:definition "A simple stainless steel clam-shell sediment grab designed to retrieve sediment samples from shallow and deep waters. On descent two levers with buckets at their ends are spread like open scissors that unlock on hitting the seabed. When pulled upwards the two buckets close and grab a sample. This is subject to more disturbance than by Craib or box corers. The double grab configuration allows for more efficient sampling operation. It comes mounted to a purpose-built deck stand and galvanised seabed frame. It has a typical sampling area of approximately 0.2 m2 (10 litre capacity per bucket)."@en ;
  skos:inScheme <http://vocab.nerc.ac.uk/scheme/SDNDEV/current> ;
  skos:notation "SDN:L22::TOOL1535" ;
  skos:note "accepted"@en ;
  skos:prefLabel "Ocean Ecology Dual Van Veen Grab"@en ;
  skos:related <http://vocab.nerc.ac.uk/collection/B75/current/ORG01734> ;
  skos:related <http://vocab.nerc.ac.uk/collection/L35/current/MAN0111> ;
.
inst:TOOL1536
  rdf:type skos:Concept ;
  dcterm:date "2020-09-01 16:16:42.0" ;
  dcterm:identifier "SDN:L22::TOOL1536" ;
  pav:hasCurrentVersion <http://vocab.nerc.ac.uk/collection/L22/current/TOOL1536/1> ;
  owl:versionInfo "1" ;
  skos:altLabel "Plastic intertidal corer"@en ;
  skos:broader <http://vocab.nerc.ac.uk/collection/L05/current/51> ;
  skos:definition "A small plastic corer designed to retrieve samples from the very surface layers of shallow intertidal sediments. Samples are retrieved by pushing the corer into the sediment by hand down to a specified depth. The corer is then pulled out by hand. It has a sampling area of 0.038 m2."@en ;
  skos:inScheme <http://vocab.nerc.ac.uk/scheme/SDNDEV/current> ;
  skos:notation "SDN:L22::TOOL1536" ;
  skos:note "accepted"@en ;
  skos:prefLabel "Unspecified plastic intertidal corer"@en ;
  skos:related <http://vocab.nerc.ac.uk/collection/B75/current/UNSPEC> ;
  skos:related <http://vocab.nerc.ac.uk/collection/L35/current/MAN0001> ;
.
inst:TOOL1537
  rdf:type skos:Concept ;
  dcterm:date "2020-09-01 16:16:42.0" ;
  dcterm:identifier "SDN:L22::TOOL1537" ;
  pav:hasCurrentVersion <http://vocab.nerc.ac.uk/collection/L22/current/TOOL1537/1> ;
  owl:versionInfo "1" ;
  skos:altLabel "Stainless steel intertidal corer"@en ;
  skos:broader <http://vocab.nerc.ac.uk/collection/L05/current/51> ;
  skos:definition "A small stainless steel corer designed to retrieve samples from the very surface layers of shallow intertidal sediments. Samples are retrieved by pushing the corer into the sediment by hand down to a specified depth. The corer is then pulled out by hand. It has a sampling area of 0.01 m2."@en ;
  skos:inScheme <http://vocab.nerc.ac.uk/scheme/SDNDEV/current> ;
  skos:notation "SDN:L22::TOOL1537" ;
  skos:note "accepted"@en ;
  skos:prefLabel "Unspecified stainless steel intertidal corer"@en ;
  skos:related <http://vocab.nerc.ac.uk/collection/B75/current/UNSPEC> ;
  skos:related <http://vocab.nerc.ac.uk/collection/L35/current/MAN0001> ;
.
inst:TOOL1560
  rdf:type skos:Concept ;
  dcterm:date "2020-11-02 13:05:15.0" ;
  dcterm:identifier "SDN:L22::TOOL1560" ;
  pav:hasCurrentVersion <http://vocab.nerc.ac.uk/collection/L22/current/TOOL1560/1> ;
  owl:versionInfo "1" ;
  skos:altLabel "JPC"@en ;
  skos:broader <http://vocab.nerc.ac.uk/collection/L05/current/51> ;
  skos:definition "The Jumbo Piston Corer (JPC) is a coring system that combines a dynamically falling heavy gravity corer with an interior piston that works to expel water and draw sediment into the corer. Piston corers, like gravity corers, are generally used in areas with soft sediment, such as clay. The addition of the internal piston allows the soft sediment to be captured without significant compression or disturbance. It is launched using a rail system, and can be configured in lengths from 3m to 12m. Its head Weight is 1,180 kg, and the total system weight (Including track system) is around 11,300 kg. The system has a minimum operational depth of 50m, but its maximum operational depth is limited only by the amount of wire on ship."@en ;
  skos:inScheme <http://vocab.nerc.ac.uk/scheme/SDNDEV/current> ;
  skos:notation "SDN:L22::TOOL1560" ;
  skos:note "accepted"@en ;
  skos:prefLabel "Navy Engineering Lab (NEL) from WHOI design jumbo piston corer"@en ;
  skos:related <http://vocab.nerc.ac.uk/collection/B75/current/UNSPEC> ;
  skos:related <http://vocab.nerc.ac.uk/collection/L35/current/MAN0002> ;
.
inst:TOOL1574
  rdf:type skos:Concept ;
  dcterm:date "2020-11-23 08:44:55.0" ;
  dcterm:identifier "SDN:L22::TOOL1574" ;
  pav:hasCurrentVersion <http://vocab.nerc.ac.uk/collection/L22/current/TOOL1574/1> ;
  owl:versionInfo "1" ;
  skos:altLabel "bottom longline fishing gear"@en ;
  skos:broader <http://vocab.nerc.ac.uk/collection/L05/current/63> ;
  skos:definition "Fishing gear designed to catch demersal fish. It consists of a long mainline set horizontally and weighted to the seafloor. A series of short branch lines with baited hooks are attached at regular intervals to the mainline. The mainline is attached at both ends to downlines which have a large buoy on the surface for locating gear, and anchors at the bottom to hold the gear in place."@en ;
  skos:inScheme <http://vocab.nerc.ac.uk/scheme/SDNDEV/current> ;
  skos:notation "SDN:L22::TOOL1574" ;
  skos:note "accepted"@en ;
  skos:prefLabel "bottom longline fishing line"@en ;
  skos:related <http://vocab.nerc.ac.uk/collection/B75/current/UNSPEC> ;
  skos:related <http://vocab.nerc.ac.uk/collection/L35/current/MAN0001> ;
.
inst:TOOL1575
  rdf:type skos:Concept ;
  dcterm:date "2020-11-23 08:44:55.0" ;
  dcterm:identifier "SDN:L22::TOOL1575" ;
  pav:hasCurrentVersion <http://vocab.nerc.ac.uk/collection/L22/current/TOOL1575/1> ;
  owl:versionInfo "1" ;
  skos:altLabel "handline fishing gear"@en ;
  skos:broader <http://vocab.nerc.ac.uk/collection/L05/current/63> ;
  skos:definition "A fishing line that is held in the hands. Typically lures or baited hooks are attached to the line."@en ;
  skos:inScheme <http://vocab.nerc.ac.uk/scheme/SDNDEV/current> ;
  skos:notation "SDN:L22::TOOL1575" ;
  skos:note "accepted"@en ;
  skos:prefLabel "handheld fishing line"@en ;
  skos:related <http://vocab.nerc.ac.uk/collection/B75/current/UNSPEC> ;
  skos:related <http://vocab.nerc.ac.uk/collection/L35/current/MAN0001> ;
.
inst:TOOL1576
  rdf:type skos:Concept ;
  dcterm:date "2020-12-07 11:09:14.0" ;
  dcterm:identifier "SDN:L22::TOOL1576" ;
  pav:hasCurrentVersion <http://vocab.nerc.ac.uk/collection/L22/current/TOOL1576/1> ;
  owl:versionInfo "1" ;
  skos:altLabel "LDPE bottle"@en ;
  skos:broader <http://vocab.nerc.ac.uk/collection/L05/current/30> ;
  skos:definition "A Low Density Polyethylene (LDPE) water bottle. Used for surface sampling from small boats. Low density polyethylene bottles provide very good chemical compatibility with a wide variety of lab reagents including most acids, bases, alcohols, aldehydes, esters, and aliphatic hydrocarbons. LDPE bottles are generally more flexible than HDPE bottles."@en ;
  skos:inScheme <http://vocab.nerc.ac.uk/scheme/SDNDEV/current> ;
  skos:notation "SDN:L22::TOOL1576" ;
  skos:note "accepted"@en ;
  skos:prefLabel "Low density polyethylene water bottle"@en ;
  skos:related <http://vocab.nerc.ac.uk/collection/B75/current/UNSPEC> ;
  skos:related <http://vocab.nerc.ac.uk/collection/L35/current/MAN0001> ;
.
inst:TOOL1644
  rdf:type skos:Concept ;
  dcterm:date "2021-02-11 16:32:18.0" ;
  dcterm:identifier "SDN:L22::TOOL1644" ;
  pav:hasCurrentVersion <http://vocab.nerc.ac.uk/collection/L22/current/TOOL1644/1> ;
  owl:versionInfo "1" ;
  skos:altLabel "Jonasson and Olausson (1966) corer"@en ;
  skos:broader <http://vocab.nerc.ac.uk/collection/L05/current/51> ;
  skos:definition "A sediment gravity corer used to obtain thick, undisturbed cores of the uppermost part of the sediment layer. It can also be used as a piston corer. The device has a nose, a barrel of polyvinyl chloride (PVC), and a weight stand. The nose consists of three parts: a core cutter, a brass tube, and a core catcher. The PVC tube used, has an outside diameter of 90.4 mm and an inner diameter of 73 mm. The lower end of the PVC tube is fixed to the nose, while its upper end is attached to the weight stand. The length of the barrel used varies between 1 and 3 m."@en ;
  skos:inScheme <http://vocab.nerc.ac.uk/scheme/SDNDEV/current> ;
  skos:notation "SDN:L22::TOOL1644" ;
  skos:note "accepted"@en ;
  skos:prefLabel "Unspecified sediment corer - Jonasson and Olausson (1966)"@en ;
  skos:related <http://vocab.nerc.ac.uk/collection/B75/current/UNSPEC> ;
  skos:related <http://vocab.nerc.ac.uk/collection/L35/current/MAN0001> ;
.
inst:TOOL1654
  rdf:type skos:Concept ;
  dcterm:date "2021-03-16 16:25:16.0" ;
  dcterm:identifier "SDN:L22::TOOL1654" ;
  pav:hasCurrentVersion <http://vocab.nerc.ac.uk/collection/L22/current/TOOL1654/1> ;
  owl:versionInfo "1" ;
  skos:altLabel "UMN Gas-Tight sampler"@en ;
  skos:broader <http://vocab.nerc.ac.uk/collection/L05/current/30> ;
  skos:definition "A custom-designed gas-tight serial water sampler developed by the University of Minnesota. The system is designed for deployment at the seafloor for long-term operation to take time-series fluid samples from deep-sea environments such as cold seeps and hydrothermal vents. The serial sampler is a modular system that is based on independent and identical sampling modules, which are designed to collect six 160 ml gas-tight fluid samples maintained at high pressure to a depth of 4000 meters. With two working modes, the sampler can be deployed either as part of a seafloor cabled observatory for remote control, or as a stand-alone device for autonomous operation. The titanium housing of the system is pressure rated to 6000 m, but the gas-tight samples are only maintained at high pressures to a depth of 4000 m."@en ;
  skos:inScheme <http://vocab.nerc.ac.uk/scheme/SDNDEV/current> ;
  skos:notation "SDN:L22::TOOL1654" ;
  skos:note "accepted"@en ;
  skos:prefLabel "University of Minnesota [custom] Gas-Tight serial sampler - Wu et al. (2015)"@en ;
  skos:related <http://vocab.nerc.ac.uk/collection/B75/current/ORG00593> ;
  skos:related <http://vocab.nerc.ac.uk/collection/L35/current/MAN0056> ;
.
inst:TOOL1668
  rdf:type skos:Concept ;
  dcterm:date "2021-03-23 17:29:08.0" ;
  dcterm:identifier "SDN:L22::TOOL1668" ;
  pav:hasCurrentVersion <http://vocab.nerc.ac.uk/collection/L22/current/TOOL1668/1> ;
  owl:versionInfo "1" ;
  skos:altLabel "Technicap PPS 3-3 24S"@en ;
  skos:broader <http://vocab.nerc.ac.uk/collection/L05/current/33> ;
  skos:definition "A mooring sediment trap designed for long-term continuous deployments. It is used for the determine the flux of settling particles in-situ. It uses a funnel to collect passing settled particles into one of a set of bottles mounted on a carousel. The bottles are changed after a set period of time. It consists of a cylindro-conical funnel (collecting area of 0.125 m2) with a phenolic composite baffle (cell dia. 9.5 mm) to prevent large objects clogging the system. The trap is fitted with 24 x 250 ml or 24 x 500 ml polypropylen sampling bottles. It is capable of 18 month deployments (24 months with Lithium batteries) and has a sampling interval of 1 minute. It has a maximum operating depth of 1000 m (PETP) or 5000m (Aluminium) or 6000m (Titanium)."@en ;
  skos:inScheme <http://vocab.nerc.ac.uk/scheme/SDNDEV/current> ;
  skos:notation "SDN:L22::TOOL1668" ;
  skos:note "accepted"@en ;
  skos:prefLabel "Technicap PPS 3-3 24S sediment trap series"@en ;
  skos:related <http://vocab.nerc.ac.uk/collection/B75/current/ORG01178> ;
  skos:related <http://vocab.nerc.ac.uk/collection/L35/current/MAN0172> ;
.
inst:TOOL1703
  rdf:type skos:Concept ;
  dcterm:date "2021-06-17 16:48:16.0" ;
  dcterm:identifier "SDN:L22::TOOL1703" ;
  pav:hasCurrentVersion <http://vocab.nerc.ac.uk/collection/L22/current/TOOL1703/1> ;
  owl:versionInfo "1" ;
  skos:altLabel "HCMR gravity corer"@en ;
  skos:broader <http://vocab.nerc.ac.uk/collection/L05/current/51> ;
  skos:definition "Marine geological coring device that uses a lead weight system to penetrate the seabed and collect sediment samples. Custom-built at the Hellenic Centre for Marine Research (HCMR)."@en ;
  skos:inScheme <http://vocab.nerc.ac.uk/scheme/SDNDEV/current> ;
  skos:notation "SDN:L22::TOOL1703" ;
  skos:note "accepted"@en ;
  skos:prefLabel "Hellenic Centre for Marine Research [custom] gravity corer"@en ;
  skos:related <http://vocab.nerc.ac.uk/collection/B75/current/ORG01016> ;
  skos:related <http://vocab.nerc.ac.uk/collection/L35/current/MAN0181> ;
.
inst:TOOL1727
  rdf:type skos:Concept ;
  dcterm:date "2021-09-08 10:14:17.0" ;
  dcterm:identifier "SDN:L22::TOOL1727" ;
  pav:hasCurrentVersion <http://vocab.nerc.ac.uk/collection/L22/current/TOOL1727/1> ;
  owl:versionInfo "1" ;
  skos:altLabel "Husky 1050e"@en ;
  skos:broader <http://vocab.nerc.ac.uk/collection/L05/current/31> ;
  skos:definition "An electric operated diaphragm pump for collection of water samples. These pumps have a 1-inch (25.4 mm) connection. They are available in Aluminium, Polypropylene and Stainless Steel, and are available in 3 gearbox options: 130, 215 & 330 L/min. The maximum fluid flow is 42 gpm (158 l/min); the maximum fluid working pressure is 70 psi (4.8 bar, 0.48 MPa); maximum size of pumpable solids is 3.2 mm; and fluid displacement per cycle is 0.15 g (0.65 litre)."@en ;
  skos:inScheme <http://vocab.nerc.ac.uk/scheme/SDNDEV/current> ;
  skos:notation "SDN:L22::TOOL1727" ;
  skos:note "accepted"@en ;
  skos:prefLabel "Graco Husky 1050 E pump series"@en ;
  skos:related <http://vocab.nerc.ac.uk/collection/B75/current/ORG01830> ;
  skos:related <http://vocab.nerc.ac.uk/collection/L35/current/MAN0188> ;
.
inst:TOOL1741
  rdf:type skos:Concept ;
  dcterm:date "2021-10-28 15:59:29.0" ;
  dcterm:identifier "SDN:L22::TOOL1741" ;
  pav:hasCurrentVersion <http://vocab.nerc.ac.uk/collection/L22/current/TOOL1741/2> ;
  pav:hasVersion <http://vocab.nerc.ac.uk/collection/L22/current/TOOL1741/1> ;
  owl:versionInfo "2" ;
  skos:altLabel "KC pore-water pressing bench"@en ;
  skos:broader <http://vocab.nerc.ac.uk/collection/L05/current/52> ;
  skos:definition "The KC Pore-water pressing bench allows pore-water extraction of any kind of sediments, from sediments rich in organic material, to sandy sediments. Sediment cores are segmented and placed in the pressing house, which is closed by means of the handle on top of the house. An over-pressure is applied (fed-in) at the reduction valve and the valves of the houses in operation are opened. The resulting compression of the sediment matrix leads to expelling of the pore-water, which is sampled in containers beneath the pressing house. Operation in a glove bag prevents atmospheric contamination with, for example, oxygen, so anaerobic analysis of the pore-water is possible. The standard cylinders are made from black Polyoxymethylene (POM). However, the cylinders and all accessories are also available as AISI 316 stainless steel for special purposes. The pressing bench consists of 5 pressing houses, each 100 ml. They can hold a maximum sample diameter of 40 mm. The instrument has a maximum operating pressure of 4 bar (400 kPa)."@en ;
  skos:inScheme <http://vocab.nerc.ac.uk/scheme/SDNDEV/current> ;
  skos:notation "SDN:L22::TOOL1741" ;
  skos:note "accepted"@en ;
  skos:prefLabel "KC Denmark Research Equipment KC pore-water pressing bench sediment porewater extractor"@en ;
  skos:related <http://vocab.nerc.ac.uk/collection/B75/current/ORG00909> ;
  skos:related <http://vocab.nerc.ac.uk/collection/L35/current/MAN0108> ;
.
inst:TOOL1815
  rdf:type skos:Concept ;
  dcterm:date "2022-06-28 09:52:51.0" ;
  dcterm:identifier "SDN:L22::TOOL1815" ;
  pav:hasCurrentVersion <http://vocab.nerc.ac.uk/collection/L22/current/TOOL1815/1> ;
  owl:versionInfo "1" ;
  skos:altLabel "MANOSS"@en ;
  skos:broader <http://vocab.nerc.ac.uk/collection/L05/current/24> ;
  skos:definition "MANOSS is a manually operated suction sampler designed for sampling aquatic epibionts on hard substrates and it is manually operated by SCUBA divers. It is based on the basic design of a slurp gun, which allows for sequential pump actions to effectively scoop a certain sampling area and incorporates interchangeable sample collection pouches. It is independent from air supplies or motorised pumps and therefore compact, lightweight and easy to handle. The intake nozzle has a diameter of 4.5 cm which permits the collection of large fragments of algae or even small pebbles without blocking the valves."@en ;
  skos:inScheme <http://vocab.nerc.ac.uk/scheme/SDNDEV/current> ;
  skos:notation "SDN:L22::TOOL1815" ;
  skos:note "accepted"@en ;
  skos:prefLabel "Hellenic Centre for Marine Research - IMBBC manually operated suction sampler for hard bottom benthos - Chatzigeorgiou, G., Dailianis, T., Faulwetter, S., Pettas, M., & Arvanitidis, C. (2013)"@en ;
  skos:related <http://vocab.nerc.ac.uk/collection/B75/current/ORG01970> ;
  skos:related <http://vocab.nerc.ac.uk/collection/L35/current/MAN0181> ;
.
inst:TOOL1853
  rdf:type skos:Concept ;
  dcterm:date "2022-10-10 14:39:24.0" ;
  dcterm:identifier "SDN:L22::TOOL1853" ;
  pav:hasCurrentVersion <http://vocab.nerc.ac.uk/collection/L22/current/TOOL1853/1> ;
  owl:versionInfo "1" ;
  skos:altLabel "Unspecified Dredge"@en ;
  skos:broader <http://vocab.nerc.ac.uk/collection/L05/current/60> ;
  skos:definition "A type of sampler designed for collecting a sample of bottom substrate, usually by towing it through the substrate. It can be suitable for mud, sand, shell, and gravel substrates. Samples can be used to study benthic macroinvertebrates and algae as well as the chemistry and structure of the sediments themselves."@en ;
  skos:inScheme <http://vocab.nerc.ac.uk/scheme/SDNDEV/current> ;
  skos:notation "SDN:L22::TOOL1853" ;
  skos:note "accepted"@en ;
  skos:prefLabel "Unspecified Dredge"@en ;
  skos:related <http://vocab.nerc.ac.uk/collection/B75/current/UNSPEC> ;
  skos:related <http://vocab.nerc.ac.uk/collection/L35/current/MAN0001> ;
.
inst:TOOL1854
  rdf:type skos:Concept ;
  dcterm:date "2022-10-10 14:39:24.0" ;
  dcterm:identifier "SDN:L22::TOOL1854" ;
  pav:hasCurrentVersion <http://vocab.nerc.ac.uk/collection/L22/current/TOOL1854/1> ;
  owl:versionInfo "1" ;
  skos:altLabel "Unspecified Anchor Dredge"@en ;
  skos:broader <http://vocab.nerc.ac.uk/collection/L05/current/60> ;
  skos:definition "A type of dredge sampler developed to sample deep burrowing animals. It is not towed but digs in, and is released, in the manner of an anchor."@en ;
  skos:inScheme <http://vocab.nerc.ac.uk/scheme/SDNDEV/current> ;
  skos:notation "SDN:L22::TOOL1854" ;
  skos:note "accepted"@en ;
  skos:prefLabel "Unspecified Anchor Dredge"@en ;
  skos:related <http://vocab.nerc.ac.uk/collection/B75/current/UNSPEC> ;
  skos:related <http://vocab.nerc.ac.uk/collection/L35/current/MAN0001> ;
.
inst:TOOLZZZ
  rdf:type skos:Concept ;
  dcterm:date "2009-11-26 12:14:36.0" ;
  dcterm:identifier "SDN:L22::TOOLZZZ" ;
  pav:hasCurrentVersion <http://vocab.nerc.ac.uk/collection/L22/current/TOOLZZZ/1> ;
  owl:versionInfo "1" ;
  skos:altLabel "unknown"@en ;
  skos:broader <http://vocab.nerc.ac.uk/collection/L05/current/999> ;
  skos:definition "The correct value is not known to, and not computable by, the creator of this information. However, a correct value probably exists."@en ;
  skos:inScheme <http://vocab.nerc.ac.uk/scheme/SDNDEV/current> ;
  skos:notation "SDN:L22::TOOLZZZ" ;
  skos:note "accepted"@en ;
  skos:prefLabel "unknown"@en ;
.
inst:seavoxdevicecatalog
  rdf:type skos:Collection ;
  dcterm:alternative "SeaVoX Device Catalogue" ;
  dcterm:creator "SeaDataNet and MarineXML Vocabulary Content Governance Group" ;
  dcterm:date "2023-03-07 02:00:03.0" ;
  dcterm:description "Terms for distinct sampling or measuring devices that may be identified in the real world in terms of manufacturer and model number." ;
  dcterm:license <https://creativecommons.org/licenses/by/4.0> ;
  dcterm:publisher "Natural Environment Research Council" ;
  dcterm:title "SeaVoX Device Catalogue" ;
  grg:RE_RegisterManager "British Oceanographic Data Centre" ;
  grg:RE_RegisterOwner "SeaDataNet and MarineXML Vocabulary Content Governance Group" ;
  rdfs:comment "Group set up under the joint auspices of the SeaDataNet project and the Intergovernmental Oceanographic Commission MarineXML Steering Group for controlled vocabulary governance in the marine domain" ;
  rdfs:seeAlso <https://github.com/nvs-vocabs/L22> ;
  owl:versionInfo "613" ;
  skos:altLabel "SeaVoX Device Catalogue" ;
  skos:member inst:NETT0001 ;
  skos:member inst:NETT0002 ;
  skos:member inst:NETT0003 ;
  skos:member inst:NETT0005 ;
  skos:member inst:NETT0006 ;
  skos:member inst:NETT0009 ;
  skos:member inst:NETT0010 ;
  skos:member inst:NETT0012 ;
  skos:member inst:NETT0016 ;
  skos:member inst:NETT0019 ;
  skos:member inst:NETT0020 ;
  skos:member inst:NETT0022 ;
  skos:member inst:NETT0023 ;
  skos:member inst:NETT0024 ;
  skos:member inst:NETT0026 ;
  skos:member inst:NETT0027 ;
  skos:member inst:NETT0030 ;
  skos:member inst:NETT0031 ;
  skos:member inst:NETT0032 ;
  skos:member inst:NETT0034 ;
  skos:member inst:NETT0035 ;
  skos:member inst:NETT0036 ;
  skos:member inst:NETT0039 ;
  skos:member inst:NETT0040 ;
  skos:member inst:NETT0041 ;
  skos:member inst:NETT0042 ;
  skos:member inst:NETT0043 ;
  skos:member inst:NETT0044 ;
  skos:member inst:NETT0045 ;
  skos:member inst:NETT0047 ;
  skos:member inst:NETT0052 ;
  skos:member inst:NETT0053 ;
  skos:member inst:NETT0054 ;
  skos:member inst:NETT0055 ;
  skos:member inst:NETT0056 ;
  skos:member inst:NETT0057 ;
  skos:member inst:NETT0058 ;
  skos:member inst:NETT0059 ;
  skos:member inst:NETT0060 ;
  skos:member inst:NETT0061 ;
  skos:member inst:NETT0062 ;
  skos:member inst:NETT0063 ;
  skos:member inst:NETT0065 ;
  skos:member inst:NETT0066 ;
  skos:member inst:NETT0067 ;
  skos:member inst:NETT0068 ;
  skos:member inst:NETT0071 ;
  skos:member inst:NETT0072 ;
  skos:member inst:NETT0073 ;
  skos:member inst:NETT0074 ;
  skos:member inst:NETT0075 ;
  skos:member inst:NETT0077 ;
  skos:member inst:NETT0078 ;
  skos:member inst:NETT0079 ;
  skos:member inst:NETT0080 ;
  skos:member inst:NETT0090 ;
  skos:member inst:NETT0091 ;
  skos:member inst:NETT0092 ;
  skos:member inst:NETT0095 ;
  skos:member inst:NETT0096 ;
  skos:member inst:NETT0098 ;
  skos:member inst:NETT0100 ;
  skos:member inst:NETT0102 ;
  skos:member inst:NETT0103 ;
  skos:member inst:NETT0104 ;
  skos:member inst:NETT0105 ;
  skos:member inst:NETT0106 ;
  skos:member inst:NETT0108 ;
  skos:member inst:NETT0109 ;
  skos:member inst:NETT0111 ;
  skos:member inst:NETT0112 ;
  skos:member inst:NETT0113 ;
  skos:member inst:NETT0114 ;
  skos:member inst:NETT0115 ;
  skos:member inst:NETT0116 ;
  skos:member inst:NETT0118 ;
  skos:member inst:NETT0122 ;
  skos:member inst:NETT0124 ;
  skos:member inst:NETT0125 ;
  skos:member inst:NETT0126 ;
  skos:member inst:NETT0127 ;
  skos:member inst:NETT0128 ;
  skos:member inst:NETT0129 ;
  skos:member inst:NETT0131 ;
  skos:member inst:NETT0132 ;
  skos:member inst:NETT0133 ;
  skos:member inst:NETT0134 ;
  skos:member inst:NETT0135 ;
  skos:member inst:NETT0136 ;
  skos:member inst:NETT0137 ;
  skos:member inst:NETT0138 ;
  skos:member inst:NETT0139 ;
  skos:member inst:NETT0140 ;
  skos:member inst:NETT0141 ;
  skos:member inst:NETT0142 ;
  skos:member inst:NETT0143 ;
  skos:member inst:NETT0144 ;
  skos:member inst:NETT0145 ;
  skos:member inst:NETT0147 ;
  skos:member inst:NETT0150 ;
  skos:member inst:NETT0151 ;
  skos:member inst:NETT0153 ;
  skos:member inst:NETT0154 ;
  skos:member inst:NETT0155 ;
  skos:member inst:NETT0161 ;
  skos:member inst:NETT0162 ;
  skos:member inst:NETT0163 ;
  skos:member inst:NETT0164 ;
  skos:member inst:NETT0165 ;
  skos:member inst:NETT0166 ;
  skos:member inst:NETT0167 ;
  skos:member inst:NETT0169 ;
  skos:member inst:NETT0171 ;
  skos:member inst:NETT0173 ;
  skos:member inst:NETT0174 ;
  skos:member inst:NETT0175 ;
  skos:member inst:NETT0176 ;
  skos:member inst:NETT0177 ;
  skos:member inst:NETT0178 ;
  skos:member inst:NETT0179 ;
  skos:member inst:NETT0180 ;
  skos:member inst:NETT0181 ;
  skos:member inst:NETT0182 ;
  skos:member inst:NETT0183 ;
  skos:member inst:NETT0184 ;
  skos:member inst:NETT0186 ;
  skos:member inst:NETT0188 ;
  skos:member inst:NETT0189 ;
  skos:member inst:NETT0190 ;
  skos:member inst:NETT0191 ;
  skos:member inst:NETT0192 ;
  skos:member inst:NETT0193 ;
  skos:member inst:NETT0194 ;
  skos:member inst:NETT0195 ;
  skos:member inst:NETT0196 ;
  skos:member inst:NETT0197 ;
  skos:member inst:NETT0198 ;
  skos:member inst:NETT0199 ;
  skos:member inst:NETT0200 ;
  skos:member inst:NETT0201 ;
  skos:member inst:NETT0202 ;
  skos:member inst:TOOL000X ;
  skos:member inst:TOOL0078 ;
  skos:member inst:TOOL0199 ;
  skos:member inst:TOOL0235 ;
  skos:member inst:TOOL0236 ;
  skos:member inst:TOOL0248 ;
  skos:member inst:TOOL0304 ;
  skos:member inst:TOOL0313 ;
  skos:member inst:TOOL0337 ;
  skos:member inst:TOOL0348 ;
  skos:member inst:TOOL0349 ;
  skos:member inst:TOOL0353 ;
  skos:member inst:TOOL0354 ;
  skos:member inst:TOOL0355 ;
  skos:member inst:TOOL0356 ;
  skos:member inst:TOOL0357 ;
  skos:member inst:TOOL0358 ;
  skos:member inst:TOOL0359 ;
  skos:member inst:TOOL0381 ;
  skos:member inst:TOOL0388 ;
  skos:member inst:TOOL0389 ;
  skos:member inst:TOOL0390 ;
  skos:member inst:TOOL0391 ;
  skos:member inst:TOOL0412 ;
  skos:member inst:TOOL0413 ;
  skos:member inst:TOOL0418 ;
  skos:member inst:TOOL0420 ;
  skos:member inst:TOOL0427 ;
  skos:member inst:TOOL0457 ;
  skos:member inst:TOOL0469 ;
  skos:member inst:TOOL0472 ;
  skos:member inst:TOOL0482 ;
  skos:member inst:TOOL0491 ;
  skos:member inst:TOOL0500 ;
  skos:member inst:TOOL0501 ;
  skos:member inst:TOOL0502 ;
  skos:member inst:TOOL0503 ;
  skos:member inst:TOOL0504 ;
  skos:member inst:TOOL0505 ;
  skos:member inst:TOOL0506 ;
  skos:member inst:TOOL0507 ;
  skos:member inst:TOOL0508 ;
  skos:member inst:TOOL0524 ;
  skos:member inst:TOOL0535 ;
  skos:member inst:TOOL0536 ;
  skos:member inst:TOOL0537 ;
  skos:member inst:TOOL0538 ;
  skos:member inst:TOOL0539 ;
  skos:member inst:TOOL0540 ;
  skos:member inst:TOOL0541 ;
  skos:member inst:TOOL0542 ;
  skos:member inst:TOOL0543 ;
  skos:member inst:TOOL0544 ;
  skos:member inst:TOOL0545 ;
  skos:member inst:TOOL0546 ;
  skos:member inst:TOOL0547 ;
  skos:member inst:TOOL0548 ;
  skos:member inst:TOOL0550 ;
  skos:member inst:TOOL0551 ;
  skos:member inst:TOOL0552 ;
  skos:member inst:TOOL0553 ;
  skos:member inst:TOOL0554 ;
  skos:member inst:TOOL0555 ;
  skos:member inst:TOOL0556 ;
  skos:member inst:TOOL0557 ;
  skos:member inst:TOOL0561 ;
  skos:member inst:TOOL0562 ;
  skos:member inst:TOOL0563 ;
  skos:member inst:TOOL0567 ;
  skos:member inst:TOOL0571 ;
  skos:member inst:TOOL0573 ;
  skos:member inst:TOOL0588 ;
  skos:member inst:TOOL0601 ;
  skos:member inst:TOOL0623 ;
  skos:member inst:TOOL0651 ;
  skos:member inst:TOOL0652 ;
  skos:member inst:TOOL0653 ;
  skos:member inst:TOOL0660 ;
  skos:member inst:TOOL0695 ;
  skos:member inst:TOOL0698 ;
  skos:member inst:TOOL0702 ;
  skos:member inst:TOOL0703 ;
  skos:member inst:TOOL0722 ;
  skos:member inst:TOOL0723 ;
  skos:member inst:TOOL0735 ;
  skos:member inst:TOOL0742 ;
  skos:member inst:TOOL0743 ;
  skos:member inst:TOOL0751 ;
  skos:member inst:TOOL0753 ;
  skos:member inst:TOOL0758 ;
  skos:member inst:TOOL0759 ;
  skos:member inst:TOOL0760 ;
  skos:member inst:TOOL0761 ;
  skos:member inst:TOOL0762 ;
  skos:member inst:TOOL0763 ;
  skos:member inst:TOOL0764 ;
  skos:member inst:TOOL0765 ;
  skos:member inst:TOOL0766 ;
  skos:member inst:TOOL0767 ;
  skos:member inst:TOOL0768 ;
  skos:member inst:TOOL0769 ;
  skos:member inst:TOOL0784 ;
  skos:member inst:TOOL0785 ;
  skos:member inst:TOOL0786 ;
  skos:member inst:TOOL0787 ;
  skos:member inst:TOOL0788 ;
  skos:member inst:TOOL0792 ;
  skos:member inst:TOOL0798 ;
  skos:member inst:TOOL0799 ;
  skos:member inst:TOOL0800 ;
  skos:member inst:TOOL0801 ;
  skos:member inst:TOOL0802 ;
  skos:member inst:TOOL0803 ;
  skos:member inst:TOOL0806 ;
  skos:member inst:TOOL0807 ;
  skos:member inst:TOOL0817 ;
  skos:member inst:TOOL0818 ;
  skos:member inst:TOOL0819 ;
  skos:member inst:TOOL0828 ;
  skos:member inst:TOOL0833 ;
  skos:member inst:TOOL0843 ;
  skos:member inst:TOOL0862 ;
  skos:member inst:TOOL0882 ;
  skos:member inst:TOOL0885 ;
  skos:member inst:TOOL0899 ;
  skos:member inst:TOOL0900 ;
  skos:member inst:TOOL0912 ;
  skos:member inst:TOOL0917 ;
  skos:member inst:TOOL0926 ;
  skos:member inst:TOOL0933 ;
  skos:member inst:TOOL0934 ;
  skos:member inst:TOOL0935 ;
  skos:member inst:TOOL0936 ;
  skos:member inst:TOOL0939 ;
  skos:member inst:TOOL0940 ;
  skos:member inst:TOOL0960 ;
  skos:member inst:TOOL0961 ;
  skos:member inst:TOOL0962 ;
  skos:member inst:TOOL0963 ;
  skos:member inst:TOOL0978 ;
  skos:member inst:TOOL0979 ;
  skos:member inst:TOOL0980 ;
  skos:member inst:TOOL0981 ;
  skos:member inst:TOOL0982 ;
  skos:member inst:TOOL0983 ;
  skos:member inst:TOOL0984 ;
  skos:member inst:TOOL0985 ;
  skos:member inst:TOOL0986 ;
  skos:member inst:TOOL0987 ;
  skos:member inst:TOOL0988 ;
  skos:member inst:TOOL0989 ;
  skos:member inst:TOOL0990 ;
  skos:member inst:TOOL0991 ;
  skos:member inst:TOOL0992 ;
  skos:member inst:TOOL0993 ;
  skos:member inst:TOOL0994 ;
  skos:member inst:TOOL0995 ;
  skos:member inst:TOOL0996 ;
  skos:member inst:TOOL0997 ;
  skos:member inst:TOOL1012 ;
  skos:member inst:TOOL1034 ;
  skos:member inst:TOOL1042 ;
  skos:member inst:TOOL1049 ;
  skos:member inst:TOOL1052 ;
  skos:member inst:TOOL1053 ;
  skos:member inst:TOOL1054 ;
  skos:member inst:TOOL1058 ;
  skos:member inst:TOOL1063 ;
  skos:member inst:TOOL1067 ;
  skos:member inst:TOOL1068 ;
  skos:member inst:TOOL1084 ;
  skos:member inst:TOOL1085 ;
  skos:member inst:TOOL1090 ;
  skos:member inst:TOOL1091 ;
  skos:member inst:TOOL1111 ;
  skos:member inst:TOOL1135 ;
  skos:member inst:TOOL1165 ;
  skos:member inst:TOOL1166 ;
  skos:member inst:TOOL1169 ;
  skos:member inst:TOOL1170 ;
  skos:member inst:TOOL1171 ;
  skos:member inst:TOOL1172 ;
  skos:member inst:TOOL1173 ;
  skos:member inst:TOOL1174 ;
  skos:member inst:TOOL1175 ;
  skos:member inst:TOOL1176 ;
  skos:member inst:TOOL1177 ;
  skos:member inst:TOOL1178 ;
  skos:member inst:TOOL1179 ;
  skos:member inst:TOOL1181 ;
  skos:member inst:TOOL1191 ;
  skos:member inst:TOOL1199 ;
  skos:member inst:TOOL1204 ;
  skos:member inst:TOOL1214 ;
  skos:member inst:TOOL1215 ;
  skos:member inst:TOOL1216 ;
  skos:member inst:TOOL1227 ;
  skos:member inst:TOOL1228 ;
  skos:member inst:TOOL1235 ;
  skos:member inst:TOOL1249 ;
  skos:member inst:TOOL1252 ;
  skos:member inst:TOOL1253 ;
  skos:member inst:TOOL1259 ;
  skos:member inst:TOOL1260 ;
  skos:member inst:TOOL1261 ;
  skos:member inst:TOOL1272 ;
  skos:member inst:TOOL1274 ;
  skos:member inst:TOOL1280 ;
  skos:member inst:TOOL1285 ;
  skos:member inst:TOOL1299 ;
  skos:member inst:TOOL1304 ;
  skos:member inst:TOOL1326 ;
  skos:member inst:TOOL1339 ;
  skos:member inst:TOOL1348 ;
  skos:member inst:TOOL1371 ;
  skos:member inst:TOOL1372 ;
  skos:member inst:TOOL1373 ;
  skos:member inst:TOOL1374 ;
  skos:member inst:TOOL1375 ;
  skos:member inst:TOOL1376 ;
  skos:member inst:TOOL1378 ;
  skos:member inst:TOOL1379 ;
  skos:member inst:TOOL1405 ;
  skos:member inst:TOOL1413 ;
  skos:member inst:TOOL1414 ;
  skos:member inst:TOOL1415 ;
  skos:member inst:TOOL1416 ;
  skos:member inst:TOOL1417 ;
  skos:member inst:TOOL1433 ;
  skos:member inst:TOOL1434 ;
  skos:member inst:TOOL1435 ;
  skos:member inst:TOOL1446 ;
  skos:member inst:TOOL1454 ;
  skos:member inst:TOOL1455 ;
  skos:member inst:TOOL1462 ;
  skos:member inst:TOOL1463 ;
  skos:member inst:TOOL1464 ;
  skos:member inst:TOOL1465 ;
  skos:member inst:TOOL1466 ;
  skos:member inst:TOOL1467 ;
  skos:member inst:TOOL1468 ;
  skos:member inst:TOOL1469 ;
  skos:member inst:TOOL1477 ;
  skos:member inst:TOOL1478 ;
  skos:member inst:TOOL1480 ;
  skos:member inst:TOOL1485 ;
  skos:member inst:TOOL1486 ;
  skos:member inst:TOOL1487 ;
  skos:member inst:TOOL1521 ;
  skos:member inst:TOOL1524 ;
  skos:member inst:TOOL1527 ;
  skos:member inst:TOOL1533 ;
  skos:member inst:TOOL1535 ;
  skos:member inst:TOOL1536 ;
  skos:member inst:TOOL1537 ;
  skos:member inst:TOOL1547 ;
  skos:member inst:TOOL1553 ;
  skos:member inst:TOOL1554 ;
  skos:member inst:TOOL1560 ;
  skos:member inst:TOOL1574 ;
  skos:member inst:TOOL1575 ;
  skos:member inst:TOOL1576 ;
  skos:member inst:TOOL1606 ;
  skos:member inst:TOOL1621 ;
  skos:member inst:TOOL1623 ;
  skos:member inst:TOOL1636 ;
  skos:member inst:TOOL1637 ;
  skos:member inst:TOOL1644 ;
  skos:member inst:TOOL1654 ;
  skos:member inst:TOOL1668 ;
  skos:member inst:TOOL1684 ;
  skos:member inst:TOOL1697 ;
  skos:member inst:TOOL1698 ;
  skos:member inst:TOOL1699 ;
  skos:member inst:TOOL1703 ;
  skos:member inst:TOOL1709 ;
  skos:member inst:TOOL1727 ;
  skos:member inst:TOOL1734 ;
  skos:member inst:TOOL1741 ;
  skos:member inst:TOOL1755 ;
  skos:member inst:TOOL1756 ;
  skos:member inst:TOOL1757 ;
  skos:member inst:TOOL1790 ;
  skos:member inst:TOOL1791 ;
  skos:member inst:TOOL1815 ;
  skos:member inst:TOOL1820 ;
  skos:member inst:TOOL1823 ;
  skos:member inst:TOOL1848 ;
  skos:member inst:TOOL1853 ;
  skos:member inst:TOOL1854 ;
  skos:member inst:TOOL1857 ;
  skos:member inst:TOOL1858 ;
  skos:member inst:TOOL1859 ;
  skos:member inst:TOOL1860 ;
  skos:member inst:TOOL1861 ;
  skos:member inst:TOOL1873 ;
  skos:member inst:TOOL1879 ;
  skos:member inst:TOOL1899 ;
  skos:member inst:TOOLZZZ ;
  skos:prefLabel "SeaVoX Device Catalogue" ;
.
<http://vocab.nerc.ac.uk/scheme/EDMED_DCAT_THEMES/current>
  rdf:type skos:ConceptScheme ;
  dcterm:creator "SeaDataNet" ;
  dcterm:date "2023-01-04 02:00:08.0" ;
  dcterm:description "A SKOS concept scheme to allow the representation of the SeaDataNet EDMED catalogue as Linked Data following the W3C DCAT profile." ;
  dcterm:publisher "Natural Environment Research Council" ;
  dcterm:title "W3C DCAT Themes for the SeaDataNet EDMED Catalogue" ;
  owl:versionInfo "24" ;
  skos:altLabel "EDMED DCAT themes" ;
  skos:hasTopConcept <http://vocab.nerc.ac.uk/collection/D01/current/D0100001> ;
  skos:hasTopConcept <http://vocab.nerc.ac.uk/collection/D01/current/D0100002> ;
  skos:hasTopConcept <http://vocab.nerc.ac.uk/collection/D01/current/D0100003> ;
  skos:hasTopConcept <http://vocab.nerc.ac.uk/collection/D01/current/D0100004> ;
  skos:hasTopConcept <http://vocab.nerc.ac.uk/collection/D01/current/D0100005> ;
  skos:prefLabel "W3C DCAT Themes for the SeaDataNet EDMED Catalogue" ;
.
<http://vocab.nerc.ac.uk/scheme/NETMAR_OCEAN/current>
  rdf:type skos:ConceptScheme ;
  dcterm:creator "NETMAR Ontology Governance Group" ;
  dcterm:date "2023-02-04 02:00:09.0" ;
  dcterm:description "Thesaurus centred on parameter descriptions from the BODC PUV and CF Standard Names mapping to parameter discovery, units, instrument, platform, project and coverage concepts.  Underpins discovery and semantic service chain validation for the NETMAR sea ice and oceanography pilots." ;
  dcterm:publisher "Natural Environment Research Council" ;
  dcterm:title "NETMAR Oceanography Thesaurus" ;
  owl:versionInfo "91" ;
  skos:altLabel "NETMAR Oceans" ;
  skos:hasTopConcept sdnk:SDNKG02 ;
  skos:hasTopConcept sdnk:SDNKG04 ;
  skos:hasTopConcept sdnk:SDNKG05 ;
  skos:hasTopConcept sdnk:SDNKG16 ;
  skos:prefLabel "NETMAR Oceanography Thesaurus" ;
.
<http://vocab.nerc.ac.uk/scheme/NETOC_INSTRUMENT/current>
  rdf:type skos:ConceptScheme ;
  dcterm:creator "NETMAR Ontology Governance Group" ;
  dcterm:date "2020-09-18 15:00:10.0" ;
  dcterm:description "Instrument facet of a thesaurus centred on parameter descriptions from the BODC PUV and CF Standard Names mapping to parameter discovery, units, instrument, platform, project and coverage concepts.  Underpins discovery and semantic service chain validation for the NETMAR sea ice and oceanography pilots." ;
  dcterm:publisher "Natural Environment Research Council" ;
  dcterm:title "NETMAR Oceanography Thesaurus Instrument Facet" ;
  owl:versionInfo "10" ;
  skos:altLabel "NETMAR Oceans Instrument" ;
  skos:prefLabel "NETMAR Oceanography Thesaurus Instrument Facet" ;
.
<http://vocab.nerc.ac.uk/scheme/NETOC_ORTHO/current>
  rdf:type skos:ConceptScheme ;
  dcterm:creator "NETMAR Ontology Governance Group" ;
  dcterm:date "2022-12-03 02:00:06.0" ;
  dcterm:description "Linking concepts and concepts external to the NVS of a thesaurus centred on parameter descriptions from the BODC PUV and CF Standard Names mapping to parameter discovery, units, instrument, platform, project and coverage concepts.  Underpins discovery and semantic service chain validation for the NETMAR sea ice and oceanography pilots." ;
  dcterm:publisher "Natural Environment Research Council" ;
  dcterm:title "NETMAR Oceanography Thesaurus Facet linkages and external concepts" ;
  owl:versionInfo "15" ;
  skos:altLabel "NETMAR Oceans Orthogonal" ;
  skos:prefLabel "NETMAR Oceanography Thesaurus Facet linkages and external concepts" ;
.
<http://vocab.nerc.ac.uk/scheme/NETOC_PARAM/current>
  rdf:type skos:ConceptScheme ;
  dcterm:creator "NETMAR Ontology Governance Group" ;
  dcterm:date "2023-02-04 02:00:09.0" ;
  dcterm:description "Parameter facet of a thesaurus centred on parameter descriptions from the BODC PUV and CF Standard Names mapping to parameter discovery, units, instrument, platform, project and coverage concepts.  Underpins discovery and semantic service chain validation for the NETMAR sea ice and oceanography pilots." ;
  dcterm:publisher "Natural Environment Research Council" ;
  dcterm:title "NETMAR Oceanography Thesaurus Parameter Facet" ;
  owl:versionInfo "70" ;
  skos:altLabel "NETMAR Oceans Parameter" ;
  skos:prefLabel "NETMAR Oceanography Thesaurus Parameter Facet" ;
.
<http://vocab.nerc.ac.uk/scheme/SDNDEV/current>
  rdf:type skos:ConceptScheme ;
  dcterm:creator "SeaDataNet" ;
  dcterm:date "2023-03-09 02:00:06.0" ;
  dcterm:description "A thesarus comprising categorisations of devices (sensors, instrument packages and sample collectors) developed by SeaDataNet mapped to a catalogue of specific devices maintained by SeaVoX." ;
  dcterm:publisher "Natural Environment Research Council" ;
  dcterm:title "SeaDataNet Device Thesaurus" ;
  owl:versionInfo "541" ;
  skos:altLabel "Devices" ;
  skos:hasTopConcept sdnc:ICAT01 ;
  skos:prefLabel "SeaDataNet Device Thesaurus" ;
.
<http://w3id.org/def/nerc/discipline-P08/collection>

  rdf:type skos:Collection ;
  dcterm:alternative "SeaDataNet Disciplines" ;
  dcterm:creator "SeaDataNet" ;
  dcterm:date "2017-02-03 02:00:03.0" ;
  dcterm:description "Terms used to classify SeaDataNet Agreed Parameter Groups to provide topic/theme level terms in a hierarchical parameter discovery interface." ;
  dcterm:license <https://creativecommons.org/licenses/by/4.0> ;
  dcterm:publisher "Natural Environment Research Council" ;
  dcterm:title "SeaDataNet Parameter Disciplines" ;
  grg:RE_RegisterManager "British Oceanographic Data Centre" ;
  grg:RE_RegisterOwner "SeaDataNet" ;
  rdfs:comment "Governance for vocabularies used in the EU SeaDataNet project implemented as consultation between BODC and the members of the SeaDataNet Technical Task Team" ;
  owl:imports <http://www.w3.org/2004/02/skos/core> ;
  owl:versionInfo "5" ;
  skos:altLabel "SeaDataNet Disciplines" ;
  skos:member dspl:DS06 ;
  skos:member dspl:DS07 ;
  skos:member dspl:DS08 ;
  skos:member dspl:DS12 ;
  skos:prefLabel "SeaDataNet Parameter Disciplines" ;
.
<http://w3id.org/def/nerc/instrument-L05/collection>

  rdf:type skos:Collection ;
  <http://purl.org/dc/terms/:alternative> "SDN devices" ;
  <http://purl.org/dc/terms/:creator> "SeaDataNet" ;
  <http://purl.org/dc/terms/:description> "Terms used to classify groups of sensors, instruments, sources of algorithmically computed data (numerical models) or samplers (collectors of water, SPM, sediment, rock, air or biota samples)." ;
  <http://purl.org/dc/terms/:license> <https://creativecommons.org/licenses/by/4.0/> ;
  <http://purl.org/dc/terms/:publisher> "Natural Environment Research Council" ;
  <http://purl.org/dc/terms/:title> "SeaDataNet device categories" ;
  dcterm:date "2023-02-17 02:00:01.0" ;
  grg:RE_RegisterManager "British Oceanographic Data Centre" ;
  grg:RE_RegisterOwner "SeaDataNet" ;
  rdfs:comment "Governance for vocabularies used in the EU SeaDataNet project implemented as consultation between BODC and the members of the SeaDataNet Technical Task Team" ;
  rdfs:seeAlso <https://github.com/nvs-vocabs/L05> ;
  owl:imports <http://w3id.org/def/nerc/sdncategories-L21/conceptscheme> ;
  owl:imports <http://w3id.org/def/nerc/seadatanetdatacat/collection> ;
  owl:imports <http://www.w3.org/2004/02/skos/core> ;
  owl:versionInfo "86" ;
  skos:altLabel "SDN devices" ;
  skos:historyNote "original URI http://vocab.nerc.ac.uk/collection/L05/current/, SMR change to put instrument vocabs together"@en ;
  skos:member <http://vocab.nerc.ac.uk/collection/L05/current/101> ;
  skos:member <http://vocab.nerc.ac.uk/collection/L05/current/103> ;
  skos:member <http://vocab.nerc.ac.uk/collection/L05/current/11> ;
  skos:member <http://vocab.nerc.ac.uk/collection/L05/current/110> ;
  skos:member <http://vocab.nerc.ac.uk/collection/L05/current/111> ;
  skos:member <http://vocab.nerc.ac.uk/collection/L05/current/112> ;
  skos:member <http://vocab.nerc.ac.uk/collection/L05/current/113> ;
  skos:member <http://vocab.nerc.ac.uk/collection/L05/current/114> ;
  skos:member <http://vocab.nerc.ac.uk/collection/L05/current/115> ;
  skos:member <http://vocab.nerc.ac.uk/collection/L05/current/116> ;
  skos:member <http://vocab.nerc.ac.uk/collection/L05/current/12> ;
  skos:member <http://vocab.nerc.ac.uk/collection/L05/current/122> ;
  skos:member <http://vocab.nerc.ac.uk/collection/L05/current/123> ;
  skos:member <http://vocab.nerc.ac.uk/collection/L05/current/13> ;
  skos:member <http://vocab.nerc.ac.uk/collection/L05/current/130> ;
  skos:member <http://vocab.nerc.ac.uk/collection/L05/current/131> ;
  skos:member <http://vocab.nerc.ac.uk/collection/L05/current/133> ;
  skos:member <http://vocab.nerc.ac.uk/collection/L05/current/135> ;
  skos:member <http://vocab.nerc.ac.uk/collection/L05/current/14> ;
  skos:member <http://vocab.nerc.ac.uk/collection/L05/current/150> ;
  skos:member <http://vocab.nerc.ac.uk/collection/L05/current/152> ;
  skos:member <http://vocab.nerc.ac.uk/collection/L05/current/155> ;
  skos:member <http://vocab.nerc.ac.uk/collection/L05/current/156> ;
  skos:member <http://vocab.nerc.ac.uk/collection/L05/current/157> ;
  skos:member <http://vocab.nerc.ac.uk/collection/L05/current/158> ;
  skos:member <http://vocab.nerc.ac.uk/collection/L05/current/159> ;
  skos:member <http://vocab.nerc.ac.uk/collection/L05/current/181> ;
  skos:member <http://vocab.nerc.ac.uk/collection/L05/current/182> ;
  skos:member <http://vocab.nerc.ac.uk/collection/L05/current/183> ;
  skos:member <http://vocab.nerc.ac.uk/collection/L05/current/184> ;
  skos:member <http://vocab.nerc.ac.uk/collection/L05/current/185> ;
  skos:member <http://vocab.nerc.ac.uk/collection/L05/current/21> ;
  skos:member <http://vocab.nerc.ac.uk/collection/L05/current/22> ;
  skos:member <http://vocab.nerc.ac.uk/collection/L05/current/23> ;
  skos:member <http://vocab.nerc.ac.uk/collection/L05/current/24> ;
  skos:member <http://vocab.nerc.ac.uk/collection/L05/current/30> ;
  skos:member <http://vocab.nerc.ac.uk/collection/L05/current/303> ;
  skos:member <http://vocab.nerc.ac.uk/collection/L05/current/31> ;
  skos:member <http://vocab.nerc.ac.uk/collection/L05/current/312> ;
  skos:member <http://vocab.nerc.ac.uk/collection/L05/current/313> ;
  skos:member <http://vocab.nerc.ac.uk/collection/L05/current/315> ;
  skos:member <http://vocab.nerc.ac.uk/collection/L05/current/32> ;
  skos:member <http://vocab.nerc.ac.uk/collection/L05/current/33> ;
  skos:member <http://vocab.nerc.ac.uk/collection/L05/current/351> ;
  skos:member <http://vocab.nerc.ac.uk/collection/L05/current/352> ;
  skos:member <http://vocab.nerc.ac.uk/collection/L05/current/353> ;
  skos:member <http://vocab.nerc.ac.uk/collection/L05/current/354> ;
  skos:member <http://vocab.nerc.ac.uk/collection/L05/current/355> ;
  skos:member <http://vocab.nerc.ac.uk/collection/L05/current/356> ;
  skos:member <http://vocab.nerc.ac.uk/collection/L05/current/358> ;
  skos:member <http://vocab.nerc.ac.uk/collection/L05/current/359> ;
  skos:member <http://vocab.nerc.ac.uk/collection/L05/current/360> ;
  skos:member <http://vocab.nerc.ac.uk/collection/L05/current/361> ;
  skos:member <http://vocab.nerc.ac.uk/collection/L05/current/367> ;
  skos:member <http://vocab.nerc.ac.uk/collection/L05/current/368> ;
  skos:member <http://vocab.nerc.ac.uk/collection/L05/current/370> ;
  skos:member <http://vocab.nerc.ac.uk/collection/L05/current/376> ;
  skos:member <http://vocab.nerc.ac.uk/collection/L05/current/377> ;
  skos:member <http://vocab.nerc.ac.uk/collection/L05/current/379> ;
  skos:member <http://vocab.nerc.ac.uk/collection/L05/current/380> ;
  skos:member <http://vocab.nerc.ac.uk/collection/L05/current/381> ;
  skos:member <http://vocab.nerc.ac.uk/collection/L05/current/382> ;
  skos:member <http://vocab.nerc.ac.uk/collection/L05/current/383> ;
  skos:member <http://vocab.nerc.ac.uk/collection/L05/current/384> ;
  skos:member <http://vocab.nerc.ac.uk/collection/L05/current/385> ;
  skos:member <http://vocab.nerc.ac.uk/collection/L05/current/386> ;
  skos:member <http://vocab.nerc.ac.uk/collection/L05/current/387> ;
  skos:member <http://vocab.nerc.ac.uk/collection/L05/current/388> ;
  skos:member <http://vocab.nerc.ac.uk/collection/L05/current/389> ;
  skos:member <http://vocab.nerc.ac.uk/collection/L05/current/390> ;
  skos:member <http://vocab.nerc.ac.uk/collection/L05/current/391> ;
  skos:member <http://vocab.nerc.ac.uk/collection/L05/current/392> ;
  skos:member <http://vocab.nerc.ac.uk/collection/L05/current/395> ;
  skos:member <http://vocab.nerc.ac.uk/collection/L05/current/50> ;
  skos:member <http://vocab.nerc.ac.uk/collection/L05/current/51> ;
  skos:member <http://vocab.nerc.ac.uk/collection/L05/current/52> ;
  skos:member <http://vocab.nerc.ac.uk/collection/L05/current/53> ;
  skos:member <http://vocab.nerc.ac.uk/collection/L05/current/54> ;
  skos:member <http://vocab.nerc.ac.uk/collection/L05/current/55> ;
  skos:member <http://vocab.nerc.ac.uk/collection/L05/current/56> ;
  skos:member <http://vocab.nerc.ac.uk/collection/L05/current/57> ;
  skos:member <http://vocab.nerc.ac.uk/collection/L05/current/58> ;
  skos:member <http://vocab.nerc.ac.uk/collection/L05/current/59> ;
  skos:member <http://vocab.nerc.ac.uk/collection/L05/current/60> ;
  skos:member <http://vocab.nerc.ac.uk/collection/L05/current/61> ;
  skos:member <http://vocab.nerc.ac.uk/collection/L05/current/62> ;
  skos:member <http://vocab.nerc.ac.uk/collection/L05/current/63> ;
  skos:member <http://vocab.nerc.ac.uk/collection/L05/current/64> ;
  skos:member <http://vocab.nerc.ac.uk/collection/L05/current/65> ;
  skos:member <http://vocab.nerc.ac.uk/collection/L05/current/66> ;
  skos:member <http://vocab.nerc.ac.uk/collection/L05/current/67> ;
  skos:member <http://vocab.nerc.ac.uk/collection/L05/current/68> ;
  skos:member <http://vocab.nerc.ac.uk/collection/L05/current/69> ;
  skos:member <http://vocab.nerc.ac.uk/collection/L05/current/70> ;
  skos:member <http://vocab.nerc.ac.uk/collection/L05/current/71> ;
  skos:member <http://vocab.nerc.ac.uk/collection/L05/current/72> ;
  skos:member <http://vocab.nerc.ac.uk/collection/L05/current/86> ;
  skos:member <http://vocab.nerc.ac.uk/collection/L05/current/90> ;
  skos:member <http://vocab.nerc.ac.uk/collection/L05/current/91> ;
  skos:member <http://vocab.nerc.ac.uk/collection/L05/current/999> ;
  skos:member sdev:ATRANS ;
  skos:member sdev:BLUMS ;
  skos:member sdev:CCOV ;
  skos:member sdev:COLCMP ;
  skos:member sdev:CSEM ;
  skos:member sdev:DLOG ;
  skos:member sdev:EMSR ;
  skos:member sdev:FFES ;
  skos:member sdev:ICEP ;
  skos:member sdev:LAB01 ;
  skos:member sdev:LAB02 ;
  skos:member sdev:LAB03 ;
  skos:member sdev:LAB04 ;
  skos:member sdev:LAB06 ;
  skos:member sdev:LAB07 ;
  skos:member sdev:LAB08 ;
  skos:member sdev:LAB09 ;
  skos:member sdev:LAB10 ;
  skos:member sdev:LAB11 ;
  skos:member sdev:LAB12 ;
  skos:member sdev:LAB13 ;
  skos:member sdev:LAB14 ;
  skos:member sdev:LAB15 ;
  skos:member sdev:LAB17 ;
  skos:member sdev:LAB18 ;
  skos:member sdev:LAB19 ;
  skos:member sdev:LAB21 ;
  skos:member sdev:LAB22 ;
  skos:member sdev:LAB23 ;
  skos:member sdev:LAB24 ;
  skos:member sdev:LAB25 ;
  skos:member sdev:LAB26 ;
  skos:member sdev:LAB27 ;
  skos:member sdev:LAB28 ;
  skos:member sdev:LAB29 ;
  skos:member sdev:LAB30 ;
  skos:member sdev:LAB31 ;
  skos:member sdev:LAB32 ;
  skos:member sdev:LAB33 ;
  skos:member sdev:LAB34 ;
  skos:member sdev:LAB35 ;
  skos:member sdev:LAB36 ;
  skos:member sdev:LAB37 ;
  skos:member sdev:LAB38 ;
  skos:member sdev:LAB39 ;
  skos:member sdev:LAB40 ;
  skos:member sdev:LAB42 ;
  skos:member sdev:LAB43 ;
  skos:member sdev:LAB44 ;
  skos:member sdev:LAB45 ;
  skos:member sdev:LAB46 ;
  skos:member sdev:LAB47 ;
  skos:member sdev:LAB48 ;
  skos:member sdev:LAB49 ;
  skos:member sdev:LAB51 ;
  skos:member sdev:LVLST ;
  skos:member sdev:MMIS ;
  skos:member sdev:MPIS ;
  skos:member sdev:PERMON ;
  skos:member sdev:TFSAMP ;
  skos:member sdev:TRTG ;
  skos:member sdev:WDRG ;
  skos:member sdev:WPS ;
  skos:prefLabel "SeaDataNet device categories" ;
.
<http://w3id.org/def/nerc/instrumenttype/ontology>

  rdf:type skos:ConceptScheme ;
  rdfs:label "nerc collection W06"@en ;
  owl:imports <http://www.w3.org/2004/02/skos/core> ;
  skos:prefLabel "nerc collection W06"@en ;
.
<http://w3id.org/def/nerc/keyword-L19/collection>

  rdf:type skos:Collection ;
  dcterm:alternative "SDN keyword types" ;
  dcterm:creator "SeaDataNet" ;
  dcterm:date "2021-07-07 15:21:48.0" ;
  dcterm:description "Terms used in SeaDataNet metadata to describe the purpose of a keyword.  An extension of the ISO19115 KeywordTypeCode codelist." ;
  dcterm:license <https://creativecommons.org/licenses/by/4.0> ;
  dcterm:publisher "Natural Environment Research Council" ;
  dcterm:title "SeaDataNet keyword types" ;
  grg:RE_RegisterManager "British Oceanographic Data Centre" ;
  grg:RE_RegisterOwner "SeaDataNet" ;
  rdfs:comment "Governance for vocabularies used in the EU SeaDataNet project implemented as consultation between BODC and the members of the SeaDataNet Technical Task Team" ;
  owl:imports <http://www.w3.org/2004/02/skos/core> ;
  owl:versionInfo "4" ;
  skos:altLabel "SDN keyword types" ;
  skos:historyNote "original URI was http://vocab.nerc.ac.uk/collection/L19/current/"@en ;
  skos:member <http://vocab.nerc.ac.uk/collection/L19/current/002> ;
  skos:member <http://vocab.nerc.ac.uk/collection/L19/current/003> ;
  skos:member <http://vocab.nerc.ac.uk/collection/L19/current/004> ;
  skos:member sdnk:SDNKG02 ;
  skos:member sdnk:SDNKG04 ;
  skos:member sdnk:SDNKG05 ;
  skos:member sdnk:SDNKG06 ;
  skos:member sdnk:SDNKG07 ;
  skos:member sdnk:SDNKG08 ;
  skos:member sdnk:SDNKG09 ;
  skos:member sdnk:SDNKG10 ;
  skos:member sdnk:SDNKG11 ;
  skos:member sdnk:SDNKG12 ;
  skos:member sdnk:SDNKG13 ;
  skos:member sdnk:SDNKG14 ;
  skos:member sdnk:SDNKG15 ;
  skos:member sdnk:SDNKG16 ;
  skos:member sdnk:SDNKG17 ;
  skos:prefLabel "SeaDataNet keyword types" ;
.
<http://w3id.org/def/nerc/sdncategories-L21/conceptscheme>

  rdf:type skos:ConceptScheme ;
  rdfs:label "categories for SeaDataNet resources"@en ;
  owl:imports <http://www.w3.org/2004/02/skos/core> ;
.
<http://w3id.org/def/nerc/seadatanetdatacat/collection>

  rdf:type skos:Collection ;
  dcterm:alternative "SeaDataNet CSR data categories" ;
  dcterm:creator "SeaDataNet" ;
  dcterm:date "2022-09-27 03:00:02.0" ;
  dcterm:description "Terms used to describe shipboard activities (sometimes inaccurately described as parameters) by SeaDataNet in Cruise Summary Report (formerly known as ROSCOP) metadata." ;
  dcterm:license <https://creativecommons.org/licenses/by/4.0> ;
  dcterm:publisher "Natural Environment Research Council" ;
  dcterm:title "SeaDataNet Cruise Summary Report data categories" ;
  grg:RE_RegisterManager "British Oceanographic Data Centre" ;
  grg:RE_RegisterOwner "SeaDataNet" ;
  rdfs:comment "Governance for vocabularies used in the EU SeaDataNet project implemented as consultation between BODC and the members of the SeaDataNet Technical Task Team" ;
  owl:imports <http://w3id.org/def/nerc/discipline-P08/collection> ;
  owl:imports <http://w3id.org/def/nerc/instrument-L05/collection> ;
  owl:imports <http://w3id.org/def/nerc/keyword-L19/collection> ;
  owl:imports <http://www.w3.org/2004/02/skos/core> ;
  skos:altLabel "SeaDataNet CSR data categories" ;
  skos:historyNote "original URI was http://vocab.nerc.ac.uk/collection/C77/current/"@en ;
  skos:member sdnd:B01 ;
  skos:member sdnd:B02 ;
  skos:member sdnd:B03 ;
  skos:member sdnd:B06 ;
  skos:member sdnd:B07 ;
  skos:member sdnd:B08 ;
  skos:member sdnd:B09 ;
  skos:member sdnd:B10 ;
  skos:member sdnd:B11 ;
  skos:member sdnd:B13 ;
  skos:member sdnd:B14 ;
  skos:member sdnd:B16 ;
  skos:member sdnd:B17 ;
  skos:member sdnd:B18 ;
  skos:member sdnd:B19 ;
  skos:member sdnd:B20 ;
  skos:member sdnd:B21 ;
  skos:member sdnd:B25 ;
  skos:member sdnd:B26 ;
  skos:member sdnd:B28 ;
  skos:member sdnd:B37 ;
  skos:member sdnd:B64 ;
  skos:member sdnd:B65 ;
  skos:member sdnd:B71 ;
  skos:member sdnd:B72 ;
  skos:member sdnd:B73 ;
  skos:member sdnd:B90 ;
  skos:member sdnd:G01 ;
  skos:member sdnd:G02 ;
  skos:member sdnd:G03 ;
  skos:member sdnd:G04 ;
  skos:member sdnd:G08 ;
  skos:member sdnd:G24 ;
  skos:member sdnd:G26 ;
  skos:member sdnd:G27 ;
  skos:member sdnd:G28 ;
  skos:member sdnd:G71 ;
  skos:member sdnd:G72 ;
  skos:member sdnd:G73 ;
  skos:member sdnd:G74 ;
  skos:member sdnd:G75 ;
  skos:member sdnd:G76 ;
  skos:member sdnd:G90 ;
  skos:member sdnd:H21 ;
  skos:member sdnd:H22 ;
  skos:member sdnd:H23 ;
  skos:member sdnd:H24 ;
  skos:member sdnd:H25 ;
  skos:member sdnd:H26 ;
  skos:member sdnd:H27 ;
  skos:member sdnd:H28 ;
  skos:member sdnd:H30 ;
  skos:member sdnd:H31 ;
  skos:member sdnd:H32 ;
  skos:member sdnd:H33 ;
  skos:member sdnd:H74 ;
  skos:member sdnd:H75 ;
  skos:member sdnd:H76 ;
  skos:member sdnd:H90 ;
  skos:member sdnd:M04 ;
  skos:member sdnd:R01 ;
  skos:member sdnd:R02 ;
  skos:member sdnd:R03 ;
  skos:member sdnd:R04 ;
  skos:prefLabel "SeaDataNet Cruise Summary Report data categories" ;
.
<http://w3id.org/def/numericalmodel/conceptscheme>
  rdf:type skos:ConceptScheme ;
  rdfs:label "Numeric Model" ;
  skos:definition " " ;
  skos:prefLabel "Numeric Model" ;
.
<http://w3id.org/def/positioningsystem/conceptscheme>
  rdf:type skos:ConceptScheme ;
  rdfs:label "Positioning system "@en ;
  skos:definition " " ;
  skos:prefLabel "Positioning system "@en ;
.
<http://w3id.org/def/samplecollectioninstrument/conceptscheme>
  rdf:type skos:ConceptScheme ;
  rdfs:label "Sample collection instrument "@en ;
  skos:definition " " ;
  skos:prefLabel "Sample collection instrument "@en ;
.
<http://w3id.org/def/sampleprepreationinstrument/conceptscheme>
  rdf:type skos:ConceptScheme ;
  rdfs:label "Sample preparation instrument "@en ;
  skos:definition " " ;
  skos:prefLabel "Sample preparation instrument "@en ;
.
<http://w3id.org/def/seismicsource/conceptscheme>
  rdf:type skos:ConceptScheme ;
  rdfs:label "Seismic source instrument "@en ;
  skos:definition " " ;
  skos:prefLabel "Seismic source instrument "@en ;
.
<http://w3id.org/ogeochem/def/samplecollection/measurement/conceptscheme>
  rdf:type skos:ConceptScheme ;
  rdfs:label "Measurement instruments" ;
  skos:definition " " ;
  skos:prefLabel "Measurement instruments" ;
.
<http://w3id.org/ogeochem/def/samplecollection/ontology>
  rdf:type owl:Ontology ;
  dcterm:created "2023-02-09"^^xsd:date ;
  dcterm:creator "SMR" ;
  dcterm:modified "2023-03-09"^^xsd:date ;
  dcterm:publisher "TBD" ;
  dcterm:source "Compiled NERC vocabularies related to measurement instyruments" ;
  rdfs:label "Measurement instruments for geochemistry"@en ;
  owl:imports <http://purl.org/dc/elements/1.1/> ;
  owl:imports <http://www.w3.org/2000/01/rdf-schema> ;
  owl:imports <http://www.w3.org/2004/02/skos/core> ;
  skos:definition "TBD"@en ;
  skos:prefLabel "Measurement instruments for geochemistry"@en ;
.
<http://w3id.org/ogeochem/def/samplecollection/parameters/conceptscheme>
  rdf:type skos:ConceptScheme ;
  rdfs:label "Measurement type" ;
  skos:definition " " ;
  skos:prefLabel "Measurement type" ;
.
grg:RE_RegisterManager
  rdf:type owl:AnnotationProperty ;
.
grg:RE_RegisterOwner
  rdf:type owl:AnnotationProperty ;
.
skos:Collection
  rdf:type owl:Class ;
.
skos:Concept
  rdf:type owl:Class ;
.
skos:altLabel
  rdf:type owl:AnnotationProperty ;
.
skos:definition
  rdf:type owl:AnnotationProperty ;
.
skos:narrower
  rdf:type owl:AnnotationProperty ;
.
skos:notation
  rdf:type owl:AnnotationProperty ;
.
skos:note
  rdf:type owl:AnnotationProperty ;
.
skos:prefLabel
  rdf:type owl:AnnotationProperty ;
.
