# baseURI: http://w3id.org/def/mmisw/models/ontology
# imports: http://www.w3.org/2004/02/skos/core

@prefix : <http://mmisw.org/ont/trdi/models/> .
@prefix dc: <http://purl.org/dc/elements/1.1/> .
@prefix dcterm: <http://purl.org/dc/terms/> .
@prefix omv: <http://omv.ontoware.org/2005/05/ontology#> .
@prefix omvmmi: <http://mmisw.org/ont/mmi/20081020/ontologyMetadata/> .
@prefix owl: <http://www.w3.org/2002/07/owl#> .
@prefix rdf: <http://www.w3.org/1999/02/22-rdf-syntax-ns#> .
@prefix rdfs: <http://www.w3.org/2000/01/rdf-schema#> .
@prefix skos: <http://www.w3.org/2004/02/skos/core#> .
@prefix xsd: <http://www.w3.org/2001/XMLSchema#> .

:
  rdf:type owl:Ontology ;
.
:Category
  rdf:type owl:DatatypeProperty ;
  rdfs:domain :ModelName ;
  rdfs:label "Category" ;
.
:ChannelMaster
  rdf:type :ModelName ;
  :ID "ChannelMaster" ;
  :LongName "ChannelMaster" ;
  rdfs:label "ChannelMaster" ;
  skos:definition "Teledyne Rd Instruments model name for an ADCP designed to use horizontal profiling for flow monitoring in inland waterways." ;
  skos:inScheme <http://w3id.org/def/mmisw/models/ontology> ;
  skos:prefLabel "ChannelMaster" ;
.
:Equations_s
  rdf:type owl:DatatypeProperty ;
  rdfs:domain :ModelName ;
  rdfs:label "Equations(s)" ;
.
:Figure_s
  rdf:type owl:DatatypeProperty ;
  rdfs:domain :ModelName ;
  rdfs:label "Figure(s)" ;
.
:HorizontalADCP
  rdf:type :ModelName ;
  :ID "HorizontalADCP" ;
  :LongName "Horizontal ADCP" ;
  :ShortName "HADCP" ;
  rdfs:label "HorizontalADCP" ;
  skos:definition "Instrument designed to measure velocity profiles in a horizontal plane." ;
  skos:inScheme <http://w3id.org/def/mmisw/models/ontology> ;
  skos:prefLabel "HorizontalADCP" ;
.
:ID
  rdf:type owl:DatatypeProperty ;
  rdfs:domain :ModelName ;
  rdfs:label "ID" ;
.
:LongName
  rdf:type owl:DatatypeProperty ;
  rdfs:domain :ModelName ;
  rdfs:label "LongName" ;
.
:LongRanger
  rdf:type :ModelName ;
  :ID "LongRanger" ;
  :LongName "Long Ranger" ;
  rdfs:label "LongRanger" ;
  skos:definition "Model name for Teledyne RD Instruments Workhorse ADCPs of frequency 75 kHz." ;
  skos:inScheme <http://w3id.org/def/mmisw/models/ontology> ;
  skos:prefLabel "LongRanger" ;
.
:Mariner
  rdf:type :ModelName ;
  :ID "Mariner" ;
  :LongName "Mariner" ;
  rdfs:label "Mariner" ;
  skos:definition "Model name for a Teledyne RD Instruments Workhorse Monitor ADCP configured for underway current measurement in shallow water (as opposed to the deep water Ocean Surveyor systems)." ;
  skos:inScheme <http://w3id.org/def/mmisw/models/ontology> ;
  skos:prefLabel "Mariner" ;
.
:ModelName
  rdf:type owl:Class ;
  rdfs:label "ModelName" ;
  rdfs:subClassOf skos:Concept ;
  skos:historyNote "change from owl:Class to skos:Concept SMR 2023-03-07" ;
.
:Monitor
  rdf:type :ModelName ;
  :ID "Monitor" ;
  :LongName "Monitor" ;
  :Relationship_s "DirectReadingADCP" ;
  rdfs:label "Monitor" ;
  skos:definition "Teledyne RD Instruments model name for a direct reading Workhorse ADCP." ;
  skos:inScheme <http://w3id.org/def/mmisw/models/ontology> ;
  skos:prefLabel "Monitor" ;
.
:Navigator
  rdf:type :ModelName ;
  :ID "Navigator" ;
  :LongName "Navigator" ;
  rdfs:label "Navigator" ;
  skos:definition "Teledyne RD Instruments model name for the Teledyne RDI Doppler Velocity Log." ;
  skos:inScheme <http://w3id.org/def/mmisw/models/ontology> ;
  skos:prefLabel "Navigator" ;
.
:Notes
  rdf:type owl:DatatypeProperty ;
  rdfs:domain :ModelName ;
  rdfs:label "Notes" ;
.
:OceanObserver
  rdf:type :ModelName ;
  :ID "OceanObserver" ;
  :LongName "Ocean Observer" ;
  :ShortName "OO" ;
  rdfs:label "OceanObserver" ;
  skos:definition "Teledyne RD Instruments model name for a low frequency Phased Array ADCP for cabled deployment, usually from an oil rig." ;
  skos:inScheme <http://w3id.org/def/mmisw/models/ontology> ;
  skos:prefLabel "OceanObserver" ;
.
:OceanSurveyor
  rdf:type :ModelName ;
  :ID "OceanSurveyor" ;
  :LongName "Ocean Surveyor" ;
  :ShortName "OS" ;
  rdfs:label "OceanSurveyor" ;
  skos:definition "Teledyne RD Instruments model name for a low frequency Phased Array ADCP for vessel mounted operations." ;
  skos:inScheme <http://w3id.org/def/mmisw/models/ontology> ;
  skos:prefLabel "OceanSurveyor" ;
.
:Reference
  rdf:type owl:DatatypeProperty ;
  rdfs:domain :ModelName ;
  rdfs:label "Reference" ;
.
:Relationship_s
  rdf:type owl:DatatypeProperty ;
  rdfs:domain :ModelName ;
  rdfs:label "Relationship(s)" ;
.
:RioGrandeADCP
  rdf:type :ModelName ;
  :ID "RioGrandeADCP" ;
  :LongName "Rio Grande ADCP" ;
  rdfs:label "RioGrandeADCP" ;
  skos:definition "Teledyne RD Instruments model name for an ADCP optimally configured for measurement of river discharge. A distinguishing feature of Rio Grande ADCPs is that they are designed to operate from a 12 VDC power supply (all other ADCPs operate from 20 - 60 VDC)." ;
  skos:inScheme <http://w3id.org/def/mmisw/models/ontology> ;
  skos:prefLabel "RioGrandeADCP" ;
.
:Sentinel
  rdf:type :ModelName ;
  :ID "Sentinel" ;
  :LongName "Sentinel" ;
  rdfs:label "Sentinel" ;
  skos:definition "Teledyne RD Instruments model name for a self-contained Workhorse ADCP." ;
  skos:inScheme <http://w3id.org/def/mmisw/models/ontology> ;
  skos:prefLabel "Sentinel" ;
.
:ShortName
  rdf:type owl:DatatypeProperty ;
  rdfs:domain :ModelName ;
  rdfs:label "ShortName" ;
.
:StreamPro
  rdf:type :ModelName ;
  :ID "StreamPro" ;
  :LongName "StreamPro" ;
  rdfs:label "StreamPro" ;
  skos:definition "Teledyne RD Instruments model name for a miniaturized ADCP packaged into a streamlined float designed to be towed by hand across very shallow streams for quick and efficient discharge measurements." ;
  skos:inScheme <http://w3id.org/def/mmisw/models/ontology> ;
  skos:prefLabel "StreamPro" ;
.
:Symbol
  rdf:type owl:DatatypeProperty ;
  rdfs:domain :ModelName ;
  rdfs:label "Symbol" ;
.
:VesselMount
  rdf:type :ModelName ;
  :ID "VesselMount" ;
  :LongName "Vessel Mount" ;
  rdfs:label "VesselMount" ;
  skos:definition "An ADCP mounted to the hull of a vessel, typically in a sea chest, and having inputs from the vessel's navigation equipment." ;
  skos:inScheme <http://w3id.org/def/mmisw/models/ontology> ;
  skos:prefLabel "VesselMount" ;
.
:WorkhorseADCP
  rdf:type :ModelName ;
  :ID "WorkhorseADCP" ;
  :LongName "Workhorse ADCP" ;
  :ShortName "WH" ;
  rdfs:label "WorkhorseADCP" ;
  skos:definition "The generic model name for all of the non-phased array broadband ADCPs currently produced by Teledyne RD Instruments" ;
  skos:inScheme <http://w3id.org/def/mmisw/models/ontology> ;
  skos:prefLabel "WorkhorseADCP" ;
.
:ZedHead
  rdf:type :ModelName ;
  :ID "ZedHead" ;
  :LongName "ZedHead" ;
  rdfs:label "ZedHead" ;
  skos:definition "Teledyne RD Instruments trade name for a transducer designed to minimize ringing." ;
  skos:inScheme <http://w3id.org/def/mmisw/models/ontology> ;
  skos:prefLabel "ZedHead" ;
.
<http://w3id.org/def/mmisw/models/ontology>
  rdf:type owl:Ontology ;
  rdf:type skos:ConceptScheme ;
  omvmmi:creditRequired "not specified" ;
  omvmmi:hasResourceType "sensor" ;
  omvmmi:origMaintainerCode "trdi" ;
  omvmmi:shortNameUri "http://mmisw.org/ont/mmi/resourcetype/sensor" ;
  omv:acronym "models" ;
  omv:creationDate "2012-04-19T19:25:05+0000" ;
  omv:description "Names and descriptions of various Teledyne RD Instruments Sensor Models" ;
  omv:hasCreator "Jerry Mullison" ;
  omv:keywords "ADCP, Doppler, Waves, Ocean Currents" ;
  omv:name "Teledyne RD Instruments Model Names" ;
  omv:uri "http://mmisw.org/ont/trdi/models" ;
  omv:usedOntologyEngineeringTool omvmmi:voc2rdf ;
  omv:version "20120419T192505" ;
  dcterm:creator "Jerry Mullison" ;
  dcterm:date "2012-04-19T19:25:05+0000" ;
  dcterm:description "Names and descriptions of various Teledyne RD Instruments Sensor Models" ;
  owl:imports <http://www.w3.org/2004/02/skos/core> ;
.
skos:definition
  rdf:type owl:DatatypeProperty ;
.
